<?xml version="1.0"?>
<rdf:RDF xmlns="http://semanticbible.org/ns/2006/NTNames#"
     xml:base="http://semanticbible.org/ns/2006/NTNames"
     xmlns:dc="http://purl.org/dc/elements/1.1/"
     xmlns:owl="http://www.w3.org/2002/07/owl#"
     xmlns:rdf="http://www.w3.org/1999/02/22-rdf-syntax-ns#"
     xmlns:rss="http://purl.org/rss/1.0/"
     xmlns:xml="http://www.w3.org/XML/1998/namespace"
     xmlns:xsd="http://www.w3.org/2001/XMLSchema#"
     xmlns:rdfs="http://www.w3.org/2000/01/rdf-schema#">
    <owl:Ontology rdf:about="http://semanticbible.org/ns/2006/NTNames">
        <rdfs:comment xml:lang="en">The names here are as
transliterated in the English Standard Version (ESV), copyright Â©
2001 by Crossway Bibles, a division of Good News Publishers.

Reuse note: where feasible, class names coincide with SUMO (Suggested
Upper Merged Ontology), as developed within the IEEE Standard Upper
Ontology Working Group, described at http://www.ontologyportal.org/,
and available as OWL at http://reliant.teknowledge.com/DAML/SUMO.owl
(but not without some problems). I&apos;ve copied, rather than re-used, but
this provides a future migration path toward coordinating the two
ontologies.

</rdfs:comment>
        <owl:versionInfo rdf:datatype="http://www.w3.org/2001/XMLSchema#string">1.0</owl:versionInfo>
    </owl:Ontology>
    


    <!-- 
    ///////////////////////////////////////////////////////////////////////////////////////
    //
    // Object Properties
    //
    ///////////////////////////////////////////////////////////////////////////////////////
     -->

    


    <!-- http://semanticbible.org/ns/2006/NTNames#antagonistOf -->

    <owl:ObjectProperty rdf:about="http://semanticbible.org/ns/2006/NTNames#antagonistOf">
        <rdfs:subPropertyOf rdf:resource="http://semanticbible.org/ns/2006/NTNames#knows"/>
        <owl:inverseOf rdf:resource="http://semanticbible.org/ns/2006/NTNames#hasAntagonist"/>
        <rdfs:comment xml:lang="en">&quot;A person who opposes and contends against this person&quot;, similar to http://purl.org/vocab/relationship vocabulary, but with different domain and range. For clarity, &lt;X antagonistOf Y&gt; means X opposes, etc. Y, and also (by inference) &lt;Y hasAntagonist X&gt;. However, it does _not_ necessarily mean &lt;Y antagonistOf X&gt;, i.e. it is not necessarily reciprocal.</rdfs:comment>
        <rdfs:label xml:lang="en">antagonist of</rdfs:label>
    </owl:ObjectProperty>
    


    <!-- http://semanticbible.org/ns/2006/NTNames#childOf -->

    <owl:ObjectProperty rdf:about="http://semanticbible.org/ns/2006/NTNames#childOf">
        <rdfs:subPropertyOf rdf:resource="http://semanticbible.org/ns/2006/NTNames#relativeOf"/>
        <owl:inverseOf rdf:resource="http://semanticbible.org/ns/2006/NTNames#parentOf"/>
        <rdfs:domain rdf:resource="http://semanticbible.org/ns/2006/NTNames#Human"/>
        <rdfs:range rdf:resource="http://semanticbible.org/ns/2006/NTNames#Human"/>
        <rdfs:comment xml:lang="en">Similar to http://purl.org/vocab/relationship vocabulary, but with different domain and range. In-laws are considered relatives. </rdfs:comment>
        <rdfs:label xml:lang="en">child of</rdfs:label>
    </owl:ObjectProperty>
    


    <!-- http://semanticbible.org/ns/2006/NTNames#collaboratesWith -->

    <owl:ObjectProperty rdf:about="http://semanticbible.org/ns/2006/NTNames#collaboratesWith">
        <rdfs:subPropertyOf rdf:resource="http://semanticbible.org/ns/2006/NTNames#knows"/>
        <owl:inverseOf rdf:resource="http://semanticbible.org/ns/2006/NTNames#collaboratesWith"/>
        <rdf:type rdf:resource="http://www.w3.org/2002/07/owl#SymmetricProperty"/>
        <rdfs:domain rdf:resource="http://semanticbible.org/ns/2006/NTNames#Human"/>
        <rdfs:range rdf:resource="http://semanticbible.org/ns/2006/NTNames#Human"/>
        <rdfs:comment xml:lang="en">&quot;A person who works toward a common goal with this person&quot;, similar to http://purl.org/vocab/relationship vocabulary, but with different domain and range. Those to whom the author of a New Testament Epistle send greetings are assumed to be collaborators, though this is perhaps broader than the general sense of the word. However, simple Christian fellowship or conversion do not constitute collaboration in this sense. </rdfs:comment>
        <rdfs:label xml:lang="en">collaborates with</rdfs:label>
    </owl:ObjectProperty>
    


    <!-- http://semanticbible.org/ns/2006/NTNames#enemyOf -->

    <owl:ObjectProperty rdf:about="http://semanticbible.org/ns/2006/NTNames#enemyOf">
        <rdfs:subPropertyOf rdf:resource="http://semanticbible.org/ns/2006/NTNames#knows"/>
        <owl:inverseOf rdf:resource="http://semanticbible.org/ns/2006/NTNames#hasEnemy"/>
        <rdfs:comment xml:lang="en">&quot;A person towards whom this person feels hatred, intends injury to, or opposes the interests of&quot;, similar to http://purl.org/vocab/relationship vocabulary, but with different domain and range. For clarity, &lt;X, enemyOf, Y&gt; means X feels hatred, etc. towards Y, and also (by inference) &lt;Y, hasEnemy, X&gt;. However, it does _not_ necessarily mean &lt;Y, enemyOf, X&gt;, i.e. it is not necessarily reciprocal.</rdfs:comment>
        <rdfs:label xml:lang="en">enemy of</rdfs:label>
    </owl:ObjectProperty>
    


    <!-- http://semanticbible.org/ns/2006/NTNames#ethnicity -->

    <owl:ObjectProperty rdf:about="http://semanticbible.org/ns/2006/NTNames#ethnicity">
        <owl:inverseOf rdf:resource="http://semanticbible.org/ns/2006/NTNames#ethnicityOf"/>
        <rdfs:domain rdf:resource="http://semanticbible.org/ns/2006/NTNames#Human"/>
        <rdfs:range rdf:resource="http://semanticbible.org/ns/2006/NTNames#EthnicityAttribute"/>
        <rdfs:comment xml:lang="en">The ethnicity or, more generally, cultural heritage of a person. This can overlap with both religiousBelief (which may, however, change over time) and nativePlace (which, like ethnicity, does not change, though residency might). Whether a given property represents ethnicity or citizenship (nativePlace) can be a difficult decision, but in general, ethnic identities like &quot;Jewish&quot; or &quot;Greek&quot; take precedence. For example, we consider the Apostle Paul to have Jewish ethnicity, though he was a citizen of Tarsus, because he was raised as a Jew. Ethnicity is not specified without specific evidence, either textual or reliable tradition: for example, having a Greek name is not sufficient. </rdfs:comment>
        <rdfs:label xml:lang="en">ethnicity</rdfs:label>
    </owl:ObjectProperty>
    


    <!-- http://semanticbible.org/ns/2006/NTNames#ethnicityOf -->

    <owl:ObjectProperty rdf:about="http://semanticbible.org/ns/2006/NTNames#ethnicityOf">
        <rdfs:domain rdf:resource="http://semanticbible.org/ns/2006/NTNames#EthnicityAttribute"/>
        <rdfs:range rdf:resource="http://semanticbible.org/ns/2006/NTNames#Human"/>
        <rdfs:label xml:lang="en">ethnicity of</rdfs:label>
    </owl:ObjectProperty>
    


    <!-- http://semanticbible.org/ns/2006/NTNames#hasAntagonist -->

    <owl:ObjectProperty rdf:about="http://semanticbible.org/ns/2006/NTNames#hasAntagonist">
        <rdfs:subPropertyOf rdf:resource="http://semanticbible.org/ns/2006/NTNames#knows"/>
        <rdfs:domain rdf:resource="http://semanticbible.org/ns/2006/NTNames#Human"/>
        <rdfs:comment xml:lang="en">inverse of antagonistOf, which is not necessarily reciprocal</rdfs:comment>
        <rdfs:label xml:lang="en">has antagonist</rdfs:label>
    </owl:ObjectProperty>
    


    <!-- http://semanticbible.org/ns/2006/NTNames#hasEnemy -->

    <owl:ObjectProperty rdf:about="http://semanticbible.org/ns/2006/NTNames#hasEnemy">
        <rdfs:subPropertyOf rdf:resource="http://semanticbible.org/ns/2006/NTNames#knows"/>
        <rdfs:domain rdf:resource="http://semanticbible.org/ns/2006/NTNames#Human"/>
        <rdfs:range rdf:resource="http://semanticbible.org/ns/2006/NTNames#Human"/>
        <rdfs:comment xml:lang="en">inverse of enemyOf, which is not necessarily reciprocal</rdfs:comment>
        <rdfs:label xml:lang="en">has enemy</rdfs:label>
    </owl:ObjectProperty>
    


    <!-- http://semanticbible.org/ns/2006/NTNames#knows -->

    <owl:ObjectProperty rdf:about="http://semanticbible.org/ns/2006/NTNames#knows">
        <owl:inverseOf rdf:resource="http://semanticbible.org/ns/2006/NTNames#knows"/>
        <rdf:type rdf:resource="http://www.w3.org/2002/07/owl#SymmetricProperty"/>
        <rdfs:domain rdf:resource="http://semanticbible.org/ns/2006/NTNames#Human"/>
        <rdfs:range rdf:resource="http://semanticbible.org/ns/2006/NTNames#Human"/>
        <rdfs:comment xml:lang="en">&quot;A person known by this person (indicating some level of reciprocated interaction between the parties)&quot;, similar to http://purl.org/vocab/relationship vocabulary, but with different domain and range. Therefore this is a symmetric relationship: if I know you, you also know me (or else we don&apos;t &quot;know&quot; each other in this sense). </rdfs:comment>
        <rdfs:label xml:lang="en">knows</rdfs:label>
    </owl:ObjectProperty>
    


    <!-- http://semanticbible.org/ns/2006/NTNames#location -->

    <owl:ObjectProperty rdf:about="http://semanticbible.org/ns/2006/NTNames#location">
        <owl:inverseOf rdf:resource="http://semanticbible.org/ns/2006/NTNames#locationOf"/>
        <rdf:type rdf:resource="http://www.w3.org/2002/07/owl#FunctionalProperty"/>
        <rdf:type rdf:resource="http://www.w3.org/2002/07/owl#InverseFunctionalProperty"/>
        <rdfs:domain rdf:resource="http://semanticbible.org/ns/2006/NTNames#GeographicArea"/>
        <rdfs:range rdf:resource="http://semanticbible.org/ns/2006/NTNames#GeographicLocation"/>
        <rdfs:comment xml:lang="en">The location property relates a GeographicArea to a GeographicLocation. Each GeographicArea is assumed to have only one location, and no GeographicAreas share a location. </rdfs:comment>
        <rdfs:label xml:lang="en">location</rdfs:label>
    </owl:ObjectProperty>
    


    <!-- http://semanticbible.org/ns/2006/NTNames#locationOf -->

    <owl:ObjectProperty rdf:about="http://semanticbible.org/ns/2006/NTNames#locationOf">
        <rdf:type rdf:resource="http://www.w3.org/2002/07/owl#InverseFunctionalProperty"/>
        <rdfs:domain rdf:resource="http://semanticbible.org/ns/2006/NTNames#GeographicLocation"/>
        <rdfs:range rdf:resource="http://semanticbible.org/ns/2006/NTNames#GeographicArea"/>
    </owl:ObjectProperty>
    


    <!-- http://semanticbible.org/ns/2006/NTNames#member -->

    <owl:ObjectProperty rdf:about="http://semanticbible.org/ns/2006/NTNames#member">
        <owl:inverseOf rdf:resource="http://semanticbible.org/ns/2006/NTNames#memberOf"/>
        <rdfs:domain rdf:resource="http://semanticbible.org/ns/2006/NTNames#Group"/>
        <rdfs:range rdf:resource="http://semanticbible.org/ns/2006/NTNames#Human"/>
        <rdfs:comment xml:lang="en">Group has member Human. Inverse of memberOf. No provision for membership changes over time.</rdfs:comment>
        <rdfs:label xml:lang="en">member</rdfs:label>
    </owl:ObjectProperty>
    


    <!-- http://semanticbible.org/ns/2006/NTNames#memberOf -->

    <owl:ObjectProperty rdf:about="http://semanticbible.org/ns/2006/NTNames#memberOf">
        <rdfs:domain rdf:resource="http://semanticbible.org/ns/2006/NTNames#Human"/>
        <rdfs:range rdf:resource="http://semanticbible.org/ns/2006/NTNames#Group"/>
        <rdfs:comment xml:lang="en">Human is a memberOf a Group. Inverse of member. There are subtleties about Collections in SUMO that i&apos;m omiting here.</rdfs:comment>
        <rdfs:label xml:lang="en">member of</rdfs:label>
    </owl:ObjectProperty>
    


    <!-- http://semanticbible.org/ns/2006/NTNames#nativePlace -->

    <owl:ObjectProperty rdf:about="http://semanticbible.org/ns/2006/NTNames#nativePlace">
        <rdfs:subPropertyOf rdf:resource="http://semanticbible.org/ns/2006/NTNames#visitedPlace"/>
        <owl:inverseOf rdf:resource="http://semanticbible.org/ns/2006/NTNames#nativePlaceOf"/>
        <rdf:type rdf:resource="http://www.w3.org/2002/07/owl#FunctionalProperty"/>
        <rdfs:domain>
            <owl:Class>
                <owl:unionOf rdf:parseType="Collection">
                    <rdf:Description rdf:about="http://semanticbible.org/ns/2006/NTNames#GroupOfPeople"/>
                    <rdf:Description rdf:about="http://semanticbible.org/ns/2006/NTNames#Human"/>
                </owl:unionOf>
            </owl:Class>
        </rdfs:domain>
        <rdfs:range rdf:resource="http://semanticbible.org/ns/2006/NTNames#Region"/>
        <rdfs:comment xml:lang="en">Birthplace, or place in which a person grows up. Unlike residentOf, only one possible value. residentPlace is to be preferred unless the birthplace relationship is clearly identified.</rdfs:comment>
        <rdfs:label xml:lang="en">native place</rdfs:label>
    </owl:ObjectProperty>
    


    <!-- http://semanticbible.org/ns/2006/NTNames#nativePlaceOf -->

    <owl:ObjectProperty rdf:about="http://semanticbible.org/ns/2006/NTNames#nativePlaceOf">
        <rdfs:subPropertyOf rdf:resource="http://semanticbible.org/ns/2006/NTNames#visitedPlaceOf"/>
        <rdf:type rdf:resource="http://www.w3.org/2002/07/owl#InverseFunctionalProperty"/>
        <rdfs:domain rdf:resource="http://semanticbible.org/ns/2006/NTNames#GeographicArea"/>
        <rdfs:range>
            <owl:Class>
                <owl:unionOf rdf:parseType="Collection">
                    <rdf:Description rdf:about="http://semanticbible.org/ns/2006/NTNames#GroupOfPeople"/>
                    <rdf:Description rdf:about="http://semanticbible.org/ns/2006/NTNames#Human"/>
                </owl:unionOf>
            </owl:Class>
        </rdfs:range>
    </owl:ObjectProperty>
    


    <!-- http://semanticbible.org/ns/2006/NTNames#parentOf -->

    <owl:ObjectProperty rdf:about="http://semanticbible.org/ns/2006/NTNames#parentOf">
        <rdfs:subPropertyOf rdf:resource="http://semanticbible.org/ns/2006/NTNames#relativeOf"/>
        <rdfs:domain rdf:resource="http://semanticbible.org/ns/2006/NTNames#Human"/>
        <rdfs:range rdf:resource="http://semanticbible.org/ns/2006/NTNames#Human"/>
        <rdfs:comment xml:lang="en">Similar to http://purl.org/vocab/relationship vocabulary, but with different domain and range.</rdfs:comment>
        <rdfs:label xml:lang="en">parent of</rdfs:label>
    </owl:ObjectProperty>
    


    <!-- http://semanticbible.org/ns/2006/NTNames#politicalBelief -->

    <owl:ObjectProperty rdf:about="http://semanticbible.org/ns/2006/NTNames#politicalBelief">
        <rdfs:domain>
            <owl:Class>
                <owl:unionOf rdf:parseType="Collection">
                    <rdf:Description rdf:about="http://semanticbible.org/ns/2006/NTNames#GroupOfPeople"/>
                    <rdf:Description rdf:about="http://semanticbible.org/ns/2006/NTNames#Human"/>
                </owl:unionOf>
            </owl:Class>
        </rdfs:domain>
        <rdfs:range rdf:resource="http://semanticbible.org/ns/2006/NTNames#PoliticalBeliefSystem"/>
        <rdfs:comment xml:lang="en">Holding to a PoliticalBelief</rdfs:comment>
        <rdfs:label xml:lang="en">political belief</rdfs:label>
    </owl:ObjectProperty>
    


    <!-- http://semanticbible.org/ns/2006/NTNames#possiblySamePersonAs -->

    <owl:ObjectProperty rdf:about="http://semanticbible.org/ns/2006/NTNames#possiblySamePersonAs">
        <owl:inverseOf rdf:resource="http://semanticbible.org/ns/2006/NTNames#possiblySamePersonAs"/>
        <rdf:type rdf:resource="http://www.w3.org/2002/07/owl#SymmetricProperty"/>
        <rdfs:domain rdf:resource="http://semanticbible.org/ns/2006/NTNames#Human"/>
        <rdfs:range rdf:resource="http://semanticbible.org/ns/2006/NTNames#Human"/>
        <rdfs:comment xml:lang="en">This person may be the same as the other person, though there isn&apos;t enough evidence to definitively say so. Typically the individuals will have the same name, and some overlap of circumstances that makes it possible. </rdfs:comment>
        <rdfs:label xml:lang="en">possibly same person as</rdfs:label>
    </owl:ObjectProperty>
    


    <!-- http://semanticbible.org/ns/2006/NTNames#relativeOf -->

    <owl:ObjectProperty rdf:about="http://semanticbible.org/ns/2006/NTNames#relativeOf">
        <owl:inverseOf rdf:resource="http://semanticbible.org/ns/2006/NTNames#relativeOf"/>
        <rdf:type rdf:resource="http://www.w3.org/2002/07/owl#SymmetricProperty"/>
        <rdfs:domain rdf:resource="http://semanticbible.org/ns/2006/NTNames#Human"/>
        <rdfs:range rdf:resource="http://semanticbible.org/ns/2006/NTNames#Human"/>
        <rdfs:comment xml:lang="en">A person who is related by kinship to this person. No attempt is made to delineate precisely which kinship relations qualify: this is used when a description indicates two people are &quot;related&quot;. parent/child/siblingOf are subproperties of this, properly speaking. </rdfs:comment>
        <rdfs:label xml:lang="en">relative of</rdfs:label>
    </owl:ObjectProperty>
    


    <!-- http://semanticbible.org/ns/2006/NTNames#religiousBelief -->

    <owl:ObjectProperty rdf:about="http://semanticbible.org/ns/2006/NTNames#religiousBelief">
        <owl:inverseOf rdf:resource="http://semanticbible.org/ns/2006/NTNames#religiousBeliefOf"/>
        <rdfs:domain>
            <owl:Class>
                <owl:unionOf rdf:parseType="Collection">
                    <rdf:Description rdf:about="http://semanticbible.org/ns/2006/NTNames#GroupOfPeople"/>
                    <rdf:Description rdf:about="http://semanticbible.org/ns/2006/NTNames#Human"/>
                </owl:unionOf>
            </owl:Class>
        </rdfs:domain>
        <rdfs:range rdf:resource="http://semanticbible.org/ns/2006/NTNames#ReligiousBeliefSystem"/>
        <rdfs:comment xml:lang="en">Having a ReligiousBelief as an attribute</rdfs:comment>
        <rdfs:label xml:lang="en">religious belief</rdfs:label>
    </owl:ObjectProperty>
    


    <!-- http://semanticbible.org/ns/2006/NTNames#religiousBeliefOf -->

    <owl:ObjectProperty rdf:about="http://semanticbible.org/ns/2006/NTNames#religiousBeliefOf">
        <rdfs:domain rdf:resource="http://semanticbible.org/ns/2006/NTNames#ReligiousBeliefSystem"/>
        <rdfs:range>
            <owl:Class>
                <owl:unionOf rdf:parseType="Collection">
                    <rdf:Description rdf:about="http://semanticbible.org/ns/2006/NTNames#GroupOfPeople"/>
                    <rdf:Description rdf:about="http://semanticbible.org/ns/2006/NTNames#Human"/>
                </owl:unionOf>
            </owl:Class>
        </rdfs:range>
        <rdfs:label xml:lang="en">religious belief of</rdfs:label>
    </owl:ObjectProperty>
    


    <!-- http://semanticbible.org/ns/2006/NTNames#residentPlace -->

    <owl:ObjectProperty rdf:about="http://semanticbible.org/ns/2006/NTNames#residentPlace">
        <rdfs:subPropertyOf rdf:resource="http://semanticbible.org/ns/2006/NTNames#visitedPlace"/>
        <owl:inverseOf rdf:resource="http://semanticbible.org/ns/2006/NTNames#residentPlaceOf"/>
        <rdfs:domain>
            <owl:Class>
                <owl:unionOf rdf:parseType="Collection">
                    <rdf:Description rdf:about="http://semanticbible.org/ns/2006/NTNames#GroupOfPeople"/>
                    <rdf:Description rdf:about="http://semanticbible.org/ns/2006/NTNames#Human"/>
                </owl:unionOf>
            </owl:Class>
        </rdfs:domain>
        <rdfs:range rdf:resource="http://semanticbible.org/ns/2006/NTNames#Region"/>
        <rdfs:comment xml:lang="en">The location a person or group of people resides in. Range values may change over time: no attempt is made to capture this. Transient residence of very short duration is assumed to be visited, not resident. People addressed in a letter bound for a specific destination (e.g. the epistle of Paul to the Romans) are assumed to be resident there unless there is indication to the contrary (since the timing of a letter&apos;s arrival could not be determined with high precision). </rdfs:comment>
        <rdfs:label xml:lang="en">resident place</rdfs:label>
    </owl:ObjectProperty>
    


    <!-- http://semanticbible.org/ns/2006/NTNames#residentPlaceOf -->

    <owl:ObjectProperty rdf:about="http://semanticbible.org/ns/2006/NTNames#residentPlaceOf">
        <rdfs:subPropertyOf rdf:resource="http://semanticbible.org/ns/2006/NTNames#visitedPlaceOf"/>
        <rdfs:domain rdf:resource="http://semanticbible.org/ns/2006/NTNames#Region"/>
        <rdfs:range>
            <owl:Class>
                <owl:unionOf rdf:parseType="Collection">
                    <rdf:Description rdf:about="http://semanticbible.org/ns/2006/NTNames#GroupOfPeople"/>
                    <rdf:Description rdf:about="http://semanticbible.org/ns/2006/NTNames#Human"/>
                </owl:unionOf>
            </owl:Class>
        </rdfs:range>
    </owl:ObjectProperty>
    


    <!-- http://semanticbible.org/ns/2006/NTNames#siblingOf -->

    <owl:ObjectProperty rdf:about="http://semanticbible.org/ns/2006/NTNames#siblingOf">
        <rdfs:subPropertyOf rdf:resource="http://semanticbible.org/ns/2006/NTNames#relativeOf"/>
        <owl:inverseOf rdf:resource="http://semanticbible.org/ns/2006/NTNames#siblingOf"/>
        <rdf:type rdf:resource="http://www.w3.org/2002/07/owl#SymmetricProperty"/>
        <rdf:type rdf:resource="http://www.w3.org/2002/07/owl#TransitiveProperty"/>
        <rdfs:domain rdf:resource="http://semanticbible.org/ns/2006/NTNames#Human"/>
        <rdfs:range rdf:resource="http://semanticbible.org/ns/2006/NTNames#Human"/>
        <rdfs:comment xml:lang="en">Similar to http://purl.org/vocab/relationship vocabulary, but with different domain and range.</rdfs:comment>
        <rdfs:label xml:lang="en">sibling of</rdfs:label>
    </owl:ObjectProperty>
    


    <!-- http://semanticbible.org/ns/2006/NTNames#spouseOf -->

    <owl:ObjectProperty rdf:about="http://semanticbible.org/ns/2006/NTNames#spouseOf">
        <owl:inverseOf rdf:resource="http://semanticbible.org/ns/2006/NTNames#spouseOf"/>
        <rdf:type rdf:resource="http://www.w3.org/2002/07/owl#SymmetricProperty"/>
        <rdfs:domain rdf:resource="http://semanticbible.org/ns/2006/NTNames#Human"/>
        <rdfs:range rdf:resource="http://semanticbible.org/ns/2006/NTNames#Human"/>
        <rdfs:comment xml:lang="en">Similar to http://purl.org/vocab/relationship vocabulary, but with different domain and range. Multiple spouses are all included, whether sequential (Herodias) or simultaneous (the woman at the well). </rdfs:comment>
        <rdfs:label xml:lang="en">spouse of</rdfs:label>
    </owl:ObjectProperty>
    


    <!-- http://semanticbible.org/ns/2006/NTNames#subregion -->

    <owl:ObjectProperty rdf:about="http://semanticbible.org/ns/2006/NTNames#subregion">
        <owl:inverseOf rdf:resource="http://semanticbible.org/ns/2006/NTNames#subregionOf"/>
        <rdf:type rdf:resource="http://www.w3.org/2002/07/owl#TransitiveProperty"/>
        <rdfs:domain rdf:resource="http://semanticbible.org/ns/2006/NTNames#GeographicArea"/>
        <rdfs:range rdf:resource="http://semanticbible.org/ns/2006/NTNames#GeographicArea"/>
        <rdfs:comment xml:lang="en">Inverse of subregionOf</rdfs:comment>
        <rdfs:label xml:lang="en">subregion</rdfs:label>
    </owl:ObjectProperty>
    


    <!-- http://semanticbible.org/ns/2006/NTNames#subregionOf -->

    <owl:ObjectProperty rdf:about="http://semanticbible.org/ns/2006/NTNames#subregionOf">
        <rdf:type rdf:resource="http://www.w3.org/2002/07/owl#TransitiveProperty"/>
        <rdfs:domain rdf:resource="http://semanticbible.org/ns/2006/NTNames#GeographicArea"/>
        <rdfs:range rdf:resource="http://semanticbible.org/ns/2006/NTNames#GeographicArea"/>
        <rdfs:comment xml:lang="en">A smaller GeographicArea is a subregionOf a larger one (e.g. Jerusalem is a subregionOf Israel).</rdfs:comment>
        <rdfs:label xml:lang="en">subregion of</rdfs:label>
    </owl:ObjectProperty>
    


    <!-- http://semanticbible.org/ns/2006/NTNames#visitedPlace -->

    <owl:ObjectProperty rdf:about="http://semanticbible.org/ns/2006/NTNames#visitedPlace">
        <owl:inverseOf rdf:resource="http://semanticbible.org/ns/2006/NTNames#visitedPlaceOf"/>
        <rdfs:domain>
            <owl:Class>
                <owl:unionOf rdf:parseType="Collection">
                    <rdf:Description rdf:about="http://semanticbible.org/ns/2006/NTNames#GroupOfPeople"/>
                    <rdf:Description rdf:about="http://semanticbible.org/ns/2006/NTNames#Human"/>
                </owl:unionOf>
            </owl:Class>
        </rdfs:domain>
        <rdfs:range rdf:resource="http://semanticbible.org/ns/2006/NTNames#Region"/>
        <rdfs:comment xml:lang="en">Places that a human visited. For current purposes, only instances which are explicitly mentioned in Scripture are included, not those that might be inferred (e.g. if going from from A to B implies visiting C, C would not be listed). </rdfs:comment>
        <rdfs:label xml:lang="en">visited place</rdfs:label>
    </owl:ObjectProperty>
    


    <!-- http://semanticbible.org/ns/2006/NTNames#visitedPlaceOf -->

    <owl:ObjectProperty rdf:about="http://semanticbible.org/ns/2006/NTNames#visitedPlaceOf">
        <rdfs:domain rdf:resource="http://semanticbible.org/ns/2006/NTNames#Region"/>
        <rdfs:range>
            <owl:Class>
                <owl:unionOf rdf:parseType="Collection">
                    <rdf:Description rdf:about="http://semanticbible.org/ns/2006/NTNames#GroupOfPeople"/>
                    <rdf:Description rdf:about="http://semanticbible.org/ns/2006/NTNames#Human"/>
                </owl:unionOf>
            </owl:Class>
        </rdfs:range>
    </owl:ObjectProperty>
    


    <!-- 
    ///////////////////////////////////////////////////////////////////////////////////////
    //
    // Data properties
    //
    ///////////////////////////////////////////////////////////////////////////////////////
     -->

    


    <!-- http://semanticbible.org/ns/2006/NTNames#LNID -->

    <owl:DatatypeProperty rdf:about="http://semanticbible.org/ns/2006/NTNames#LNID">
        <rdf:type rdf:resource="http://www.w3.org/2002/07/owl#FunctionalProperty"/>
        <rdfs:range rdf:resource="http://www.w3.org/2001/XMLSchema#string"/>
        <rdfs:comment xml:lang="en">Louw-Nida identifier, keying specific Greek terms (and their English translations) to their taxonomy of semantic domains. A string like &quot;33.X&apos;.439&quot; identifies the term sumballo, which can be translated as &quot;to express differences of opinion in a forceful way&quot;. In their scheme, this has domain index 33 (Communication), with sub-domain index X&apos; (Dispute, Debate). The final integer index uniquely defines this term (but the same term may have multiple senses). The sub-domain index can be determined from the term index, but it seems helpful to include both. Note the possible values of the sub-domain index are A-Z, then A&apos;-Z&apos;, etc.</rdfs:comment>
        <rdfs:label xml:lang="en">Louw-Nida identifier</rdfs:label>
    </owl:DatatypeProperty>
    


    <!-- http://semanticbible.org/ns/2006/NTNames#altitude -->

    <owl:DatatypeProperty rdf:about="http://semanticbible.org/ns/2006/NTNames#altitude">
        <rdfs:domain rdf:resource="http://semanticbible.org/ns/2006/NTNames#GeographicLocation"/>
        <rdfs:range rdf:resource="http://www.w3.org/2001/XMLSchema#int"/>
        <rdfs:comment xml:lang="en">The altitude component of a GeographicLocation</rdfs:comment>
        <rdfs:label xml:lang="en">altitude</rdfs:label>
    </owl:DatatypeProperty>
    


    <!-- http://semanticbible.org/ns/2006/NTNames#description -->

    <owl:DatatypeProperty rdf:about="http://semanticbible.org/ns/2006/NTNames#description">
        <rdfs:domain rdf:resource="http://semanticbible.org/ns/2006/NTNames#Human"/>
        <rdfs:range rdf:resource="http://www.w3.org/2001/XMLSchema#string"/>
        <rdfs:comment xml:lang="en">A brief description of the salient aspects of a Human, based on their being mentioned in Scripture. This is not the way to enter dictionary-style definitions.</rdfs:comment>
        <rdfs:label xml:lang="en">description</rdfs:label>
    </owl:DatatypeProperty>
    


    <!-- http://semanticbible.org/ns/2006/NTNames#hasOnlyGenealogyMention -->

    <owl:DatatypeProperty rdf:about="http://semanticbible.org/ns/2006/NTNames#hasOnlyGenealogyMention">
        <rdf:type rdf:resource="http://www.w3.org/2002/07/owl#FunctionalProperty"/>
        <rdfs:domain rdf:resource="http://semanticbible.org/ns/2006/NTNames#Human"/>
        <rdfs:range rdf:resource="http://www.w3.org/2001/XMLSchema#boolean"/>
        <rdfs:comment xml:lang="en">The only mention of this person in the New Testament text is the genealogies of Jesus recorded in Matthew 1 and/or Luke 3. Since only limited information (their ancestry) is available about this special subset of names, this property exists to support filtering them out (or in). </rdfs:comment>
        <rdfs:label xml:lang="en">has only genealogy mention</rdfs:label>
    </owl:DatatypeProperty>
    


    <!-- http://semanticbible.org/ns/2006/NTNames#latitude -->

    <owl:DatatypeProperty rdf:about="http://semanticbible.org/ns/2006/NTNames#latitude">
        <rdfs:domain rdf:resource="http://semanticbible.org/ns/2006/NTNames#GeographicLocation"/>
        <rdfs:range rdf:resource="http://www.w3.org/2001/XMLSchema#double"/>
        <rdfs:comment xml:lang="en">The latitude component of a GeographicLocation</rdfs:comment>
        <rdfs:label xml:lang="en">latitude</rdfs:label>
    </owl:DatatypeProperty>
    


    <!-- http://semanticbible.org/ns/2006/NTNames#longitude -->

    <owl:DatatypeProperty rdf:about="http://semanticbible.org/ns/2006/NTNames#longitude">
        <rdfs:domain rdf:resource="http://semanticbible.org/ns/2006/NTNames#GeographicLocation"/>
        <rdfs:range rdf:resource="http://www.w3.org/2001/XMLSchema#double"/>
        <rdfs:comment xml:lang="en">The longiitude component of a GeographicLocation</rdfs:comment>
        <rdfs:label xml:lang="en">longitude</rdfs:label>
    </owl:DatatypeProperty>
    


    <!-- http://semanticbible.org/ns/2006/NTNames#name_en -->

    <owl:DatatypeProperty rdf:about="http://semanticbible.org/ns/2006/NTNames#name_en">
        <rdfs:domain>
            <owl:Class>
                <owl:unionOf rdf:parseType="Collection">
                    <rdf:Description rdf:about="http://semanticbible.org/ns/2006/NTNames#BeliefSystem"/>
                    <rdf:Description rdf:about="http://semanticbible.org/ns/2006/NTNames#FixedHoliday"/>
                    <rdf:Description rdf:about="http://semanticbible.org/ns/2006/NTNames#HumanAttribute"/>
                    <rdf:Description rdf:about="http://semanticbible.org/ns/2006/NTNames#Object"/>
                </owl:unionOf>
            </owl:Class>
        </rdfs:domain>
        <rdfs:range rdf:resource="http://www.w3.org/2001/XMLSchema#string"/>
        <rdfs:comment xml:lang="en">The human language name of an Object in English. 
Since Protege (3.0 build 141) doesn&apos;t seem to support loading and saving xml:lang attributes on properties, different subproperties are used for representing names in different languages.</rdfs:comment>
        <rdfs:label xml:lang="en">English name</rdfs:label>
    </owl:DatatypeProperty>
    


    <!-- http://semanticbible.org/ns/2006/NTNames#name_grc -->

    <owl:DatatypeProperty rdf:about="http://semanticbible.org/ns/2006/NTNames#name_grc">
        <rdfs:domain>
            <owl:Class>
                <owl:unionOf rdf:parseType="Collection">
                    <rdf:Description rdf:about="http://semanticbible.org/ns/2006/NTNames#BeliefSystem"/>
                    <rdf:Description rdf:about="http://semanticbible.org/ns/2006/NTNames#FixedHoliday"/>
                    <rdf:Description rdf:about="http://semanticbible.org/ns/2006/NTNames#HumanAttribute"/>
                    <rdf:Description rdf:about="http://semanticbible.org/ns/2006/NTNames#Object"/>
                </owl:unionOf>
            </owl:Class>
        </rdfs:domain>
        <rdfs:range rdf:resource="http://www.w3.org/2001/XMLSchema#string"/>
        <rdfs:comment xml:lang="en">The human language name of an Object in Koine (not Modern) Greek, in the standard dictionary form (nominative case). 
 Since Protege (3.0 build 141) doesn&apos;t seem to support loading and saving xml:lang attributes on properties, different subproperties are used for representing names in different languages. &quot;grc&quot; is the three-letter ISO-639-2 standard designator for Koine Greek.</rdfs:comment>
        <rdfs:label xml:lang="en">Greek name</rdfs:label>
    </owl:DatatypeProperty>
    


    <!-- http://semanticbible.org/ns/2006/NTNames#occupation -->

    <owl:DatatypeProperty rdf:about="http://semanticbible.org/ns/2006/NTNames#occupation">
        <rdfs:domain rdf:resource="http://semanticbible.org/ns/2006/NTNames#Human"/>
        <rdfs:range rdf:resource="http://www.w3.org/2001/XMLSchema#string"/>
        <rdfs:label xml:lang="en">occupation</rdfs:label>
    </owl:DatatypeProperty>
    


    <!-- 
    ///////////////////////////////////////////////////////////////////////////////////////
    //
    // Classes
    //
    ///////////////////////////////////////////////////////////////////////////////////////
     -->

    


    <!-- http://semanticbible.org/ns/2006/NTNames#Agent -->

    <owl:Class rdf:about="http://semanticbible.org/ns/2006/NTNames#Agent">
        <rdfs:subClassOf rdf:resource="http://semanticbible.org/ns/2006/NTNames#Object"/>
        <rdfs:comment xml:lang="en">Comparable to http://reliant.teknowledge.com/DAML/SUMO.owl#Agent
SUO 1.55: July 14, 2003
Something or someone that can act on its own and 
produce changes in the world.</rdfs:comment>
        <rdfs:label xml:lang="en">Agent</rdfs:label>
    </owl:Class>
    


    <!-- http://semanticbible.org/ns/2006/NTNames#Angel -->

    <owl:Class rdf:about="http://semanticbible.org/ns/2006/NTNames#Angel">
        <rdfs:subClassOf rdf:resource="http://semanticbible.org/ns/2006/NTNames#SupernaturalBeing"/>
        <owl:disjointWith rdf:resource="http://semanticbible.org/ns/2006/NTNames#God"/>
        <rdfs:comment xml:lang="en">Supernatural beings that work to support God&apos;s purposes as his agents.</rdfs:comment>
        <rdfs:label xml:lang="en">Angel</rdfs:label>
    </owl:Class>
    


    <!-- http://semanticbible.org/ns/2006/NTNames#BeliefGroup -->

    <owl:Class rdf:about="http://semanticbible.org/ns/2006/NTNames#BeliefGroup">
        <rdfs:subClassOf rdf:resource="http://semanticbible.org/ns/2006/NTNames#GroupOfPeople"/>
        <rdfs:comment xml:lang="en">Comparable to http://reliant.teknowledge.com/DAML/SUMO.owl#BeliefGroup
SUO 1.55: July 14, 2003
A &amp;%Group whose &amp;%members share a belief or
set of beliefs.
For NTN, this covers groups defined by a particular set of beliefs (orthodox or heretical) which are informal, rather than formal, in membership and activity.</rdfs:comment>
        <rdfs:label xml:lang="en">Belief Group</rdfs:label>
    </owl:Class>
    


    <!-- http://semanticbible.org/ns/2006/NTNames#BeliefSystem -->

    <owl:Class rdf:about="http://semanticbible.org/ns/2006/NTNames#BeliefSystem">
        <rdfs:comment xml:lang="en">An organization of propositions into an identifiable belief system. A person who holds to a belief system can be considered a member of the corresponding BeliefGroup.

The notion of Proposition here is derived from http://reliant.teknowledge.com/DAML/SUMO.owl#Proposition.</rdfs:comment>
        <rdfs:label xml:lang="en">Belief system</rdfs:label>
    </owl:Class>
    


    <!-- http://semanticbible.org/ns/2006/NTNames#Character -->

    <owl:Class rdf:about="http://semanticbible.org/ns/2006/NTNames#Character">
        <rdfs:subClassOf rdf:resource="http://semanticbible.org/ns/2006/NTNames#ContentBearingObject"/>
        <rdfs:comment xml:lang="en">Broadly the same as http://reliant.teknowledge.com/DAML/SUMO.owl#Character
SUO 1.55: July 14, 2003
An element of an alphabet, a set of numerals, etc.
Note that a &amp;%Character may or may not be part of a &amp;%Language.  &amp;%Character
is a subclass of &amp;%SymbolicString, because every instance of &amp;%Character is
an alphanumeric sequence consisting of a single element.</rdfs:comment>
        <rdfs:label xml:lang="en">Character</rdfs:label>
    </owl:Class>
    


    <!-- http://semanticbible.org/ns/2006/NTNames#CitizenshipAttribute -->

    <owl:Class rdf:about="http://semanticbible.org/ns/2006/NTNames#CitizenshipAttribute">
        <rdfs:subClassOf rdf:resource="http://semanticbible.org/ns/2006/NTNames#HumanAttribute"/>
        <rdfs:comment xml:lang="en">Belonging to the citizenry of a country (e.g. Roman). There may be parallel ethnicity attributes (Roman being the primary example) which are not easily distinguished. In the case of Roman, while all ethnic Romans (in the general sense, though not necessarily legal sense [e.g. slaves]) are Roman citizens, there are other Roman citizens (e.g. Paul) who have different ethnicity. </rdfs:comment>
        <rdfs:label rdf:datatype="http://www.w3.org/2001/XMLSchema#string">Citizenship attribute</rdfs:label>
    </owl:Class>
    


    <!-- http://semanticbible.org/ns/2006/NTNames#City -->

    <owl:Class rdf:about="http://semanticbible.org/ns/2006/NTNames#City">
        <rdfs:subClassOf rdf:resource="http://semanticbible.org/ns/2006/NTNames#GeopoliticalArea"/>
        <rdfs:subClassOf rdf:resource="http://semanticbible.org/ns/2006/NTNames#LandArea"/>
        <rdfs:comment xml:lang="en">Based on SUMO, http://reliant.teknowledge.com/DAML/SUMO.owl#City
SUO 1.55: July 14, 2003
A &amp;%LandArea of relatively small size, inhabited
by a community of people, and having some sort of political structure.
Note that this class includes both large cities and small settlements
like towns, villages, hamlets, etc.</rdfs:comment>
        <rdfs:label xml:lang="en">City</rdfs:label>
    </owl:Class>
    


    <!-- http://semanticbible.org/ns/2006/NTNames#CognitiveAgent -->

    <owl:Class rdf:about="http://semanticbible.org/ns/2006/NTNames#CognitiveAgent">
        <rdfs:subClassOf rdf:resource="http://semanticbible.org/ns/2006/NTNames#Agent"/>
        <rdfs:comment xml:lang="en">Comparable to http://reliant.teknowledge.com/DAML/SUMO.owl#CognitiveAgent
SUO 1.55: July 14, 2003
A &amp;%SentientAgent with responsibilities 
and the ability to reason, deliberate, make plans, etc.  This is 
essentially the legal/ethical notion of a person.  Note that, although 
&amp;%Human is a subclass of &amp;%CognitiveAgent, there may be instances of 
&amp;%CognitiveAgent which are not also instances of &amp;%Human.  For example, 
chimpanzees, gorillas, dolphins, whales, and some extraterrestrials 
(if they exist) may be &amp;%CognitiveAgents.</rdfs:comment>
        <rdfs:label xml:lang="en">Cognitive Agent</rdfs:label>
    </owl:Class>
    


    <!-- http://semanticbible.org/ns/2006/NTNames#ContentBearingObject -->

    <owl:Class rdf:about="http://semanticbible.org/ns/2006/NTNames#ContentBearingObject">
        <rdfs:subClassOf rdf:resource="http://semanticbible.org/ns/2006/NTNames#Object"/>
        <rdfs:comment xml:lang="en">Broadly the same as http://reliant.teknowledge.com/DAML/SUMO.owl#ContentBearingObject
SUO 1.55: July 14, 2003
Any &amp;%SelfConnectedObject that expresses 
information.</rdfs:comment>
        <rdfs:label xml:lang="en">Content Bearing Object</rdfs:label>
    </owl:Class>
    


    <!-- http://semanticbible.org/ns/2006/NTNames#EthnicGroup -->

    <owl:Class rdf:about="http://semanticbible.org/ns/2006/NTNames#EthnicGroup">
        <rdfs:subClassOf rdf:resource="http://semanticbible.org/ns/2006/NTNames#GroupOfPeople"/>
        <rdfs:comment xml:lang="en">Comparable to http://reliant.teknowledge.com/DAML/SUMO.owl#EthnicGroup
SUO 1.55: July 14, 2003
A &amp;%Group whose &amp;%members originate from
the same &amp;%GeographicArea or share the same &amp;%Language and/or cultural
practices.</rdfs:comment>
        <rdfs:label xml:lang="en">Ethnic Group</rdfs:label>
    </owl:Class>
    


    <!-- http://semanticbible.org/ns/2006/NTNames#EthnicityAttribute -->

    <owl:Class rdf:about="http://semanticbible.org/ns/2006/NTNames#EthnicityAttribute">
        <rdfs:subClassOf rdf:resource="http://semanticbible.org/ns/2006/NTNames#HumanAttribute"/>
        <rdfs:comment xml:lang="en">The attribute of belonging to a particular ethnic group, or originating from a GeographicArea. Unlike Residency, which can change, Ethnicity is considered permanent.</rdfs:comment>
        <rdfs:label xml:lang="en">Ethnicity attribute</rdfs:label>
    </owl:Class>
    


    <!-- http://semanticbible.org/ns/2006/NTNames#EvilSupernaturalBeing -->

    <owl:Class rdf:about="http://semanticbible.org/ns/2006/NTNames#EvilSupernaturalBeing">
        <rdfs:subClassOf rdf:resource="http://semanticbible.org/ns/2006/NTNames#SupernaturalBeing"/>
        <owl:disjointWith rdf:resource="http://semanticbible.org/ns/2006/NTNames#God"/>
        <rdfs:comment xml:lang="en">Class of malevolent supernatural beings, whose instances include Satan and demons. </rdfs:comment>
        <rdfs:label xml:lang="en">Evil Supernatural Being</rdfs:label>
    </owl:Class>
    


    <!-- http://semanticbible.org/ns/2006/NTNames#FixedHoliday -->

    <owl:Class rdf:about="http://semanticbible.org/ns/2006/NTNames#FixedHoliday">
        <rdfs:comment xml:lang="en">Would be a subclass of http://reliant.teknowledge.com/DAML/SUMO.owl#TimeInterval, but is specified within MILO.
MILO: &amp;%FixedHoliday is the class of &amp;%Holidays 
whose observance is fixed to recurrences of the calendar day that the 
holiday commemorates.</rdfs:comment>
        <rdfs:label xml:lang="en">Fixed holiday</rdfs:label>
    </owl:Class>
    


    <!-- http://semanticbible.org/ns/2006/NTNames#FreshWaterArea -->

    <owl:Class rdf:about="http://semanticbible.org/ns/2006/NTNames#FreshWaterArea">
        <rdfs:subClassOf rdf:resource="http://semanticbible.org/ns/2006/NTNames#WaterArea"/>
        <owl:disjointWith rdf:resource="http://semanticbible.org/ns/2006/NTNames#SaltWaterArea"/>
        <rdfs:comment xml:lang="en">Based on SUMO, http://reliant.teknowledge.com/DAML/SUMO.owl#FreshWaterArea

SUO 1.55: July 14, 2003
A &amp;%WaterArea whose &amp;%Water is not saline,
e.g. most rivers and lakes.</rdfs:comment>
        <rdfs:label xml:lang="en">Fresh Water Area</rdfs:label>
    </owl:Class>
    


    <!-- http://semanticbible.org/ns/2006/NTNames#GeographicArea -->

    <owl:Class rdf:about="http://semanticbible.org/ns/2006/NTNames#GeographicArea">
        <rdfs:subClassOf rdf:resource="http://semanticbible.org/ns/2006/NTNames#Region"/>
        <rdfs:comment xml:lang="en">Based on SUMO, http://reliant.teknowledge.com/DAML/SUMO.owl#GeographicArea
SUO 1.55: July 14, 2003
A geographic location, generally having 
definite boundaries.  Note that this differs from its immediate superclass 
&amp;%Region in that a &amp;%GeographicArea is a three-dimensional &amp;%Region of the 
earth.  Accordingly, all astronomical objects other than earth and all 
one-dimensional and two-dimensional &amp;%Regions are not classed under 
&amp;%GeographicArea.</rdfs:comment>
        <rdfs:label xml:lang="en">Geographic Area</rdfs:label>
    </owl:Class>
    


    <!-- http://semanticbible.org/ns/2006/NTNames#GeographicLocation -->

    <owl:Class rdf:about="http://semanticbible.org/ns/2006/NTNames#GeographicLocation">
        <rdfs:comment rdf:datatype="http://www.w3.org/2001/XMLSchema#string">A collection of properties describing geographic location. </rdfs:comment>
        <rdfs:label xml:lang="en">Geographic Location</rdfs:label>
    </owl:Class>
    


    <!-- http://semanticbible.org/ns/2006/NTNames#GeopoliticalArea -->

    <owl:Class rdf:about="http://semanticbible.org/ns/2006/NTNames#GeopoliticalArea">
        <rdfs:subClassOf rdf:resource="http://semanticbible.org/ns/2006/NTNames#GeographicArea"/>
        <rdfs:comment xml:lang="en">Based on SUMO, http://reliant.teknowledge.com/DAML/SUMO.owl#GeopoliticalArea
SUO 1.55: July 14, 2003
Any &amp;%GeographicArea which is associated 
with some sort of political structure.  This class includes &amp;%Lands, 
&amp;%Cities, districts of cities, counties, etc.  Note that the identity 
of a &amp;%GeopoliticalArea may remain constant after a change in borders.</rdfs:comment>
        <rdfs:label xml:lang="en">Geopolitical Area</rdfs:label>
    </owl:Class>
    


    <!-- http://semanticbible.org/ns/2006/NTNames#God -->

    <owl:Class rdf:about="http://semanticbible.org/ns/2006/NTNames#God">
        <rdfs:subClassOf rdf:resource="http://semanticbible.org/ns/2006/NTNames#SupernaturalBeing"/>
        <rdfs:comment xml:lang="en">Self-documenting</rdfs:comment>
        <rdfs:label xml:lang="en">God</rdfs:label>
    </owl:Class>
    


    <!-- http://semanticbible.org/ns/2006/NTNames#Group -->

    <owl:Class rdf:about="http://semanticbible.org/ns/2006/NTNames#Group">
        <rdfs:subClassOf rdf:resource="http://semanticbible.org/ns/2006/NTNames#Agent"/>
        <rdfs:comment xml:lang="en">Comparable to http://reliant.teknowledge.com/DAML/SUMO.owl#Group
SUO 1.55: July 14, 2003
A &amp;%Collection of &amp;%Agents, e.g. a flock
of sheep, a herd of goats, or the local Boy Scout troop.</rdfs:comment>
        <rdfs:label xml:lang="en">Group</rdfs:label>
    </owl:Class>
    


    <!-- http://semanticbible.org/ns/2006/NTNames#GroupOfPeople -->

    <owl:Class rdf:about="http://semanticbible.org/ns/2006/NTNames#GroupOfPeople">
        <rdfs:subClassOf rdf:resource="http://semanticbible.org/ns/2006/NTNames#Group"/>
        <rdfs:comment xml:lang="en">Comparable to http://reliant.teknowledge.com/DAML/SUMO.owl#GroupOfPeople
SUO 1.55: July 14, 2003
Any &amp;%Group whose &amp;%members are
exclusively &amp;%Humans.</rdfs:comment>
        <rdfs:label xml:lang="en">Group of People</rdfs:label>
    </owl:Class>
    


    <!-- http://semanticbible.org/ns/2006/NTNames#Human -->

    <owl:Class rdf:about="http://semanticbible.org/ns/2006/NTNames#Human">
        <rdfs:subClassOf rdf:resource="http://semanticbible.org/ns/2006/NTNames#CognitiveAgent"/>
        <rdfs:comment xml:lang="en">Comparable to http://reliant.teknowledge.com/DAML/SUMO.owl#Human
SUO 1.55: July 14, 2003
Modern man, the only remaining species of the Homo genus.</rdfs:comment>
        <rdfs:label xml:lang="en">Human</rdfs:label>
    </owl:Class>
    


    <!-- http://semanticbible.org/ns/2006/NTNames#HumanAttribute -->

    <owl:Class rdf:about="http://semanticbible.org/ns/2006/NTNames#HumanAttribute">
        <rdfs:comment xml:lang="en">Attributes of people, overlapping with the class hierarchy under suo:Group: this is unsatisfactory.</rdfs:comment>
        <rdfs:label xml:lang="en">Human attribute</rdfs:label>
    </owl:Class>
    


    <!-- http://semanticbible.org/ns/2006/NTNames#Island -->

    <owl:Class rdf:about="http://semanticbible.org/ns/2006/NTNames#Island">
        <rdfs:subClassOf rdf:resource="http://semanticbible.org/ns/2006/NTNames#LandArea"/>
        <rdfs:comment xml:lang="en">Based on SUMO, http://reliant.teknowledge.com/DAML/SUMO.owl#Island
SUO 1.55: July 14, 2003
A &amp;%LandArea that is completely surrounded by a &amp;%WaterArea.</rdfs:comment>
        <rdfs:label xml:lang="en">Island</rdfs:label>
    </owl:Class>
    


    <!-- http://semanticbible.org/ns/2006/NTNames#LandArea -->

    <owl:Class rdf:about="http://semanticbible.org/ns/2006/NTNames#LandArea">
        <rdfs:subClassOf rdf:resource="http://semanticbible.org/ns/2006/NTNames#GeographicArea"/>
        <owl:disjointWith rdf:resource="http://semanticbible.org/ns/2006/NTNames#WaterArea"/>
        <rdfs:comment xml:lang="en">Based on SUMO, http://reliant.teknowledge.com/DAML/SUMO.owl#LandArea
SUO 1.55: July 14, 2003
An area which is predominantly solid ground,
e.g. a &amp;%Nation, a mountain, a desert, etc.  Note that a &amp;%LandArea may
contain some relatively small &amp;%WaterAreas.  For example, Australia is
a &amp;%LandArea even though it contains various rivers and lakes.</rdfs:comment>
        <rdfs:label xml:lang="en">Land Area</rdfs:label>
    </owl:Class>
    


    <!-- http://semanticbible.org/ns/2006/NTNames#Man -->

    <owl:Class rdf:about="http://semanticbible.org/ns/2006/NTNames#Man">
        <rdfs:subClassOf rdf:resource="http://semanticbible.org/ns/2006/NTNames#Human"/>
        <rdfs:subClassOf>
            <owl:Restriction>
                <owl:onProperty rdf:resource="http://semanticbible.org/ns/2006/NTNames#spouseOf"/>
                <owl:allValuesFrom rdf:resource="http://semanticbible.org/ns/2006/NTNames#Woman"/>
            </owl:Restriction>
        </rdfs:subClassOf>
        <owl:disjointWith rdf:resource="http://semanticbible.org/ns/2006/NTNames#Woman"/>
        <rdfs:comment xml:lang="en">SUO 1.55: July 14, 2003
The class of &amp;%Male &amp;%Humans.</rdfs:comment>
        <rdfs:label xml:lang="en">Man</rdfs:label>
    </owl:Class>
    


    <!-- http://semanticbible.org/ns/2006/NTNames#Mountain -->

    <owl:Class rdf:about="http://semanticbible.org/ns/2006/NTNames#Mountain">
        <rdfs:subClassOf rdf:resource="http://semanticbible.org/ns/2006/NTNames#LandArea"/>
        <rdfs:comment xml:lang="en">Wordnet: &quot;a land mass that projects well above its surroundings; higher than a hill. &quot;
Used here for things referred to as &quot;mount&quot;, even though some of these might seem
like hills to well-traveled observers. </rdfs:comment>
        <rdfs:label xml:lang="en">Mountain</rdfs:label>
    </owl:Class>
    


    <!-- http://semanticbible.org/ns/2006/NTNames#Nation -->

    <owl:Class rdf:about="http://semanticbible.org/ns/2006/NTNames#Nation">
        <rdfs:subClassOf rdf:resource="http://semanticbible.org/ns/2006/NTNames#GeopoliticalArea"/>
        <rdfs:subClassOf rdf:resource="http://semanticbible.org/ns/2006/NTNames#LandArea"/>
        <rdfs:comment xml:lang="en">Based on SUMO, http://reliant.teknowledge.com/DAML/SUMO.owl#Nation
SUO 1.55: July 14, 2003
The broadest &amp;%GeopoliticalArea, i.e. &amp;%Nations are
&amp;%GeopoliticalAreas that are not part of any other overarching and
comprehensive governance structure (excepting commonwealths and other sorts
of loose international organizations).
Note that modern nations referred to in the New Testament (Spain,
Italy, Libya) are typically not instances of Nation, but rather
of Region (if the borders are indefinite) or of LandArea.</rdfs:comment>
        <rdfs:label xml:lang="en">Nation</rdfs:label>
    </owl:Class>
    


    <!-- http://semanticbible.org/ns/2006/NTNames#NaturalLanguage -->

    <owl:Class rdf:about="http://semanticbible.org/ns/2006/NTNames#NaturalLanguage">
        <rdfs:subClassOf rdf:resource="http://semanticbible.org/ns/2006/NTNames#ContentBearingObject"/>
        <rdfs:comment xml:lang="en">Broadly the same as http://reliant.teknowledge.com/DAML/SUMO.owl#NaturalLanguage
SUO 1.55: July 14, 2003
The &amp;%subclass of &amp;%HumanLanguages which
are not designed and which evolve from generation to generation.  This
&amp;%Class includes all of the national languages, e.g. English, Spanish,
Japanese, etc.  Note that this class includes dialects of natural
languages.</rdfs:comment>
        <rdfs:label xml:lang="en">Natural Language</rdfs:label>
    </owl:Class>
    


    <!-- http://semanticbible.org/ns/2006/NTNames#Object -->

    <owl:Class rdf:about="http://semanticbible.org/ns/2006/NTNames#Object">
        <rdfs:comment xml:lang="en">Following http://reliant.teknowledge.com/DAML/SUMO.owl#Object, this &quot;Corresponds roughly to the class of ordinary 
objects.  Examples include normal physical objects, geographical regions, 
and locations of &amp;%Processes, the complement of &amp;%Objects in the &amp;%Physical class. &quot;</rdfs:comment>
        <rdfs:label xml:lang="en">Object</rdfs:label>
    </owl:Class>
    


    <!-- http://semanticbible.org/ns/2006/NTNames#Organization -->

    <owl:Class rdf:about="http://semanticbible.org/ns/2006/NTNames#Organization">
        <rdfs:subClassOf rdf:resource="http://semanticbible.org/ns/2006/NTNames#GroupOfPeople"/>
        <rdfs:comment xml:lang="en">Comparable to http://reliant.teknowledge.com/DAML/SUMO.owl#Organization
SUO 1.55: July 14, 2003
An &amp;%Organization is a corporate or similar institution. The &amp;%members of an &amp;%Organization typically have a common purpose or function. Note that this class also covers divisions, departments, etc. of organizations.  For example, both the Shell Corporation and the accounting department at Shell would both be instances of &amp;%Organization.  Note too that the existence of an &amp;%Organization is dependent on the existence of at least one &amp;%member (since &amp;%Organization is a subclass of &amp;%Collection).  Accordingly, in cases of purely legal organizations, a fictitious &amp;%member 
should be assumed.</rdfs:comment>
        <rdfs:label xml:lang="en">Organization</rdfs:label>
    </owl:Class>
    


    <!-- http://semanticbible.org/ns/2006/NTNames#PoliticalAttribute -->

    <owl:Class rdf:about="http://semanticbible.org/ns/2006/NTNames#PoliticalAttribute">
        <rdfs:subClassOf rdf:resource="http://semanticbible.org/ns/2006/NTNames#HumanAttribute"/>
        <rdfs:comment xml:lang="en">The attribute of ascribing to a PoliticalBeliefSystem, or belonging to a political party or system.</rdfs:comment>
        <rdfs:label xml:lang="en">Political attribute</rdfs:label>
    </owl:Class>
    


    <!-- http://semanticbible.org/ns/2006/NTNames#PoliticalBeliefSystem -->

    <owl:Class rdf:about="http://semanticbible.org/ns/2006/NTNames#PoliticalBeliefSystem">
        <rdfs:subClassOf rdf:resource="http://semanticbible.org/ns/2006/NTNames#BeliefSystem"/>
        <rdfs:label xml:lang="en">Political belief system</rdfs:label>
    </owl:Class>
    


    <!-- http://semanticbible.org/ns/2006/NTNames#PoliticalOrganization -->

    <owl:Class rdf:about="http://semanticbible.org/ns/2006/NTNames#PoliticalOrganization">
        <rdfs:subClassOf rdf:resource="http://semanticbible.org/ns/2006/NTNames#Organization"/>
        <rdfs:comment xml:lang="en">Comparable to http://reliant.teknowledge.com/DAML/SUMO.owl#PoliticalOrganization
SUO 1.55: July 14, 2003
An &amp;%Organization that is a &amp;%Government,
a &amp;%subOrganization of a &amp;%Government, or an &amp;%Organization that is attempting
to bring about some sort of political change.</rdfs:comment>
        <rdfs:label xml:lang="en">Political Organization</rdfs:label>
    </owl:Class>
    


    <!-- http://semanticbible.org/ns/2006/NTNames#Region -->

    <owl:Class rdf:about="http://semanticbible.org/ns/2006/NTNames#Region">
        <rdfs:subClassOf rdf:resource="http://semanticbible.org/ns/2006/NTNames#Object"/>
        <rdfs:comment xml:lang="en">Comparable to http://reliant.teknowledge.com/DAML/SUMO.owl#Region: &quot;A topographic location.  Regions encompass surfaces of Objects, imaginary places, and GeographicAreas. &quot;</rdfs:comment>
        <rdfs:label xml:lang="en">Region</rdfs:label>
    </owl:Class>
    


    <!-- http://semanticbible.org/ns/2006/NTNames#ReligiousBelief -->

    <owl:Class rdf:about="http://semanticbible.org/ns/2006/NTNames#ReligiousBelief">
        <rdfs:subClassOf rdf:resource="http://semanticbible.org/ns/2006/NTNames#HumanAttribute"/>
        <rdfs:comment xml:lang="en">The attribute of ascribing to a ReligiousBeliefSystem (which includes philosophies).</rdfs:comment>
        <rdfs:label xml:lang="en">Religious belief</rdfs:label>
    </owl:Class>
    


    <!-- http://semanticbible.org/ns/2006/NTNames#ReligiousBeliefSystem -->

    <owl:Class rdf:about="http://semanticbible.org/ns/2006/NTNames#ReligiousBeliefSystem">
        <rdfs:subClassOf rdf:resource="http://semanticbible.org/ns/2006/NTNames#BeliefSystem"/>
        <rdfs:comment xml:lang="en">A system of religious beliefs, or a philosophy.</rdfs:comment>
        <rdfs:label xml:lang="en">Religious belief system</rdfs:label>
    </owl:Class>
    


    <!-- http://semanticbible.org/ns/2006/NTNames#ReligiousOrganization -->

    <owl:Class rdf:about="http://semanticbible.org/ns/2006/NTNames#ReligiousOrganization">
        <rdfs:subClassOf rdf:resource="http://semanticbible.org/ns/2006/NTNames#BeliefGroup"/>
        <rdfs:subClassOf rdf:resource="http://semanticbible.org/ns/2006/NTNames#Organization"/>
        <rdfs:comment xml:lang="en">Comparable to http://reliant.teknowledge.com/DAML/SUMO.owl#ReligiousOrganization
SUO 1.55: July 14, 2003
An &amp;%Organization whose members
share a set of religious beliefs.</rdfs:comment>
        <rdfs:label xml:lang="en">Religious Organization</rdfs:label>
    </owl:Class>
    


    <!-- http://semanticbible.org/ns/2006/NTNames#ResidenceGroup -->

    <owl:Class rdf:about="http://semanticbible.org/ns/2006/NTNames#ResidenceGroup">
        <rdfs:subClassOf rdf:resource="http://semanticbible.org/ns/2006/NTNames#GroupOfPeople"/>
        <rdfs:comment xml:lang="en">A group identified by common residence in a City or StateOrProvince. At the level of Nation, this should generally be EthnicGroup. Unlike EthnicGroup, they need not have cultural or ethnic features in common.</rdfs:comment>
        <rdfs:label xml:lang="en">Residence Group</rdfs:label>
    </owl:Class>
    


    <!-- http://semanticbible.org/ns/2006/NTNames#ResidencyAttribute -->

    <owl:Class rdf:about="http://semanticbible.org/ns/2006/NTNames#ResidencyAttribute">
        <rdfs:subClassOf rdf:resource="http://semanticbible.org/ns/2006/NTNames#HumanAttribute"/>
        <rdfs:comment xml:lang="en">The attribute of living in a particular City or Province. Unlike Ethnicity, which is permanent, Residency can change.</rdfs:comment>
        <rdfs:label xml:lang="en">Residency attribute</rdfs:label>
    </owl:Class>
    


    <!-- http://semanticbible.org/ns/2006/NTNames#SaltWaterArea -->

    <owl:Class rdf:about="http://semanticbible.org/ns/2006/NTNames#SaltWaterArea">
        <rdfs:subClassOf rdf:resource="http://semanticbible.org/ns/2006/NTNames#WaterArea"/>
        <rdfs:comment xml:lang="en">Based on SUMO, http://reliant.teknowledge.com/DAML/SUMO.owl#SaltWaterArea
SUO 1.55: July 14, 2003
A &amp;%WaterArea whose &amp;%Water is saline, e.g.
oceans and seas.</rdfs:comment>
        <rdfs:label xml:lang="en">Salt Water Area</rdfs:label>
    </owl:Class>
    


    <!-- http://semanticbible.org/ns/2006/NTNames#Series -->

    <owl:Class rdf:about="http://semanticbible.org/ns/2006/NTNames#Series">
        <rdfs:subClassOf rdf:resource="http://semanticbible.org/ns/2006/NTNames#ContentBearingObject"/>
        <rdfs:comment xml:lang="en">Broadly the same as http://reliant.teknowledge.com/DAML/SUMO.owl#Series
SUO 1.55: July 14, 2003
A &amp;%Text consisting of multiple self-contained units.  
Some examples are an encyclopedia containing a couple dozen volumes, a television 
series made up of many episodes, a film serial, etc.</rdfs:comment>
        <rdfs:label xml:lang="en">Series</rdfs:label>
    </owl:Class>
    


    <!-- http://semanticbible.org/ns/2006/NTNames#SonOfGod -->

    <owl:Class rdf:about="http://semanticbible.org/ns/2006/NTNames#SonOfGod">
        <rdfs:subClassOf rdf:resource="http://semanticbible.org/ns/2006/NTNames#God"/>
        <rdfs:subClassOf rdf:resource="http://semanticbible.org/ns/2006/NTNames#Human"/>
        <rdfs:comment xml:lang="en">Both Human and God</rdfs:comment>
        <rdfs:label xml:lang="en">Son of God</rdfs:label>
    </owl:Class>
    


    <!-- http://semanticbible.org/ns/2006/NTNames#StateOrProvince -->

    <owl:Class rdf:about="http://semanticbible.org/ns/2006/NTNames#StateOrProvince">
        <rdfs:subClassOf rdf:resource="http://semanticbible.org/ns/2006/NTNames#GeopoliticalArea"/>
        <rdfs:subClassOf rdf:resource="http://semanticbible.org/ns/2006/NTNames#LandArea"/>
        <rdfs:comment xml:lang="en">Based on SUMO, http://reliant.teknowledge.com/DAML/SUMO.owl#StateOrProvince
SUO 1.55: July 14, 2003
Administrative subdivisions of a
&amp;%Nation that are broader than any other political subdivisions that
may exist.  This &amp;%Class includes the states of the United States, as
well as the provinces of Canada and European countries.
Here it covers both provinces and districts.</rdfs:comment>
        <rdfs:label xml:lang="en">State or Province</rdfs:label>
    </owl:Class>
    


    <!-- http://semanticbible.org/ns/2006/NTNames#SupernaturalBeing -->

    <owl:Class rdf:about="http://semanticbible.org/ns/2006/NTNames#SupernaturalBeing">
        <rdfs:subClassOf rdf:resource="http://semanticbible.org/ns/2006/NTNames#CognitiveAgent"/>
        <rdfs:comment xml:lang="en">A CognitiveAgent whose effects are not limited to the physical world. This includes the Lord Almighty, as well as supposed or imaginary deities.</rdfs:comment>
        <rdfs:label xml:lang="en">Supernatural Being</rdfs:label>
    </owl:Class>
    


    <!-- http://semanticbible.org/ns/2006/NTNames#SupernaturalRegion -->

    <owl:Class rdf:about="http://semanticbible.org/ns/2006/NTNames#SupernaturalRegion">
        <rdfs:subClassOf rdf:resource="http://semanticbible.org/ns/2006/NTNames#Region"/>
        <rdfs:comment rdf:datatype="http://www.w3.org/2001/XMLSchema#string">Those regions that are outside normal human existence. </rdfs:comment>
    </owl:Class>
    


    <!-- http://semanticbible.org/ns/2006/NTNames#Tribe -->

    <owl:Class rdf:about="http://semanticbible.org/ns/2006/NTNames#Tribe">
        <rdfs:subClassOf rdf:resource="http://semanticbible.org/ns/2006/NTNames#EthnicGroup"/>
        <rdfs:comment xml:lang="en">Subclass for the Twelve Tribes of Israel</rdfs:comment>
        <rdfs:label xml:lang="en">Tribe</rdfs:label>
    </owl:Class>
    


    <!-- http://semanticbible.org/ns/2006/NTNames#WaterArea -->

    <owl:Class rdf:about="http://semanticbible.org/ns/2006/NTNames#WaterArea">
        <rdfs:subClassOf rdf:resource="http://semanticbible.org/ns/2006/NTNames#GeographicArea"/>
        <rdfs:subClassOf>
            <owl:Restriction>
                <owl:onProperty rdf:resource="http://semanticbible.org/ns/2006/NTNames#nativePlaceOf"/>
                <owl:cardinality rdf:datatype="http://www.w3.org/2001/XMLSchema#nonNegativeInteger">0</owl:cardinality>
            </owl:Restriction>
        </rdfs:subClassOf>
        <rdfs:comment xml:lang="en">Based on SUMO, http://reliant.teknowledge.com/DAML/SUMO.owl#WaterArea
SUO 1.55: July 14, 2003
A body which is made up predominantly of water,
e.g. rivers, lakes, oceans, etc.</rdfs:comment>
        <rdfs:label xml:lang="en">Water Area</rdfs:label>
    </owl:Class>
    


    <!-- http://semanticbible.org/ns/2006/NTNames#Woman -->

    <owl:Class rdf:about="http://semanticbible.org/ns/2006/NTNames#Woman">
        <rdfs:subClassOf rdf:resource="http://semanticbible.org/ns/2006/NTNames#Human"/>
        <rdfs:subClassOf>
            <owl:Restriction>
                <owl:onProperty rdf:resource="http://semanticbible.org/ns/2006/NTNames#spouseOf"/>
                <owl:allValuesFrom rdf:resource="http://semanticbible.org/ns/2006/NTNames#Man"/>
            </owl:Restriction>
        </rdfs:subClassOf>
        <rdfs:comment xml:lang="en">SUO 1.55: July 14, 2003
The class of &amp;%Female &amp;%Humans.</rdfs:comment>
        <rdfs:label xml:lang="en">Woman</rdfs:label>
    </owl:Class>
    


    <!-- 
    ///////////////////////////////////////////////////////////////////////////////////////
    //
    // Individuals
    //
    ///////////////////////////////////////////////////////////////////////////////////////
     -->

    


    <!-- http://semanticbible.org/ns/2006/NTNames#Aaron -->

    <owl:NamedIndividual rdf:about="http://semanticbible.org/ns/2006/NTNames#Aaron">
        <rdf:type rdf:resource="http://semanticbible.org/ns/2006/NTNames#Man"/>
        <ethnicity rdf:resource="http://semanticbible.org/ns/2006/NTNames#Jewish"/>
        <siblingOf rdf:resource="http://semanticbible.org/ns/2006/NTNames#Moses"/>
        <description rdf:datatype="http://www.w3.org/2001/XMLSchema#string">Moses&apos; assistant during the Exodus</description>
        <hasOnlyGenealogyMention rdf:datatype="http://www.w3.org/2001/XMLSchema#boolean">false</hasOnlyGenealogyMention>
        <rdfs:label xml:lang="en">Aaron</rdfs:label>
    </owl:NamedIndividual>
    


    <!-- http://semanticbible.org/ns/2006/NTNames#Abel -->

    <owl:NamedIndividual rdf:about="http://semanticbible.org/ns/2006/NTNames#Abel">
        <rdf:type rdf:resource="http://semanticbible.org/ns/2006/NTNames#Man"/>
        <childOf rdf:resource="http://semanticbible.org/ns/2006/NTNames#Adam"/>
        <childOf rdf:resource="http://semanticbible.org/ns/2006/NTNames#Eve"/>
        <siblingOf rdf:resource="http://semanticbible.org/ns/2006/NTNames#Cain"/>
        <rdfs:label xml:lang="en">Abel</rdfs:label>
    </owl:NamedIndividual>
    


    <!-- http://semanticbible.org/ns/2006/NTNames#Abiathar -->

    <owl:NamedIndividual rdf:about="http://semanticbible.org/ns/2006/NTNames#Abiathar">
        <rdf:type rdf:resource="http://semanticbible.org/ns/2006/NTNames#Man"/>
        <ethnicity rdf:resource="http://semanticbible.org/ns/2006/NTNames#Levite"/>
        <description rdf:datatype="http://www.w3.org/2001/XMLSchema#string">High priest during the lifetime of King David</description>
        <occupation rdf:datatype="http://www.w3.org/2001/XMLSchema#string">high priest</occupation>
        <rdfs:label xml:lang="en">Abiathar</rdfs:label>
    </owl:NamedIndividual>
    


    <!-- http://semanticbible.org/ns/2006/NTNames#AbijahSonOfRehoboam -->

    <owl:NamedIndividual rdf:about="http://semanticbible.org/ns/2006/NTNames#AbijahSonOfRehoboam">
        <rdf:type rdf:resource="http://semanticbible.org/ns/2006/NTNames#Man"/>
        <childOf rdf:resource="http://semanticbible.org/ns/2006/NTNames#Rehoboam"/>
        <ethnicity rdf:resource="http://semanticbible.org/ns/2006/NTNames#Jewish"/>
        <parentOf rdf:resource="http://semanticbible.org/ns/2006/NTNames#Asaph"/>
        <relativeOf rdf:resource="http://semanticbible.org/ns/2006/NTNames#Asaph"/>
        <relativeOf rdf:resource="http://semanticbible.org/ns/2006/NTNames#Rehoboam"/>
        <description rdf:datatype="http://www.w3.org/2001/XMLSchema#string">One of the ancestors of Jesus mentioned in Matthew&apos;s geneaology</description>
        <hasOnlyGenealogyMention rdf:datatype="http://www.w3.org/2001/XMLSchema#boolean">true</hasOnlyGenealogyMention>
        <occupation rdf:datatype="http://www.w3.org/2001/XMLSchema#string">king of Judah</occupation>
        <rdfs:comment xml:lang="en">His occupation as king comes from Old Testament sources, 2Chr.12-13.</rdfs:comment>
        <rdfs:label xml:lang="en">Abijah</rdfs:label>
    </owl:NamedIndividual>
    


    <!-- http://semanticbible.org/ns/2006/NTNames#AbijahthePriest -->

    <owl:NamedIndividual rdf:about="http://semanticbible.org/ns/2006/NTNames#AbijahthePriest">
        <rdf:type rdf:resource="http://semanticbible.org/ns/2006/NTNames#Man"/>
        <ethnicity rdf:resource="http://semanticbible.org/ns/2006/NTNames#Levite"/>
        <knows rdf:resource="http://semanticbible.org/ns/2006/NTNames#David"/>
        <description rdf:datatype="http://www.w3.org/2001/XMLSchema#string">A priest appointed by King David</description>
        <occupation rdf:datatype="http://www.w3.org/2001/XMLSchema#string">priest</occupation>
        <rdfs:comment xml:lang="en">Zacharias, father of John the Baptist, was a descendant of Abijah.</rdfs:comment>
        <rdfs:label xml:lang="en">Abijah</rdfs:label>
    </owl:NamedIndividual>
    


    <!-- http://semanticbible.org/ns/2006/NTNames#Abilene -->

    <owl:NamedIndividual rdf:about="http://semanticbible.org/ns/2006/NTNames#Abilene">
        <rdf:type rdf:resource="http://semanticbible.org/ns/2006/NTNames#StateOrProvince"/>
        <subregion rdf:resource="http://semanticbible.org/ns/2006/NTNames#Damascus"/>
        <rdfs:label xml:lang="en">Abilene</rdfs:label>
    </owl:NamedIndividual>
    


    <!-- http://semanticbible.org/ns/2006/NTNames#Abiud -->

    <owl:NamedIndividual rdf:about="http://semanticbible.org/ns/2006/NTNames#Abiud">
        <rdf:type rdf:resource="http://semanticbible.org/ns/2006/NTNames#Man"/>
        <childOf rdf:resource="http://semanticbible.org/ns/2006/NTNames#Zerubbabel"/>
        <ethnicity rdf:resource="http://semanticbible.org/ns/2006/NTNames#Jewish"/>
        <parentOf rdf:resource="http://semanticbible.org/ns/2006/NTNames#EliakimSonOfAbiud"/>
        <rdfs:label xml:lang="en">Abiud</rdfs:label>
    </owl:NamedIndividual>
    


    <!-- http://semanticbible.org/ns/2006/NTNames#Abraham -->

    <owl:NamedIndividual rdf:about="http://semanticbible.org/ns/2006/NTNames#Abraham">
        <rdf:type rdf:resource="http://semanticbible.org/ns/2006/NTNames#Man"/>
        <childOf rdf:resource="http://semanticbible.org/ns/2006/NTNames#Terah"/>
        <ethnicity rdf:resource="http://semanticbible.org/ns/2006/NTNames#Jewish"/>
        <parentOf rdf:resource="http://semanticbible.org/ns/2006/NTNames#Isaac"/>
        <residentPlace rdf:resource="http://semanticbible.org/ns/2006/NTNames#Canaan"/>
        <spouseOf rdf:resource="http://semanticbible.org/ns/2006/NTNames#Sarah"/>
        <description rdf:datatype="http://www.w3.org/2001/XMLSchema#string">The founder of the Hebrew nation.</description>
        <hasOnlyGenealogyMention rdf:datatype="http://www.w3.org/2001/XMLSchema#boolean">false</hasOnlyGenealogyMention>
        <rdfs:label xml:lang="en">Abraham</rdfs:label>
        <rdfs:label xml:lang="en">Abram</rdfs:label>
    </owl:NamedIndividual>
    


    <!-- http://semanticbible.org/ns/2006/NTNames#Achaia -->

    <owl:NamedIndividual rdf:about="http://semanticbible.org/ns/2006/NTNames#Achaia">
        <rdf:type rdf:resource="http://semanticbible.org/ns/2006/NTNames#StateOrProvince"/>
        <residentPlaceOf rdf:resource="http://semanticbible.org/ns/2006/NTNames#Gallio"/>
        <rdfs:label xml:lang="en">Achaia</rdfs:label>
    </owl:NamedIndividual>
    


    <!-- http://semanticbible.org/ns/2006/NTNames#Achaicus -->

    <owl:NamedIndividual rdf:about="http://semanticbible.org/ns/2006/NTNames#Achaicus">
        <rdf:type rdf:resource="http://semanticbible.org/ns/2006/NTNames#Man"/>
        <collaboratesWith rdf:resource="http://semanticbible.org/ns/2006/NTNames#Fortunatus"/>
        <collaboratesWith rdf:resource="http://semanticbible.org/ns/2006/NTNames#Paul"/>
        <collaboratesWith rdf:resource="http://semanticbible.org/ns/2006/NTNames#Stephanas"/>
        <religiousBelief rdf:resource="http://semanticbible.org/ns/2006/NTNames#Christianity"/>
        <residentPlace rdf:resource="http://semanticbible.org/ns/2006/NTNames#Corinth"/>
        <visitedPlace rdf:resource="http://semanticbible.org/ns/2006/NTNames#Ephesus"/>
        <description rdf:datatype="http://www.w3.org/2001/XMLSchema#string">A member of Corinthian church who visited the Apostle Paul in Ephesus, perhaps bearing a letter to him.</description>
        <rdfs:comment rdf:datatype="http://www.w3.org/2001/XMLSchema#string">His residence in Corinth and visit to Ephesus follow from Paul&apos;s statement in 1Cor.16.17, and the assumption that Paul was in Ephesus when he wrote 1 Corinthians. </rdfs:comment>
        <rdfs:label xml:lang="en">Achaicus</rdfs:label>
    </owl:NamedIndividual>
    


    <!-- http://semanticbible.org/ns/2006/NTNames#Achim -->

    <owl:NamedIndividual rdf:about="http://semanticbible.org/ns/2006/NTNames#Achim">
        <rdf:type rdf:resource="http://semanticbible.org/ns/2006/NTNames#Man"/>
        <childOf rdf:resource="http://semanticbible.org/ns/2006/NTNames#Zadok"/>
        <ethnicity rdf:resource="http://semanticbible.org/ns/2006/NTNames#Jewish"/>
        <parentOf rdf:resource="http://semanticbible.org/ns/2006/NTNames#Eliud"/>
        <rdfs:label xml:lang="en">Achim</rdfs:label>
    </owl:NamedIndividual>
    


    <!-- http://semanticbible.org/ns/2006/NTNames#Adam -->

    <owl:NamedIndividual rdf:about="http://semanticbible.org/ns/2006/NTNames#Adam">
        <rdf:type rdf:resource="http://semanticbible.org/ns/2006/NTNames#Man"/>
        <parentOf rdf:resource="http://semanticbible.org/ns/2006/NTNames#Abel"/>
        <parentOf rdf:resource="http://semanticbible.org/ns/2006/NTNames#Cain"/>
        <parentOf rdf:resource="http://semanticbible.org/ns/2006/NTNames#Seth"/>
        <spouseOf rdf:resource="http://semanticbible.org/ns/2006/NTNames#Eve"/>
        <description rdf:datatype="http://www.w3.org/2001/XMLSchema#string">The first created human</description>
        <rdfs:comment xml:lang="en">Though Luke&apos;s geneaology lists Adam as &quot;the son of God&quot;, this is not in the biological sense of childOf</rdfs:comment>
        <rdfs:label xml:lang="en">Adam</rdfs:label>
    </owl:NamedIndividual>
    


    <!-- http://semanticbible.org/ns/2006/NTNames#Addi -->

    <owl:NamedIndividual rdf:about="http://semanticbible.org/ns/2006/NTNames#Addi">
        <rdf:type rdf:resource="http://semanticbible.org/ns/2006/NTNames#Man"/>
        <childOf rdf:resource="http://semanticbible.org/ns/2006/NTNames#Cosam"/>
        <ethnicity rdf:resource="http://semanticbible.org/ns/2006/NTNames#Jewish"/>
        <parentOf rdf:resource="http://semanticbible.org/ns/2006/NTNames#MelchiSonOfAddi"/>
        <hasOnlyGenealogyMention rdf:datatype="http://www.w3.org/2001/XMLSchema#boolean">true</hasOnlyGenealogyMention>
        <rdfs:label xml:lang="en">Addi</rdfs:label>
    </owl:NamedIndividual>
    


    <!-- http://semanticbible.org/ns/2006/NTNames#Admin -->

    <owl:NamedIndividual rdf:about="http://semanticbible.org/ns/2006/NTNames#Admin">
        <rdf:type rdf:resource="http://semanticbible.org/ns/2006/NTNames#Man"/>
        <childOf rdf:resource="http://semanticbible.org/ns/2006/NTNames#Arni"/>
        <ethnicity rdf:resource="http://semanticbible.org/ns/2006/NTNames#Jewish"/>
        <parentOf rdf:resource="http://semanticbible.org/ns/2006/NTNames#Amminadab"/>
        <hasOnlyGenealogyMention rdf:datatype="http://www.w3.org/2001/XMLSchema#boolean">true</hasOnlyGenealogyMention>
        <rdfs:label xml:lang="en">Admin</rdfs:label>
        <rdfs:label xml:lang="en">Aram</rdfs:label>
    </owl:NamedIndividual>
    


    <!-- http://semanticbible.org/ns/2006/NTNames#Adramyttium -->

    <owl:NamedIndividual rdf:about="http://semanticbible.org/ns/2006/NTNames#Adramyttium">
        <rdf:type rdf:resource="http://semanticbible.org/ns/2006/NTNames#City"/>
        <rdfs:label xml:lang="en">Adramyttium</rdfs:label>
    </owl:NamedIndividual>
    


    <!-- http://semanticbible.org/ns/2006/NTNames#Adriatic -->

    <owl:NamedIndividual rdf:about="http://semanticbible.org/ns/2006/NTNames#Adriatic">
        <rdf:type rdf:resource="http://semanticbible.org/ns/2006/NTNames#SaltWaterArea"/>
        <rdfs:label xml:lang="en">Adriatic</rdfs:label>
    </owl:NamedIndividual>
    


    <!-- http://semanticbible.org/ns/2006/NTNames#Aeneas -->

    <owl:NamedIndividual rdf:about="http://semanticbible.org/ns/2006/NTNames#Aeneas">
        <rdf:type rdf:resource="http://semanticbible.org/ns/2006/NTNames#Man"/>
        <knows rdf:resource="http://semanticbible.org/ns/2006/NTNames#SimonPeter"/>
        <description rdf:datatype="http://www.w3.org/2001/XMLSchema#string">A paralytic healed by Peter</description>
        <rdfs:label xml:lang="en">Aeneas</rdfs:label>
    </owl:NamedIndividual>
    


    <!-- http://semanticbible.org/ns/2006/NTNames#Aenon -->

    <owl:NamedIndividual rdf:about="http://semanticbible.org/ns/2006/NTNames#Aenon">
        <rdf:type rdf:resource="http://semanticbible.org/ns/2006/NTNames#LandArea"/>
        <rdfs:label xml:lang="en">Aenon</rdfs:label>
    </owl:NamedIndividual>
    


    <!-- http://semanticbible.org/ns/2006/NTNames#Agabus -->

    <owl:NamedIndividual rdf:about="http://semanticbible.org/ns/2006/NTNames#Agabus">
        <rdf:type rdf:resource="http://semanticbible.org/ns/2006/NTNames#Man"/>
        <collaboratesWith rdf:resource="http://semanticbible.org/ns/2006/NTNames#Barabbas"/>
        <collaboratesWith rdf:resource="http://semanticbible.org/ns/2006/NTNames#Paul"/>
        <description rdf:datatype="http://www.w3.org/2001/XMLSchema#string">A prophet in the Jerusalem church who visited Antioch and foretold of a coming famine.</description>
        <occupation rdf:datatype="http://www.w3.org/2001/XMLSchema#string">prophet</occupation>
        <rdfs:label xml:lang="en">Agabus</rdfs:label>
    </owl:NamedIndividual>
    


    <!-- http://semanticbible.org/ns/2006/NTNames#Ahaz -->

    <owl:NamedIndividual rdf:about="http://semanticbible.org/ns/2006/NTNames#Ahaz">
        <rdf:type rdf:resource="http://semanticbible.org/ns/2006/NTNames#Man"/>
        <childOf rdf:resource="http://semanticbible.org/ns/2006/NTNames#Jotham"/>
        <ethnicity rdf:resource="http://semanticbible.org/ns/2006/NTNames#Jewish"/>
        <parentOf rdf:resource="http://semanticbible.org/ns/2006/NTNames#Hezekiah"/>
        <description rdf:datatype="http://www.w3.org/2001/XMLSchema#string">King of Judah during the time of Isaiah</description>
        <hasOnlyGenealogyMention rdf:datatype="http://www.w3.org/2001/XMLSchema#boolean">true</hasOnlyGenealogyMention>
        <occupation rdf:datatype="http://www.w3.org/2001/XMLSchema#string">king</occupation>
        <rdfs:comment xml:lang="en">See OT descriptions in 2 Kings 16; Isa. 7-9; 2 Chr. 28.</rdfs:comment>
        <rdfs:label xml:lang="en">Ahaz</rdfs:label>
    </owl:NamedIndividual>
    


    <!-- http://semanticbible.org/ns/2006/NTNames#Akeldama -->

    <owl:NamedIndividual rdf:about="http://semanticbible.org/ns/2006/NTNames#Akeldama">
        <rdf:type rdf:resource="http://semanticbible.org/ns/2006/NTNames#LandArea"/>
        <rdfs:label xml:lang="en">Akeldama</rdfs:label>
    </owl:NamedIndividual>
    


    <!-- http://semanticbible.org/ns/2006/NTNames#Alexander -->

    <owl:NamedIndividual rdf:about="http://semanticbible.org/ns/2006/NTNames#Alexander">
        <rdf:type rdf:resource="http://semanticbible.org/ns/2006/NTNames#Man"/>
        <childOf rdf:resource="http://semanticbible.org/ns/2006/NTNames#SimonOfCyrene"/>
        <siblingOf rdf:resource="http://semanticbible.org/ns/2006/NTNames#Rufus"/>
        <description rdf:datatype="http://www.w3.org/2001/XMLSchema#string">Probably an early Christian known to Mark, who mentions him as the son of Simon of Cyrene, who was compelled to carry Jesus&apos; cross</description>
        <hasOnlyGenealogyMention rdf:datatype="http://www.w3.org/2001/XMLSchema#boolean">false</hasOnlyGenealogyMention>
        <rdfs:label xml:lang="en">Alexander</rdfs:label>
    </owl:NamedIndividual>
    


    <!-- http://semanticbible.org/ns/2006/NTNames#AlexanderOfEphesus -->

    <owl:NamedIndividual rdf:about="http://semanticbible.org/ns/2006/NTNames#AlexanderOfEphesus">
        <rdf:type rdf:resource="http://semanticbible.org/ns/2006/NTNames#Man"/>
        <ethnicity rdf:resource="http://semanticbible.org/ns/2006/NTNames#Jewish"/>
        <description rdf:datatype="http://www.w3.org/2001/XMLSchema#string">A Jew in Ephesus who was put forward to quiet the crowd during the riot caused by Demetrius</description>
        <hasOnlyGenealogyMention rdf:datatype="http://www.w3.org/2001/XMLSchema#boolean">false</hasOnlyGenealogyMention>
        <rdfs:label xml:lang="en">Alexander</rdfs:label>
    </owl:NamedIndividual>
    


    <!-- http://semanticbible.org/ns/2006/NTNames#AlexanderOfTheSanhedrin -->

    <owl:NamedIndividual rdf:about="http://semanticbible.org/ns/2006/NTNames#AlexanderOfTheSanhedrin">
        <rdf:type rdf:resource="http://semanticbible.org/ns/2006/NTNames#Man"/>
        <collaboratesWith rdf:resource="http://semanticbible.org/ns/2006/NTNames#JohnOfTheSanhedrin"/>
        <enemyOf rdf:resource="http://semanticbible.org/ns/2006/NTNames#JohnSonOfZebedee"/>
        <enemyOf rdf:resource="http://semanticbible.org/ns/2006/NTNames#SimonPeter"/>
        <ethnicity rdf:resource="http://semanticbible.org/ns/2006/NTNames#Judean"/>
        <memberOf rdf:resource="http://semanticbible.org/ns/2006/NTNames#Sanhedrin"/>
        <relativeOf rdf:resource="http://semanticbible.org/ns/2006/NTNames#Annas"/>
        <relativeOf rdf:resource="http://semanticbible.org/ns/2006/NTNames#JohnOfTheSanhedrin"/>
        <description rdf:datatype="http://www.w3.org/2001/XMLSchema#string">A relative of Annas the High Priest who was present when Peter and John were questioned about healing a lame man</description>
        <hasOnlyGenealogyMention rdf:datatype="http://www.w3.org/2001/XMLSchema#boolean">false</hasOnlyGenealogyMention>
        <rdfs:label xml:lang="en">Alexander</rdfs:label>
    </owl:NamedIndividual>
    


    <!-- http://semanticbible.org/ns/2006/NTNames#AlexanderTheCoppersmith -->

    <owl:NamedIndividual rdf:about="http://semanticbible.org/ns/2006/NTNames#AlexanderTheCoppersmith">
        <rdf:type rdf:resource="http://semanticbible.org/ns/2006/NTNames#Man"/>
        <enemyOf rdf:resource="http://semanticbible.org/ns/2006/NTNames#Paul"/>
        <possiblySamePersonAs rdf:resource="http://semanticbible.org/ns/2006/NTNames#AlexanderTheHeretic"/>
        <description rdf:datatype="http://www.w3.org/2001/XMLSchema#string">A resident of Ephesus who caused Paul &quot;great harm&quot;</description>
        <hasOnlyGenealogyMention rdf:datatype="http://www.w3.org/2001/XMLSchema#boolean">false</hasOnlyGenealogyMention>
        <occupation rdf:datatype="http://www.w3.org/2001/XMLSchema#string">coppersmith</occupation>
        <rdfs:comment xml:lang="en">This may be the same as AlexanderTheHeretic, since they are both identified as opponents of Paul and the Gospel, and they both resided in Ephesus.</rdfs:comment>
        <rdfs:label xml:lang="en">Alexander</rdfs:label>
    </owl:NamedIndividual>
    


    <!-- http://semanticbible.org/ns/2006/NTNames#AlexanderTheHeretic -->

    <owl:NamedIndividual rdf:about="http://semanticbible.org/ns/2006/NTNames#AlexanderTheHeretic">
        <rdf:type rdf:resource="http://semanticbible.org/ns/2006/NTNames#Man"/>
        <collaboratesWith rdf:resource="http://semanticbible.org/ns/2006/NTNames#Hymenaeus"/>
        <possiblySamePersonAs rdf:resource="http://semanticbible.org/ns/2006/NTNames#AlexanderTheCoppersmith"/>
        <description rdf:datatype="http://www.w3.org/2001/XMLSchema#string">Described to Timothy by Paul as having &quot;rejected conscience&quot;</description>
        <rdfs:label xml:lang="en">Alexander</rdfs:label>
    </owl:NamedIndividual>
    


    <!-- http://semanticbible.org/ns/2006/NTNames#Alexandria -->

    <owl:NamedIndividual rdf:about="http://semanticbible.org/ns/2006/NTNames#Alexandria">
        <rdf:type rdf:resource="http://semanticbible.org/ns/2006/NTNames#City"/>
        <location rdf:resource="http://semanticbible.org/ns/2006/NTNames#AlexandriaGeodata"/>
        <nativePlaceOf rdf:resource="http://semanticbible.org/ns/2006/NTNames#Apollos"/>
        <rdfs:label xml:lang="en">Alexandria</rdfs:label>
    </owl:NamedIndividual>
    


    <!-- http://semanticbible.org/ns/2006/NTNames#AlexandriaGeodata -->

    <owl:NamedIndividual rdf:about="http://semanticbible.org/ns/2006/NTNames#AlexandriaGeodata">
        <rdf:type rdf:resource="http://semanticbible.org/ns/2006/NTNames#GeographicLocation"/>
        <altitude rdf:datatype="http://www.w3.org/2001/XMLSchema#int">0</altitude>
        <latitude rdf:datatype="http://www.w3.org/2001/XMLSchema#double">31.1869228814314</latitude>
        <longitude rdf:datatype="http://www.w3.org/2001/XMLSchema#double">30.09869047792926</longitude>
        <rdfs:label xml:lang="en">geodata for Alexandria</rdfs:label>
    </owl:NamedIndividual>
    


    <!-- http://semanticbible.org/ns/2006/NTNames#Alexandrians -->

    <owl:NamedIndividual rdf:about="http://semanticbible.org/ns/2006/NTNames#Alexandrians">
        <rdf:type rdf:resource="http://semanticbible.org/ns/2006/NTNames#ResidenceGroup"/>
        <rdfs:label xml:lang="en">Alexandrians</rdfs:label>
    </owl:NamedIndividual>
    


    <!-- http://semanticbible.org/ns/2006/NTNames#Almighty -->

    <owl:NamedIndividual rdf:about="http://semanticbible.org/ns/2006/NTNames#Almighty">
        <rdf:type rdf:resource="http://semanticbible.org/ns/2006/NTNames#God"/>
        <rdfs:comment rdf:datatype="http://www.w3.org/2001/XMLSchema#string">&quot;Eli&quot; is Aramaic for &quot;My God&quot;. </rdfs:comment>
        <rdfs:label xml:lang="en">Almighty</rdfs:label>
    </owl:NamedIndividual>
    


    <!-- http://semanticbible.org/ns/2006/NTNames#Alpha -->

    <owl:NamedIndividual rdf:about="http://semanticbible.org/ns/2006/NTNames#Alpha">
        <rdf:type rdf:resource="http://semanticbible.org/ns/2006/NTNames#Character"/>
        <rdfs:label xml:lang="en">Alpha</rdfs:label>
    </owl:NamedIndividual>
    


    <!-- http://semanticbible.org/ns/2006/NTNames#Alphaeus -->

    <owl:NamedIndividual rdf:about="http://semanticbible.org/ns/2006/NTNames#Alphaeus">
        <rdf:type rdf:resource="http://semanticbible.org/ns/2006/NTNames#Man"/>
        <ethnicity rdf:resource="http://semanticbible.org/ns/2006/NTNames#Galilean"/>
        <parentOf rdf:resource="http://semanticbible.org/ns/2006/NTNames#JamesSonOfAlphaeus"/>
        <spouseOf rdf:resource="http://semanticbible.org/ns/2006/NTNames#MaryWifeOfClopas"/>
        <description rdf:datatype="http://www.w3.org/2001/XMLSchema#string">The father of James, one of the Twelve</description>
        <rdfs:comment rdf:datatype="http://www.w3.org/2001/XMLSchema#string">The identification of Alphaeus with Clopas is not completely certain: see ISBE for Alphaeus.</rdfs:comment>
        <rdfs:label xml:lang="en">Alphaeus</rdfs:label>
    </owl:NamedIndividual>
    


    <!-- http://semanticbible.org/ns/2006/NTNames#AlphaeusFatherOfLevi -->

    <owl:NamedIndividual rdf:about="http://semanticbible.org/ns/2006/NTNames#AlphaeusFatherOfLevi">
        <rdf:type rdf:resource="http://semanticbible.org/ns/2006/NTNames#Man"/>
        <ethnicity rdf:resource="http://semanticbible.org/ns/2006/NTNames#Galilean"/>
        <parentOf rdf:resource="http://semanticbible.org/ns/2006/NTNames#Levi"/>
        <description rdf:datatype="http://www.w3.org/2001/XMLSchema#string">The father of Levi, one of the Twelve</description>
        <rdfs:comment xml:lang="en">That both James the Less and Levi had fathers named Alphaeus has led some to speculate they were brothers, but this seems unlikely.</rdfs:comment>
        <rdfs:label xml:lang="en">Alphaeus</rdfs:label>
    </owl:NamedIndividual>
    


    <!-- http://semanticbible.org/ns/2006/NTNames#Amminadab -->

    <owl:NamedIndividual rdf:about="http://semanticbible.org/ns/2006/NTNames#Amminadab">
        <rdf:type rdf:resource="http://semanticbible.org/ns/2006/NTNames#Man"/>
        <childOf rdf:resource="http://semanticbible.org/ns/2006/NTNames#Admin"/>
        <childOf rdf:resource="http://semanticbible.org/ns/2006/NTNames#Ram"/>
        <ethnicity rdf:resource="http://semanticbible.org/ns/2006/NTNames#Jewish"/>
        <parentOf rdf:resource="http://semanticbible.org/ns/2006/NTNames#Nahshon"/>
        <description rdf:datatype="http://www.w3.org/2001/XMLSchema#string">One of the ancestors of Jesus mentioned in Matthew&apos;s geneaology</description>
        <hasOnlyGenealogyMention rdf:datatype="http://www.w3.org/2001/XMLSchema#boolean">true</hasOnlyGenealogyMention>
        <rdfs:label xml:lang="en">Amminadab</rdfs:label>
    </owl:NamedIndividual>
    


    <!-- http://semanticbible.org/ns/2006/NTNames#Amos -->

    <owl:NamedIndividual rdf:about="http://semanticbible.org/ns/2006/NTNames#Amos">
        <rdf:type rdf:resource="http://semanticbible.org/ns/2006/NTNames#Man"/>
        <childOf rdf:resource="http://semanticbible.org/ns/2006/NTNames#Manasseh"/>
        <ethnicity rdf:resource="http://semanticbible.org/ns/2006/NTNames#Jewish"/>
        <parentOf rdf:resource="http://semanticbible.org/ns/2006/NTNames#Josiah"/>
        <rdfs:label xml:lang="en">Amos</rdfs:label>
    </owl:NamedIndividual>
    


    <!-- http://semanticbible.org/ns/2006/NTNames#AmosSonOfNahum -->

    <owl:NamedIndividual rdf:about="http://semanticbible.org/ns/2006/NTNames#AmosSonOfNahum">
        <rdf:type rdf:resource="http://semanticbible.org/ns/2006/NTNames#Man"/>
        <childOf rdf:resource="http://semanticbible.org/ns/2006/NTNames#Nahum"/>
        <ethnicity rdf:resource="http://semanticbible.org/ns/2006/NTNames#Jewish"/>
        <parentOf rdf:resource="http://semanticbible.org/ns/2006/NTNames#MattathaisSonOfAmos"/>
        <description rdf:datatype="http://www.w3.org/2001/XMLSchema#string">One of the ancestors of Jesus mentioned in Luke&apos;s geneaology</description>
        <hasOnlyGenealogyMention rdf:datatype="http://www.w3.org/2001/XMLSchema#boolean">true</hasOnlyGenealogyMention>
        <rdfs:comment xml:lang="en">There&apos;s no evidence other than the similar (and not uncommon) name to suggest this man is the same Amos as the Old Testament prophet. </rdfs:comment>
        <rdfs:label xml:lang="en">Amos</rdfs:label>
    </owl:NamedIndividual>
    


    <!-- http://semanticbible.org/ns/2006/NTNames#Amphipolis -->

    <owl:NamedIndividual rdf:about="http://semanticbible.org/ns/2006/NTNames#Amphipolis">
        <rdf:type rdf:resource="http://semanticbible.org/ns/2006/NTNames#City"/>
        <location rdf:resource="http://semanticbible.org/ns/2006/NTNames#AmphipolisGeodata"/>
        <subregionOf rdf:resource="http://semanticbible.org/ns/2006/NTNames#Macedonia"/>
        <rdfs:label xml:lang="en">Amphipolis</rdfs:label>
    </owl:NamedIndividual>
    


    <!-- http://semanticbible.org/ns/2006/NTNames#AmphipolisGeodata -->

    <owl:NamedIndividual rdf:about="http://semanticbible.org/ns/2006/NTNames#AmphipolisGeodata">
        <rdf:type rdf:resource="http://semanticbible.org/ns/2006/NTNames#GeographicLocation"/>
        <locationOf rdf:resource="http://semanticbible.org/ns/2006/NTNames#Amphipolis"/>
        <altitude rdf:datatype="http://www.w3.org/2001/XMLSchema#int">0</altitude>
        <latitude rdf:datatype="http://www.w3.org/2001/XMLSchema#double">40.82086523068722</latitude>
        <longitude rdf:datatype="http://www.w3.org/2001/XMLSchema#double">23.83947945942736</longitude>
        <rdfs:label xml:lang="en">geodata for Amphipolis</rdfs:label>
    </owl:NamedIndividual>
    


    <!-- http://semanticbible.org/ns/2006/NTNames#Ampliatus -->

    <owl:NamedIndividual rdf:about="http://semanticbible.org/ns/2006/NTNames#Ampliatus">
        <rdf:type rdf:resource="http://semanticbible.org/ns/2006/NTNames#Man"/>
        <knows rdf:resource="http://semanticbible.org/ns/2006/NTNames#Paul"/>
        <knows rdf:resource="http://semanticbible.org/ns/2006/NTNames#Priscilla"/>
        <religiousBelief rdf:resource="http://semanticbible.org/ns/2006/NTNames#Christianity"/>
        <residentPlace rdf:resource="http://semanticbible.org/ns/2006/NTNames#Rome"/>
        <hasOnlyGenealogyMention rdf:datatype="http://www.w3.org/2001/XMLSchema#boolean">false</hasOnlyGenealogyMention>
        <rdfs:label xml:lang="en">Ampliatus</rdfs:label>
    </owl:NamedIndividual>
    


    <!-- http://semanticbible.org/ns/2006/NTNames#Ananias -->

    <owl:NamedIndividual rdf:about="http://semanticbible.org/ns/2006/NTNames#Ananias">
        <rdf:type rdf:resource="http://semanticbible.org/ns/2006/NTNames#Man"/>
        <ethnicity rdf:resource="http://semanticbible.org/ns/2006/NTNames#Jewish"/>
        <hasAntagonist rdf:resource="http://semanticbible.org/ns/2006/NTNames#SimonPeter"/>
        <knows rdf:resource="http://semanticbible.org/ns/2006/NTNames#SimonPeter"/>
        <spouseOf rdf:resource="http://semanticbible.org/ns/2006/NTNames#Sapphira"/>
        <description rdf:datatype="http://www.w3.org/2001/XMLSchema#string">A member of the early church in Jerusalem who conspired with his wife to deceive the church about a gift of property, and who was consequently struck dead.</description>
        <rdfs:comment rdf:datatype="http://www.w3.org/2001/XMLSchema#string">Residence in Jerusalem is assumed by the account in Acts 5, where the church is still primarily Jersualem-based. </rdfs:comment>
        <rdfs:label xml:lang="en">Ananias</rdfs:label>
    </owl:NamedIndividual>
    


    <!-- http://semanticbible.org/ns/2006/NTNames#AnaniasOfDamascus -->

    <owl:NamedIndividual rdf:about="http://semanticbible.org/ns/2006/NTNames#AnaniasOfDamascus">
        <rdf:type rdf:resource="http://semanticbible.org/ns/2006/NTNames#Man"/>
        <collaboratesWith rdf:resource="http://semanticbible.org/ns/2006/NTNames#Paul"/>
        <ethnicity rdf:resource="http://semanticbible.org/ns/2006/NTNames#Jewish"/>
        <description rdf:datatype="http://www.w3.org/2001/XMLSchema#string">Ananias was sent to Paul to restore his sight, after his encounter with Christ on the road to Damascus</description>
        <rdfs:label xml:lang="en">Ananias</rdfs:label>
    </owl:NamedIndividual>
    


    <!-- http://semanticbible.org/ns/2006/NTNames#AnaniasTheHighPriest -->

    <owl:NamedIndividual rdf:about="http://semanticbible.org/ns/2006/NTNames#AnaniasTheHighPriest">
        <rdf:type rdf:resource="http://semanticbible.org/ns/2006/NTNames#Man"/>
        <collaboratesWith rdf:resource="http://semanticbible.org/ns/2006/NTNames#Tertullus"/>
        <enemyOf rdf:resource="http://semanticbible.org/ns/2006/NTNames#Paul"/>
        <ethnicity rdf:resource="http://semanticbible.org/ns/2006/NTNames#Judean"/>
        <ethnicity rdf:resource="http://semanticbible.org/ns/2006/NTNames#Levite"/>
        <knows rdf:resource="http://semanticbible.org/ns/2006/NTNames#Felix"/>
        <memberOf rdf:resource="http://semanticbible.org/ns/2006/NTNames#Sanhedrin"/>
        <description rdf:datatype="http://www.w3.org/2001/XMLSchema#string">Jewish High Priest during the time of the Apostle Paul </description>
        <occupation rdf:datatype="http://www.w3.org/2001/XMLSchema#string">High priest</occupation>
        <rdfs:comment rdf:datatype="http://www.w3.org/2001/XMLSchema#string">ISBE describes him as a Sadducee, though it&apos;s not clear why.</rdfs:comment>
        <rdfs:label xml:lang="en">Ananias</rdfs:label>
    </owl:NamedIndividual>
    


    <!-- http://semanticbible.org/ns/2006/NTNames#Andrew -->

    <owl:NamedIndividual rdf:about="http://semanticbible.org/ns/2006/NTNames#Andrew">
        <rdf:type rdf:resource="http://semanticbible.org/ns/2006/NTNames#Man"/>
        <childOf rdf:resource="http://semanticbible.org/ns/2006/NTNames#JonahOfBethsaida"/>
        <collaboratesWith rdf:resource="http://semanticbible.org/ns/2006/NTNames#Bartholomew"/>
        <collaboratesWith rdf:resource="http://semanticbible.org/ns/2006/NTNames#JamesSonOfAlphaeus"/>
        <collaboratesWith rdf:resource="http://semanticbible.org/ns/2006/NTNames#JamesSonOfZebedee"/>
        <collaboratesWith rdf:resource="http://semanticbible.org/ns/2006/NTNames#Jesus"/>
        <collaboratesWith rdf:resource="http://semanticbible.org/ns/2006/NTNames#JohnSonOfZebedee"/>
        <collaboratesWith rdf:resource="http://semanticbible.org/ns/2006/NTNames#JohntheBaptist"/>
        <collaboratesWith rdf:resource="http://semanticbible.org/ns/2006/NTNames#Levi"/>
        <collaboratesWith rdf:resource="http://semanticbible.org/ns/2006/NTNames#Philip"/>
        <collaboratesWith rdf:resource="http://semanticbible.org/ns/2006/NTNames#SimonPeter"/>
        <collaboratesWith rdf:resource="http://semanticbible.org/ns/2006/NTNames#Thaddaeus"/>
        <collaboratesWith rdf:resource="http://semanticbible.org/ns/2006/NTNames#Thomas"/>
        <ethnicity rdf:resource="http://semanticbible.org/ns/2006/NTNames#Galilean"/>
        <relativeOf rdf:resource="http://semanticbible.org/ns/2006/NTNames#SimonTheZealot"/>
        <siblingOf rdf:resource="http://semanticbible.org/ns/2006/NTNames#SimonPeter"/>
        <description rdf:datatype="http://www.w3.org/2001/XMLSchema#string">One of Jesus&apos; twelve apostles, and the first one called.</description>
        <occupation rdf:datatype="http://www.w3.org/2001/XMLSchema#string">apostle</occupation>
        <occupation rdf:datatype="http://www.w3.org/2001/XMLSchema#string">fisherman</occupation>
        <rdfs:comment xml:lang="en">One could infer that Andrew followed Jesus back from Bethany to Galilee in his early ministry, and therefore visited Cana and Capernaum. But this is not explicitly described.</rdfs:comment>
        <rdfs:label xml:lang="en">Andrew</rdfs:label>
    </owl:NamedIndividual>
    


    <!-- http://semanticbible.org/ns/2006/NTNames#Andronicus -->

    <owl:NamedIndividual rdf:about="http://semanticbible.org/ns/2006/NTNames#Andronicus">
        <rdf:type rdf:resource="http://semanticbible.org/ns/2006/NTNames#Man"/>
        <collaboratesWith rdf:resource="http://semanticbible.org/ns/2006/NTNames#Junia"/>
        <collaboratesWith rdf:resource="http://semanticbible.org/ns/2006/NTNames#Paul"/>
        <knows rdf:resource="http://semanticbible.org/ns/2006/NTNames#Priscilla"/>
        <religiousBelief rdf:resource="http://semanticbible.org/ns/2006/NTNames#Christianity"/>
        <residentPlace rdf:resource="http://semanticbible.org/ns/2006/NTNames#Rome"/>
        <description rdf:datatype="http://www.w3.org/2001/XMLSchema#string">A Christian in Rome to whom Paul sent greetings</description>
        <hasOnlyGenealogyMention rdf:datatype="http://www.w3.org/2001/XMLSchema#boolean">false</hasOnlyGenealogyMention>
        <rdfs:comment xml:lang="en">Paul&apos;s description of Andronicus as &quot;my kinsman&quot; is taken in the general snese (e.g. coming from the same region), rather than literally. As a &quot;fellow-prisoner&quot;, he and Junia are assumed to be collaborators with Paul. </rdfs:comment>
        <rdfs:label xml:lang="en">Andronicus</rdfs:label>
    </owl:NamedIndividual>
    


    <!-- http://semanticbible.org/ns/2006/NTNames#Anna -->

    <owl:NamedIndividual rdf:about="http://semanticbible.org/ns/2006/NTNames#Anna">
        <rdf:type rdf:resource="http://semanticbible.org/ns/2006/NTNames#Woman"/>
        <childOf rdf:resource="http://semanticbible.org/ns/2006/NTNames#Phanuel"/>
        <ethnicity rdf:resource="http://semanticbible.org/ns/2006/NTNames#Jewish"/>
        <memberOf rdf:resource="http://semanticbible.org/ns/2006/NTNames#TribeOfAsher"/>
        <religiousBelief rdf:resource="http://semanticbible.org/ns/2006/NTNames#Judaism"/>
        <description rdf:datatype="http://www.w3.org/2001/XMLSchema#string">a prophetess who spoke about the infant Jesus in the temple</description>
        <hasOnlyGenealogyMention rdf:datatype="http://www.w3.org/2001/XMLSchema#boolean">false</hasOnlyGenealogyMention>
        <occupation rdf:datatype="http://www.w3.org/2001/XMLSchema#string">prophetess</occupation>
        <rdfs:label xml:lang="en">Anna</rdfs:label>
    </owl:NamedIndividual>
    


    <!-- http://semanticbible.org/ns/2006/NTNames#Annas -->

    <owl:NamedIndividual rdf:about="http://semanticbible.org/ns/2006/NTNames#Annas">
        <rdf:type rdf:resource="http://semanticbible.org/ns/2006/NTNames#Man"/>
        <collaboratesWith rdf:resource="http://semanticbible.org/ns/2006/NTNames#Caiaphas"/>
        <collaboratesWith rdf:resource="http://semanticbible.org/ns/2006/NTNames#JohnOfTheSanhedrin"/>
        <enemyOf rdf:resource="http://semanticbible.org/ns/2006/NTNames#JohnSonOfZebedee"/>
        <enemyOf rdf:resource="http://semanticbible.org/ns/2006/NTNames#SimonPeter"/>
        <memberOf rdf:resource="http://semanticbible.org/ns/2006/NTNames#Sanhedrin"/>
        <relativeOf rdf:resource="http://semanticbible.org/ns/2006/NTNames#AlexanderOfTheSanhedrin"/>
        <relativeOf rdf:resource="http://semanticbible.org/ns/2006/NTNames#Caiaphas"/>
        <relativeOf rdf:resource="http://semanticbible.org/ns/2006/NTNames#JohnOfTheSanhedrin"/>
        <description rdf:datatype="http://www.w3.org/2001/XMLSchema#string">Jewish high-priest (prior to Jesus&apos; ministry)</description>
        <occupation rdf:datatype="http://www.w3.org/2001/XMLSchema#string">Priestly leader</occupation>
        <rdfs:comment xml:lang="en">Annas&apos; highpriesthood ended in 15 AD, but he continued to be described as high-priest after his son-in-law, Caiaphas, had taken the position.</rdfs:comment>
        <rdfs:label xml:lang="en">Annas</rdfs:label>
    </owl:NamedIndividual>
    


    <!-- http://semanticbible.org/ns/2006/NTNames#Antioch -->

    <owl:NamedIndividual rdf:about="http://semanticbible.org/ns/2006/NTNames#Antioch">
        <rdf:type rdf:resource="http://semanticbible.org/ns/2006/NTNames#City"/>
        <location rdf:resource="http://semanticbible.org/ns/2006/NTNames#AntiochGeodata"/>
        <rdfs:label xml:lang="en">Antioch</rdfs:label>
    </owl:NamedIndividual>
    


    <!-- http://semanticbible.org/ns/2006/NTNames#AntiochGeodata -->

    <owl:NamedIndividual rdf:about="http://semanticbible.org/ns/2006/NTNames#AntiochGeodata">
        <rdf:type rdf:resource="http://semanticbible.org/ns/2006/NTNames#GeographicLocation"/>
        <altitude rdf:datatype="http://www.w3.org/2001/XMLSchema#int">0</altitude>
        <latitude rdf:datatype="http://www.w3.org/2001/XMLSchema#double">36.20712275818978</latitude>
        <longitude rdf:datatype="http://www.w3.org/2001/XMLSchema#double">36.16196869636812</longitude>
        <rdfs:label xml:lang="en">geodata for Antioch</rdfs:label>
    </owl:NamedIndividual>
    


    <!-- http://semanticbible.org/ns/2006/NTNames#AntiochInPisidia -->

    <owl:NamedIndividual rdf:about="http://semanticbible.org/ns/2006/NTNames#AntiochInPisidia">
        <rdf:type rdf:resource="http://semanticbible.org/ns/2006/NTNames#City"/>
        <location rdf:resource="http://semanticbible.org/ns/2006/NTNames#AntiochInPisidiaGeodata"/>
        <rdfs:comment xml:lang="en">This Antioch is located in the Pisidian region of Asia Minor, a different place from the town of the same name in Syria</rdfs:comment>
        <rdfs:label xml:lang="en">Antioch</rdfs:label>
        <rdfs:label xml:lang="en">Antioch in Pisidia</rdfs:label>
    </owl:NamedIndividual>
    


    <!-- http://semanticbible.org/ns/2006/NTNames#AntiochInPisidiaGeodata -->

    <owl:NamedIndividual rdf:about="http://semanticbible.org/ns/2006/NTNames#AntiochInPisidiaGeodata">
        <rdf:type rdf:resource="http://semanticbible.org/ns/2006/NTNames#GeographicLocation"/>
        <altitude rdf:datatype="http://www.w3.org/2001/XMLSchema#int">0</altitude>
        <latitude rdf:datatype="http://www.w3.org/2001/XMLSchema#double">38.35065381137431</latitude>
        <longitude rdf:datatype="http://www.w3.org/2001/XMLSchema#double">31.216030760332</longitude>
        <rdfs:label xml:lang="en">geodata for Antioch</rdfs:label>
    </owl:NamedIndividual>
    


    <!-- http://semanticbible.org/ns/2006/NTNames#Antipas -->

    <owl:NamedIndividual rdf:about="http://semanticbible.org/ns/2006/NTNames#Antipas">
        <rdf:type rdf:resource="http://semanticbible.org/ns/2006/NTNames#Man"/>
        <description rdf:datatype="http://www.w3.org/2001/XMLSchema#string">a martyr</description>
        <rdfs:label xml:lang="en">Antipas</rdfs:label>
    </owl:NamedIndividual>
    


    <!-- http://semanticbible.org/ns/2006/NTNames#Antipatris -->

    <owl:NamedIndividual rdf:about="http://semanticbible.org/ns/2006/NTNames#Antipatris">
        <rdf:type rdf:resource="http://semanticbible.org/ns/2006/NTNames#City"/>
        <location rdf:resource="http://semanticbible.org/ns/2006/NTNames#AntipatrisGeodata"/>
        <subregionOf rdf:resource="http://semanticbible.org/ns/2006/NTNames#Judea"/>
        <rdfs:label xml:lang="en">Antipatris</rdfs:label>
    </owl:NamedIndividual>
    


    <!-- http://semanticbible.org/ns/2006/NTNames#AntipatrisGeodata -->

    <owl:NamedIndividual rdf:about="http://semanticbible.org/ns/2006/NTNames#AntipatrisGeodata">
        <rdf:type rdf:resource="http://semanticbible.org/ns/2006/NTNames#GeographicLocation"/>
        <altitude rdf:datatype="http://www.w3.org/2001/XMLSchema#int">0</altitude>
        <latitude rdf:datatype="http://www.w3.org/2001/XMLSchema#double">32.10685678492184</latitude>
        <longitude rdf:datatype="http://www.w3.org/2001/XMLSchema#double">34.95460542969052</longitude>
        <rdfs:label xml:lang="en">geodata for Antipatris</rdfs:label>
    </owl:NamedIndividual>
    


    <!-- http://semanticbible.org/ns/2006/NTNames#Apelles -->

    <owl:NamedIndividual rdf:about="http://semanticbible.org/ns/2006/NTNames#Apelles">
        <rdf:type rdf:resource="http://semanticbible.org/ns/2006/NTNames#Man"/>
        <knows rdf:resource="http://semanticbible.org/ns/2006/NTNames#Paul"/>
        <knows rdf:resource="http://semanticbible.org/ns/2006/NTNames#Priscilla"/>
        <religiousBelief rdf:resource="http://semanticbible.org/ns/2006/NTNames#Christianity"/>
        <residentPlace rdf:resource="http://semanticbible.org/ns/2006/NTNames#Rome"/>
        <description rdf:datatype="http://www.w3.org/2001/XMLSchema#string">a Christian in Rome whom Paul greeted</description>
        <hasOnlyGenealogyMention rdf:datatype="http://www.w3.org/2001/XMLSchema#boolean">false</hasOnlyGenealogyMention>
        <rdfs:label xml:lang="en">Apelles</rdfs:label>
    </owl:NamedIndividual>
    


    <!-- http://semanticbible.org/ns/2006/NTNames#Apollonia -->

    <owl:NamedIndividual rdf:about="http://semanticbible.org/ns/2006/NTNames#Apollonia">
        <rdf:type rdf:resource="http://semanticbible.org/ns/2006/NTNames#City"/>
        <location rdf:resource="http://semanticbible.org/ns/2006/NTNames#ApolloniaGeodata"/>
        <subregionOf rdf:resource="http://semanticbible.org/ns/2006/NTNames#Macedonia"/>
        <rdfs:label xml:lang="en">Apollonia</rdfs:label>
    </owl:NamedIndividual>
    


    <!-- http://semanticbible.org/ns/2006/NTNames#ApolloniaGeodata -->

    <owl:NamedIndividual rdf:about="http://semanticbible.org/ns/2006/NTNames#ApolloniaGeodata">
        <rdf:type rdf:resource="http://semanticbible.org/ns/2006/NTNames#GeographicLocation"/>
        <altitude rdf:datatype="http://www.w3.org/2001/XMLSchema#int">0</altitude>
        <latitude rdf:datatype="http://www.w3.org/2001/XMLSchema#double">40.5876325134332</latitude>
        <longitude rdf:datatype="http://www.w3.org/2001/XMLSchema#double">23.35335168557564</longitude>
        <rdfs:label xml:lang="en">geodata for Apollonia</rdfs:label>
    </owl:NamedIndividual>
    


    <!-- http://semanticbible.org/ns/2006/NTNames#Apollos -->

    <owl:NamedIndividual rdf:about="http://semanticbible.org/ns/2006/NTNames#Apollos">
        <rdf:type rdf:resource="http://semanticbible.org/ns/2006/NTNames#Man"/>
        <collaboratesWith rdf:resource="http://semanticbible.org/ns/2006/NTNames#Aquila"/>
        <collaboratesWith rdf:resource="http://semanticbible.org/ns/2006/NTNames#Paul"/>
        <collaboratesWith rdf:resource="http://semanticbible.org/ns/2006/NTNames#Priscilla"/>
        <nativePlace rdf:resource="http://semanticbible.org/ns/2006/NTNames#Alexandria"/>
        <religiousBelief rdf:resource="http://semanticbible.org/ns/2006/NTNames#Christianity"/>
        <visitedPlace rdf:resource="http://semanticbible.org/ns/2006/NTNames#Corinth"/>
        <visitedPlace rdf:resource="http://semanticbible.org/ns/2006/NTNames#Ephesus"/>
        <description rdf:datatype="http://www.w3.org/2001/XMLSchema#string">an eloquent evangelist whose ministry was initially based only on the teachings of John the Baptist</description>
        <hasOnlyGenealogyMention rdf:datatype="http://www.w3.org/2001/XMLSchema#boolean">false</hasOnlyGenealogyMention>
        <rdfs:label xml:lang="en">Apollos</rdfs:label>
    </owl:NamedIndividual>
    


    <!-- http://semanticbible.org/ns/2006/NTNames#Apphia -->

    <owl:NamedIndividual rdf:about="http://semanticbible.org/ns/2006/NTNames#Apphia">
        <rdf:type rdf:resource="http://semanticbible.org/ns/2006/NTNames#Woman"/>
        <collaboratesWith rdf:resource="http://semanticbible.org/ns/2006/NTNames#Archippus"/>
        <religiousBelief rdf:resource="http://semanticbible.org/ns/2006/NTNames#Christianity"/>
        <spouseOf rdf:resource="http://semanticbible.org/ns/2006/NTNames#Philemon"/>
        <hasOnlyGenealogyMention rdf:datatype="http://www.w3.org/2001/XMLSchema#boolean">false</hasOnlyGenealogyMention>
        <rdfs:comment xml:lang="en">Being the spouseOf Philemon is implied by their mention together in the salutation of the Letter to Philemon, though it is not definite. 
Paul describes her as &quot;our sister&quot;, presumably in Christ rather than literally. See Philemon about ResidentPlace.</rdfs:comment>
        <rdfs:label xml:lang="en">Apphia</rdfs:label>
    </owl:NamedIndividual>
    


    <!-- http://semanticbible.org/ns/2006/NTNames#Appius -->

    <owl:NamedIndividual rdf:about="http://semanticbible.org/ns/2006/NTNames#Appius">
        <rdf:type rdf:resource="http://semanticbible.org/ns/2006/NTNames#City"/>
        <rdfs:label xml:lang="en">Appius</rdfs:label>
    </owl:NamedIndividual>
    


    <!-- http://semanticbible.org/ns/2006/NTNames#Aquila -->

    <owl:NamedIndividual rdf:about="http://semanticbible.org/ns/2006/NTNames#Aquila">
        <rdf:type rdf:resource="http://semanticbible.org/ns/2006/NTNames#Man"/>
        <collaboratesWith rdf:resource="http://semanticbible.org/ns/2006/NTNames#Apollos"/>
        <collaboratesWith rdf:resource="http://semanticbible.org/ns/2006/NTNames#Paul"/>
        <ethnicity rdf:resource="http://semanticbible.org/ns/2006/NTNames#Jewish"/>
        <nativePlace rdf:resource="http://semanticbible.org/ns/2006/NTNames#Pontus"/>
        <religiousBelief rdf:resource="http://semanticbible.org/ns/2006/NTNames#Christianity"/>
        <residentPlace rdf:resource="http://semanticbible.org/ns/2006/NTNames#Corinth"/>
        <residentPlace rdf:resource="http://semanticbible.org/ns/2006/NTNames#Ephesus"/>
        <residentPlace rdf:resource="http://semanticbible.org/ns/2006/NTNames#Rome"/>
        <spouseOf rdf:resource="http://semanticbible.org/ns/2006/NTNames#Priscilla"/>
        <description rdf:datatype="http://www.w3.org/2001/XMLSchema#string">a tentmaked converted by Paul who, together with his wife, became evangelists</description>
        <hasOnlyGenealogyMention rdf:datatype="http://www.w3.org/2001/XMLSchema#boolean">false</hasOnlyGenealogyMention>
        <occupation rdf:datatype="http://www.w3.org/2001/XMLSchema#string">tentmaker</occupation>
        <rdfs:label xml:lang="en">Aquila</rdfs:label>
    </owl:NamedIndividual>
    


    <!-- http://semanticbible.org/ns/2006/NTNames#Arabia -->

    <owl:NamedIndividual rdf:about="http://semanticbible.org/ns/2006/NTNames#Arabia">
        <rdf:type rdf:resource="http://semanticbible.org/ns/2006/NTNames#Region"/>
        <rdfs:label xml:lang="en">Arabia</rdfs:label>
    </owl:NamedIndividual>
    


    <!-- http://semanticbible.org/ns/2006/NTNames#Arabians -->

    <owl:NamedIndividual rdf:about="http://semanticbible.org/ns/2006/NTNames#Arabians">
        <rdf:type rdf:resource="http://semanticbible.org/ns/2006/NTNames#EthnicGroup"/>
        <rdfs:label xml:lang="en">Arabians</rdfs:label>
    </owl:NamedIndividual>
    


    <!-- http://semanticbible.org/ns/2006/NTNames#Aramaic -->

    <owl:NamedIndividual rdf:about="http://semanticbible.org/ns/2006/NTNames#Aramaic">
        <rdf:type rdf:resource="http://semanticbible.org/ns/2006/NTNames#NaturalLanguage"/>
        <rdfs:label xml:lang="en">Aramaic</rdfs:label>
    </owl:NamedIndividual>
    


    <!-- http://semanticbible.org/ns/2006/NTNames#Archelaus -->

    <owl:NamedIndividual rdf:about="http://semanticbible.org/ns/2006/NTNames#Archelaus">
        <rdf:type rdf:resource="http://semanticbible.org/ns/2006/NTNames#Man"/>
        <childOf rdf:resource="http://semanticbible.org/ns/2006/NTNames#HerodTheGreat"/>
        <collaboratesWith rdf:resource="http://semanticbible.org/ns/2006/NTNames#PontiusPilate"/>
        <siblingOf rdf:resource="http://semanticbible.org/ns/2006/NTNames#HerodAntipas"/>
        <siblingOf rdf:resource="http://semanticbible.org/ns/2006/NTNames#PhilipSonOfHerod"/>
        <description rdf:datatype="http://www.w3.org/2001/XMLSchema#string">one of the sons of Herod the Great who ruled Judea for a time</description>
        <occupation rdf:datatype="http://www.w3.org/2001/XMLSchema#string">ruler</occupation>
        <rdfs:label xml:lang="en">Archelaus</rdfs:label>
    </owl:NamedIndividual>
    


    <!-- http://semanticbible.org/ns/2006/NTNames#Archippus -->

    <owl:NamedIndividual rdf:about="http://semanticbible.org/ns/2006/NTNames#Archippus">
        <rdf:type rdf:resource="http://semanticbible.org/ns/2006/NTNames#Man"/>
        <collaboratesWith rdf:resource="http://semanticbible.org/ns/2006/NTNames#Apphia"/>
        <collaboratesWith rdf:resource="http://semanticbible.org/ns/2006/NTNames#Philemon"/>
        <description rdf:datatype="http://www.w3.org/2001/XMLSchema#string">a Christian in Colossae whom Paul describes as &quot;our fellow soldier&quot;</description>
        <rdfs:comment xml:lang="en">Paul describes Archippus as &quot;our fellow soldier&quot; in Philemon 1:2, perhaps based on service together in Ephesus (RWP).</rdfs:comment>
        <rdfs:label xml:lang="en">Archippus</rdfs:label>
    </owl:NamedIndividual>
    


    <!-- http://semanticbible.org/ns/2006/NTNames#Areopagite -->

    <owl:NamedIndividual rdf:about="http://semanticbible.org/ns/2006/NTNames#Areopagite">
        <rdf:type rdf:resource="http://semanticbible.org/ns/2006/NTNames#PoliticalAttribute"/>
        <rdfs:label xml:lang="en">Areopagite</rdfs:label>
    </owl:NamedIndividual>
    


    <!-- http://semanticbible.org/ns/2006/NTNames#Areopagus -->

    <owl:NamedIndividual rdf:about="http://semanticbible.org/ns/2006/NTNames#Areopagus">
        <rdf:type rdf:resource="http://semanticbible.org/ns/2006/NTNames#PoliticalOrganization"/>
        <rdfs:label xml:lang="en">Areopagus</rdfs:label>
    </owl:NamedIndividual>
    


    <!-- http://semanticbible.org/ns/2006/NTNames#Aretas -->

    <owl:NamedIndividual rdf:about="http://semanticbible.org/ns/2006/NTNames#Aretas">
        <rdf:type rdf:resource="http://semanticbible.org/ns/2006/NTNames#Man"/>
        <relativeOf rdf:resource="http://semanticbible.org/ns/2006/NTNames#HerodAntipas"/>
        <description rdf:datatype="http://www.w3.org/2001/XMLSchema#string">a king in Paul&apos;s time whose rule included Damascus</description>
        <occupation rdf:datatype="http://www.w3.org/2001/XMLSchema#string">king</occupation>
        <rdfs:label xml:lang="en">Aretas</rdfs:label>
    </owl:NamedIndividual>
    


    <!-- http://semanticbible.org/ns/2006/NTNames#Arimathea -->

    <owl:NamedIndividual rdf:about="http://semanticbible.org/ns/2006/NTNames#Arimathea">
        <rdf:type rdf:resource="http://semanticbible.org/ns/2006/NTNames#City"/>
        <location rdf:resource="http://semanticbible.org/ns/2006/NTNames#ArimatheaGeodata"/>
        <subregionOf rdf:resource="http://semanticbible.org/ns/2006/NTNames#Judea"/>
        <rdfs:comment xml:lang="en">Arimathea is known as the native place of Joseph, a member of the Sanhedrin and a disciple who put Jesus&apos; body in his own tomb after the crucifixion.</rdfs:comment>
        <rdfs:label xml:lang="en">Arimathea</rdfs:label>
    </owl:NamedIndividual>
    


    <!-- http://semanticbible.org/ns/2006/NTNames#ArimatheaGeodata -->

    <owl:NamedIndividual rdf:about="http://semanticbible.org/ns/2006/NTNames#ArimatheaGeodata">
        <rdf:type rdf:resource="http://semanticbible.org/ns/2006/NTNames#GeographicLocation"/>
        <altitude rdf:datatype="http://www.w3.org/2001/XMLSchema#int">0</altitude>
        <latitude rdf:datatype="http://www.w3.org/2001/XMLSchema#double">31.97778934332933</latitude>
        <longitude rdf:datatype="http://www.w3.org/2001/XMLSchema#double">34.94445199398103</longitude>
        <rdfs:label xml:lang="en">geodata for Arimathea</rdfs:label>
    </owl:NamedIndividual>
    


    <!-- http://semanticbible.org/ns/2006/NTNames#Aristarchus -->

    <owl:NamedIndividual rdf:about="http://semanticbible.org/ns/2006/NTNames#Aristarchus">
        <rdf:type rdf:resource="http://semanticbible.org/ns/2006/NTNames#Man"/>
        <collaboratesWith rdf:resource="http://semanticbible.org/ns/2006/NTNames#GaiusOfDerbe"/>
        <collaboratesWith rdf:resource="http://semanticbible.org/ns/2006/NTNames#GaiusOfMacedonia"/>
        <collaboratesWith rdf:resource="http://semanticbible.org/ns/2006/NTNames#Paul"/>
        <collaboratesWith rdf:resource="http://semanticbible.org/ns/2006/NTNames#Secundus"/>
        <collaboratesWith rdf:resource="http://semanticbible.org/ns/2006/NTNames#Sopater"/>
        <collaboratesWith rdf:resource="http://semanticbible.org/ns/2006/NTNames#Timothy"/>
        <collaboratesWith rdf:resource="http://semanticbible.org/ns/2006/NTNames#Trophimus"/>
        <collaboratesWith rdf:resource="http://semanticbible.org/ns/2006/NTNames#Tychicus"/>
        <ethnicity rdf:resource="http://semanticbible.org/ns/2006/NTNames#Macedonian"/>
        <religiousBelief rdf:resource="http://semanticbible.org/ns/2006/NTNames#Christianity"/>
        <visitedPlace rdf:resource="http://semanticbible.org/ns/2006/NTNames#Ephesus"/>
        <description rdf:datatype="http://www.w3.org/2001/XMLSchema#string">a traveling companion of Paul</description>
        <hasOnlyGenealogyMention rdf:datatype="http://www.w3.org/2001/XMLSchema#boolean">false</hasOnlyGenealogyMention>
        <rdfs:label xml:lang="en">Aristarchus</rdfs:label>
    </owl:NamedIndividual>
    


    <!-- http://semanticbible.org/ns/2006/NTNames#Aristobulus -->

    <owl:NamedIndividual rdf:about="http://semanticbible.org/ns/2006/NTNames#Aristobulus">
        <rdf:type rdf:resource="http://semanticbible.org/ns/2006/NTNames#Man"/>
        <residentPlace rdf:resource="http://semanticbible.org/ns/2006/NTNames#Rome"/>
        <description rdf:datatype="http://www.w3.org/2001/XMLSchema#string">an inhabitant of Rome</description>
        <hasOnlyGenealogyMention rdf:datatype="http://www.w3.org/2001/XMLSchema#boolean">false</hasOnlyGenealogyMention>
        <rdfs:comment xml:lang="en">Paul addresses &quot;the family/household of Aristobulus&quot;, which may refer to slaves: so we have no evidence about the beliefs or other attributes of Aristobulus himself, other than his residence in Rome. One of the grandsons of Herod the Great had this name, though the name was common enough that this need not be the same man. </rdfs:comment>
        <rdfs:label xml:lang="en">Aristobulus</rdfs:label>
    </owl:NamedIndividual>
    


    <!-- http://semanticbible.org/ns/2006/NTNames#Armageddon -->

    <owl:NamedIndividual rdf:about="http://semanticbible.org/ns/2006/NTNames#Armageddon">
        <rdf:type rdf:resource="http://semanticbible.org/ns/2006/NTNames#City"/>
        <rdfs:label xml:lang="en">Armageddon</rdfs:label>
    </owl:NamedIndividual>
    


    <!-- http://semanticbible.org/ns/2006/NTNames#Arni -->

    <owl:NamedIndividual rdf:about="http://semanticbible.org/ns/2006/NTNames#Arni">
        <rdf:type rdf:resource="http://semanticbible.org/ns/2006/NTNames#Man"/>
        <childOf rdf:resource="http://semanticbible.org/ns/2006/NTNames#Hezron"/>
        <ethnicity rdf:resource="http://semanticbible.org/ns/2006/NTNames#Jewish"/>
        <parentOf rdf:resource="http://semanticbible.org/ns/2006/NTNames#Admin"/>
        <possiblySamePersonAs rdf:resource="http://semanticbible.org/ns/2006/NTNames#Ram"/>
        <description rdf:datatype="http://www.w3.org/2001/XMLSchema#string">One of the ancestors of Jesus mentioned in Luke&apos;s geneaology</description>
        <hasOnlyGenealogyMention rdf:datatype="http://www.w3.org/2001/XMLSchema#boolean">true</hasOnlyGenealogyMention>
        <rdfs:comment xml:lang="en">Likely a variant form of Ram, as Hezron&apos;s son is called in Matthew&apos;s genealogy. </rdfs:comment>
        <rdfs:label xml:lang="en">Arni</rdfs:label>
    </owl:NamedIndividual>
    


    <!-- http://semanticbible.org/ns/2006/NTNames#Arphaxad -->

    <owl:NamedIndividual rdf:about="http://semanticbible.org/ns/2006/NTNames#Arphaxad">
        <rdf:type rdf:resource="http://semanticbible.org/ns/2006/NTNames#Man"/>
        <childOf rdf:resource="http://semanticbible.org/ns/2006/NTNames#Shem"/>
        <parentOf rdf:resource="http://semanticbible.org/ns/2006/NTNames#CainanSonOfArphaxad"/>
        <description rdf:datatype="http://www.w3.org/2001/XMLSchema#string">One of the ancestors of Jesus mentioned in Luke&apos;s geneaology</description>
        <hasOnlyGenealogyMention rdf:datatype="http://www.w3.org/2001/XMLSchema#boolean">true</hasOnlyGenealogyMention>
        <rdfs:label xml:lang="en">Arphaxad</rdfs:label>
    </owl:NamedIndividual>
    


    <!-- http://semanticbible.org/ns/2006/NTNames#Artemas -->

    <owl:NamedIndividual rdf:about="http://semanticbible.org/ns/2006/NTNames#Artemas">
        <rdf:type rdf:resource="http://semanticbible.org/ns/2006/NTNames#Man"/>
        <collaboratesWith rdf:resource="http://semanticbible.org/ns/2006/NTNames#Paul"/>
        <rdfs:label xml:lang="en">Artemas</rdfs:label>
    </owl:NamedIndividual>
    


    <!-- http://semanticbible.org/ns/2006/NTNames#Artemis -->

    <owl:NamedIndividual rdf:about="http://semanticbible.org/ns/2006/NTNames#Artemis">
        <rdf:type rdf:resource="http://semanticbible.org/ns/2006/NTNames#SupernaturalBeing"/>
        <rdfs:label xml:lang="en">Artemis</rdfs:label>
    </owl:NamedIndividual>
    


    <!-- http://semanticbible.org/ns/2006/NTNames#Asaph -->

    <owl:NamedIndividual rdf:about="http://semanticbible.org/ns/2006/NTNames#Asaph">
        <rdf:type rdf:resource="http://semanticbible.org/ns/2006/NTNames#Man"/>
        <childOf rdf:resource="http://semanticbible.org/ns/2006/NTNames#AbijahSonOfRehoboam"/>
        <ethnicity rdf:resource="http://semanticbible.org/ns/2006/NTNames#Jewish"/>
        <parentOf rdf:resource="http://semanticbible.org/ns/2006/NTNames#Jehoshaphat"/>
        <relativeOf rdf:resource="http://semanticbible.org/ns/2006/NTNames#AbijahSonOfRehoboam"/>
        <description rdf:datatype="http://www.w3.org/2001/XMLSchema#string">One of the ancestors of Jesus mentioned in Matthew&apos;s geneaology</description>
        <hasOnlyGenealogyMention rdf:datatype="http://www.w3.org/2001/XMLSchema#boolean">true</hasOnlyGenealogyMention>
        <occupation rdf:datatype="http://www.w3.org/2001/XMLSchema#string">king of Judah</occupation>
        <rdfs:comment xml:lang="en">Not the same as the psalmist and leader of King David&apos;s choir in 1Chr.6.39.</rdfs:comment>
        <rdfs:label xml:lang="en">Asaph</rdfs:label>
    </owl:NamedIndividual>
    


    <!-- http://semanticbible.org/ns/2006/NTNames#Asher -->

    <owl:NamedIndividual rdf:about="http://semanticbible.org/ns/2006/NTNames#Asher">
        <rdf:type rdf:resource="http://semanticbible.org/ns/2006/NTNames#Man"/>
        <childOf rdf:resource="http://semanticbible.org/ns/2006/NTNames#Jacob"/>
        <ethnicity rdf:resource="http://semanticbible.org/ns/2006/NTNames#Jewish"/>
        <siblingOf rdf:resource="http://semanticbible.org/ns/2006/NTNames#Gad"/>
        <description rdf:datatype="http://www.w3.org/2001/XMLSchema#string">One of the 12 Patriarchs of Israel</description>
        <rdfs:comment xml:lang="en">One of the sons of Judah</rdfs:comment>
        <rdfs:label xml:lang="en">Asher</rdfs:label>
    </owl:NamedIndividual>
    


    <!-- http://semanticbible.org/ns/2006/NTNames#Asia -->

    <owl:NamedIndividual rdf:about="http://semanticbible.org/ns/2006/NTNames#Asia">
        <rdf:type rdf:resource="http://semanticbible.org/ns/2006/NTNames#GeopoliticalArea"/>
        <visitedPlaceOf rdf:resource="http://semanticbible.org/ns/2006/NTNames#Epaenetus"/>
        <rdfs:label xml:lang="en">Asia</rdfs:label>
    </owl:NamedIndividual>
    


    <!-- http://semanticbible.org/ns/2006/NTNames#Asians -->

    <owl:NamedIndividual rdf:about="http://semanticbible.org/ns/2006/NTNames#Asians">
        <rdf:type rdf:resource="http://semanticbible.org/ns/2006/NTNames#EthnicGroup"/>
        <rdfs:label xml:lang="en">Asians</rdfs:label>
    </owl:NamedIndividual>
    


    <!-- http://semanticbible.org/ns/2006/NTNames#Asiarchs -->

    <owl:NamedIndividual rdf:about="http://semanticbible.org/ns/2006/NTNames#Asiarchs">
        <rdf:type rdf:resource="http://semanticbible.org/ns/2006/NTNames#GroupOfPeople"/>
        <rdfs:label xml:lang="en">Asiarchs</rdfs:label>
    </owl:NamedIndividual>
    


    <!-- http://semanticbible.org/ns/2006/NTNames#Assassins -->

    <owl:NamedIndividual rdf:about="http://semanticbible.org/ns/2006/NTNames#Assassins">
        <rdf:type rdf:resource="http://semanticbible.org/ns/2006/NTNames#PoliticalOrganization"/>
        <rdfs:label xml:lang="en">Assassins</rdfs:label>
    </owl:NamedIndividual>
    


    <!-- http://semanticbible.org/ns/2006/NTNames#Assos -->

    <owl:NamedIndividual rdf:about="http://semanticbible.org/ns/2006/NTNames#Assos">
        <rdf:type rdf:resource="http://semanticbible.org/ns/2006/NTNames#City"/>
        <location rdf:resource="http://semanticbible.org/ns/2006/NTNames#AssosGeodata"/>
        <rdfs:label xml:lang="en">Assos</rdfs:label>
    </owl:NamedIndividual>
    


    <!-- http://semanticbible.org/ns/2006/NTNames#AssosGeodata -->

    <owl:NamedIndividual rdf:about="http://semanticbible.org/ns/2006/NTNames#AssosGeodata">
        <rdf:type rdf:resource="http://semanticbible.org/ns/2006/NTNames#GeographicLocation"/>
        <altitude rdf:datatype="http://www.w3.org/2001/XMLSchema#int">0</altitude>
        <latitude rdf:datatype="http://www.w3.org/2001/XMLSchema#double">39.48955031303715</latitude>
        <longitude rdf:datatype="http://www.w3.org/2001/XMLSchema#double">26.33586734239906</longitude>
        <rdfs:label xml:lang="en">geodata for Assos</rdfs:label>
    </owl:NamedIndividual>
    


    <!-- http://semanticbible.org/ns/2006/NTNames#Asyncritus -->

    <owl:NamedIndividual rdf:about="http://semanticbible.org/ns/2006/NTNames#Asyncritus">
        <rdf:type rdf:resource="http://semanticbible.org/ns/2006/NTNames#Man"/>
        <knows rdf:resource="http://semanticbible.org/ns/2006/NTNames#Paul"/>
        <knows rdf:resource="http://semanticbible.org/ns/2006/NTNames#Priscilla"/>
        <religiousBelief rdf:resource="http://semanticbible.org/ns/2006/NTNames#Christianity"/>
        <residentPlace rdf:resource="http://semanticbible.org/ns/2006/NTNames#Rome"/>
        <description rdf:datatype="http://www.w3.org/2001/XMLSchema#string">a Roman to whom Paul sent greetings</description>
        <hasOnlyGenealogyMention rdf:datatype="http://www.w3.org/2001/XMLSchema#boolean">false</hasOnlyGenealogyMention>
        <rdfs:label xml:lang="en">Asyncritus</rdfs:label>
    </owl:NamedIndividual>
    


    <!-- http://semanticbible.org/ns/2006/NTNames#Athenians -->

    <owl:NamedIndividual rdf:about="http://semanticbible.org/ns/2006/NTNames#Athenians">
        <rdf:type rdf:resource="http://semanticbible.org/ns/2006/NTNames#ResidenceGroup"/>
        <rdfs:label xml:lang="en">Athenians</rdfs:label>
    </owl:NamedIndividual>
    


    <!-- http://semanticbible.org/ns/2006/NTNames#Athens -->

    <owl:NamedIndividual rdf:about="http://semanticbible.org/ns/2006/NTNames#Athens">
        <rdf:type rdf:resource="http://semanticbible.org/ns/2006/NTNames#City"/>
        <residentPlaceOf rdf:resource="http://semanticbible.org/ns/2006/NTNames#Damaris"/>
        <rdfs:label xml:lang="en">Athens</rdfs:label>
    </owl:NamedIndividual>
    


    <!-- http://semanticbible.org/ns/2006/NTNames#Attalia -->

    <owl:NamedIndividual rdf:about="http://semanticbible.org/ns/2006/NTNames#Attalia">
        <rdf:type rdf:resource="http://semanticbible.org/ns/2006/NTNames#City"/>
        <location rdf:resource="http://semanticbible.org/ns/2006/NTNames#AttaliaGeodata"/>
        <rdfs:label xml:lang="en">Attalia</rdfs:label>
    </owl:NamedIndividual>
    


    <!-- http://semanticbible.org/ns/2006/NTNames#AttaliaGeodata -->

    <owl:NamedIndividual rdf:about="http://semanticbible.org/ns/2006/NTNames#AttaliaGeodata">
        <rdf:type rdf:resource="http://semanticbible.org/ns/2006/NTNames#GeographicLocation"/>
        <altitude rdf:datatype="http://www.w3.org/2001/XMLSchema#int">0</altitude>
        <latitude rdf:datatype="http://www.w3.org/2001/XMLSchema#double">36.91461876374842</latitude>
        <longitude rdf:datatype="http://www.w3.org/2001/XMLSchema#double">30.7182409422051</longitude>
        <rdfs:label xml:lang="en">geodata for Attalia</rdfs:label>
    </owl:NamedIndividual>
    


    <!-- http://semanticbible.org/ns/2006/NTNames#AugustanCohort -->

    <owl:NamedIndividual rdf:about="http://semanticbible.org/ns/2006/NTNames#AugustanCohort">
        <rdf:type rdf:resource="http://semanticbible.org/ns/2006/NTNames#PoliticalOrganization"/>
        <rdfs:comment xml:lang="en">A Roman legion.</rdfs:comment>
        <rdfs:label xml:lang="en">Augustan Cohort</rdfs:label>
    </owl:NamedIndividual>
    


    <!-- http://semanticbible.org/ns/2006/NTNames#Augustus -->

    <owl:NamedIndividual rdf:about="http://semanticbible.org/ns/2006/NTNames#Augustus">
        <rdf:type rdf:resource="http://semanticbible.org/ns/2006/NTNames#Man"/>
        <description rdf:datatype="http://www.w3.org/2001/XMLSchema#string">Emperor of Rome at the time of Jesus&apos; birth</description>
        <occupation rdf:datatype="http://www.w3.org/2001/XMLSchema#string">emperor</occupation>
        <rdfs:label xml:lang="en">Augustus</rdfs:label>
    </owl:NamedIndividual>
    


    <!-- http://semanticbible.org/ns/2006/NTNames#Azor -->

    <owl:NamedIndividual rdf:about="http://semanticbible.org/ns/2006/NTNames#Azor">
        <rdf:type rdf:resource="http://semanticbible.org/ns/2006/NTNames#Man"/>
        <childOf rdf:resource="http://semanticbible.org/ns/2006/NTNames#EliakimSonOfAbiud"/>
        <ethnicity rdf:resource="http://semanticbible.org/ns/2006/NTNames#Jewish"/>
        <parentOf rdf:resource="http://semanticbible.org/ns/2006/NTNames#Zadok"/>
        <rdfs:label xml:lang="en">Azor</rdfs:label>
    </owl:NamedIndividual>
    


    <!-- http://semanticbible.org/ns/2006/NTNames#Azotus -->

    <owl:NamedIndividual rdf:about="http://semanticbible.org/ns/2006/NTNames#Azotus">
        <rdf:type rdf:resource="http://semanticbible.org/ns/2006/NTNames#City"/>
        <subregionOf rdf:resource="http://semanticbible.org/ns/2006/NTNames#Judea"/>
        <rdfs:label xml:lang="en">Azotus</rdfs:label>
    </owl:NamedIndividual>
    


    <!-- http://semanticbible.org/ns/2006/NTNames#Babylon -->

    <owl:NamedIndividual rdf:about="http://semanticbible.org/ns/2006/NTNames#Babylon">
        <rdf:type rdf:resource="http://semanticbible.org/ns/2006/NTNames#City"/>
        <location rdf:resource="http://semanticbible.org/ns/2006/NTNames#BabylonGeodata"/>
        <rdfs:comment xml:lang="en">Babylon also has a metaphorical usage as a symbol of the world system opposed to God</rdfs:comment>
        <rdfs:label xml:lang="en">Babylon</rdfs:label>
    </owl:NamedIndividual>
    


    <!-- http://semanticbible.org/ns/2006/NTNames#BabylonGeodata -->

    <owl:NamedIndividual rdf:about="http://semanticbible.org/ns/2006/NTNames#BabylonGeodata">
        <rdf:type rdf:resource="http://semanticbible.org/ns/2006/NTNames#GeographicLocation"/>
        <altitude rdf:datatype="http://www.w3.org/2001/XMLSchema#int">0</altitude>
        <latitude rdf:datatype="http://www.w3.org/2001/XMLSchema#double">32.53660983263659</latitude>
        <longitude rdf:datatype="http://www.w3.org/2001/XMLSchema#double">44.42007455918414</longitude>
        <rdfs:label xml:lang="en">geodata for Babylon</rdfs:label>
    </owl:NamedIndividual>
    


    <!-- http://semanticbible.org/ns/2006/NTNames#Balaam -->

    <owl:NamedIndividual rdf:about="http://semanticbible.org/ns/2006/NTNames#Balaam">
        <rdf:type rdf:resource="http://semanticbible.org/ns/2006/NTNames#Man"/>
        <childOf rdf:resource="http://semanticbible.org/ns/2006/NTNames#Beor"/>
        <description rdf:datatype="http://www.w3.org/2001/XMLSchema#string">an Old Testament figure and negative example</description>
        <rdfs:label xml:lang="en">Balaam</rdfs:label>
    </owl:NamedIndividual>
    


    <!-- http://semanticbible.org/ns/2006/NTNames#Balak -->

    <owl:NamedIndividual rdf:about="http://semanticbible.org/ns/2006/NTNames#Balak">
        <rdf:type rdf:resource="http://semanticbible.org/ns/2006/NTNames#Man"/>
        <ethnicity rdf:resource="http://semanticbible.org/ns/2006/NTNames#Moabite"/>
        <description rdf:datatype="http://www.w3.org/2001/XMLSchema#string">king of Moab who hired Balaam</description>
        <occupation rdf:datatype="http://www.w3.org/2001/XMLSchema#string">king</occupation>
        <rdfs:label xml:lang="en">Balak</rdfs:label>
    </owl:NamedIndividual>
    


    <!-- http://semanticbible.org/ns/2006/NTNames#Bar-Jesus -->

    <owl:NamedIndividual rdf:about="http://semanticbible.org/ns/2006/NTNames#Bar-Jesus">
        <rdf:type rdf:resource="http://semanticbible.org/ns/2006/NTNames#Man"/>
        <antagonistOf rdf:resource="http://semanticbible.org/ns/2006/NTNames#Paul"/>
        <antagonistOf rdf:resource="http://semanticbible.org/ns/2006/NTNames#Silas"/>
        <ethnicity rdf:resource="http://semanticbible.org/ns/2006/NTNames#Jewish"/>
        <knows rdf:resource="http://semanticbible.org/ns/2006/NTNames#Paul"/>
        <knows rdf:resource="http://semanticbible.org/ns/2006/NTNames#SergiusPaulus"/>
        <knows rdf:resource="http://semanticbible.org/ns/2006/NTNames#Silas"/>
        <description rdf:datatype="http://www.w3.org/2001/XMLSchema#string">a magician and false prophet who Paul and Silas encountered on Cyprus</description>
        <occupation rdf:datatype="http://www.w3.org/2001/XMLSchema#string">magician</occupation>
        <rdfs:comment xml:lang="en">Elymas is a transliteration of an Aramaic or Arabic word equivalent to &apos;magician&apos;.</rdfs:comment>
        <rdfs:label xml:lang="en">Bar-Jesus</rdfs:label>
    </owl:NamedIndividual>
    


    <!-- http://semanticbible.org/ns/2006/NTNames#Barabbas -->

    <owl:NamedIndividual rdf:about="http://semanticbible.org/ns/2006/NTNames#Barabbas">
        <rdf:type rdf:resource="http://semanticbible.org/ns/2006/NTNames#Man"/>
        <collaboratesWith rdf:resource="http://semanticbible.org/ns/2006/NTNames#Agabus"/>
        <ethnicity rdf:resource="http://semanticbible.org/ns/2006/NTNames#Jewish"/>
        <description rdf:datatype="http://www.w3.org/2001/XMLSchema#string">a criminal, released in place of Jesus</description>
        <rdfs:label xml:lang="en">Barabbas</rdfs:label>
    </owl:NamedIndividual>
    


    <!-- http://semanticbible.org/ns/2006/NTNames#Barachiah -->

    <owl:NamedIndividual rdf:about="http://semanticbible.org/ns/2006/NTNames#Barachiah">
        <rdf:type rdf:resource="http://semanticbible.org/ns/2006/NTNames#Man"/>
        <ethnicity rdf:resource="http://semanticbible.org/ns/2006/NTNames#Jewish"/>
        <parentOf rdf:resource="http://semanticbible.org/ns/2006/NTNames#ZechariahSonOfBarachiah"/>
        <rdfs:label xml:lang="en">Barachiah</rdfs:label>
    </owl:NamedIndividual>
    


    <!-- http://semanticbible.org/ns/2006/NTNames#Barak -->

    <owl:NamedIndividual rdf:about="http://semanticbible.org/ns/2006/NTNames#Barak">
        <rdf:type rdf:resource="http://semanticbible.org/ns/2006/NTNames#Man"/>
        <description rdf:datatype="http://www.w3.org/2001/XMLSchema#string">an Old Testament military leader from the book of Judges</description>
        <name_en rdf:datatype="http://www.w3.org/2001/XMLSchema#string">Barak</name_en>
        <occupation rdf:datatype="http://www.w3.org/2001/XMLSchema#string">general</occupation>
        <rdfs:label xml:lang="en">Barak</rdfs:label>
    </owl:NamedIndividual>
    


    <!-- http://semanticbible.org/ns/2006/NTNames#Barnabas -->

    <owl:NamedIndividual rdf:about="http://semanticbible.org/ns/2006/NTNames#Barnabas">
        <rdf:type rdf:resource="http://semanticbible.org/ns/2006/NTNames#Man"/>
        <collaboratesWith rdf:resource="http://semanticbible.org/ns/2006/NTNames#JohnMark"/>
        <collaboratesWith rdf:resource="http://semanticbible.org/ns/2006/NTNames#JudasOfAntioch"/>
        <collaboratesWith rdf:resource="http://semanticbible.org/ns/2006/NTNames#LuciusOfCyrene"/>
        <collaboratesWith rdf:resource="http://semanticbible.org/ns/2006/NTNames#Manaen"/>
        <collaboratesWith rdf:resource="http://semanticbible.org/ns/2006/NTNames#Paul"/>
        <collaboratesWith rdf:resource="http://semanticbible.org/ns/2006/NTNames#Silas"/>
        <collaboratesWith rdf:resource="http://semanticbible.org/ns/2006/NTNames#SimeonNiger"/>
        <collaboratesWith rdf:resource="http://semanticbible.org/ns/2006/NTNames#SimonPeter"/>
        <ethnicity rdf:resource="http://semanticbible.org/ns/2006/NTNames#Levite"/>
        <relativeOf rdf:resource="http://semanticbible.org/ns/2006/NTNames#JohnMark"/>
        <siblingOf rdf:resource="http://semanticbible.org/ns/2006/NTNames#MaryMotherOfJohnMark"/>
        <description rdf:datatype="http://www.w3.org/2001/XMLSchema#string">a close companion of the Apostle Paul</description>
        <occupation rdf:datatype="http://www.w3.org/2001/XMLSchema#string">apostle</occupation>
        <rdfs:label xml:lang="en">Barnabas</rdfs:label>
    </owl:NamedIndividual>
    


    <!-- http://semanticbible.org/ns/2006/NTNames#Bartholomew -->

    <owl:NamedIndividual rdf:about="http://semanticbible.org/ns/2006/NTNames#Bartholomew">
        <rdf:type rdf:resource="http://semanticbible.org/ns/2006/NTNames#Man"/>
        <collaboratesWith rdf:resource="http://semanticbible.org/ns/2006/NTNames#Andrew"/>
        <ethnicity rdf:resource="http://semanticbible.org/ns/2006/NTNames#Galilean"/>
        <description rdf:datatype="http://www.w3.org/2001/XMLSchema#string">One of Jesus&apos; twelve apostles</description>
        <occupation rdf:datatype="http://www.w3.org/2001/XMLSchema#string">apostle</occupation>
        <rdfs:comment xml:lang="en">Many believe Bartholemew is another name for Nathanael, though their identity is deduced rather than stated.</rdfs:comment>
        <rdfs:label xml:lang="en">Bartholomew</rdfs:label>
    </owl:NamedIndividual>
    


    <!-- http://semanticbible.org/ns/2006/NTNames#Bartimaeus -->

    <owl:NamedIndividual rdf:about="http://semanticbible.org/ns/2006/NTNames#Bartimaeus">
        <rdf:type rdf:resource="http://semanticbible.org/ns/2006/NTNames#Man"/>
        <childOf rdf:resource="http://semanticbible.org/ns/2006/NTNames#Timaeus"/>
        <description rdf:datatype="http://www.w3.org/2001/XMLSchema#string">a blind beggar whom Jesus healed</description>
        <rdfs:label xml:lang="en">Bartimaeus</rdfs:label>
    </owl:NamedIndividual>
    


    <!-- http://semanticbible.org/ns/2006/NTNames#Bathsheba -->

    <owl:NamedIndividual rdf:about="http://semanticbible.org/ns/2006/NTNames#Bathsheba">
        <rdf:type rdf:resource="http://semanticbible.org/ns/2006/NTNames#Woman"/>
        <ethnicity rdf:resource="http://semanticbible.org/ns/2006/NTNames#Jewish"/>
        <parentOf rdf:resource="http://semanticbible.org/ns/2006/NTNames#Solomon"/>
        <spouseOf rdf:resource="http://semanticbible.org/ns/2006/NTNames#David"/>
        <spouseOf rdf:resource="http://semanticbible.org/ns/2006/NTNames#Uriah"/>
        <hasOnlyGenealogyMention rdf:datatype="http://www.w3.org/2001/XMLSchema#boolean">true</hasOnlyGenealogyMention>
        <rdfs:comment xml:lang="en">Not named in the New Testament, but referred to in Matt.1.6 as &quot;the wife of Uriah&quot;. Since Uriah was a Hittite, it&apos;s not clear what her religiousBelief might have been. </rdfs:comment>
        <rdfs:label xml:lang="en">Bathsheba</rdfs:label>
    </owl:NamedIndividual>
    


    <!-- http://semanticbible.org/ns/2006/NTNames#Benjamin -->

    <owl:NamedIndividual rdf:about="http://semanticbible.org/ns/2006/NTNames#Benjamin">
        <rdf:type rdf:resource="http://semanticbible.org/ns/2006/NTNames#Man"/>
        <childOf rdf:resource="http://semanticbible.org/ns/2006/NTNames#Jacob"/>
        <childOf rdf:resource="http://semanticbible.org/ns/2006/NTNames#Rachel"/>
        <ethnicity rdf:resource="http://semanticbible.org/ns/2006/NTNames#Jewish"/>
        <siblingOf rdf:resource="http://semanticbible.org/ns/2006/NTNames#Gad"/>
        <description rdf:datatype="http://www.w3.org/2001/XMLSchema#string">One of the 12 Patriarchs of Israel</description>
        <rdfs:label xml:lang="en">Benjamin</rdfs:label>
    </owl:NamedIndividual>
    


    <!-- http://semanticbible.org/ns/2006/NTNames#Beor -->

    <owl:NamedIndividual rdf:about="http://semanticbible.org/ns/2006/NTNames#Beor">
        <rdf:type rdf:resource="http://semanticbible.org/ns/2006/NTNames#Man"/>
        <parentOf rdf:resource="http://semanticbible.org/ns/2006/NTNames#Balaam"/>
        <rdfs:label xml:lang="en">Beor</rdfs:label>
    </owl:NamedIndividual>
    


    <!-- http://semanticbible.org/ns/2006/NTNames#Berea -->

    <owl:NamedIndividual rdf:about="http://semanticbible.org/ns/2006/NTNames#Berea">
        <rdf:type rdf:resource="http://semanticbible.org/ns/2006/NTNames#City"/>
        <location rdf:resource="http://semanticbible.org/ns/2006/NTNames#BereaGeodata"/>
        <subregionOf rdf:resource="http://semanticbible.org/ns/2006/NTNames#Macedonia"/>
        <rdfs:label xml:lang="en">Berea</rdfs:label>
    </owl:NamedIndividual>
    


    <!-- http://semanticbible.org/ns/2006/NTNames#BereaGeodata -->

    <owl:NamedIndividual rdf:about="http://semanticbible.org/ns/2006/NTNames#BereaGeodata">
        <rdf:type rdf:resource="http://semanticbible.org/ns/2006/NTNames#GeographicLocation"/>
        <altitude rdf:datatype="http://www.w3.org/2001/XMLSchema#int">0</altitude>
        <latitude rdf:datatype="http://www.w3.org/2001/XMLSchema#double">40.43708022312837</latitude>
        <longitude rdf:datatype="http://www.w3.org/2001/XMLSchema#double">22.25122790151288</longitude>
        <rdfs:label xml:lang="en">geodata for Berea</rdfs:label>
    </owl:NamedIndividual>
    


    <!-- http://semanticbible.org/ns/2006/NTNames#Bernice -->

    <owl:NamedIndividual rdf:about="http://semanticbible.org/ns/2006/NTNames#Bernice">
        <rdf:type rdf:resource="http://semanticbible.org/ns/2006/NTNames#Woman"/>
        <childOf rdf:resource="http://semanticbible.org/ns/2006/NTNames#HerodAgrippaI"/>
        <ethnicity rdf:resource="http://semanticbible.org/ns/2006/NTNames#Jewish"/>
        <siblingOf rdf:resource="http://semanticbible.org/ns/2006/NTNames#Drusilla"/>
        <siblingOf rdf:resource="http://semanticbible.org/ns/2006/NTNames#HerodAgrippaII"/>
        <description rdf:datatype="http://www.w3.org/2001/XMLSchema#string">a daughter of Herod Agrippa I who heard Paul&apos;s defense to her brother, Herod Agrippa II</description>
        <hasOnlyGenealogyMention rdf:datatype="http://www.w3.org/2001/XMLSchema#boolean">false</hasOnlyGenealogyMention>
        <rdfs:comment xml:lang="en">Smith notes that Bernice &quot;lived  under circumstances of great suspicion&quot; with her brother Herod Agrippa II, i.e. they may have had an incestuous relationship. </rdfs:comment>
        <rdfs:label xml:lang="en">Bernice</rdfs:label>
    </owl:NamedIndividual>
    


    <!-- http://semanticbible.org/ns/2006/NTNames#Bethany -->

    <owl:NamedIndividual rdf:about="http://semanticbible.org/ns/2006/NTNames#Bethany">
        <rdf:type rdf:resource="http://semanticbible.org/ns/2006/NTNames#City"/>
        <residentPlaceOf rdf:resource="http://semanticbible.org/ns/2006/NTNames#Lazarus"/>
        <residentPlaceOf rdf:resource="http://semanticbible.org/ns/2006/NTNames#Martha"/>
        <residentPlaceOf rdf:resource="http://semanticbible.org/ns/2006/NTNames#MaryOfBethany"/>
        <subregionOf rdf:resource="http://semanticbible.org/ns/2006/NTNames#Judea"/>
        <rdfs:label xml:lang="en">Bethany</rdfs:label>
    </owl:NamedIndividual>
    


    <!-- http://semanticbible.org/ns/2006/NTNames#BethanyBeyondtheJordan -->

    <owl:NamedIndividual rdf:about="http://semanticbible.org/ns/2006/NTNames#BethanyBeyondtheJordan">
        <rdf:type rdf:resource="http://semanticbible.org/ns/2006/NTNames#City"/>
        <location rdf:resource="http://semanticbible.org/ns/2006/NTNames#BethanyBeyondtheJordanGeodata"/>
        <rdfs:comment xml:lang="en">Distinguished from the Bethany near Jerusalem: since the time of Origen, the location has been unknown.</rdfs:comment>
        <rdfs:label xml:lang="en">Bethany beyond the Jordan</rdfs:label>
    </owl:NamedIndividual>
    


    <!-- http://semanticbible.org/ns/2006/NTNames#BethanyBeyondtheJordanGeodata -->

    <owl:NamedIndividual rdf:about="http://semanticbible.org/ns/2006/NTNames#BethanyBeyondtheJordanGeodata">
        <rdf:type rdf:resource="http://semanticbible.org/ns/2006/NTNames#GeographicLocation"/>
        <altitude rdf:datatype="http://www.w3.org/2001/XMLSchema#int">0</altitude>
        <latitude rdf:datatype="http://www.w3.org/2001/XMLSchema#double">31.83673784971973</latitude>
        <longitude rdf:datatype="http://www.w3.org/2001/XMLSchema#double">35.55008611318313</longitude>
        <rdfs:label xml:lang="en">geodata for Bethany Beyond the Jordan</rdfs:label>
    </owl:NamedIndividual>
    


    <!-- http://semanticbible.org/ns/2006/NTNames#Bethesda -->

    <owl:NamedIndividual rdf:about="http://semanticbible.org/ns/2006/NTNames#Bethesda">
        <rdf:type rdf:resource="http://semanticbible.org/ns/2006/NTNames#FreshWaterArea"/>
        <subregionOf rdf:resource="http://semanticbible.org/ns/2006/NTNames#Jerusalem"/>
        <rdfs:label xml:lang="en">Bethesda</rdfs:label>
    </owl:NamedIndividual>
    


    <!-- http://semanticbible.org/ns/2006/NTNames#Bethlehem -->

    <owl:NamedIndividual rdf:about="http://semanticbible.org/ns/2006/NTNames#Bethlehem">
        <rdf:type rdf:resource="http://semanticbible.org/ns/2006/NTNames#City"/>
        <location rdf:resource="http://semanticbible.org/ns/2006/NTNames#BethlehemGeodata"/>
        <subregionOf rdf:resource="http://semanticbible.org/ns/2006/NTNames#Judea"/>
        <visitedPlaceOf rdf:resource="http://semanticbible.org/ns/2006/NTNames#Mary"/>
        <rdfs:label xml:lang="en">Bethlehem</rdfs:label>
    </owl:NamedIndividual>
    


    <!-- http://semanticbible.org/ns/2006/NTNames#BethlehemGeodata -->

    <owl:NamedIndividual rdf:about="http://semanticbible.org/ns/2006/NTNames#BethlehemGeodata">
        <rdf:type rdf:resource="http://semanticbible.org/ns/2006/NTNames#GeographicLocation"/>
        <altitude rdf:datatype="http://www.w3.org/2001/XMLSchema#int">0</altitude>
        <latitude rdf:datatype="http://www.w3.org/2001/XMLSchema#double">31.71507355246746</latitude>
        <longitude rdf:datatype="http://www.w3.org/2001/XMLSchema#double">35.20536282503156</longitude>
        <rdfs:label xml:lang="en">geodata for Bethlehem</rdfs:label>
    </owl:NamedIndividual>
    


    <!-- http://semanticbible.org/ns/2006/NTNames#Bethphage -->

    <owl:NamedIndividual rdf:about="http://semanticbible.org/ns/2006/NTNames#Bethphage">
        <rdf:type rdf:resource="http://semanticbible.org/ns/2006/NTNames#City"/>
        <subregionOf rdf:resource="http://semanticbible.org/ns/2006/NTNames#Judea"/>
        <rdfs:label xml:lang="en">Bethphage</rdfs:label>
    </owl:NamedIndividual>
    


    <!-- http://semanticbible.org/ns/2006/NTNames#Bethsaida -->

    <owl:NamedIndividual rdf:about="http://semanticbible.org/ns/2006/NTNames#Bethsaida">
        <rdf:type rdf:resource="http://semanticbible.org/ns/2006/NTNames#City"/>
        <location rdf:resource="http://semanticbible.org/ns/2006/NTNames#BethsaidaGeodata"/>
        <subregionOf rdf:resource="http://semanticbible.org/ns/2006/NTNames#Galilee"/>
        <rdfs:comment xml:lang="en">NNE of Sea of Galilee, &quot;Bethsaida Julia&quot;. ISBE has a thorough account
of whether, given Mark 6.45 and John&apos;s &quot;Bethsaida of Galilee&quot;, 
there were two such towns (with a second, smaller one on the west side),
or only one</rdfs:comment>
        <rdfs:label xml:lang="en">Bethsaida</rdfs:label>
    </owl:NamedIndividual>
    


    <!-- http://semanticbible.org/ns/2006/NTNames#BethsaidaGeodata -->

    <owl:NamedIndividual rdf:about="http://semanticbible.org/ns/2006/NTNames#BethsaidaGeodata">
        <rdf:type rdf:resource="http://semanticbible.org/ns/2006/NTNames#GeographicLocation"/>
        <altitude rdf:datatype="http://www.w3.org/2001/XMLSchema#int">0</altitude>
        <latitude rdf:datatype="http://www.w3.org/2001/XMLSchema#double">32.87856448546807</latitude>
        <longitude rdf:datatype="http://www.w3.org/2001/XMLSchema#double">35.61284401358682</longitude>
        <rdfs:label xml:lang="en">geodata for Bethsaida</rdfs:label>
    </owl:NamedIndividual>
    


    <!-- http://semanticbible.org/ns/2006/NTNames#Bithynia -->

    <owl:NamedIndividual rdf:about="http://semanticbible.org/ns/2006/NTNames#Bithynia">
        <rdf:type rdf:resource="http://semanticbible.org/ns/2006/NTNames#StateOrProvince"/>
        <rdfs:label xml:lang="en">Bithynia</rdfs:label>
    </owl:NamedIndividual>
    


    <!-- http://semanticbible.org/ns/2006/NTNames#Blastus -->

    <owl:NamedIndividual rdf:about="http://semanticbible.org/ns/2006/NTNames#Blastus">
        <rdf:type rdf:resource="http://semanticbible.org/ns/2006/NTNames#Man"/>
        <knows rdf:resource="http://semanticbible.org/ns/2006/NTNames#HerodAgrippaI"/>
        <description rdf:datatype="http://www.w3.org/2001/XMLSchema#string">the chamberlain of Herod Agrippa</description>
        <occupation rdf:datatype="http://www.w3.org/2001/XMLSchema#string">chamberlain</occupation>
        <rdfs:label xml:lang="en">Blastus</rdfs:label>
    </owl:NamedIndividual>
    


    <!-- http://semanticbible.org/ns/2006/NTNames#Boanerges -->

    <owl:NamedIndividual rdf:about="http://semanticbible.org/ns/2006/NTNames#Boanerges">
        <rdf:type rdf:resource="http://semanticbible.org/ns/2006/NTNames#GroupOfPeople"/>
        <rdfs:comment xml:lang="en">Jesus&apos; nickname for two of his disciples: James, the son of Zebedee, and John, his brother.</rdfs:comment>
        <rdfs:label xml:lang="en">Boanerges</rdfs:label>
        <rdfs:label xml:lang="en">Sons of Thunder</rdfs:label>
    </owl:NamedIndividual>
    


    <!-- http://semanticbible.org/ns/2006/NTNames#Boaz -->

    <owl:NamedIndividual rdf:about="http://semanticbible.org/ns/2006/NTNames#Boaz">
        <rdf:type rdf:resource="http://semanticbible.org/ns/2006/NTNames#Man"/>
        <childOf rdf:resource="http://semanticbible.org/ns/2006/NTNames#Rahab"/>
        <childOf rdf:resource="http://semanticbible.org/ns/2006/NTNames#Salmon"/>
        <ethnicity rdf:resource="http://semanticbible.org/ns/2006/NTNames#Jewish"/>
        <parentOf rdf:resource="http://semanticbible.org/ns/2006/NTNames#Obed"/>
        <spouseOf rdf:resource="http://semanticbible.org/ns/2006/NTNames#Ruth"/>
        <description rdf:datatype="http://www.w3.org/2001/XMLSchema#string">One of the ancestors of Jesus mentioned in Matthew&apos;s geneaology</description>
        <hasOnlyGenealogyMention rdf:datatype="http://www.w3.org/2001/XMLSchema#boolean">true</hasOnlyGenealogyMention>
        <rdfs:label xml:lang="en">Boaz</rdfs:label>
    </owl:NamedIndividual>
    


    <!-- http://semanticbible.org/ns/2006/NTNames#CaesarAugustus -->

    <owl:NamedIndividual rdf:about="http://semanticbible.org/ns/2006/NTNames#CaesarAugustus">
        <rdf:type rdf:resource="http://semanticbible.org/ns/2006/NTNames#Man"/>
        <ethnicity rdf:resource="http://semanticbible.org/ns/2006/NTNames#Roman"/>
        <description rdf:datatype="http://www.w3.org/2001/XMLSchema#string">Roman Emperor at the time of Jesus&apos; birth</description>
        <occupation rdf:datatype="http://www.w3.org/2001/XMLSchema#string">emperor</occupation>
        <rdfs:comment rdf:datatype="http://www.w3.org/2001/XMLSchema#string">Caesar is used as a name for several different individuals in the New Testament</rdfs:comment>
        <rdfs:label xml:lang="en">Caesar</rdfs:label>
    </owl:NamedIndividual>
    


    <!-- http://semanticbible.org/ns/2006/NTNames#CaesarNero -->

    <owl:NamedIndividual rdf:about="http://semanticbible.org/ns/2006/NTNames#CaesarNero">
        <rdf:type rdf:resource="http://semanticbible.org/ns/2006/NTNames#Man"/>
        <ethnicity rdf:resource="http://semanticbible.org/ns/2006/NTNames#Roman"/>
        <description rdf:datatype="http://www.w3.org/2001/XMLSchema#string">Roman Emperor during Paul&apos;s ministry</description>
        <occupation rdf:datatype="http://www.w3.org/2001/XMLSchema#string">emperor</occupation>
        <rdfs:comment rdf:datatype="http://www.w3.org/2001/XMLSchema#string">Caesar is used as a name for several different individuals in the New Testament</rdfs:comment>
        <rdfs:label xml:lang="en">Caesar</rdfs:label>
    </owl:NamedIndividual>
    


    <!-- http://semanticbible.org/ns/2006/NTNames#Caesarea -->

    <owl:NamedIndividual rdf:about="http://semanticbible.org/ns/2006/NTNames#Caesarea">
        <rdf:type rdf:resource="http://semanticbible.org/ns/2006/NTNames#City"/>
        <location rdf:resource="http://semanticbible.org/ns/2006/NTNames#CaesareaGeodata"/>
        <residentPlaceOf rdf:resource="http://semanticbible.org/ns/2006/NTNames#Drusilla"/>
        <residentPlaceOf rdf:resource="http://semanticbible.org/ns/2006/NTNames#Felix"/>
        <residentPlaceOf rdf:resource="http://semanticbible.org/ns/2006/NTNames#Festus"/>
        <subregionOf rdf:resource="http://semanticbible.org/ns/2006/NTNames#Samaria"/>
        <rdfs:label xml:lang="en">Caesarea</rdfs:label>
    </owl:NamedIndividual>
    


    <!-- http://semanticbible.org/ns/2006/NTNames#CaesareaGeodata -->

    <owl:NamedIndividual rdf:about="http://semanticbible.org/ns/2006/NTNames#CaesareaGeodata">
        <rdf:type rdf:resource="http://semanticbible.org/ns/2006/NTNames#GeographicLocation"/>
        <altitude rdf:datatype="http://www.w3.org/2001/XMLSchema#int">0</altitude>
        <latitude rdf:datatype="http://www.w3.org/2001/XMLSchema#double">32.48365887401189</latitude>
        <longitude rdf:datatype="http://www.w3.org/2001/XMLSchema#double">34.93994395174937</longitude>
        <rdfs:label xml:lang="en">geodata for Caesarea</rdfs:label>
    </owl:NamedIndividual>
    


    <!-- http://semanticbible.org/ns/2006/NTNames#CaesareaPhilippi -->

    <owl:NamedIndividual rdf:about="http://semanticbible.org/ns/2006/NTNames#CaesareaPhilippi">
        <rdf:type rdf:resource="http://semanticbible.org/ns/2006/NTNames#City"/>
        <location rdf:resource="http://semanticbible.org/ns/2006/NTNames#CaesareaPhilippiGeodata"/>
        <subregionOf rdf:resource="http://semanticbible.org/ns/2006/NTNames#Ituraea"/>
        <rdfs:label xml:lang="en">Caesarea Philippi</rdfs:label>
    </owl:NamedIndividual>
    


    <!-- http://semanticbible.org/ns/2006/NTNames#CaesareaPhilippiGeodata -->

    <owl:NamedIndividual rdf:about="http://semanticbible.org/ns/2006/NTNames#CaesareaPhilippiGeodata">
        <rdf:type rdf:resource="http://semanticbible.org/ns/2006/NTNames#GeographicLocation"/>
        <altitude rdf:datatype="http://www.w3.org/2001/XMLSchema#int">0</altitude>
        <latitude rdf:datatype="http://www.w3.org/2001/XMLSchema#double">33.25100774530771</latitude>
        <longitude rdf:datatype="http://www.w3.org/2001/XMLSchema#double">35.69397573529149</longitude>
        <rdfs:label xml:lang="en">geodata for Caesarea Philippi</rdfs:label>
    </owl:NamedIndividual>
    


    <!-- http://semanticbible.org/ns/2006/NTNames#Caiaphas -->

    <owl:NamedIndividual rdf:about="http://semanticbible.org/ns/2006/NTNames#Caiaphas">
        <rdf:type rdf:resource="http://semanticbible.org/ns/2006/NTNames#Man"/>
        <collaboratesWith rdf:resource="http://semanticbible.org/ns/2006/NTNames#Annas"/>
        <ethnicity rdf:resource="http://semanticbible.org/ns/2006/NTNames#Jewish"/>
        <knows rdf:resource="http://semanticbible.org/ns/2006/NTNames#PontiusPilate"/>
        <relativeOf rdf:resource="http://semanticbible.org/ns/2006/NTNames#Annas"/>
        <description rdf:datatype="http://www.w3.org/2001/XMLSchema#string">Jewish high priest during Jesus&apos; ministry</description>
        <occupation rdf:datatype="http://www.w3.org/2001/XMLSchema#string">high priest</occupation>
        <rdfs:label xml:lang="en">Caiaphas</rdfs:label>
    </owl:NamedIndividual>
    


    <!-- http://semanticbible.org/ns/2006/NTNames#Cain -->

    <owl:NamedIndividual rdf:about="http://semanticbible.org/ns/2006/NTNames#Cain">
        <rdf:type rdf:resource="http://semanticbible.org/ns/2006/NTNames#Man"/>
        <childOf rdf:resource="http://semanticbible.org/ns/2006/NTNames#Adam"/>
        <childOf rdf:resource="http://semanticbible.org/ns/2006/NTNames#Eve"/>
        <siblingOf rdf:resource="http://semanticbible.org/ns/2006/NTNames#Abel"/>
        <description rdf:datatype="http://www.w3.org/2001/XMLSchema#string">the first son of Adam and Eve, who killed his brother Abel</description>
        <rdfs:label xml:lang="en">Cain</rdfs:label>
    </owl:NamedIndividual>
    


    <!-- http://semanticbible.org/ns/2006/NTNames#CainanSonOfArphaxad -->

    <owl:NamedIndividual rdf:about="http://semanticbible.org/ns/2006/NTNames#CainanSonOfArphaxad">
        <rdf:type rdf:resource="http://semanticbible.org/ns/2006/NTNames#Man"/>
        <childOf rdf:resource="http://semanticbible.org/ns/2006/NTNames#Arphaxad"/>
        <parentOf rdf:resource="http://semanticbible.org/ns/2006/NTNames#Shelah"/>
        <description rdf:datatype="http://www.w3.org/2001/XMLSchema#string">One of the ancestors of Jesus mentioned in Luke&apos;s geneaology</description>
        <hasOnlyGenealogyMention rdf:datatype="http://www.w3.org/2001/XMLSchema#boolean">true</hasOnlyGenealogyMention>
        <rdfs:label xml:lang="en">Cainan</rdfs:label>
    </owl:NamedIndividual>
    


    <!-- http://semanticbible.org/ns/2006/NTNames#CainanSonOfEnosh -->

    <owl:NamedIndividual rdf:about="http://semanticbible.org/ns/2006/NTNames#CainanSonOfEnosh">
        <rdf:type rdf:resource="http://semanticbible.org/ns/2006/NTNames#Man"/>
        <childOf rdf:resource="http://semanticbible.org/ns/2006/NTNames#Enos"/>
        <parentOf rdf:resource="http://semanticbible.org/ns/2006/NTNames#Mahalaleel"/>
        <description rdf:datatype="http://www.w3.org/2001/XMLSchema#string">One of the ancestors of Jesus mentioned in Luke&apos;s geneaology</description>
        <hasOnlyGenealogyMention rdf:datatype="http://www.w3.org/2001/XMLSchema#boolean">true</hasOnlyGenealogyMention>
        <rdfs:comment xml:lang="en">Kenan in the NIV</rdfs:comment>
        <rdfs:label xml:lang="en">Cainan</rdfs:label>
    </owl:NamedIndividual>
    


    <!-- http://semanticbible.org/ns/2006/NTNames#Caiphas -->

    <owl:NamedIndividual rdf:about="http://semanticbible.org/ns/2006/NTNames#Caiphas">
        <rdf:type rdf:resource="http://semanticbible.org/ns/2006/NTNames#Man"/>
        <rdfs:comment xml:lang="en">see Caiaphas</rdfs:comment>
        <rdfs:label xml:lang="en">Caiphas</rdfs:label>
    </owl:NamedIndividual>
    


    <!-- http://semanticbible.org/ns/2006/NTNames#Cana -->

    <owl:NamedIndividual rdf:about="http://semanticbible.org/ns/2006/NTNames#Cana">
        <rdf:type rdf:resource="http://semanticbible.org/ns/2006/NTNames#City"/>
        <location rdf:resource="http://semanticbible.org/ns/2006/NTNames#CanaGeodata"/>
        <subregionOf rdf:resource="http://semanticbible.org/ns/2006/NTNames#Galilee"/>
        <visitedPlaceOf rdf:resource="http://semanticbible.org/ns/2006/NTNames#Mary"/>
        <rdfs:label xml:lang="en">Cana</rdfs:label>
    </owl:NamedIndividual>
    


    <!-- http://semanticbible.org/ns/2006/NTNames#CanaGeodata -->

    <owl:NamedIndividual rdf:about="http://semanticbible.org/ns/2006/NTNames#CanaGeodata">
        <rdf:type rdf:resource="http://semanticbible.org/ns/2006/NTNames#GeographicLocation"/>
        <altitude rdf:datatype="http://www.w3.org/2001/XMLSchema#int">0</altitude>
        <latitude rdf:datatype="http://www.w3.org/2001/XMLSchema#double">32.75209569199829</latitude>
        <longitude rdf:datatype="http://www.w3.org/2001/XMLSchema#double">35.34180211400924</longitude>
        <rdfs:label xml:lang="en">geodata for Cana</rdfs:label>
    </owl:NamedIndividual>
    


    <!-- http://semanticbible.org/ns/2006/NTNames#Canaan -->

    <owl:NamedIndividual rdf:about="http://semanticbible.org/ns/2006/NTNames#Canaan">
        <rdf:type rdf:resource="http://semanticbible.org/ns/2006/NTNames#Region"/>
        <residentPlaceOf rdf:resource="http://semanticbible.org/ns/2006/NTNames#Abraham"/>
        <residentPlaceOf rdf:resource="http://semanticbible.org/ns/2006/NTNames#Hagar"/>
        <residentPlaceOf rdf:resource="http://semanticbible.org/ns/2006/NTNames#Sarah"/>
        <rdfs:label xml:lang="en">Canaan</rdfs:label>
    </owl:NamedIndividual>
    


    <!-- http://semanticbible.org/ns/2006/NTNames#Canaanite -->

    <owl:NamedIndividual rdf:about="http://semanticbible.org/ns/2006/NTNames#Canaanite">
        <rdf:type rdf:resource="http://semanticbible.org/ns/2006/NTNames#EthnicityAttribute"/>
        <ethnicityOf rdf:resource="http://semanticbible.org/ns/2006/NTNames#Hamor"/>
        <rdfs:comment xml:lang="en">In the Old Testament, a people living west of the Jordan river who were partially displaced by the Israelites. In New Testament times, Canaanites lived primarily in the area of Phoenicia. Cananean, in contrast, is almost certainly political, rather than ethnic. </rdfs:comment>
        <rdfs:label xml:lang="en">Canaanite</rdfs:label>
    </owl:NamedIndividual>
    


    <!-- http://semanticbible.org/ns/2006/NTNames#Cananaean -->

    <owl:NamedIndividual rdf:about="http://semanticbible.org/ns/2006/NTNames#Cananaean">
        <rdf:type rdf:resource="http://semanticbible.org/ns/2006/NTNames#PoliticalAttribute"/>
        <rdfs:comment xml:lang="en">This attribute is only used by Matthew and Mark to describe Simon, one of Jesus&apos; disciples. Given what else we know of Simon, it almost certainly designates a political attribute, rather than ethnicity.</rdfs:comment>
        <rdfs:label xml:lang="en">Cananaean</rdfs:label>
    </owl:NamedIndividual>
    


    <!-- http://semanticbible.org/ns/2006/NTNames#Candace -->

    <owl:NamedIndividual rdf:about="http://semanticbible.org/ns/2006/NTNames#Candace">
        <rdf:type rdf:resource="http://semanticbible.org/ns/2006/NTNames#Woman"/>
        <ethnicity rdf:resource="http://semanticbible.org/ns/2006/NTNames#Ethiopian"/>
        <hasOnlyGenealogyMention rdf:datatype="http://www.w3.org/2001/XMLSchema#boolean">false</hasOnlyGenealogyMention>
        <occupation rdf:datatype="http://www.w3.org/2001/XMLSchema#string">queen</occupation>
        <rdfs:comment xml:lang="en">Candace is actually a title like &quot;Pharaoh&quot; rather than a personal name, hence her occupation as queen.</rdfs:comment>
        <rdfs:label xml:lang="en">Candace</rdfs:label>
    </owl:NamedIndividual>
    


    <!-- http://semanticbible.org/ns/2006/NTNames#Capernaum -->

    <owl:NamedIndividual rdf:about="http://semanticbible.org/ns/2006/NTNames#Capernaum">
        <rdf:type rdf:resource="http://semanticbible.org/ns/2006/NTNames#City"/>
        <location rdf:resource="http://semanticbible.org/ns/2006/NTNames#CapernaumGeodata"/>
        <subregionOf rdf:resource="http://semanticbible.org/ns/2006/NTNames#Galilee"/>
        <rdfs:label xml:lang="en">Capernaum</rdfs:label>
    </owl:NamedIndividual>
    


    <!-- http://semanticbible.org/ns/2006/NTNames#CapernaumGeodata -->

    <owl:NamedIndividual rdf:about="http://semanticbible.org/ns/2006/NTNames#CapernaumGeodata">
        <rdf:type rdf:resource="http://semanticbible.org/ns/2006/NTNames#GeographicLocation"/>
        <altitude rdf:datatype="http://www.w3.org/2001/XMLSchema#int">0</altitude>
        <latitude rdf:datatype="http://www.w3.org/2001/XMLSchema#double">32.88081694660667</latitude>
        <longitude rdf:datatype="http://www.w3.org/2001/XMLSchema#double">35.57534055705805</longitude>
        <rdfs:label xml:lang="en">geodata for Capernaum</rdfs:label>
    </owl:NamedIndividual>
    


    <!-- http://semanticbible.org/ns/2006/NTNames#Cappadocia -->

    <owl:NamedIndividual rdf:about="http://semanticbible.org/ns/2006/NTNames#Cappadocia">
        <rdf:type rdf:resource="http://semanticbible.org/ns/2006/NTNames#StateOrProvince"/>
        <rdfs:label xml:lang="en">Cappadocia</rdfs:label>
    </owl:NamedIndividual>
    


    <!-- http://semanticbible.org/ns/2006/NTNames#Carpus -->

    <owl:NamedIndividual rdf:about="http://semanticbible.org/ns/2006/NTNames#Carpus">
        <rdf:type rdf:resource="http://semanticbible.org/ns/2006/NTNames#Man"/>
        <collaboratesWith rdf:resource="http://semanticbible.org/ns/2006/NTNames#Paul"/>
        <description rdf:datatype="http://www.w3.org/2001/XMLSchema#string">an associate of Paul&apos;s, whom the Apostle entrusted with books, parchments, and his cloak</description>
        <rdfs:label xml:lang="en">Carpus</rdfs:label>
    </owl:NamedIndividual>
    


    <!-- http://semanticbible.org/ns/2006/NTNames#Cauda -->

    <owl:NamedIndividual rdf:about="http://semanticbible.org/ns/2006/NTNames#Cauda">
        <rdf:type rdf:resource="http://semanticbible.org/ns/2006/NTNames#Island"/>
        <rdfs:label xml:lang="en">Cauda</rdfs:label>
    </owl:NamedIndividual>
    


    <!-- http://semanticbible.org/ns/2006/NTNames#Cenchreae -->

    <owl:NamedIndividual rdf:about="http://semanticbible.org/ns/2006/NTNames#Cenchreae">
        <rdf:type rdf:resource="http://semanticbible.org/ns/2006/NTNames#City"/>
        <location rdf:resource="http://semanticbible.org/ns/2006/NTNames#CenchreaeGeodata"/>
        <residentPlaceOf rdf:resource="http://semanticbible.org/ns/2006/NTNames#Phoebe"/>
        <rdfs:label xml:lang="en">Cenchreae</rdfs:label>
    </owl:NamedIndividual>
    


    <!-- http://semanticbible.org/ns/2006/NTNames#CenchreaeGeodata -->

    <owl:NamedIndividual rdf:about="http://semanticbible.org/ns/2006/NTNames#CenchreaeGeodata">
        <rdf:type rdf:resource="http://semanticbible.org/ns/2006/NTNames#GeographicLocation"/>
        <altitude rdf:datatype="http://www.w3.org/2001/XMLSchema#int">0</altitude>
        <latitude rdf:datatype="http://www.w3.org/2001/XMLSchema#double">37.90791013400233</latitude>
        <longitude rdf:datatype="http://www.w3.org/2001/XMLSchema#double">22.96102305563464</longitude>
        <rdfs:label xml:lang="en">geodata for Cenchreae</rdfs:label>
    </owl:NamedIndividual>
    


    <!-- http://semanticbible.org/ns/2006/NTNames#Chaldeans -->

    <owl:NamedIndividual rdf:about="http://semanticbible.org/ns/2006/NTNames#Chaldeans">
        <rdf:type rdf:resource="http://semanticbible.org/ns/2006/NTNames#EthnicGroup"/>
        <rdfs:label xml:lang="en">Chaldeans</rdfs:label>
    </owl:NamedIndividual>
    


    <!-- http://semanticbible.org/ns/2006/NTNames#Chios -->

    <owl:NamedIndividual rdf:about="http://semanticbible.org/ns/2006/NTNames#Chios">
        <rdf:type rdf:resource="http://semanticbible.org/ns/2006/NTNames#Island"/>
        <rdfs:label xml:lang="en">Chios</rdfs:label>
    </owl:NamedIndividual>
    


    <!-- http://semanticbible.org/ns/2006/NTNames#Chloe -->

    <owl:NamedIndividual rdf:about="http://semanticbible.org/ns/2006/NTNames#Chloe">
        <rdf:type rdf:resource="http://semanticbible.org/ns/2006/NTNames#Woman"/>
        <hasOnlyGenealogyMention rdf:datatype="http://www.w3.org/2001/XMLSchema#boolean">false</hasOnlyGenealogyMention>
        <rdfs:comment rdf:datatype="http://www.w3.org/2001/XMLSchema#string">&quot;Chloe&apos;s people&quot; are mentioned in 1Cor.1.11: so while they were clearly Christians who knew the church in Corinth, nothing more specific is known about her. She may have resided in Ephesus instead of Corinth. </rdfs:comment>
        <rdfs:label xml:lang="en">Chloe</rdfs:label>
    </owl:NamedIndividual>
    


    <!-- http://semanticbible.org/ns/2006/NTNames#Chorazin -->

    <owl:NamedIndividual rdf:about="http://semanticbible.org/ns/2006/NTNames#Chorazin">
        <rdf:type rdf:resource="http://semanticbible.org/ns/2006/NTNames#City"/>
        <subregionOf rdf:resource="http://semanticbible.org/ns/2006/NTNames#Galilee"/>
        <rdfs:label xml:lang="en">Chorazin</rdfs:label>
    </owl:NamedIndividual>
    


    <!-- http://semanticbible.org/ns/2006/NTNames#Christian -->

    <owl:NamedIndividual rdf:about="http://semanticbible.org/ns/2006/NTNames#Christian">
        <rdf:type rdf:resource="http://semanticbible.org/ns/2006/NTNames#ReligiousBelief"/>
        <rdfs:label xml:lang="en">Christian</rdfs:label>
    </owl:NamedIndividual>
    


    <!-- http://semanticbible.org/ns/2006/NTNames#Christianity -->

    <owl:NamedIndividual rdf:about="http://semanticbible.org/ns/2006/NTNames#Christianity">
        <rdf:type rdf:resource="http://semanticbible.org/ns/2006/NTNames#ReligiousBeliefSystem"/>
        <rdfs:comment xml:lang="en">Not referenced as a belief system in the New Testament.</rdfs:comment>
        <rdfs:label xml:lang="en">Christianity</rdfs:label>
    </owl:NamedIndividual>
    


    <!-- http://semanticbible.org/ns/2006/NTNames#Christians -->

    <owl:NamedIndividual rdf:about="http://semanticbible.org/ns/2006/NTNames#Christians">
        <rdf:type rdf:resource="http://semanticbible.org/ns/2006/NTNames#BeliefGroup"/>
        <rdfs:label xml:lang="en">Christians</rdfs:label>
    </owl:NamedIndividual>
    


    <!-- http://semanticbible.org/ns/2006/NTNames#Chuza -->

    <owl:NamedIndividual rdf:about="http://semanticbible.org/ns/2006/NTNames#Chuza">
        <rdf:type rdf:resource="http://semanticbible.org/ns/2006/NTNames#Man"/>
        <knows rdf:resource="http://semanticbible.org/ns/2006/NTNames#HerodAntipas"/>
        <spouseOf rdf:resource="http://semanticbible.org/ns/2006/NTNames#Joanna"/>
        <description rdf:datatype="http://www.w3.org/2001/XMLSchema#string">Household manager of Herod Antipas</description>
        <occupation rdf:datatype="http://www.w3.org/2001/XMLSchema#string">household manager</occupation>
        <rdfs:comment xml:lang="en">Though Chuza&apos;s wife was a devoted follower of Jesus, there&apos;s no evidence as to Chuza&apos;s belief.</rdfs:comment>
        <rdfs:label xml:lang="en">Chuza</rdfs:label>
    </owl:NamedIndividual>
    


    <!-- http://semanticbible.org/ns/2006/NTNames#Cilicia -->

    <owl:NamedIndividual rdf:about="http://semanticbible.org/ns/2006/NTNames#Cilicia">
        <rdf:type rdf:resource="http://semanticbible.org/ns/2006/NTNames#StateOrProvince"/>
        <rdfs:label xml:lang="en">Cilicia</rdfs:label>
    </owl:NamedIndividual>
    


    <!-- http://semanticbible.org/ns/2006/NTNames#Claudia -->

    <owl:NamedIndividual rdf:about="http://semanticbible.org/ns/2006/NTNames#Claudia">
        <rdf:type rdf:resource="http://semanticbible.org/ns/2006/NTNames#Woman"/>
        <knows rdf:resource="http://semanticbible.org/ns/2006/NTNames#Eubulus"/>
        <knows rdf:resource="http://semanticbible.org/ns/2006/NTNames#Linus"/>
        <knows rdf:resource="http://semanticbible.org/ns/2006/NTNames#Paul"/>
        <knows rdf:resource="http://semanticbible.org/ns/2006/NTNames#Pudens"/>
        <knows rdf:resource="http://semanticbible.org/ns/2006/NTNames#Timothy"/>
        <religiousBelief rdf:resource="http://semanticbible.org/ns/2006/NTNames#Christianity"/>
        <residentPlace rdf:resource="http://semanticbible.org/ns/2006/NTNames#Rome"/>
        <description rdf:datatype="http://www.w3.org/2001/XMLSchema#string">a Christian who sent greeetings to Timothy in Paul&apos;s second epislte.</description>
        <hasOnlyGenealogyMention rdf:datatype="http://www.w3.org/2001/XMLSchema#boolean">false</hasOnlyGenealogyMention>
        <rdfs:comment rdf:datatype="http://www.w3.org/2001/XMLSchema#string">Rome as ResidentPlace because Paul was imprisoned there when writing to Timothy.</rdfs:comment>
        <rdfs:label xml:lang="en">Claudia</rdfs:label>
    </owl:NamedIndividual>
    


    <!-- http://semanticbible.org/ns/2006/NTNames#Claudius -->

    <owl:NamedIndividual rdf:about="http://semanticbible.org/ns/2006/NTNames#Claudius">
        <rdf:type rdf:resource="http://semanticbible.org/ns/2006/NTNames#Man"/>
        <description rdf:datatype="http://www.w3.org/2001/XMLSchema#string">One of the emperors of Rome</description>
        <occupation rdf:datatype="http://www.w3.org/2001/XMLSchema#string">emperor</occupation>
        <rdfs:label xml:lang="en">Claudius</rdfs:label>
    </owl:NamedIndividual>
    


    <!-- http://semanticbible.org/ns/2006/NTNames#ClaudiusLysias -->

    <owl:NamedIndividual rdf:about="http://semanticbible.org/ns/2006/NTNames#ClaudiusLysias">
        <rdf:type rdf:resource="http://semanticbible.org/ns/2006/NTNames#Man"/>
        <knows rdf:resource="http://semanticbible.org/ns/2006/NTNames#Felix"/>
        <knows rdf:resource="http://semanticbible.org/ns/2006/NTNames#Paul"/>
        <residentPlace rdf:resource="http://semanticbible.org/ns/2006/NTNames#Jerusalem"/>
        <description rdf:datatype="http://www.w3.org/2001/XMLSchema#string">the military tribune commanding the Roman forces in Jerusalem</description>
        <hasOnlyGenealogyMention rdf:datatype="http://www.w3.org/2001/XMLSchema#boolean">false</hasOnlyGenealogyMention>
        <occupation rdf:datatype="http://www.w3.org/2001/XMLSchema#string">tribune</occupation>
        <rdfs:comment xml:lang="en">Greek ethnicity is suggested by his surname. </rdfs:comment>
        <rdfs:label xml:lang="en">Claudius Lysias</rdfs:label>
    </owl:NamedIndividual>
    


    <!-- http://semanticbible.org/ns/2006/NTNames#Clement -->

    <owl:NamedIndividual rdf:about="http://semanticbible.org/ns/2006/NTNames#Clement">
        <rdf:type rdf:resource="http://semanticbible.org/ns/2006/NTNames#Man"/>
        <collaboratesWith rdf:resource="http://semanticbible.org/ns/2006/NTNames#Euodia"/>
        <collaboratesWith rdf:resource="http://semanticbible.org/ns/2006/NTNames#Paul"/>
        <collaboratesWith rdf:resource="http://semanticbible.org/ns/2006/NTNames#Syntyche"/>
        <religiousBelief rdf:resource="http://semanticbible.org/ns/2006/NTNames#Christianity"/>
        <description rdf:datatype="http://www.w3.org/2001/XMLSchema#string">a companion of the Apostle Paul</description>
        <hasOnlyGenealogyMention rdf:datatype="http://www.w3.org/2001/XMLSchema#boolean">false</hasOnlyGenealogyMention>
        <rdfs:label xml:lang="en">Clement</rdfs:label>
    </owl:NamedIndividual>
    


    <!-- http://semanticbible.org/ns/2006/NTNames#Cleopas -->

    <owl:NamedIndividual rdf:about="http://semanticbible.org/ns/2006/NTNames#Cleopas">
        <rdf:type rdf:resource="http://semanticbible.org/ns/2006/NTNames#Man"/>
        <collaboratesWith rdf:resource="http://semanticbible.org/ns/2006/NTNames#Jesus"/>
        <religiousBelief rdf:resource="http://semanticbible.org/ns/2006/NTNames#Christianity"/>
        <visitedPlace rdf:resource="http://semanticbible.org/ns/2006/NTNames#Jerusalem"/>
        <description rdf:datatype="http://www.w3.org/2001/XMLSchema#string">one of the two travellers on the road to Emmaus to whom Jesus appeared after his resurrection</description>
        <hasOnlyGenealogyMention rdf:datatype="http://www.w3.org/2001/XMLSchema#boolean">false</hasOnlyGenealogyMention>
        <rdfs:comment xml:lang="en">&quot;The name is a contraction of Cleopatros, not identical with Clopas of Joh 19:25.&quot; (ISBE) Jerusalem could have been his place of residence. </rdfs:comment>
        <rdfs:label xml:lang="en">Cleopas</rdfs:label>
        <owl:versionInfo rdf:datatype="http://www.w3.org/2001/XMLSchema#string">TODO: Cleopas knew the 11, and the women who went to the tomb</owl:versionInfo>
    </owl:NamedIndividual>
    


    <!-- http://semanticbible.org/ns/2006/NTNames#Cnidus -->

    <owl:NamedIndividual rdf:about="http://semanticbible.org/ns/2006/NTNames#Cnidus">
        <rdf:type rdf:resource="http://semanticbible.org/ns/2006/NTNames#City"/>
        <location rdf:resource="http://semanticbible.org/ns/2006/NTNames#CnidusGeodata"/>
        <rdfs:label xml:lang="en">Cnidus</rdfs:label>
    </owl:NamedIndividual>
    


    <!-- http://semanticbible.org/ns/2006/NTNames#CnidusGeodata -->

    <owl:NamedIndividual rdf:about="http://semanticbible.org/ns/2006/NTNames#CnidusGeodata">
        <rdf:type rdf:resource="http://semanticbible.org/ns/2006/NTNames#GeographicLocation"/>
        <altitude rdf:datatype="http://www.w3.org/2001/XMLSchema#int">0</altitude>
        <latitude rdf:datatype="http://www.w3.org/2001/XMLSchema#double">36.68500139032388</latitude>
        <longitude rdf:datatype="http://www.w3.org/2001/XMLSchema#double">27.37335756835654</longitude>
        <rdfs:label xml:lang="en">geodata for Cnidus</rdfs:label>
    </owl:NamedIndividual>
    


    <!-- http://semanticbible.org/ns/2006/NTNames#Colossae -->

    <owl:NamedIndividual rdf:about="http://semanticbible.org/ns/2006/NTNames#Colossae">
        <rdf:type rdf:resource="http://semanticbible.org/ns/2006/NTNames#City"/>
        <location rdf:resource="http://semanticbible.org/ns/2006/NTNames#ColossaeGeodata"/>
        <rdfs:label xml:lang="en">Colossae</rdfs:label>
    </owl:NamedIndividual>
    


    <!-- http://semanticbible.org/ns/2006/NTNames#ColossaeGeodata -->

    <owl:NamedIndividual rdf:about="http://semanticbible.org/ns/2006/NTNames#ColossaeGeodata">
        <rdf:type rdf:resource="http://semanticbible.org/ns/2006/NTNames#GeographicLocation"/>
        <altitude rdf:datatype="http://www.w3.org/2001/XMLSchema#int">0</altitude>
        <latitude rdf:datatype="http://www.w3.org/2001/XMLSchema#double">37.82980850278283</latitude>
        <longitude rdf:datatype="http://www.w3.org/2001/XMLSchema#double">29.19879351988703</longitude>
        <rdfs:label xml:lang="en">geodata for Colossae</rdfs:label>
    </owl:NamedIndividual>
    


    <!-- http://semanticbible.org/ns/2006/NTNames#Corinth -->

    <owl:NamedIndividual rdf:about="http://semanticbible.org/ns/2006/NTNames#Corinth">
        <rdf:type rdf:resource="http://semanticbible.org/ns/2006/NTNames#City"/>
        <location rdf:resource="http://semanticbible.org/ns/2006/NTNames#CorinthGeodata"/>
        <residentPlaceOf rdf:resource="http://semanticbible.org/ns/2006/NTNames#Achaicus"/>
        <residentPlaceOf rdf:resource="http://semanticbible.org/ns/2006/NTNames#Aquila"/>
        <residentPlaceOf rdf:resource="http://semanticbible.org/ns/2006/NTNames#Fortunatus"/>
        <residentPlaceOf rdf:resource="http://semanticbible.org/ns/2006/NTNames#GaiusOfCorinth"/>
        <residentPlaceOf rdf:resource="http://semanticbible.org/ns/2006/NTNames#Jason"/>
        <residentPlaceOf rdf:resource="http://semanticbible.org/ns/2006/NTNames#Lucius"/>
        <residentPlaceOf rdf:resource="http://semanticbible.org/ns/2006/NTNames#Priscilla"/>
        <residentPlaceOf rdf:resource="http://semanticbible.org/ns/2006/NTNames#Sosipater"/>
        <residentPlaceOf rdf:resource="http://semanticbible.org/ns/2006/NTNames#Stephanas"/>
        <residentPlaceOf rdf:resource="http://semanticbible.org/ns/2006/NTNames#Tertius"/>
        <residentPlaceOf rdf:resource="http://semanticbible.org/ns/2006/NTNames#Timothy"/>
        <visitedPlaceOf rdf:resource="http://semanticbible.org/ns/2006/NTNames#Apollos"/>
        <visitedPlaceOf rdf:resource="http://semanticbible.org/ns/2006/NTNames#Erastus"/>
        <rdfs:label xml:lang="en">Corinth</rdfs:label>
    </owl:NamedIndividual>
    


    <!-- http://semanticbible.org/ns/2006/NTNames#CorinthGeodata -->

    <owl:NamedIndividual rdf:about="http://semanticbible.org/ns/2006/NTNames#CorinthGeodata">
        <rdf:type rdf:resource="http://semanticbible.org/ns/2006/NTNames#GeographicLocation"/>
        <altitude rdf:datatype="http://www.w3.org/2001/XMLSchema#int">0</altitude>
        <latitude rdf:datatype="http://www.w3.org/2001/XMLSchema#double">37.89771145673512</latitude>
        <longitude rdf:datatype="http://www.w3.org/2001/XMLSchema#double">22.88904528961036</longitude>
        <rdfs:label xml:lang="en">geodata for Corinth</rdfs:label>
    </owl:NamedIndividual>
    


    <!-- http://semanticbible.org/ns/2006/NTNames#Corinthians -->

    <owl:NamedIndividual rdf:about="http://semanticbible.org/ns/2006/NTNames#Corinthians">
        <rdf:type rdf:resource="http://semanticbible.org/ns/2006/NTNames#ResidenceGroup"/>
        <rdfs:label xml:lang="en">Corinthians</rdfs:label>
    </owl:NamedIndividual>
    


    <!-- http://semanticbible.org/ns/2006/NTNames#Cornelius -->

    <owl:NamedIndividual rdf:about="http://semanticbible.org/ns/2006/NTNames#Cornelius">
        <rdf:type rdf:resource="http://semanticbible.org/ns/2006/NTNames#Man"/>
        <ethnicity rdf:resource="http://semanticbible.org/ns/2006/NTNames#Roman"/>
        <knows rdf:resource="http://semanticbible.org/ns/2006/NTNames#SimonPeter"/>
        <occupation rdf:datatype="http://www.w3.org/2001/XMLSchema#string">centurion</occupation>
        <rdfs:label xml:lang="en">Cornelius</rdfs:label>
    </owl:NamedIndividual>
    


    <!-- http://semanticbible.org/ns/2006/NTNames#Cos -->

    <owl:NamedIndividual rdf:about="http://semanticbible.org/ns/2006/NTNames#Cos">
        <rdf:type rdf:resource="http://semanticbible.org/ns/2006/NTNames#City"/>
        <location rdf:resource="http://semanticbible.org/ns/2006/NTNames#CosGeodata"/>
        <rdfs:label xml:lang="en">Cos</rdfs:label>
    </owl:NamedIndividual>
    


    <!-- http://semanticbible.org/ns/2006/NTNames#CosGeodata -->

    <owl:NamedIndividual rdf:about="http://semanticbible.org/ns/2006/NTNames#CosGeodata">
        <rdf:type rdf:resource="http://semanticbible.org/ns/2006/NTNames#GeographicLocation"/>
        <altitude rdf:datatype="http://www.w3.org/2001/XMLSchema#int">0</altitude>
        <latitude rdf:datatype="http://www.w3.org/2001/XMLSchema#double">36.79289004177876</latitude>
        <longitude rdf:datatype="http://www.w3.org/2001/XMLSchema#double">27.08847233780648</longitude>
        <rdfs:label xml:lang="en">geodata for Cos</rdfs:label>
    </owl:NamedIndividual>
    


    <!-- http://semanticbible.org/ns/2006/NTNames#Cosam -->

    <owl:NamedIndividual rdf:about="http://semanticbible.org/ns/2006/NTNames#Cosam">
        <rdf:type rdf:resource="http://semanticbible.org/ns/2006/NTNames#Man"/>
        <childOf rdf:resource="http://semanticbible.org/ns/2006/NTNames#Elmadam"/>
        <ethnicity rdf:resource="http://semanticbible.org/ns/2006/NTNames#Jewish"/>
        <parentOf rdf:resource="http://semanticbible.org/ns/2006/NTNames#Addi"/>
        <hasOnlyGenealogyMention rdf:datatype="http://www.w3.org/2001/XMLSchema#boolean">true</hasOnlyGenealogyMention>
        <rdfs:label xml:lang="en">Cosam</rdfs:label>
    </owl:NamedIndividual>
    


    <!-- http://semanticbible.org/ns/2006/NTNames#Crescens -->

    <owl:NamedIndividual rdf:about="http://semanticbible.org/ns/2006/NTNames#Crescens">
        <rdf:type rdf:resource="http://semanticbible.org/ns/2006/NTNames#Man"/>
        <collaboratesWith rdf:resource="http://semanticbible.org/ns/2006/NTNames#Paul"/>
        <description rdf:datatype="http://www.w3.org/2001/XMLSchema#string">a companion of the Apostle Paul</description>
        <rdfs:comment xml:lang="en">Crescens may have been from Rome originally</rdfs:comment>
        <rdfs:label xml:lang="en">Crescens</rdfs:label>
    </owl:NamedIndividual>
    


    <!-- http://semanticbible.org/ns/2006/NTNames#Cretans -->

    <owl:NamedIndividual rdf:about="http://semanticbible.org/ns/2006/NTNames#Cretans">
        <rdf:type rdf:resource="http://semanticbible.org/ns/2006/NTNames#EthnicGroup"/>
        <rdfs:label xml:lang="en">Cretans</rdfs:label>
    </owl:NamedIndividual>
    


    <!-- http://semanticbible.org/ns/2006/NTNames#Crete -->

    <owl:NamedIndividual rdf:about="http://semanticbible.org/ns/2006/NTNames#Crete">
        <rdf:type rdf:resource="http://semanticbible.org/ns/2006/NTNames#Island"/>
        <rdfs:label xml:lang="en">Crete</rdfs:label>
    </owl:NamedIndividual>
    


    <!-- http://semanticbible.org/ns/2006/NTNames#Crispus -->

    <owl:NamedIndividual rdf:about="http://semanticbible.org/ns/2006/NTNames#Crispus">
        <rdf:type rdf:resource="http://semanticbible.org/ns/2006/NTNames#Man"/>
        <knows rdf:resource="http://semanticbible.org/ns/2006/NTNames#Aquila"/>
        <knows rdf:resource="http://semanticbible.org/ns/2006/NTNames#GaiusOfCorinth"/>
        <knows rdf:resource="http://semanticbible.org/ns/2006/NTNames#Priscilla"/>
        <knows rdf:resource="http://semanticbible.org/ns/2006/NTNames#Silas"/>
        <knows rdf:resource="http://semanticbible.org/ns/2006/NTNames#Timothy"/>
        <description rdf:datatype="http://www.w3.org/2001/XMLSchema#string">a Corinthian Christian, and former ruler of the synagogue there</description>
        <rdfs:comment rdf:datatype="http://www.w3.org/2001/XMLSchema#string">As a prominent member of the church at Corinth, it seems reasonable to assume Crispus would know the other people from Corinth mentioned in the New Testament. </rdfs:comment>
        <rdfs:label xml:lang="en">Crispus</rdfs:label>
    </owl:NamedIndividual>
    


    <!-- http://semanticbible.org/ns/2006/NTNames#Cyprus -->

    <owl:NamedIndividual rdf:about="http://semanticbible.org/ns/2006/NTNames#Cyprus">
        <rdf:type rdf:resource="http://semanticbible.org/ns/2006/NTNames#Island"/>
        <rdfs:label xml:lang="en">Cyprus</rdfs:label>
    </owl:NamedIndividual>
    


    <!-- http://semanticbible.org/ns/2006/NTNames#Cyrene -->

    <owl:NamedIndividual rdf:about="http://semanticbible.org/ns/2006/NTNames#Cyrene">
        <rdf:type rdf:resource="http://semanticbible.org/ns/2006/NTNames#City"/>
        <rdfs:label xml:lang="en">Cyrene</rdfs:label>
    </owl:NamedIndividual>
    


    <!-- http://semanticbible.org/ns/2006/NTNames#Cyrenians -->

    <owl:NamedIndividual rdf:about="http://semanticbible.org/ns/2006/NTNames#Cyrenians">
        <rdf:type rdf:resource="http://semanticbible.org/ns/2006/NTNames#ResidenceGroup"/>
        <rdfs:label xml:lang="en">Cyrenians</rdfs:label>
    </owl:NamedIndividual>
    


    <!-- http://semanticbible.org/ns/2006/NTNames#Dalmanutha -->

    <owl:NamedIndividual rdf:about="http://semanticbible.org/ns/2006/NTNames#Dalmanutha">
        <rdf:type rdf:resource="http://semanticbible.org/ns/2006/NTNames#City"/>
        <location rdf:resource="http://semanticbible.org/ns/2006/NTNames#DalmanuthaGeodata"/>
        <rdfs:label xml:lang="en">Dalmanutha</rdfs:label>
    </owl:NamedIndividual>
    


    <!-- http://semanticbible.org/ns/2006/NTNames#DalmanuthaGeodata -->

    <owl:NamedIndividual rdf:about="http://semanticbible.org/ns/2006/NTNames#DalmanuthaGeodata">
        <rdf:type rdf:resource="http://semanticbible.org/ns/2006/NTNames#GeographicLocation"/>
        <altitude rdf:datatype="http://www.w3.org/2001/XMLSchema#int">0</altitude>
        <latitude rdf:datatype="http://www.w3.org/2001/XMLSchema#double">32.84830682682786</latitude>
        <longitude rdf:datatype="http://www.w3.org/2001/XMLSchema#double">35.52350046026037</longitude>
        <rdfs:label xml:lang="en">geodata for Dalmanutha</rdfs:label>
    </owl:NamedIndividual>
    


    <!-- http://semanticbible.org/ns/2006/NTNames#Dalmatia -->

    <owl:NamedIndividual rdf:about="http://semanticbible.org/ns/2006/NTNames#Dalmatia">
        <rdf:type rdf:resource="http://semanticbible.org/ns/2006/NTNames#StateOrProvince"/>
        <rdfs:label xml:lang="en">Dalmatia</rdfs:label>
    </owl:NamedIndividual>
    


    <!-- http://semanticbible.org/ns/2006/NTNames#Damaris -->

    <owl:NamedIndividual rdf:about="http://semanticbible.org/ns/2006/NTNames#Damaris">
        <rdf:type rdf:resource="http://semanticbible.org/ns/2006/NTNames#Woman"/>
        <knows rdf:resource="http://semanticbible.org/ns/2006/NTNames#Paul"/>
        <religiousBelief rdf:resource="http://semanticbible.org/ns/2006/NTNames#Christianity"/>
        <residentPlace rdf:resource="http://semanticbible.org/ns/2006/NTNames#Athens"/>
        <description rdf:datatype="http://www.w3.org/2001/XMLSchema#string">a convert from Paul&apos;s address to the Aeropagus</description>
        <hasOnlyGenealogyMention rdf:datatype="http://www.w3.org/2001/XMLSchema#boolean">false</hasOnlyGenealogyMention>
        <rdfs:comment xml:lang="en">Damaris was converted through Paul&apos;s preaching in Athens.</rdfs:comment>
        <rdfs:label xml:lang="en">Damaris</rdfs:label>
    </owl:NamedIndividual>
    


    <!-- http://semanticbible.org/ns/2006/NTNames#Damascus -->

    <owl:NamedIndividual rdf:about="http://semanticbible.org/ns/2006/NTNames#Damascus">
        <rdf:type rdf:resource="http://semanticbible.org/ns/2006/NTNames#City"/>
        <subregionOf rdf:resource="http://semanticbible.org/ns/2006/NTNames#Abilene"/>
        <rdfs:label xml:lang="en">Damascus</rdfs:label>
    </owl:NamedIndividual>
    


    <!-- http://semanticbible.org/ns/2006/NTNames#Daniel -->

    <owl:NamedIndividual rdf:about="http://semanticbible.org/ns/2006/NTNames#Daniel">
        <rdf:type rdf:resource="http://semanticbible.org/ns/2006/NTNames#Man"/>
        <description rdf:datatype="http://www.w3.org/2001/XMLSchema#string">an Old Testament prophet</description>
        <occupation rdf:datatype="http://www.w3.org/2001/XMLSchema#string">prophet</occupation>
        <rdfs:label xml:lang="en">Daniel</rdfs:label>
    </owl:NamedIndividual>
    


    <!-- http://semanticbible.org/ns/2006/NTNames#David -->

    <owl:NamedIndividual rdf:about="http://semanticbible.org/ns/2006/NTNames#David">
        <rdf:type rdf:resource="http://semanticbible.org/ns/2006/NTNames#Man"/>
        <childOf rdf:resource="http://semanticbible.org/ns/2006/NTNames#Jesse"/>
        <collaboratesWith rdf:resource="http://semanticbible.org/ns/2006/NTNames#Uriah"/>
        <enemyOf rdf:resource="http://semanticbible.org/ns/2006/NTNames#Uriah"/>
        <ethnicity rdf:resource="http://semanticbible.org/ns/2006/NTNames#Jewish"/>
        <parentOf rdf:resource="http://semanticbible.org/ns/2006/NTNames#Nathan"/>
        <parentOf rdf:resource="http://semanticbible.org/ns/2006/NTNames#Solomon"/>
        <spouseOf rdf:resource="http://semanticbible.org/ns/2006/NTNames#Bathsheba"/>
        <description rdf:datatype="http://www.w3.org/2001/XMLSchema#string">Israel&apos;s greatest king; author of many of the Old Testament Psalms</description>
        <hasOnlyGenealogyMention rdf:datatype="http://www.w3.org/2001/XMLSchema#boolean">false</hasOnlyGenealogyMention>
        <occupation rdf:datatype="http://www.w3.org/2001/XMLSchema#string">king of Israel</occupation>
        <rdfs:label xml:lang="en">David</rdfs:label>
    </owl:NamedIndividual>
    


    <!-- http://semanticbible.org/ns/2006/NTNames#Decapolis -->

    <owl:NamedIndividual rdf:about="http://semanticbible.org/ns/2006/NTNames#Decapolis">
        <rdf:type rdf:resource="http://semanticbible.org/ns/2006/NTNames#StateOrProvince"/>
        <subregion rdf:resource="http://semanticbible.org/ns/2006/NTNames#Gadara"/>
        <rdfs:label xml:lang="en">Decapolis</rdfs:label>
    </owl:NamedIndividual>
    


    <!-- http://semanticbible.org/ns/2006/NTNames#Demas -->

    <owl:NamedIndividual rdf:about="http://semanticbible.org/ns/2006/NTNames#Demas">
        <rdf:type rdf:resource="http://semanticbible.org/ns/2006/NTNames#Man"/>
        <collaboratesWith rdf:resource="http://semanticbible.org/ns/2006/NTNames#Paul"/>
        <rdfs:comment xml:lang="en">Though Paul describes Demas as &quot;my fellow worker&quot; in Philemon, later he apparently deserted him and went to Thessalonica. He was with Paul when he wrote his letter to  Philemon and the Colossians, but Paul&apos;s location when writing them is uncertain. </rdfs:comment>
        <rdfs:label xml:lang="en">Demas</rdfs:label>
    </owl:NamedIndividual>
    


    <!-- http://semanticbible.org/ns/2006/NTNames#Demetrius -->

    <owl:NamedIndividual rdf:about="http://semanticbible.org/ns/2006/NTNames#Demetrius">
        <rdf:type rdf:resource="http://semanticbible.org/ns/2006/NTNames#Man"/>
        <collaboratesWith rdf:resource="http://semanticbible.org/ns/2006/NTNames#JohnSonOfZebedee"/>
        <knows rdf:resource="http://semanticbible.org/ns/2006/NTNames#GaiusTheBeloved"/>
        <possiblySamePersonAs rdf:resource="http://semanticbible.org/ns/2006/NTNames#DemetriusTheSilversmith"/>
        <description rdf:datatype="http://www.w3.org/2001/XMLSchema#string">a disciple mentioned in 3 John as having a good reputation</description>
        <rdfs:comment xml:lang="en">See comment on DemetriusTheSilversmith. Keener suggests that 3John is a letter of support which Demetrius carried to Gaius. </rdfs:comment>
        <rdfs:label xml:lang="en">Demetrius</rdfs:label>
    </owl:NamedIndividual>
    


    <!-- http://semanticbible.org/ns/2006/NTNames#DemetriusTheSilversmith -->

    <owl:NamedIndividual rdf:about="http://semanticbible.org/ns/2006/NTNames#DemetriusTheSilversmith">
        <rdf:type rdf:resource="http://semanticbible.org/ns/2006/NTNames#Man"/>
        <enemyOf rdf:resource="http://semanticbible.org/ns/2006/NTNames#Paul"/>
        <possiblySamePersonAs rdf:resource="http://semanticbible.org/ns/2006/NTNames#Demetrius"/>
        <description rdf:datatype="http://www.w3.org/2001/XMLSchema#string">a craftsman in Ephesus who made silver shrines of Artemis</description>
        <occupation rdf:datatype="http://www.w3.org/2001/XMLSchema#string">silversmith</occupation>
        <rdfs:comment xml:lang="en">Demetrius was a common name, so it&apos;s unlikely this man is the same as the disciple mentioned in 3John.1.12.</rdfs:comment>
        <rdfs:label xml:lang="en">Demetrius</rdfs:label>
    </owl:NamedIndividual>
    


    <!-- http://semanticbible.org/ns/2006/NTNames#Derbe -->

    <owl:NamedIndividual rdf:about="http://semanticbible.org/ns/2006/NTNames#Derbe">
        <rdf:type rdf:resource="http://semanticbible.org/ns/2006/NTNames#City"/>
        <location rdf:resource="http://semanticbible.org/ns/2006/NTNames#DerbeGeodata"/>
        <nativePlaceOf rdf:resource="http://semanticbible.org/ns/2006/NTNames#GaiusOfDerbe"/>
        <rdfs:label xml:lang="en">Derbe</rdfs:label>
    </owl:NamedIndividual>
    


    <!-- http://semanticbible.org/ns/2006/NTNames#DerbeGeodata -->

    <owl:NamedIndividual rdf:about="http://semanticbible.org/ns/2006/NTNames#DerbeGeodata">
        <rdf:type rdf:resource="http://semanticbible.org/ns/2006/NTNames#GeographicLocation"/>
        <altitude rdf:datatype="http://www.w3.org/2001/XMLSchema#int">0</altitude>
        <latitude rdf:datatype="http://www.w3.org/2001/XMLSchema#double">37.37703789113421</latitude>
        <longitude rdf:datatype="http://www.w3.org/2001/XMLSchema#double">33.22035444184204</longitude>
        <rdfs:label xml:lang="en">geodata for Derbe</rdfs:label>
    </owl:NamedIndividual>
    


    <!-- http://semanticbible.org/ns/2006/NTNames#Dionysius -->

    <owl:NamedIndividual rdf:about="http://semanticbible.org/ns/2006/NTNames#Dionysius">
        <rdf:type rdf:resource="http://semanticbible.org/ns/2006/NTNames#Man"/>
        <rdfs:comment xml:lang="en">Though nothing else is recorded about Dionysius, the exclusivity and prestige of the Areopagus makes his descriptive surname significant. </rdfs:comment>
        <rdfs:label xml:lang="en">Dionysius</rdfs:label>
    </owl:NamedIndividual>
    


    <!-- http://semanticbible.org/ns/2006/NTNames#Diotrephes -->

    <owl:NamedIndividual rdf:about="http://semanticbible.org/ns/2006/NTNames#Diotrephes">
        <rdf:type rdf:resource="http://semanticbible.org/ns/2006/NTNames#Man"/>
        <antagonistOf rdf:resource="http://semanticbible.org/ns/2006/NTNames#JohnSonOfZebedee"/>
        <description rdf:datatype="http://www.w3.org/2001/XMLSchema#string">a member of the church to which 3 John was addressed</description>
        <rdfs:label xml:lang="en">Diotrephes</rdfs:label>
    </owl:NamedIndividual>
    


    <!-- http://semanticbible.org/ns/2006/NTNames#Drusilla -->

    <owl:NamedIndividual rdf:about="http://semanticbible.org/ns/2006/NTNames#Drusilla">
        <rdf:type rdf:resource="http://semanticbible.org/ns/2006/NTNames#Woman"/>
        <childOf rdf:resource="http://semanticbible.org/ns/2006/NTNames#HerodAgrippaI"/>
        <ethnicity rdf:resource="http://semanticbible.org/ns/2006/NTNames#Jewish"/>
        <residentPlace rdf:resource="http://semanticbible.org/ns/2006/NTNames#Caesarea"/>
        <siblingOf rdf:resource="http://semanticbible.org/ns/2006/NTNames#Bernice"/>
        <siblingOf rdf:resource="http://semanticbible.org/ns/2006/NTNames#HerodAgrippaII"/>
        <spouseOf rdf:resource="http://semanticbible.org/ns/2006/NTNames#Felix"/>
        <description rdf:datatype="http://www.w3.org/2001/XMLSchema#string">wife of Felix</description>
        <hasOnlyGenealogyMention rdf:datatype="http://www.w3.org/2001/XMLSchema#boolean">false</hasOnlyGenealogyMention>
        <rdfs:comment rdf:datatype="http://www.w3.org/2001/XMLSchema#string">Drusilla&apos;s locations are inferred from those of her husband. According to Josephus, she was the daughter of Herod Agrippa I. </rdfs:comment>
        <rdfs:label xml:lang="en">Drusilla</rdfs:label>
    </owl:NamedIndividual>
    


    <!-- http://semanticbible.org/ns/2006/NTNames#Eber -->

    <owl:NamedIndividual rdf:about="http://semanticbible.org/ns/2006/NTNames#Eber">
        <rdf:type rdf:resource="http://semanticbible.org/ns/2006/NTNames#Man"/>
        <childOf rdf:resource="http://semanticbible.org/ns/2006/NTNames#Shelah"/>
        <ethnicity rdf:resource="http://semanticbible.org/ns/2006/NTNames#Jewish"/>
        <parentOf rdf:resource="http://semanticbible.org/ns/2006/NTNames#Peleg"/>
        <description rdf:datatype="http://www.w3.org/2001/XMLSchema#string">One of the ancestors of Jesus mentioned in Luke&apos;s geneaology</description>
        <rdfs:label xml:lang="en">Eber</rdfs:label>
    </owl:NamedIndividual>
    


    <!-- http://semanticbible.org/ns/2006/NTNames#Egypt -->

    <owl:NamedIndividual rdf:about="http://semanticbible.org/ns/2006/NTNames#Egypt">
        <rdf:type rdf:resource="http://semanticbible.org/ns/2006/NTNames#Nation"/>
        <residentPlaceOf rdf:resource="http://semanticbible.org/ns/2006/NTNames#Mary"/>
        <rdfs:label xml:lang="en">Egypt</rdfs:label>
    </owl:NamedIndividual>
    


    <!-- http://semanticbible.org/ns/2006/NTNames#Egyptian -->

    <owl:NamedIndividual rdf:about="http://semanticbible.org/ns/2006/NTNames#Egyptian">
        <rdf:type rdf:resource="http://semanticbible.org/ns/2006/NTNames#EthnicityAttribute"/>
        <ethnicityOf rdf:resource="http://semanticbible.org/ns/2006/NTNames#Hagar"/>
        <rdfs:comment xml:lang="en">Only used in the New Testament to refer to those whose place of birth is Egypt. </rdfs:comment>
        <rdfs:label xml:lang="en">Egyptian</rdfs:label>
    </owl:NamedIndividual>
    


    <!-- http://semanticbible.org/ns/2006/NTNames#Egyptians -->

    <owl:NamedIndividual rdf:about="http://semanticbible.org/ns/2006/NTNames#Egyptians">
        <rdf:type rdf:resource="http://semanticbible.org/ns/2006/NTNames#EthnicGroup"/>
        <rdfs:label xml:lang="en">Egyptians</rdfs:label>
    </owl:NamedIndividual>
    


    <!-- http://semanticbible.org/ns/2006/NTNames#Elamites -->

    <owl:NamedIndividual rdf:about="http://semanticbible.org/ns/2006/NTNames#Elamites">
        <rdf:type rdf:resource="http://semanticbible.org/ns/2006/NTNames#EthnicGroup"/>
        <rdfs:label xml:lang="en">Elamites</rdfs:label>
    </owl:NamedIndividual>
    


    <!-- http://semanticbible.org/ns/2006/NTNames#Eleazar -->

    <owl:NamedIndividual rdf:about="http://semanticbible.org/ns/2006/NTNames#Eleazar">
        <rdf:type rdf:resource="http://semanticbible.org/ns/2006/NTNames#Man"/>
        <childOf rdf:resource="http://semanticbible.org/ns/2006/NTNames#Eliud"/>
        <ethnicity rdf:resource="http://semanticbible.org/ns/2006/NTNames#Jewish"/>
        <parentOf rdf:resource="http://semanticbible.org/ns/2006/NTNames#Matthan"/>
        <description rdf:datatype="http://www.w3.org/2001/XMLSchema#string">One of the ancestors of Jesus mentioned in Matthew&apos;s geneaology</description>
        <rdfs:label xml:lang="en">Eleazar</rdfs:label>
    </owl:NamedIndividual>
    


    <!-- http://semanticbible.org/ns/2006/NTNames#EliakimSonOfAbiud -->

    <owl:NamedIndividual rdf:about="http://semanticbible.org/ns/2006/NTNames#EliakimSonOfAbiud">
        <rdf:type rdf:resource="http://semanticbible.org/ns/2006/NTNames#Man"/>
        <childOf rdf:resource="http://semanticbible.org/ns/2006/NTNames#Abiud"/>
        <ethnicity rdf:resource="http://semanticbible.org/ns/2006/NTNames#Jewish"/>
        <parentOf rdf:resource="http://semanticbible.org/ns/2006/NTNames#Azor"/>
        <description rdf:datatype="http://www.w3.org/2001/XMLSchema#string">One of the ancestors of Jesus mentioned in Matthew&apos;s geneaology</description>
        <rdfs:label xml:lang="en">Eliakim</rdfs:label>
    </owl:NamedIndividual>
    


    <!-- http://semanticbible.org/ns/2006/NTNames#EliakimSonOfMelea -->

    <owl:NamedIndividual rdf:about="http://semanticbible.org/ns/2006/NTNames#EliakimSonOfMelea">
        <rdf:type rdf:resource="http://semanticbible.org/ns/2006/NTNames#Man"/>
        <childOf rdf:resource="http://semanticbible.org/ns/2006/NTNames#Melea"/>
        <ethnicity rdf:resource="http://semanticbible.org/ns/2006/NTNames#Jewish"/>
        <parentOf rdf:resource="http://semanticbible.org/ns/2006/NTNames#Jonam"/>
        <description rdf:datatype="http://www.w3.org/2001/XMLSchema#string">One of the ancestors of Jesus mentioned in Luke&apos;s geneaology</description>
        <hasOnlyGenealogyMention rdf:datatype="http://www.w3.org/2001/XMLSchema#boolean">true</hasOnlyGenealogyMention>
        <rdfs:label xml:lang="en">Eliakim</rdfs:label>
    </owl:NamedIndividual>
    


    <!-- http://semanticbible.org/ns/2006/NTNames#Eliezer -->

    <owl:NamedIndividual rdf:about="http://semanticbible.org/ns/2006/NTNames#Eliezer">
        <rdf:type rdf:resource="http://semanticbible.org/ns/2006/NTNames#Man"/>
        <childOf rdf:resource="http://semanticbible.org/ns/2006/NTNames#Jorim"/>
        <ethnicity rdf:resource="http://semanticbible.org/ns/2006/NTNames#Jewish"/>
        <parentOf rdf:resource="http://semanticbible.org/ns/2006/NTNames#JoshuaSonOfEliezer"/>
        <hasOnlyGenealogyMention rdf:datatype="http://www.w3.org/2001/XMLSchema#boolean">true</hasOnlyGenealogyMention>
        <rdfs:label xml:lang="en">Eliezer</rdfs:label>
    </owl:NamedIndividual>
    


    <!-- http://semanticbible.org/ns/2006/NTNames#Elijah -->

    <owl:NamedIndividual rdf:about="http://semanticbible.org/ns/2006/NTNames#Elijah">
        <rdf:type rdf:resource="http://semanticbible.org/ns/2006/NTNames#Man"/>
        <ethnicity rdf:resource="http://semanticbible.org/ns/2006/NTNames#Jewish"/>
        <knows rdf:resource="http://semanticbible.org/ns/2006/NTNames#Elisha"/>
        <description rdf:datatype="http://www.w3.org/2001/XMLSchema#string">one of the most notable prophets in the Old Testament</description>
        <rdfs:comment xml:lang="en">John the Baptist represented Elijah returned to his contemporaries, and the name is sometimes therefore used to refer to John (e.g. Matt.17.12).</rdfs:comment>
        <rdfs:label xml:lang="en">Elijah</rdfs:label>
    </owl:NamedIndividual>
    


    <!-- http://semanticbible.org/ns/2006/NTNames#Elisha -->

    <owl:NamedIndividual rdf:about="http://semanticbible.org/ns/2006/NTNames#Elisha">
        <rdf:type rdf:resource="http://semanticbible.org/ns/2006/NTNames#Man"/>
        <ethnicity rdf:resource="http://semanticbible.org/ns/2006/NTNames#Jewish"/>
        <knows rdf:resource="http://semanticbible.org/ns/2006/NTNames#Elijah"/>
        <description rdf:datatype="http://www.w3.org/2001/XMLSchema#string">an Old Testament prophet</description>
        <rdfs:label xml:lang="en">Elisha</rdfs:label>
    </owl:NamedIndividual>
    


    <!-- http://semanticbible.org/ns/2006/NTNames#Eliud -->

    <owl:NamedIndividual rdf:about="http://semanticbible.org/ns/2006/NTNames#Eliud">
        <rdf:type rdf:resource="http://semanticbible.org/ns/2006/NTNames#Man"/>
        <childOf rdf:resource="http://semanticbible.org/ns/2006/NTNames#Achim"/>
        <ethnicity rdf:resource="http://semanticbible.org/ns/2006/NTNames#Jewish"/>
        <parentOf rdf:resource="http://semanticbible.org/ns/2006/NTNames#Eleazar"/>
        <description rdf:datatype="http://www.w3.org/2001/XMLSchema#string">One of the ancestors of Jesus mentioned in Matthew&apos;s geneaology</description>
        <hasOnlyGenealogyMention rdf:datatype="http://www.w3.org/2001/XMLSchema#boolean">true</hasOnlyGenealogyMention>
        <rdfs:label xml:lang="en">Eliud</rdfs:label>
    </owl:NamedIndividual>
    


    <!-- http://semanticbible.org/ns/2006/NTNames#Elizabeth -->

    <owl:NamedIndividual rdf:about="http://semanticbible.org/ns/2006/NTNames#Elizabeth">
        <rdf:type rdf:resource="http://semanticbible.org/ns/2006/NTNames#Woman"/>
        <ethnicity rdf:resource="http://semanticbible.org/ns/2006/NTNames#Jewish"/>
        <nativePlace rdf:resource="http://semanticbible.org/ns/2006/NTNames#Judea"/>
        <parentOf rdf:resource="http://semanticbible.org/ns/2006/NTNames#JohntheBaptist"/>
        <relativeOf rdf:resource="http://semanticbible.org/ns/2006/NTNames#Mary"/>
        <religiousBelief rdf:resource="http://semanticbible.org/ns/2006/NTNames#Judaism"/>
        <residentPlace rdf:resource="http://semanticbible.org/ns/2006/NTNames#Judea"/>
        <spouseOf rdf:resource="http://semanticbible.org/ns/2006/NTNames#Zechariah"/>
        <description rdf:datatype="http://www.w3.org/2001/XMLSchema#string">the mother of John the Baptist</description>
        <hasOnlyGenealogyMention rdf:datatype="http://www.w3.org/2001/XMLSchema#boolean">false</hasOnlyGenealogyMention>
        <rdfs:comment xml:lang="en">Elizabeth was a kinswoman to Mary the mother of Jesus. Luke&apos;s gospel records that Mary visited her in a town in Judah, and that she was &quot;of the daughters of Aaron&quot;.</rdfs:comment>
        <rdfs:label xml:lang="en">Elizabeth</rdfs:label>
    </owl:NamedIndividual>
    


    <!-- http://semanticbible.org/ns/2006/NTNames#Elmadam -->

    <owl:NamedIndividual rdf:about="http://semanticbible.org/ns/2006/NTNames#Elmadam">
        <rdf:type rdf:resource="http://semanticbible.org/ns/2006/NTNames#Man"/>
        <childOf rdf:resource="http://semanticbible.org/ns/2006/NTNames#Er"/>
        <ethnicity rdf:resource="http://semanticbible.org/ns/2006/NTNames#Jewish"/>
        <parentOf rdf:resource="http://semanticbible.org/ns/2006/NTNames#Cosam"/>
        <description rdf:datatype="http://www.w3.org/2001/XMLSchema#string">One of the ancestors of Jesus mentioned in Luke&apos;s geneaology</description>
        <hasOnlyGenealogyMention rdf:datatype="http://www.w3.org/2001/XMLSchema#boolean">true</hasOnlyGenealogyMention>
        <rdfs:label xml:lang="en">Elmadam</rdfs:label>
    </owl:NamedIndividual>
    


    <!-- http://semanticbible.org/ns/2006/NTNames#Emmaus -->

    <owl:NamedIndividual rdf:about="http://semanticbible.org/ns/2006/NTNames#Emmaus">
        <rdf:type rdf:resource="http://semanticbible.org/ns/2006/NTNames#City"/>
        <location rdf:resource="http://semanticbible.org/ns/2006/NTNames#EmmausGeodata"/>
        <subregionOf rdf:resource="http://semanticbible.org/ns/2006/NTNames#Judea"/>
        <rdfs:comment xml:lang="en">Emmaus is a village about seven miles from Jerusalem. Jesus joined two disciples who were walking here, though they did not recognize Him until the end of the journey. </rdfs:comment>
        <rdfs:label xml:lang="en">Emmaus</rdfs:label>
    </owl:NamedIndividual>
    


    <!-- http://semanticbible.org/ns/2006/NTNames#EmmausGeodata -->

    <owl:NamedIndividual rdf:about="http://semanticbible.org/ns/2006/NTNames#EmmausGeodata">
        <rdf:type rdf:resource="http://semanticbible.org/ns/2006/NTNames#GeographicLocation"/>
        <altitude rdf:datatype="http://www.w3.org/2001/XMLSchema#int">0</altitude>
        <latitude rdf:datatype="http://www.w3.org/2001/XMLSchema#double">31.83790041996461</latitude>
        <longitude rdf:datatype="http://www.w3.org/2001/XMLSchema#double">34.99550449459134</longitude>
        <rdfs:label xml:lang="en">geodata for Emmaus</rdfs:label>
    </owl:NamedIndividual>
    


    <!-- http://semanticbible.org/ns/2006/NTNames#Enoch -->

    <owl:NamedIndividual rdf:about="http://semanticbible.org/ns/2006/NTNames#Enoch">
        <rdf:type rdf:resource="http://semanticbible.org/ns/2006/NTNames#Man"/>
        <childOf rdf:resource="http://semanticbible.org/ns/2006/NTNames#Jared"/>
        <parentOf rdf:resource="http://semanticbible.org/ns/2006/NTNames#Methuselah"/>
        <description rdf:datatype="http://www.w3.org/2001/XMLSchema#string">One of the ancestors of Jesus mentioned in Luke&apos;s geneaology</description>
        <hasOnlyGenealogyMention rdf:datatype="http://www.w3.org/2001/XMLSchema#boolean">false</hasOnlyGenealogyMention>
        <rdfs:comment xml:lang="en">Different from the eldest son of Cain (Gen.4:17)</rdfs:comment>
        <rdfs:label xml:lang="en">Enoch</rdfs:label>
    </owl:NamedIndividual>
    


    <!-- http://semanticbible.org/ns/2006/NTNames#Enos -->

    <owl:NamedIndividual rdf:about="http://semanticbible.org/ns/2006/NTNames#Enos">
        <rdf:type rdf:resource="http://semanticbible.org/ns/2006/NTNames#Man"/>
        <childOf rdf:resource="http://semanticbible.org/ns/2006/NTNames#Seth"/>
        <parentOf rdf:resource="http://semanticbible.org/ns/2006/NTNames#CainanSonOfEnosh"/>
        <description rdf:datatype="http://www.w3.org/2001/XMLSchema#string">One of the ancestors of Jesus mentioned in Luke&apos;s geneaology</description>
        <hasOnlyGenealogyMention rdf:datatype="http://www.w3.org/2001/XMLSchema#boolean">true</hasOnlyGenealogyMention>
        <rdfs:comment xml:lang="en">Enosh in the NIV</rdfs:comment>
        <rdfs:label xml:lang="en">Enos</rdfs:label>
    </owl:NamedIndividual>
    


    <!-- http://semanticbible.org/ns/2006/NTNames#Epaenetus -->

    <owl:NamedIndividual rdf:about="http://semanticbible.org/ns/2006/NTNames#Epaenetus">
        <rdf:type rdf:resource="http://semanticbible.org/ns/2006/NTNames#Man"/>
        <knows rdf:resource="http://semanticbible.org/ns/2006/NTNames#Paul"/>
        <knows rdf:resource="http://semanticbible.org/ns/2006/NTNames#Priscilla"/>
        <religiousBelief rdf:resource="http://semanticbible.org/ns/2006/NTNames#Christianity"/>
        <residentPlace rdf:resource="http://semanticbible.org/ns/2006/NTNames#Rome"/>
        <visitedPlace rdf:resource="http://semanticbible.org/ns/2006/NTNames#Asia"/>
        <description rdf:datatype="http://www.w3.org/2001/XMLSchema#string">A Christian in Rome whom Paul describes as &quot;the first convert to Christ in Asia&quot;</description>
        <hasOnlyGenealogyMention rdf:datatype="http://www.w3.org/2001/XMLSchema#boolean">false</hasOnlyGenealogyMention>
        <rdfs:label xml:lang="en">Epaenetus</rdfs:label>
    </owl:NamedIndividual>
    


    <!-- http://semanticbible.org/ns/2006/NTNames#Epaphras -->

    <owl:NamedIndividual rdf:about="http://semanticbible.org/ns/2006/NTNames#Epaphras">
        <rdf:type rdf:resource="http://semanticbible.org/ns/2006/NTNames#Man"/>
        <collaboratesWith rdf:resource="http://semanticbible.org/ns/2006/NTNames#Paul"/>
        <description rdf:datatype="http://www.w3.org/2001/XMLSchema#string">A fellow minister with Paul, and likely founder of the Colossian church</description>
        <occupation rdf:datatype="http://www.w3.org/2001/XMLSchema#string">missionary</occupation>
        <rdfs:comment xml:lang="en">Paul mentions that Epaphras &quot;worked hard&quot; for those in Laodicea and Hierapolis, so it&apos;s possible (but not certain) he visited there as well. </rdfs:comment>
        <rdfs:label xml:lang="en">Epaphras</rdfs:label>
    </owl:NamedIndividual>
    


    <!-- http://semanticbible.org/ns/2006/NTNames#Epaphroditus -->

    <owl:NamedIndividual rdf:about="http://semanticbible.org/ns/2006/NTNames#Epaphroditus">
        <rdf:type rdf:resource="http://semanticbible.org/ns/2006/NTNames#Man"/>
        <collaboratesWith rdf:resource="http://semanticbible.org/ns/2006/NTNames#Paul"/>
        <description rdf:datatype="http://www.w3.org/2001/XMLSchema#string">A Christian sent by the Philippian church with a gift for Paul</description>
        <rdfs:comment xml:lang="en">Though Epaphras is a contraction of Epaphroditus, this individual is distinct from the Epaphras mentioned in Colossians and Philemon.
Rome as a visitedPlace assumes Paul was there while writing Philippians. </rdfs:comment>
        <rdfs:label xml:lang="en">Epaphroditus</rdfs:label>
    </owl:NamedIndividual>
    


    <!-- http://semanticbible.org/ns/2006/NTNames#Ephesian -->

    <owl:NamedIndividual rdf:about="http://semanticbible.org/ns/2006/NTNames#Ephesian">
        <rdf:type rdf:resource="http://semanticbible.org/ns/2006/NTNames#ResidencyAttribute"/>
        <rdfs:label xml:lang="en">Ephesian</rdfs:label>
    </owl:NamedIndividual>
    


    <!-- http://semanticbible.org/ns/2006/NTNames#Ephesians -->

    <owl:NamedIndividual rdf:about="http://semanticbible.org/ns/2006/NTNames#Ephesians">
        <rdf:type rdf:resource="http://semanticbible.org/ns/2006/NTNames#ResidenceGroup"/>
        <rdfs:label xml:lang="en">Ephesians</rdfs:label>
    </owl:NamedIndividual>
    


    <!-- http://semanticbible.org/ns/2006/NTNames#Ephesus -->

    <owl:NamedIndividual rdf:about="http://semanticbible.org/ns/2006/NTNames#Ephesus">
        <rdf:type rdf:resource="http://semanticbible.org/ns/2006/NTNames#City"/>
        <location rdf:resource="http://semanticbible.org/ns/2006/NTNames#EphesusGeodata"/>
        <residentPlaceOf rdf:resource="http://semanticbible.org/ns/2006/NTNames#Aquila"/>
        <residentPlaceOf rdf:resource="http://semanticbible.org/ns/2006/NTNames#Paul"/>
        <residentPlaceOf rdf:resource="http://semanticbible.org/ns/2006/NTNames#Priscilla"/>
        <visitedPlaceOf rdf:resource="http://semanticbible.org/ns/2006/NTNames#Achaicus"/>
        <visitedPlaceOf rdf:resource="http://semanticbible.org/ns/2006/NTNames#Apollos"/>
        <visitedPlaceOf rdf:resource="http://semanticbible.org/ns/2006/NTNames#Aristarchus"/>
        <visitedPlaceOf rdf:resource="http://semanticbible.org/ns/2006/NTNames#Erastus"/>
        <visitedPlaceOf rdf:resource="http://semanticbible.org/ns/2006/NTNames#Fortunatus"/>
        <visitedPlaceOf rdf:resource="http://semanticbible.org/ns/2006/NTNames#GaiusOfMacedonia"/>
        <visitedPlaceOf rdf:resource="http://semanticbible.org/ns/2006/NTNames#Stephanas"/>
        <rdfs:label xml:lang="en">Ephesus</rdfs:label>
    </owl:NamedIndividual>
    


    <!-- http://semanticbible.org/ns/2006/NTNames#EphesusGeodata -->

    <owl:NamedIndividual rdf:about="http://semanticbible.org/ns/2006/NTNames#EphesusGeodata">
        <rdf:type rdf:resource="http://semanticbible.org/ns/2006/NTNames#GeographicLocation"/>
        <altitude rdf:datatype="http://www.w3.org/2001/XMLSchema#int">0</altitude>
        <latitude rdf:datatype="http://www.w3.org/2001/XMLSchema#double">37.95451808351513</latitude>
        <longitude rdf:datatype="http://www.w3.org/2001/XMLSchema#double">27.36811967648377</longitude>
        <rdfs:label xml:lang="en">geodata for Ephesus</rdfs:label>
    </owl:NamedIndividual>
    


    <!-- http://semanticbible.org/ns/2006/NTNames#Ephraim -->

    <owl:NamedIndividual rdf:about="http://semanticbible.org/ns/2006/NTNames#Ephraim">
        <rdf:type rdf:resource="http://semanticbible.org/ns/2006/NTNames#City"/>
        <location rdf:resource="http://semanticbible.org/ns/2006/NTNames#EphraimGeodata"/>
        <subregionOf rdf:resource="http://semanticbible.org/ns/2006/NTNames#Judea"/>
        <rdfs:comment xml:lang="en">Jesus retreated to this town with his disciples when the Jews plotted to kill him after Lazarus was raised from the dead.</rdfs:comment>
        <rdfs:label xml:lang="en">Ephraim</rdfs:label>
    </owl:NamedIndividual>
    


    <!-- http://semanticbible.org/ns/2006/NTNames#EphraimGeodata -->

    <owl:NamedIndividual rdf:about="http://semanticbible.org/ns/2006/NTNames#EphraimGeodata">
        <rdf:type rdf:resource="http://semanticbible.org/ns/2006/NTNames#GeographicLocation"/>
        <altitude rdf:datatype="http://www.w3.org/2001/XMLSchema#int">0</altitude>
        <latitude rdf:datatype="http://www.w3.org/2001/XMLSchema#double">31.94718085585583</latitude>
        <longitude rdf:datatype="http://www.w3.org/2001/XMLSchema#double">35.30400861340603</longitude>
        <rdfs:label xml:lang="en">geodata for Ephraim</rdfs:label>
    </owl:NamedIndividual>
    


    <!-- http://semanticbible.org/ns/2006/NTNames#Epicurean -->

    <owl:NamedIndividual rdf:about="http://semanticbible.org/ns/2006/NTNames#Epicurean">
        <rdf:type rdf:resource="http://semanticbible.org/ns/2006/NTNames#ReligiousBelief"/>
        <rdfs:label xml:lang="en">Epicurean</rdfs:label>
    </owl:NamedIndividual>
    


    <!-- http://semanticbible.org/ns/2006/NTNames#Er -->

    <owl:NamedIndividual rdf:about="http://semanticbible.org/ns/2006/NTNames#Er">
        <rdf:type rdf:resource="http://semanticbible.org/ns/2006/NTNames#Man"/>
        <childOf rdf:resource="http://semanticbible.org/ns/2006/NTNames#JoshuaSonOfEliezer"/>
        <ethnicity rdf:resource="http://semanticbible.org/ns/2006/NTNames#Jewish"/>
        <parentOf rdf:resource="http://semanticbible.org/ns/2006/NTNames#Elmadam"/>
        <description rdf:datatype="http://www.w3.org/2001/XMLSchema#string">One of the ancestors of Jesus mentioned in Luke&apos;s geneaology</description>
        <hasOnlyGenealogyMention rdf:datatype="http://www.w3.org/2001/XMLSchema#boolean">true</hasOnlyGenealogyMention>
        <rdfs:label xml:lang="en">Er</rdfs:label>
    </owl:NamedIndividual>
    


    <!-- http://semanticbible.org/ns/2006/NTNames#Erastus -->

    <owl:NamedIndividual rdf:about="http://semanticbible.org/ns/2006/NTNames#Erastus">
        <rdf:type rdf:resource="http://semanticbible.org/ns/2006/NTNames#Man"/>
        <collaboratesWith rdf:resource="http://semanticbible.org/ns/2006/NTNames#Paul"/>
        <collaboratesWith rdf:resource="http://semanticbible.org/ns/2006/NTNames#Timothy"/>
        <possiblySamePersonAs rdf:resource="http://semanticbible.org/ns/2006/NTNames#ErastusTheTreasurer"/>
        <visitedPlace rdf:resource="http://semanticbible.org/ns/2006/NTNames#Corinth"/>
        <visitedPlace rdf:resource="http://semanticbible.org/ns/2006/NTNames#Ephesus"/>
        <visitedPlace rdf:resource="http://semanticbible.org/ns/2006/NTNames#Macedonia"/>
        <description rdf:datatype="http://www.w3.org/2001/XMLSchema#string">a travelling companion of Paul</description>
        <hasOnlyGenealogyMention rdf:datatype="http://www.w3.org/2001/XMLSchema#boolean">false</hasOnlyGenealogyMention>
        <rdfs:comment xml:lang="en">There are two references to this Erastus: it&apos;s possible they represent two different people. See also the comment on ErastusTheTreasurer.	</rdfs:comment>
        <rdfs:label xml:lang="en">Erastus</rdfs:label>
    </owl:NamedIndividual>
    


    <!-- http://semanticbible.org/ns/2006/NTNames#ErastusTheTreasurer -->

    <owl:NamedIndividual rdf:about="http://semanticbible.org/ns/2006/NTNames#ErastusTheTreasurer">
        <rdf:type rdf:resource="http://semanticbible.org/ns/2006/NTNames#Man"/>
        <knows rdf:resource="http://semanticbible.org/ns/2006/NTNames#Paul"/>
        <possiblySamePersonAs rdf:resource="http://semanticbible.org/ns/2006/NTNames#Erastus"/>
        <hasOnlyGenealogyMention rdf:datatype="http://www.w3.org/2001/XMLSchema#boolean">false</hasOnlyGenealogyMention>
        <occupation rdf:datatype="http://www.w3.org/2001/XMLSchema#string">treasurer</occupation>
        <rdfs:comment rdf:datatype="http://www.w3.org/2001/XMLSchema#string">It is uncertain whether this Erastus is the same as Paul&apos;s travelling companion and fellow minister, though possible. </rdfs:comment>
        <rdfs:label rdf:datatype="http://www.w3.org/2001/XMLSchema#string">Erastus the city treasurer</rdfs:label>
    </owl:NamedIndividual>
    


    <!-- http://semanticbible.org/ns/2006/NTNames#Esau -->

    <owl:NamedIndividual rdf:about="http://semanticbible.org/ns/2006/NTNames#Esau">
        <rdf:type rdf:resource="http://semanticbible.org/ns/2006/NTNames#Man"/>
        <childOf rdf:resource="http://semanticbible.org/ns/2006/NTNames#Isaac"/>
        <childOf rdf:resource="http://semanticbible.org/ns/2006/NTNames#Rebecca"/>
        <ethnicity rdf:resource="http://semanticbible.org/ns/2006/NTNames#Jewish"/>
        <siblingOf rdf:resource="http://semanticbible.org/ns/2006/NTNames#Jacob"/>
        <description rdf:datatype="http://www.w3.org/2001/XMLSchema#string">a character from the Old Testament era</description>
        <rdfs:label xml:lang="en">Esau</rdfs:label>
    </owl:NamedIndividual>
    


    <!-- http://semanticbible.org/ns/2006/NTNames#Esli -->

    <owl:NamedIndividual rdf:about="http://semanticbible.org/ns/2006/NTNames#Esli">
        <rdf:type rdf:resource="http://semanticbible.org/ns/2006/NTNames#Man"/>
        <childOf rdf:resource="http://semanticbible.org/ns/2006/NTNames#Naggai"/>
        <ethnicity rdf:resource="http://semanticbible.org/ns/2006/NTNames#Jewish"/>
        <parentOf rdf:resource="http://semanticbible.org/ns/2006/NTNames#Nahum"/>
        <description rdf:datatype="http://www.w3.org/2001/XMLSchema#string">One of the ancestors of Jesus mentioned in Luke&apos;s geneaology</description>
        <hasOnlyGenealogyMention rdf:datatype="http://www.w3.org/2001/XMLSchema#boolean">true</hasOnlyGenealogyMention>
        <rdfs:label xml:lang="en">Esli</rdfs:label>
    </owl:NamedIndividual>
    


    <!-- http://semanticbible.org/ns/2006/NTNames#Ethiopia -->

    <owl:NamedIndividual rdf:about="http://semanticbible.org/ns/2006/NTNames#Ethiopia">
        <rdf:type rdf:resource="http://semanticbible.org/ns/2006/NTNames#Nation"/>
        <rdfs:comment xml:lang="en">Not named in the New Testament.</rdfs:comment>
    </owl:NamedIndividual>
    


    <!-- http://semanticbible.org/ns/2006/NTNames#Ethiopian -->

    <owl:NamedIndividual rdf:about="http://semanticbible.org/ns/2006/NTNames#Ethiopian">
        <rdf:type rdf:resource="http://semanticbible.org/ns/2006/NTNames#EthnicityAttribute"/>
        <ethnicityOf rdf:resource="http://semanticbible.org/ns/2006/NTNames#Candace"/>
        <rdfs:comment xml:lang="en">Of the country of Ethiopia. </rdfs:comment>
        <rdfs:label xml:lang="en">Ethiopian</rdfs:label>
    </owl:NamedIndividual>
    


    <!-- http://semanticbible.org/ns/2006/NTNames#Ethiopians -->

    <owl:NamedIndividual rdf:about="http://semanticbible.org/ns/2006/NTNames#Ethiopians">
        <rdf:type rdf:resource="http://semanticbible.org/ns/2006/NTNames#EthnicGroup"/>
        <rdfs:label xml:lang="en">Ethiopians</rdfs:label>
    </owl:NamedIndividual>
    


    <!-- http://semanticbible.org/ns/2006/NTNames#Eubulus -->

    <owl:NamedIndividual rdf:about="http://semanticbible.org/ns/2006/NTNames#Eubulus">
        <rdf:type rdf:resource="http://semanticbible.org/ns/2006/NTNames#Man"/>
        <collaboratesWith rdf:resource="http://semanticbible.org/ns/2006/NTNames#Paul"/>
        <religiousBelief rdf:resource="http://semanticbible.org/ns/2006/NTNames#Christianity"/>
        <residentPlace rdf:resource="http://semanticbible.org/ns/2006/NTNames#Rome"/>
        <description rdf:datatype="http://www.w3.org/2001/XMLSchema#string">a Christian companion of the Apostle Paul in his Roman imprisonment</description>
        <hasOnlyGenealogyMention rdf:datatype="http://www.w3.org/2001/XMLSchema#boolean">false</hasOnlyGenealogyMention>
        <rdfs:comment rdf:datatype="http://www.w3.org/2001/XMLSchema#string">His residence in Rome assumes </rdfs:comment>
        <rdfs:label xml:lang="en">Eubulus</rdfs:label>
    </owl:NamedIndividual>
    


    <!-- http://semanticbible.org/ns/2006/NTNames#Eunice -->

    <owl:NamedIndividual rdf:about="http://semanticbible.org/ns/2006/NTNames#Eunice">
        <rdf:type rdf:resource="http://semanticbible.org/ns/2006/NTNames#Woman"/>
        <childOf rdf:resource="http://semanticbible.org/ns/2006/NTNames#Lois"/>
        <collaboratesWith rdf:resource="http://semanticbible.org/ns/2006/NTNames#Paul"/>
        <ethnicity rdf:resource="http://semanticbible.org/ns/2006/NTNames#Jewish"/>
        <parentOf rdf:resource="http://semanticbible.org/ns/2006/NTNames#Timothy"/>
        <religiousBelief rdf:resource="http://semanticbible.org/ns/2006/NTNames#Christianity"/>
        <residentPlace rdf:resource="http://semanticbible.org/ns/2006/NTNames#Lystra"/>
        <description rdf:datatype="http://www.w3.org/2001/XMLSchema#string">the mother of Timothy</description>
        <hasOnlyGenealogyMention rdf:datatype="http://www.w3.org/2001/XMLSchema#boolean">false</hasOnlyGenealogyMention>
        <rdfs:comment xml:lang="en">Eunice&apos;s residence in Lystra is implied by Acts.16.1, though Derbe is also possible. Her Christian faith is strongly implied by Paul&apos;s commendation of it in 2Tim.1.5. </rdfs:comment>
        <rdfs:label xml:lang="en">Eunice</rdfs:label>
    </owl:NamedIndividual>
    


    <!-- http://semanticbible.org/ns/2006/NTNames#Euodia -->

    <owl:NamedIndividual rdf:about="http://semanticbible.org/ns/2006/NTNames#Euodia">
        <rdf:type rdf:resource="http://semanticbible.org/ns/2006/NTNames#Woman"/>
        <collaboratesWith rdf:resource="http://semanticbible.org/ns/2006/NTNames#Clement"/>
        <collaboratesWith rdf:resource="http://semanticbible.org/ns/2006/NTNames#Paul"/>
        <collaboratesWith rdf:resource="http://semanticbible.org/ns/2006/NTNames#Syntyche"/>
        <religiousBelief rdf:resource="http://semanticbible.org/ns/2006/NTNames#Christianity"/>
        <residentPlace rdf:resource="http://semanticbible.org/ns/2006/NTNames#Philippi"/>
        <description rdf:datatype="http://www.w3.org/2001/XMLSchema#string">a Christian in Philippi</description>
        <hasOnlyGenealogyMention rdf:datatype="http://www.w3.org/2001/XMLSchema#boolean">false</hasOnlyGenealogyMention>
        <rdfs:label xml:lang="en">Euodia</rdfs:label>
    </owl:NamedIndividual>
    


    <!-- http://semanticbible.org/ns/2006/NTNames#Euphrates -->

    <owl:NamedIndividual rdf:about="http://semanticbible.org/ns/2006/NTNames#Euphrates">
        <rdf:type rdf:resource="http://semanticbible.org/ns/2006/NTNames#FreshWaterArea"/>
        <rdfs:label xml:lang="en">Euphrates</rdfs:label>
    </owl:NamedIndividual>
    


    <!-- http://semanticbible.org/ns/2006/NTNames#Eutychus -->

    <owl:NamedIndividual rdf:about="http://semanticbible.org/ns/2006/NTNames#Eutychus">
        <rdf:type rdf:resource="http://semanticbible.org/ns/2006/NTNames#Man"/>
        <knows rdf:resource="http://semanticbible.org/ns/2006/NTNames#Paul"/>
        <residentPlace rdf:resource="http://semanticbible.org/ns/2006/NTNames#Troas"/>
        <description rdf:datatype="http://www.w3.org/2001/XMLSchema#string">a young man who fell asleep during a lengthy sermon by Paul</description>
        <hasOnlyGenealogyMention rdf:datatype="http://www.w3.org/2001/XMLSchema#boolean">false</hasOnlyGenealogyMention>
        <rdfs:label xml:lang="en">Eutychus</rdfs:label>
    </owl:NamedIndividual>
    


    <!-- http://semanticbible.org/ns/2006/NTNames#Eve -->

    <owl:NamedIndividual rdf:about="http://semanticbible.org/ns/2006/NTNames#Eve">
        <rdf:type rdf:resource="http://semanticbible.org/ns/2006/NTNames#Woman"/>
        <parentOf rdf:resource="http://semanticbible.org/ns/2006/NTNames#Abel"/>
        <parentOf rdf:resource="http://semanticbible.org/ns/2006/NTNames#Cain"/>
        <spouseOf rdf:resource="http://semanticbible.org/ns/2006/NTNames#Adam"/>
        <description rdf:datatype="http://www.w3.org/2001/XMLSchema#string">the first woman created by God</description>
        <hasOnlyGenealogyMention rdf:datatype="http://www.w3.org/2001/XMLSchema#boolean">false</hasOnlyGenealogyMention>
        <rdfs:label xml:lang="en">Eve</rdfs:label>
    </owl:NamedIndividual>
    


    <!-- http://semanticbible.org/ns/2006/NTNames#FairHavens -->

    <owl:NamedIndividual rdf:about="http://semanticbible.org/ns/2006/NTNames#FairHavens">
        <rdf:type rdf:resource="http://semanticbible.org/ns/2006/NTNames#SaltWaterArea"/>
        <location rdf:resource="http://semanticbible.org/ns/2006/NTNames#FairHavensGeodata"/>
        <rdfs:label xml:lang="en">Fair Havens</rdfs:label>
    </owl:NamedIndividual>
    


    <!-- http://semanticbible.org/ns/2006/NTNames#FairHavensGeodata -->

    <owl:NamedIndividual rdf:about="http://semanticbible.org/ns/2006/NTNames#FairHavensGeodata">
        <rdf:type rdf:resource="http://semanticbible.org/ns/2006/NTNames#GeographicLocation"/>
        <altitude rdf:datatype="http://www.w3.org/2001/XMLSchema#int">0</altitude>
        <latitude rdf:datatype="http://www.w3.org/2001/XMLSchema#double">34.93065966009429</latitude>
        <longitude rdf:datatype="http://www.w3.org/2001/XMLSchema#double">24.73534424651286</longitude>
        <rdfs:label xml:lang="en">geodata for Fair Havens</rdfs:label>
    </owl:NamedIndividual>
    


    <!-- http://semanticbible.org/ns/2006/NTNames#Felix -->

    <owl:NamedIndividual rdf:about="http://semanticbible.org/ns/2006/NTNames#Felix">
        <rdf:type rdf:resource="http://semanticbible.org/ns/2006/NTNames#Man"/>
        <enemyOf rdf:resource="http://semanticbible.org/ns/2006/NTNames#Paul"/>
        <ethnicity rdf:resource="http://semanticbible.org/ns/2006/NTNames#Roman"/>
        <residentPlace rdf:resource="http://semanticbible.org/ns/2006/NTNames#Caesarea"/>
        <spouseOf rdf:resource="http://semanticbible.org/ns/2006/NTNames#Drusilla"/>
        <description rdf:datatype="http://www.w3.org/2001/XMLSchema#string">governor of Judea during the time when Paul was arrested in the Temple</description>
        <hasOnlyGenealogyMention rdf:datatype="http://www.w3.org/2001/XMLSchema#boolean">false</hasOnlyGenealogyMention>
        <occupation rdf:datatype="http://www.w3.org/2001/XMLSchema#string">governor of Judea</occupation>
        <rdfs:comment rdf:datatype="http://www.w3.org/2001/XMLSchema#string">Properly Antonius Felix</rdfs:comment>
        <rdfs:label xml:lang="en">Felix</rdfs:label>
    </owl:NamedIndividual>
    


    <!-- http://semanticbible.org/ns/2006/NTNames#Festus -->

    <owl:NamedIndividual rdf:about="http://semanticbible.org/ns/2006/NTNames#Festus">
        <rdf:type rdf:resource="http://semanticbible.org/ns/2006/NTNames#Man"/>
        <ethnicity rdf:resource="http://semanticbible.org/ns/2006/NTNames#Roman"/>
        <knows rdf:resource="http://semanticbible.org/ns/2006/NTNames#Bernice"/>
        <knows rdf:resource="http://semanticbible.org/ns/2006/NTNames#HerodAgrippaII"/>
        <knows rdf:resource="http://semanticbible.org/ns/2006/NTNames#Paul"/>
        <residentPlace rdf:resource="http://semanticbible.org/ns/2006/NTNames#Caesarea"/>
        <visitedPlace rdf:resource="http://semanticbible.org/ns/2006/NTNames#Jerusalem"/>
        <description rdf:datatype="http://www.w3.org/2001/XMLSchema#string">governor of Judea after Felix</description>
        <hasOnlyGenealogyMention rdf:datatype="http://www.w3.org/2001/XMLSchema#boolean">false</hasOnlyGenealogyMention>
        <occupation rdf:datatype="http://www.w3.org/2001/XMLSchema#string">governor</occupation>
        <rdfs:label xml:lang="en">Festus</rdfs:label>
    </owl:NamedIndividual>
    


    <!-- http://semanticbible.org/ns/2006/NTNames#Fortunatus -->

    <owl:NamedIndividual rdf:about="http://semanticbible.org/ns/2006/NTNames#Fortunatus">
        <rdf:type rdf:resource="http://semanticbible.org/ns/2006/NTNames#Man"/>
        <collaboratesWith rdf:resource="http://semanticbible.org/ns/2006/NTNames#Achaicus"/>
        <collaboratesWith rdf:resource="http://semanticbible.org/ns/2006/NTNames#Paul"/>
        <collaboratesWith rdf:resource="http://semanticbible.org/ns/2006/NTNames#Stephanas"/>
        <religiousBelief rdf:resource="http://semanticbible.org/ns/2006/NTNames#Christianity"/>
        <residentPlace rdf:resource="http://semanticbible.org/ns/2006/NTNames#Corinth"/>
        <visitedPlace rdf:resource="http://semanticbible.org/ns/2006/NTNames#Ephesus"/>
        <description rdf:datatype="http://www.w3.org/2001/XMLSchema#string">A member of Corinthian church who visited the Apostle Paul in Ephesus, perhaps bearing a letter to him.</description>
        <hasOnlyGenealogyMention rdf:datatype="http://www.w3.org/2001/XMLSchema#boolean">false</hasOnlyGenealogyMention>
        <rdfs:comment rdf:datatype="http://www.w3.org/2001/XMLSchema#string">His residence in Corinth and visit to Ephesus follow from Paul&apos;s statement in 1Cor.16.17, and the assumption that Paul was in Ephesus when he wrote 1 Corinthians. </rdfs:comment>
        <rdfs:label xml:lang="en">Fortunatus</rdfs:label>
    </owl:NamedIndividual>
    


    <!-- http://semanticbible.org/ns/2006/NTNames#Freedmen -->

    <owl:NamedIndividual rdf:about="http://semanticbible.org/ns/2006/NTNames#Freedmen">
        <rdf:type rdf:resource="http://semanticbible.org/ns/2006/NTNames#GroupOfPeople"/>
        <rdfs:label xml:lang="en">Freedmen</rdfs:label>
    </owl:NamedIndividual>
    


    <!-- http://semanticbible.org/ns/2006/NTNames#Gabbatha -->

    <owl:NamedIndividual rdf:about="http://semanticbible.org/ns/2006/NTNames#Gabbatha">
        <rdf:type rdf:resource="http://semanticbible.org/ns/2006/NTNames#LandArea"/>
        <rdfs:label xml:lang="en">Gabbatha</rdfs:label>
    </owl:NamedIndividual>
    


    <!-- http://semanticbible.org/ns/2006/NTNames#Gabriel -->

    <owl:NamedIndividual rdf:about="http://semanticbible.org/ns/2006/NTNames#Gabriel">
        <rdf:type rdf:resource="http://semanticbible.org/ns/2006/NTNames#Angel"/>
        <rdfs:label xml:lang="en">Gabriel</rdfs:label>
    </owl:NamedIndividual>
    


    <!-- http://semanticbible.org/ns/2006/NTNames#Gad -->

    <owl:NamedIndividual rdf:about="http://semanticbible.org/ns/2006/NTNames#Gad">
        <rdf:type rdf:resource="http://semanticbible.org/ns/2006/NTNames#Man"/>
        <childOf rdf:resource="http://semanticbible.org/ns/2006/NTNames#Jacob"/>
        <ethnicity rdf:resource="http://semanticbible.org/ns/2006/NTNames#Jewish"/>
        <siblingOf rdf:resource="http://semanticbible.org/ns/2006/NTNames#Asher"/>
        <siblingOf rdf:resource="http://semanticbible.org/ns/2006/NTNames#Benjamin"/>
        <siblingOf rdf:resource="http://semanticbible.org/ns/2006/NTNames#Issachar"/>
        <siblingOf rdf:resource="http://semanticbible.org/ns/2006/NTNames#JosephThePatriarch"/>
        <siblingOf rdf:resource="http://semanticbible.org/ns/2006/NTNames#Judah"/>
        <siblingOf rdf:resource="http://semanticbible.org/ns/2006/NTNames#Levi"/>
        <siblingOf rdf:resource="http://semanticbible.org/ns/2006/NTNames#ManassehThePatriarch"/>
        <siblingOf rdf:resource="http://semanticbible.org/ns/2006/NTNames#Naphtali"/>
        <siblingOf rdf:resource="http://semanticbible.org/ns/2006/NTNames#Reuben"/>
        <siblingOf rdf:resource="http://semanticbible.org/ns/2006/NTNames#SimeonThePatriarch"/>
        <siblingOf rdf:resource="http://semanticbible.org/ns/2006/NTNames#Zebulun"/>
        <description rdf:datatype="http://www.w3.org/2001/XMLSchema#string">One of the 12 Patriarchs of Israel</description>
        <hasOnlyGenealogyMention rdf:datatype="http://www.w3.org/2001/XMLSchema#boolean">false</hasOnlyGenealogyMention>
        <rdfs:comment rdf:datatype="http://www.w3.org/2001/XMLSchema#string">His mother Zilpah, Leah&apos;s servant, is not named in the New Testament. </rdfs:comment>
        <rdfs:label xml:lang="en">Gad</rdfs:label>
    </owl:NamedIndividual>
    


    <!-- http://semanticbible.org/ns/2006/NTNames#Gadara -->

    <owl:NamedIndividual rdf:about="http://semanticbible.org/ns/2006/NTNames#Gadara">
        <rdf:type rdf:resource="http://semanticbible.org/ns/2006/NTNames#City"/>
        <subregionOf rdf:resource="http://semanticbible.org/ns/2006/NTNames#Decapolis"/>
        <rdfs:comment rdf:datatype="http://www.w3.org/2001/XMLSchema#string">City southeast of the Sea of Galilee. Not mentioned in Scripture as such, but &quot;the country of the Gadarenes&quot; (Matt 8.28) takes its name from this city. 
Part of the Decapolis.</rdfs:comment>
        <rdfs:label xml:lang="en">Gadara</rdfs:label>
    </owl:NamedIndividual>
    


    <!-- http://semanticbible.org/ns/2006/NTNames#Gadarenes -->

    <owl:NamedIndividual rdf:about="http://semanticbible.org/ns/2006/NTNames#Gadarenes">
        <rdf:type rdf:resource="http://semanticbible.org/ns/2006/NTNames#ResidenceGroup"/>
        <rdfs:label xml:lang="en">Gadarenes</rdfs:label>
    </owl:NamedIndividual>
    


    <!-- http://semanticbible.org/ns/2006/NTNames#GaiusOfCorinth -->

    <owl:NamedIndividual rdf:about="http://semanticbible.org/ns/2006/NTNames#GaiusOfCorinth">
        <rdf:type rdf:resource="http://semanticbible.org/ns/2006/NTNames#Man"/>
        <collaboratesWith rdf:resource="http://semanticbible.org/ns/2006/NTNames#Paul"/>
        <religiousBelief rdf:resource="http://semanticbible.org/ns/2006/NTNames#Christianity"/>
        <residentPlace rdf:resource="http://semanticbible.org/ns/2006/NTNames#Corinth"/>
        <description rdf:datatype="http://www.w3.org/2001/XMLSchema#string">one whom Paul baptized in Corinth</description>
        <hasOnlyGenealogyMention rdf:datatype="http://www.w3.org/2001/XMLSchema#boolean">false</hasOnlyGenealogyMention>
        <rdfs:comment xml:lang="en">Since Paul&apos;s Epistle to the Romans was written from Corinth, this is assumed to be the one Paul describes as &quot;host to me and the whole church&quot;</rdfs:comment>
        <rdfs:label xml:lang="en">Gaius</rdfs:label>
    </owl:NamedIndividual>
    


    <!-- http://semanticbible.org/ns/2006/NTNames#GaiusOfDerbe -->

    <owl:NamedIndividual rdf:about="http://semanticbible.org/ns/2006/NTNames#GaiusOfDerbe">
        <rdf:type rdf:resource="http://semanticbible.org/ns/2006/NTNames#Man"/>
        <collaboratesWith rdf:resource="http://semanticbible.org/ns/2006/NTNames#Aristarchus"/>
        <collaboratesWith rdf:resource="http://semanticbible.org/ns/2006/NTNames#Paul"/>
        <collaboratesWith rdf:resource="http://semanticbible.org/ns/2006/NTNames#Secundus"/>
        <collaboratesWith rdf:resource="http://semanticbible.org/ns/2006/NTNames#Sopater"/>
        <collaboratesWith rdf:resource="http://semanticbible.org/ns/2006/NTNames#Timothy"/>
        <collaboratesWith rdf:resource="http://semanticbible.org/ns/2006/NTNames#Trophimus"/>
        <collaboratesWith rdf:resource="http://semanticbible.org/ns/2006/NTNames#Tychicus"/>
        <nativePlace rdf:resource="http://semanticbible.org/ns/2006/NTNames#Derbe"/>
        <possiblySamePersonAs rdf:resource="http://semanticbible.org/ns/2006/NTNames#GaiusOfMacedonia"/>
        <religiousBelief rdf:resource="http://semanticbible.org/ns/2006/NTNames#Christianity"/>
        <visitedPlace rdf:resource="http://semanticbible.org/ns/2006/NTNames#Troas"/>
        <description rdf:datatype="http://www.w3.org/2001/XMLSchema#string">a travelling companion of Paul&apos;s</description>
        <hasOnlyGenealogyMention rdf:datatype="http://www.w3.org/2001/XMLSchema#boolean">false</hasOnlyGenealogyMention>
        <rdfs:comment rdf:datatype="http://www.w3.org/2001/XMLSchema#string">Luke describes him as &quot;Gaius of Derbe&quot;: that could be either his place of birth, or place of residence. It&apos;s not clear whether he (and his other companions) accompanied Paul all the way to Jerusalem. Gaius being a common name, it seems plausible that the others of the same name are distinct individuals, though the closest possible identification is with GaiusOfMacedonia (see New Bible Dictionary for discussion).</rdfs:comment>
        <rdfs:label xml:lang="en">Gaius</rdfs:label>
    </owl:NamedIndividual>
    


    <!-- http://semanticbible.org/ns/2006/NTNames#GaiusOfMacedonia -->

    <owl:NamedIndividual rdf:about="http://semanticbible.org/ns/2006/NTNames#GaiusOfMacedonia">
        <rdf:type rdf:resource="http://semanticbible.org/ns/2006/NTNames#Man"/>
        <collaboratesWith rdf:resource="http://semanticbible.org/ns/2006/NTNames#Aristarchus"/>
        <collaboratesWith rdf:resource="http://semanticbible.org/ns/2006/NTNames#Paul"/>
        <ethnicity rdf:resource="http://semanticbible.org/ns/2006/NTNames#Macedonian"/>
        <possiblySamePersonAs rdf:resource="http://semanticbible.org/ns/2006/NTNames#GaiusOfDerbe"/>
        <religiousBelief rdf:resource="http://semanticbible.org/ns/2006/NTNames#Christianity"/>
        <visitedPlace rdf:resource="http://semanticbible.org/ns/2006/NTNames#Ephesus"/>
        <description rdf:datatype="http://www.w3.org/2001/XMLSchema#string">a traveling companion of Paul&apos;s</description>
        <hasOnlyGenealogyMention rdf:datatype="http://www.w3.org/2001/XMLSchema#boolean">false</hasOnlyGenealogyMention>
        <rdfs:comment xml:lang="en">It seems likely this Gaius was a Christian since he was Paul&apos;s &quot;companion in travel&quot;, though this is not explicitly stated. </rdfs:comment>
        <rdfs:label xml:lang="en">Gaius</rdfs:label>
    </owl:NamedIndividual>
    


    <!-- http://semanticbible.org/ns/2006/NTNames#GaiusTheBeloved -->

    <owl:NamedIndividual rdf:about="http://semanticbible.org/ns/2006/NTNames#GaiusTheBeloved">
        <rdf:type rdf:resource="http://semanticbible.org/ns/2006/NTNames#Man"/>
        <collaboratesWith rdf:resource="http://semanticbible.org/ns/2006/NTNames#JohnSonOfZebedee"/>
        <knows rdf:resource="http://semanticbible.org/ns/2006/NTNames#Demetrius"/>
        <knows rdf:resource="http://semanticbible.org/ns/2006/NTNames#Diotrephes"/>
        <religiousBelief rdf:resource="http://semanticbible.org/ns/2006/NTNames#Christianity"/>
        <description rdf:datatype="http://www.w3.org/2001/XMLSchema#string">&quot;the beloved&quot; to whom John addresses his third epistle</description>
        <hasOnlyGenealogyMention rdf:datatype="http://www.w3.org/2001/XMLSchema#boolean">false</hasOnlyGenealogyMention>
        <rdfs:label xml:lang="en">Gaius</rdfs:label>
    </owl:NamedIndividual>
    


    <!-- http://semanticbible.org/ns/2006/NTNames#Galatia -->

    <owl:NamedIndividual rdf:about="http://semanticbible.org/ns/2006/NTNames#Galatia">
        <rdf:type rdf:resource="http://semanticbible.org/ns/2006/NTNames#StateOrProvince"/>
        <rdfs:label xml:lang="en">Galatia</rdfs:label>
    </owl:NamedIndividual>
    


    <!-- http://semanticbible.org/ns/2006/NTNames#Galatians -->

    <owl:NamedIndividual rdf:about="http://semanticbible.org/ns/2006/NTNames#Galatians">
        <rdf:type rdf:resource="http://semanticbible.org/ns/2006/NTNames#ResidenceGroup"/>
        <rdfs:label xml:lang="en">Galatians</rdfs:label>
    </owl:NamedIndividual>
    


    <!-- http://semanticbible.org/ns/2006/NTNames#Galilean -->

    <owl:NamedIndividual rdf:about="http://semanticbible.org/ns/2006/NTNames#Galilean">
        <rdf:type rdf:resource="http://semanticbible.org/ns/2006/NTNames#EthnicityAttribute"/>
        <ethnicityOf rdf:resource="http://semanticbible.org/ns/2006/NTNames#Alphaeus"/>
        <ethnicityOf rdf:resource="http://semanticbible.org/ns/2006/NTNames#AlphaeusFatherOfLevi"/>
        <ethnicityOf rdf:resource="http://semanticbible.org/ns/2006/NTNames#Andrew"/>
        <ethnicityOf rdf:resource="http://semanticbible.org/ns/2006/NTNames#Bartholomew"/>
        <ethnicityOf rdf:resource="http://semanticbible.org/ns/2006/NTNames#JamesSonOfAlphaeus"/>
        <ethnicityOf rdf:resource="http://semanticbible.org/ns/2006/NTNames#Levi"/>
        <ethnicityOf rdf:resource="http://semanticbible.org/ns/2006/NTNames#Philip"/>
        <ethnicityOf rdf:resource="http://semanticbible.org/ns/2006/NTNames#SimonPeter"/>
        <ethnicityOf rdf:resource="http://semanticbible.org/ns/2006/NTNames#SimonTheZealot"/>
        <ethnicityOf rdf:resource="http://semanticbible.org/ns/2006/NTNames#Thomas"/>
        <rdfs:comment xml:lang="en">In the time of Christ, Galilee was home to those of Jewish descent as well non-Jews. As used in the New Testament, the term is used primarily of Jews in distinction to Judean and Samaritan, the other major divisions of Jewish Palestine. It is therefore (in practice) a sub-ethnicity of Jewish.</rdfs:comment>
        <rdfs:label xml:lang="en">Galilean</rdfs:label>
    </owl:NamedIndividual>
    


    <!-- http://semanticbible.org/ns/2006/NTNames#Galileans -->

    <owl:NamedIndividual rdf:about="http://semanticbible.org/ns/2006/NTNames#Galileans">
        <rdf:type rdf:resource="http://semanticbible.org/ns/2006/NTNames#ResidenceGroup"/>
        <rdfs:label xml:lang="en">Galileans</rdfs:label>
    </owl:NamedIndividual>
    


    <!-- http://semanticbible.org/ns/2006/NTNames#Galilee -->

    <owl:NamedIndividual rdf:about="http://semanticbible.org/ns/2006/NTNames#Galilee">
        <rdf:type rdf:resource="http://semanticbible.org/ns/2006/NTNames#StateOrProvince"/>
        <residentPlaceOf rdf:resource="http://semanticbible.org/ns/2006/NTNames#MaryMagdalene"/>
        <subregion rdf:resource="http://semanticbible.org/ns/2006/NTNames#Bethsaida"/>
        <subregion rdf:resource="http://semanticbible.org/ns/2006/NTNames#Cana"/>
        <subregion rdf:resource="http://semanticbible.org/ns/2006/NTNames#Capernaum"/>
        <subregion rdf:resource="http://semanticbible.org/ns/2006/NTNames#Chorazin"/>
        <subregion rdf:resource="http://semanticbible.org/ns/2006/NTNames#Gennesaret"/>
        <subregion rdf:resource="http://semanticbible.org/ns/2006/NTNames#Nain"/>
        <subregion rdf:resource="http://semanticbible.org/ns/2006/NTNames#Nazareth"/>
        <subregion rdf:resource="http://semanticbible.org/ns/2006/NTNames#SeaOfGalilee"/>
        <subregion rdf:resource="http://semanticbible.org/ns/2006/NTNames#Tiberias"/>
        <subregionOf rdf:resource="http://semanticbible.org/ns/2006/NTNames#Israel"/>
        <rdfs:label xml:lang="en">Galilee</rdfs:label>
    </owl:NamedIndividual>
    


    <!-- http://semanticbible.org/ns/2006/NTNames#Gallio -->

    <owl:NamedIndividual rdf:about="http://semanticbible.org/ns/2006/NTNames#Gallio">
        <rdf:type rdf:resource="http://semanticbible.org/ns/2006/NTNames#Man"/>
        <ethnicity rdf:resource="http://semanticbible.org/ns/2006/NTNames#Roman"/>
        <residentPlace rdf:resource="http://semanticbible.org/ns/2006/NTNames#Achaia"/>
        <hasOnlyGenealogyMention rdf:datatype="http://www.w3.org/2001/XMLSchema#boolean">false</hasOnlyGenealogyMention>
        <occupation rdf:datatype="http://www.w3.org/2001/XMLSchema#string">proconsul of Achaia</occupation>
        <rdfs:comment rdf:datatype="http://www.w3.org/2001/XMLSchema#string">He is not considered an antagonist of Paul because his only involvement was indifference. </rdfs:comment>
        <rdfs:label xml:lang="en">Gallio</rdfs:label>
    </owl:NamedIndividual>
    


    <!-- http://semanticbible.org/ns/2006/NTNames#Gamaliel -->

    <owl:NamedIndividual rdf:about="http://semanticbible.org/ns/2006/NTNames#Gamaliel">
        <rdf:type rdf:resource="http://semanticbible.org/ns/2006/NTNames#Man"/>
        <ethnicity rdf:resource="http://semanticbible.org/ns/2006/NTNames#Jewish"/>
        <knows rdf:resource="http://semanticbible.org/ns/2006/NTNames#Paul"/>
        <memberOf rdf:resource="http://semanticbible.org/ns/2006/NTNames#Pharisees"/>
        <memberOf rdf:resource="http://semanticbible.org/ns/2006/NTNames#Sanhedrin"/>
        <nativePlace rdf:resource="http://semanticbible.org/ns/2006/NTNames#Israel"/>
        <religiousBelief rdf:resource="http://semanticbible.org/ns/2006/NTNames#Judaism"/>
        <religiousBelief rdf:resource="http://semanticbible.org/ns/2006/NTNames#Phariseeism"/>
        <residentPlace rdf:resource="http://semanticbible.org/ns/2006/NTNames#Jerusalem"/>
        <description rdf:datatype="http://www.w3.org/2001/XMLSchema#string">a respected Jewish teacher whom Paul studied under</description>
        <hasOnlyGenealogyMention rdf:datatype="http://www.w3.org/2001/XMLSchema#boolean">false</hasOnlyGenealogyMention>
        <occupation rdf:datatype="http://www.w3.org/2001/XMLSchema#string">teacher of the Jewish Law</occupation>
        <rdfs:label xml:lang="en">Gamaliel</rdfs:label>
    </owl:NamedIndividual>
    


    <!-- http://semanticbible.org/ns/2006/NTNames#Gaza -->

    <owl:NamedIndividual rdf:about="http://semanticbible.org/ns/2006/NTNames#Gaza">
        <rdf:type rdf:resource="http://semanticbible.org/ns/2006/NTNames#City"/>
        <location rdf:resource="http://semanticbible.org/ns/2006/NTNames#GazaGeodata"/>
        <subregionOf rdf:resource="http://semanticbible.org/ns/2006/NTNames#Judea"/>
        <rdfs:label xml:lang="en">Gaza</rdfs:label>
    </owl:NamedIndividual>
    


    <!-- http://semanticbible.org/ns/2006/NTNames#GazaGeodata -->

    <owl:NamedIndividual rdf:about="http://semanticbible.org/ns/2006/NTNames#GazaGeodata">
        <rdf:type rdf:resource="http://semanticbible.org/ns/2006/NTNames#GeographicLocation"/>
        <altitude rdf:datatype="http://www.w3.org/2001/XMLSchema#int">0</altitude>
        <latitude rdf:datatype="http://www.w3.org/2001/XMLSchema#double">31.52900696298234</latitude>
        <longitude rdf:datatype="http://www.w3.org/2001/XMLSchema#double">34.43673180421263</longitude>
        <rdfs:label xml:lang="en">geodata for Gaza</rdfs:label>
    </owl:NamedIndividual>
    


    <!-- http://semanticbible.org/ns/2006/NTNames#Gennesaret -->

    <owl:NamedIndividual rdf:about="http://semanticbible.org/ns/2006/NTNames#Gennesaret">
        <rdf:type rdf:resource="http://semanticbible.org/ns/2006/NTNames#LandArea"/>
        <subregionOf rdf:resource="http://semanticbible.org/ns/2006/NTNames#Galilee"/>
        <rdfs:comment xml:lang="en">An area on the west side of the Sea of Galilee, where Jesus healed the sick</rdfs:comment>
        <rdfs:label xml:lang="en">Gennesaret</rdfs:label>
    </owl:NamedIndividual>
    


    <!-- http://semanticbible.org/ns/2006/NTNames#Gentile -->

    <owl:NamedIndividual rdf:about="http://semanticbible.org/ns/2006/NTNames#Gentile">
        <rdf:type rdf:resource="http://semanticbible.org/ns/2006/NTNames#EthnicityAttribute"/>
        <rdfs:comment xml:lang="en">Essentially a &quot;non-ethnicity&quot; meaning not Jewish.</rdfs:comment>
        <rdfs:label xml:lang="en">Gentile</rdfs:label>
    </owl:NamedIndividual>
    


    <!-- http://semanticbible.org/ns/2006/NTNames#Gentiles -->

    <owl:NamedIndividual rdf:about="http://semanticbible.org/ns/2006/NTNames#Gentiles">
        <rdf:type rdf:resource="http://semanticbible.org/ns/2006/NTNames#GroupOfPeople"/>
        <rdfs:label xml:lang="en">Gentiles</rdfs:label>
    </owl:NamedIndividual>
    


    <!-- http://semanticbible.org/ns/2006/NTNames#Gethsemane -->

    <owl:NamedIndividual rdf:about="http://semanticbible.org/ns/2006/NTNames#Gethsemane">
        <rdf:type rdf:resource="http://semanticbible.org/ns/2006/NTNames#LandArea"/>
        <rdfs:label xml:lang="en">Gethsemane</rdfs:label>
    </owl:NamedIndividual>
    


    <!-- http://semanticbible.org/ns/2006/NTNames#Gideon -->

    <owl:NamedIndividual rdf:about="http://semanticbible.org/ns/2006/NTNames#Gideon">
        <rdf:type rdf:resource="http://semanticbible.org/ns/2006/NTNames#Man"/>
        <ethnicity rdf:resource="http://semanticbible.org/ns/2006/NTNames#Jewish"/>
        <religiousBelief rdf:resource="http://semanticbible.org/ns/2006/NTNames#Judaism"/>
        <description rdf:datatype="http://www.w3.org/2001/XMLSchema#string">a  judge of Israel prior to the monarchy</description>
        <hasOnlyGenealogyMention rdf:datatype="http://www.w3.org/2001/XMLSchema#boolean">false</hasOnlyGenealogyMention>
        <rdfs:label xml:lang="en">Gideon</rdfs:label>
    </owl:NamedIndividual>
    


    <!-- http://semanticbible.org/ns/2006/NTNames#Gog -->

    <owl:NamedIndividual rdf:about="http://semanticbible.org/ns/2006/NTNames#Gog">
        <rdf:type rdf:resource="http://semanticbible.org/ns/2006/NTNames#GroupOfPeople"/>
        <description rdf:datatype="http://www.w3.org/2001/XMLSchema#string">an apocalyptic opponent of God&apos;s people</description>
        <hasOnlyGenealogyMention rdf:datatype="http://www.w3.org/2001/XMLSchema#boolean">false</hasOnlyGenealogyMention>
        <rdfs:comment xml:lang="en">The historic background of the reference to Gog is most likely the Lydian king in the 7th Century BC. Its usage in Revelation seems to describe a group of people,  but it is hard to be certain what is intended in this apocalyptic context.</rdfs:comment>
        <rdfs:label xml:lang="en">Gog</rdfs:label>
    </owl:NamedIndividual>
    


    <!-- http://semanticbible.org/ns/2006/NTNames#Golgotha -->

    <owl:NamedIndividual rdf:about="http://semanticbible.org/ns/2006/NTNames#Golgotha">
        <rdf:type rdf:resource="http://semanticbible.org/ns/2006/NTNames#LandArea"/>
        <rdfs:label xml:lang="en">Golgotha</rdfs:label>
    </owl:NamedIndividual>
    


    <!-- http://semanticbible.org/ns/2006/NTNames#Gomorrah -->

    <owl:NamedIndividual rdf:about="http://semanticbible.org/ns/2006/NTNames#Gomorrah">
        <rdf:type rdf:resource="http://semanticbible.org/ns/2006/NTNames#City"/>
        <location rdf:resource="http://semanticbible.org/ns/2006/NTNames#GomorrahGeodata"/>
        <rdfs:label xml:lang="en">Gomorrah</rdfs:label>
    </owl:NamedIndividual>
    


    <!-- http://semanticbible.org/ns/2006/NTNames#GomorrahGeodata -->

    <owl:NamedIndividual rdf:about="http://semanticbible.org/ns/2006/NTNames#GomorrahGeodata">
        <rdf:type rdf:resource="http://semanticbible.org/ns/2006/NTNames#GeographicLocation"/>
        <altitude rdf:datatype="http://www.w3.org/2001/XMLSchema#int">0</altitude>
        <latitude rdf:datatype="http://www.w3.org/2001/XMLSchema#double">31.22573706270546</latitude>
        <longitude rdf:datatype="http://www.w3.org/2001/XMLSchema#double">35.46678974205374</longitude>
        <rdfs:label xml:lang="en">geodata for Gomorrah</rdfs:label>
    </owl:NamedIndividual>
    


    <!-- http://semanticbible.org/ns/2006/NTNames#Greece -->

    <owl:NamedIndividual rdf:about="http://semanticbible.org/ns/2006/NTNames#Greece">
        <rdf:type rdf:resource="http://semanticbible.org/ns/2006/NTNames#StateOrProvince"/>
        <rdfs:label xml:lang="en">Greece</rdfs:label>
    </owl:NamedIndividual>
    


    <!-- http://semanticbible.org/ns/2006/NTNames#Greek -->

    <owl:NamedIndividual rdf:about="http://semanticbible.org/ns/2006/NTNames#Greek">
        <rdf:type rdf:resource="http://semanticbible.org/ns/2006/NTNames#EthnicityAttribute"/>
        <ethnicityOf rdf:resource="http://semanticbible.org/ns/2006/NTNames#Timothy"/>
        <ethnicityOf rdf:resource="http://semanticbible.org/ns/2006/NTNames#Titius"/>
        <rdfs:comment xml:lang="en">Sometimes used synomymously with Gentile, but certainly means non-Jewish in ethnicity.</rdfs:comment>
        <rdfs:label xml:lang="en">Greek</rdfs:label>
    </owl:NamedIndividual>
    


    <!-- http://semanticbible.org/ns/2006/NTNames#GreekLanguage -->

    <owl:NamedIndividual rdf:about="http://semanticbible.org/ns/2006/NTNames#GreekLanguage">
        <rdf:type rdf:resource="http://semanticbible.org/ns/2006/NTNames#NaturalLanguage"/>
        <rdfs:label xml:lang="en">Greek</rdfs:label>
    </owl:NamedIndividual>
    


    <!-- http://semanticbible.org/ns/2006/NTNames#Greeks -->

    <owl:NamedIndividual rdf:about="http://semanticbible.org/ns/2006/NTNames#Greeks">
        <rdf:type rdf:resource="http://semanticbible.org/ns/2006/NTNames#EthnicGroup"/>
        <rdfs:label xml:lang="en">Greeks</rdfs:label>
    </owl:NamedIndividual>
    


    <!-- http://semanticbible.org/ns/2006/NTNames#Hades -->

    <owl:NamedIndividual rdf:about="http://semanticbible.org/ns/2006/NTNames#Hades">
        <rdf:type rdf:resource="http://semanticbible.org/ns/2006/NTNames#SupernaturalRegion"/>
        <rdfs:comment xml:lang="en">The state or place of the dead. SUO restricts use of GeographicArea to places on the earth.</rdfs:comment>
        <rdfs:label xml:lang="en">Hades</rdfs:label>
    </owl:NamedIndividual>
    


    <!-- http://semanticbible.org/ns/2006/NTNames#Hagar -->

    <owl:NamedIndividual rdf:about="http://semanticbible.org/ns/2006/NTNames#Hagar">
        <rdf:type rdf:resource="http://semanticbible.org/ns/2006/NTNames#Woman"/>
        <antagonistOf rdf:resource="http://semanticbible.org/ns/2006/NTNames#Sarah"/>
        <ethnicity rdf:resource="http://semanticbible.org/ns/2006/NTNames#Egyptian"/>
        <hasAntagonist rdf:resource="http://semanticbible.org/ns/2006/NTNames#Sarah"/>
        <knows rdf:resource="http://semanticbible.org/ns/2006/NTNames#Abraham"/>
        <residentPlace rdf:resource="http://semanticbible.org/ns/2006/NTNames#Canaan"/>
        <description rdf:datatype="http://www.w3.org/2001/XMLSchema#string">mother of Ishmael; servant to Abraham&apos;s wife Sarah </description>
        <hasOnlyGenealogyMention rdf:datatype="http://www.w3.org/2001/XMLSchema#boolean">false</hasOnlyGenealogyMention>
        <occupation rdf:datatype="http://www.w3.org/2001/XMLSchema#string">servant</occupation>
        <rdfs:comment rdf:datatype="http://www.w3.org/2001/XMLSchema#string">her son Ishmael is not named in the New Testament</rdfs:comment>
        <rdfs:label xml:lang="en">Hagar</rdfs:label>
    </owl:NamedIndividual>
    


    <!-- http://semanticbible.org/ns/2006/NTNames#Hamor -->

    <owl:NamedIndividual rdf:about="http://semanticbible.org/ns/2006/NTNames#Hamor">
        <rdf:type rdf:resource="http://semanticbible.org/ns/2006/NTNames#Man"/>
        <ethnicity rdf:resource="http://semanticbible.org/ns/2006/NTNames#Canaanite"/>
        <nativePlace rdf:resource="http://semanticbible.org/ns/2006/NTNames#Shechem"/>
        <description rdf:datatype="http://www.w3.org/2001/XMLSchema#string"></description>
        <hasOnlyGenealogyMention rdf:datatype="http://www.w3.org/2001/XMLSchema#boolean">false</hasOnlyGenealogyMention>
        <occupation rdf:datatype="http://www.w3.org/2001/XMLSchema#string">ruler</occupation>
        <rdfs:label xml:lang="en">Hamor</rdfs:label>
    </owl:NamedIndividual>
    


    <!-- http://semanticbible.org/ns/2006/NTNames#Haran -->

    <owl:NamedIndividual rdf:about="http://semanticbible.org/ns/2006/NTNames#Haran">
        <rdf:type rdf:resource="http://semanticbible.org/ns/2006/NTNames#City"/>
        <location rdf:resource="http://semanticbible.org/ns/2006/NTNames#HaranGeodata"/>
        <subregionOf rdf:resource="http://semanticbible.org/ns/2006/NTNames#Mesopotamia"/>
        <rdfs:comment xml:lang="en">In his speech before the Council, Stephen refers to Haran as a place where Abraham lived. </rdfs:comment>
        <rdfs:label xml:lang="en">Haran</rdfs:label>
    </owl:NamedIndividual>
    


    <!-- http://semanticbible.org/ns/2006/NTNames#HaranGeodata -->

    <owl:NamedIndividual rdf:about="http://semanticbible.org/ns/2006/NTNames#HaranGeodata">
        <rdf:type rdf:resource="http://semanticbible.org/ns/2006/NTNames#GeographicLocation"/>
        <altitude rdf:datatype="http://www.w3.org/2001/XMLSchema#int">0</altitude>
        <latitude rdf:datatype="http://www.w3.org/2001/XMLSchema#double">36.92937229726265</latitude>
        <longitude rdf:datatype="http://www.w3.org/2001/XMLSchema#double">39.04728757340273</longitude>
        <rdfs:label xml:lang="en">geodata for Haran</rdfs:label>
    </owl:NamedIndividual>
    


    <!-- http://semanticbible.org/ns/2006/NTNames#Hebrew -->

    <owl:NamedIndividual rdf:about="http://semanticbible.org/ns/2006/NTNames#Hebrew">
        <rdf:type rdf:resource="http://semanticbible.org/ns/2006/NTNames#NaturalLanguage"/>
        <rdfs:label xml:lang="en">Hebrew</rdfs:label>
    </owl:NamedIndividual>
    


    <!-- http://semanticbible.org/ns/2006/NTNames#Hebrews -->

    <owl:NamedIndividual rdf:about="http://semanticbible.org/ns/2006/NTNames#Hebrews">
        <rdf:type rdf:resource="http://semanticbible.org/ns/2006/NTNames#EthnicGroup"/>
        <rdfs:label xml:lang="en">Hebrews</rdfs:label>
    </owl:NamedIndividual>
    


    <!-- http://semanticbible.org/ns/2006/NTNames#Heli -->

    <owl:NamedIndividual rdf:about="http://semanticbible.org/ns/2006/NTNames#Heli">
        <rdf:type rdf:resource="http://semanticbible.org/ns/2006/NTNames#Man"/>
        <childOf rdf:resource="http://semanticbible.org/ns/2006/NTNames#MatthatSonOfLeviSonOfMelki"/>
        <ethnicity rdf:resource="http://semanticbible.org/ns/2006/NTNames#Jewish"/>
        <parentOf rdf:resource="http://semanticbible.org/ns/2006/NTNames#Joseph"/>
        <hasOnlyGenealogyMention rdf:datatype="http://www.w3.org/2001/XMLSchema#boolean">true</hasOnlyGenealogyMention>
        <rdfs:comment xml:lang="en">See the comment on Joseph for why Heli is listed as parentOf Mary, not Joseph, despite Luke 3:23.</rdfs:comment>
        <rdfs:label xml:lang="en">Heli</rdfs:label>
    </owl:NamedIndividual>
    


    <!-- http://semanticbible.org/ns/2006/NTNames#Hellenists -->

    <owl:NamedIndividual rdf:about="http://semanticbible.org/ns/2006/NTNames#Hellenists">
        <rdf:type rdf:resource="http://semanticbible.org/ns/2006/NTNames#EthnicGroup"/>
        <rdfs:label xml:lang="en">Hellenists</rdfs:label>
    </owl:NamedIndividual>
    


    <!-- http://semanticbible.org/ns/2006/NTNames#Hermas -->

    <owl:NamedIndividual rdf:about="http://semanticbible.org/ns/2006/NTNames#Hermas">
        <rdf:type rdf:resource="http://semanticbible.org/ns/2006/NTNames#Man"/>
        <knows rdf:resource="http://semanticbible.org/ns/2006/NTNames#Paul"/>
        <knows rdf:resource="http://semanticbible.org/ns/2006/NTNames#Priscilla"/>
        <religiousBelief rdf:resource="http://semanticbible.org/ns/2006/NTNames#Christianity"/>
        <residentPlace rdf:resource="http://semanticbible.org/ns/2006/NTNames#Rome"/>
        <description rdf:datatype="http://www.w3.org/2001/XMLSchema#string">a Roman to whom Paul sent greetings</description>
        <hasOnlyGenealogyMention rdf:datatype="http://www.w3.org/2001/XMLSchema#boolean">false</hasOnlyGenealogyMention>
        <rdfs:label xml:lang="en">Hermas</rdfs:label>
    </owl:NamedIndividual>
    


    <!-- http://semanticbible.org/ns/2006/NTNames#Hermes -->

    <owl:NamedIndividual rdf:about="http://semanticbible.org/ns/2006/NTNames#Hermes">
        <rdf:type rdf:resource="http://semanticbible.org/ns/2006/NTNames#Man"/>
        <knows rdf:resource="http://semanticbible.org/ns/2006/NTNames#Paul"/>
        <knows rdf:resource="http://semanticbible.org/ns/2006/NTNames#Priscilla"/>
        <religiousBelief rdf:resource="http://semanticbible.org/ns/2006/NTNames#Christianity"/>
        <residentPlace rdf:resource="http://semanticbible.org/ns/2006/NTNames#Rome"/>
        <description rdf:datatype="http://www.w3.org/2001/XMLSchema#string">a Roman to whom Paul sent greetings</description>
        <hasOnlyGenealogyMention rdf:datatype="http://www.w3.org/2001/XMLSchema#boolean">false</hasOnlyGenealogyMention>
        <rdfs:label xml:lang="en">Hermes</rdfs:label>
    </owl:NamedIndividual>
    


    <!-- http://semanticbible.org/ns/2006/NTNames#Hermogenes -->

    <owl:NamedIndividual rdf:about="http://semanticbible.org/ns/2006/NTNames#Hermogenes">
        <rdf:type rdf:resource="http://semanticbible.org/ns/2006/NTNames#Man"/>
        <knows rdf:resource="http://semanticbible.org/ns/2006/NTNames#Paul"/>
        <knows rdf:resource="http://semanticbible.org/ns/2006/NTNames#Phygelus"/>
        <religiousBelief rdf:resource="http://semanticbible.org/ns/2006/NTNames#Christianity"/>
        <description rdf:datatype="http://www.w3.org/2001/XMLSchema#string">a Christian who refused to help Paul during his Roman imprisonment</description>
        <hasOnlyGenealogyMention rdf:datatype="http://www.w3.org/2001/XMLSchema#boolean">false</hasOnlyGenealogyMention>
        <rdfs:comment xml:lang="en">The circumstances behind his &quot;turning away&quot; from Paul are unknown. Likewise, Paul&apos;s description of him as being &quot;is Asia&quot; isn&apos;t specific enough to assign a place. </rdfs:comment>
        <rdfs:label xml:lang="en">Hermogenes</rdfs:label>
    </owl:NamedIndividual>
    


    <!-- http://semanticbible.org/ns/2006/NTNames#HerodAgrippaI -->

    <owl:NamedIndividual rdf:about="http://semanticbible.org/ns/2006/NTNames#HerodAgrippaI">
        <rdf:type rdf:resource="http://semanticbible.org/ns/2006/NTNames#Man"/>
        <parentOf rdf:resource="http://semanticbible.org/ns/2006/NTNames#Bernice"/>
        <parentOf rdf:resource="http://semanticbible.org/ns/2006/NTNames#Drusilla"/>
        <hasOnlyGenealogyMention rdf:datatype="http://www.w3.org/2001/XMLSchema#boolean">false</hasOnlyGenealogyMention>
        <occupation rdf:datatype="http://www.w3.org/2001/XMLSchema#string">king</occupation>
        <rdfs:label xml:lang="en">Herod Agrippa I</rdfs:label>
    </owl:NamedIndividual>
    


    <!-- http://semanticbible.org/ns/2006/NTNames#HerodAgrippaII -->

    <owl:NamedIndividual rdf:about="http://semanticbible.org/ns/2006/NTNames#HerodAgrippaII">
        <rdf:type rdf:resource="http://semanticbible.org/ns/2006/NTNames#Man"/>
        <siblingOf rdf:resource="http://semanticbible.org/ns/2006/NTNames#Bernice"/>
        <siblingOf rdf:resource="http://semanticbible.org/ns/2006/NTNames#Drusilla"/>
        <description rdf:datatype="http://www.w3.org/2001/XMLSchema#string">King of Chalcis from AD 50-92: the last member of the Herodian dynasty</description>
        <hasOnlyGenealogyMention rdf:datatype="http://www.w3.org/2001/XMLSchema#boolean">false</hasOnlyGenealogyMention>
        <occupation rdf:datatype="http://www.w3.org/2001/XMLSchema#string">king</occupation>
        <rdfs:label xml:lang="en">Herod Agrippa II</rdfs:label>
    </owl:NamedIndividual>
    


    <!-- http://semanticbible.org/ns/2006/NTNames#HerodAntipas -->

    <owl:NamedIndividual rdf:about="http://semanticbible.org/ns/2006/NTNames#HerodAntipas">
        <rdf:type rdf:resource="http://semanticbible.org/ns/2006/NTNames#Man"/>
        <childOf rdf:resource="http://semanticbible.org/ns/2006/NTNames#HerodTheGreat"/>
        <collaboratesWith rdf:resource="http://semanticbible.org/ns/2006/NTNames#PontiusPilate"/>
        <enemyOf rdf:resource="http://semanticbible.org/ns/2006/NTNames#Jesus"/>
        <ethnicity rdf:resource="http://semanticbible.org/ns/2006/NTNames#Samaritan"/>
        <relativeOf rdf:resource="http://semanticbible.org/ns/2006/NTNames#Aretas"/>
        <siblingOf rdf:resource="http://semanticbible.org/ns/2006/NTNames#Archelaus"/>
        <siblingOf rdf:resource="http://semanticbible.org/ns/2006/NTNames#PhilipSonOfHerod"/>
        <spouseOf rdf:resource="http://semanticbible.org/ns/2006/NTNames#Herodias"/>
        <visitedPlace rdf:resource="http://semanticbible.org/ns/2006/NTNames#Jerusalem"/>
        <description rdf:datatype="http://www.w3.org/2001/XMLSchema#string">ruler of Judea during Jesus&apos; adult life</description>
        <occupation rdf:datatype="http://www.w3.org/2001/XMLSchema#string">tetrarch</occupation>
        <rdfs:comment xml:lang="en">Herod the Great was Idumean, and Antipas&apos; mother was Samaritan. According to extra-biblical history, he was educated in Rome. </rdfs:comment>
        <rdfs:label xml:lang="en">Herod</rdfs:label>
        <rdfs:label xml:lang="en">Herod the tetrarch</rdfs:label>
    </owl:NamedIndividual>
    


    <!-- http://semanticbible.org/ns/2006/NTNames#HerodTheGreat -->

    <owl:NamedIndividual rdf:about="http://semanticbible.org/ns/2006/NTNames#HerodTheGreat">
        <rdf:type rdf:resource="http://semanticbible.org/ns/2006/NTNames#Man"/>
        <parentOf rdf:resource="http://semanticbible.org/ns/2006/NTNames#Archelaus"/>
        <parentOf rdf:resource="http://semanticbible.org/ns/2006/NTNames#HerodAntipas"/>
        <parentOf rdf:resource="http://semanticbible.org/ns/2006/NTNames#PhilipSonOfHerod"/>
        <description rdf:datatype="http://www.w3.org/2001/XMLSchema#string">King of Judea at the time of Jesus&apos; birth</description>
        <hasOnlyGenealogyMention rdf:datatype="http://www.w3.org/2001/XMLSchema#boolean">false</hasOnlyGenealogyMention>
        <occupation rdf:datatype="http://www.w3.org/2001/XMLSchema#string">king</occupation>
        <rdfs:label xml:lang="en">Herod</rdfs:label>
    </owl:NamedIndividual>
    


    <!-- http://semanticbible.org/ns/2006/NTNames#Herodians -->

    <owl:NamedIndividual rdf:about="http://semanticbible.org/ns/2006/NTNames#Herodians">
        <rdf:type rdf:resource="http://semanticbible.org/ns/2006/NTNames#PoliticalOrganization"/>
        <rdfs:label xml:lang="en">Herodians</rdfs:label>
    </owl:NamedIndividual>
    


    <!-- http://semanticbible.org/ns/2006/NTNames#Herodias -->

    <owl:NamedIndividual rdf:about="http://semanticbible.org/ns/2006/NTNames#Herodias">
        <rdf:type rdf:resource="http://semanticbible.org/ns/2006/NTNames#Woman"/>
        <spouseOf rdf:resource="http://semanticbible.org/ns/2006/NTNames#HerodAntipas"/>
        <spouseOf rdf:resource="http://semanticbible.org/ns/2006/NTNames#PhilipSonOfHerod"/>
        <description rdf:datatype="http://www.w3.org/2001/XMLSchema#string">wife of Herod Antipas who had John the Baptist put to death</description>
        <hasOnlyGenealogyMention rdf:datatype="http://www.w3.org/2001/XMLSchema#boolean">false</hasOnlyGenealogyMention>
        <rdfs:comment xml:lang="en">Herodias had John the Baptist put to death</rdfs:comment>
        <rdfs:label xml:lang="en">Herodias</rdfs:label>
    </owl:NamedIndividual>
    


    <!-- http://semanticbible.org/ns/2006/NTNames#Herodion -->

    <owl:NamedIndividual rdf:about="http://semanticbible.org/ns/2006/NTNames#Herodion">
        <rdf:type rdf:resource="http://semanticbible.org/ns/2006/NTNames#Man"/>
        <knows rdf:resource="http://semanticbible.org/ns/2006/NTNames#Paul"/>
        <knows rdf:resource="http://semanticbible.org/ns/2006/NTNames#Priscilla"/>
        <religiousBelief rdf:resource="http://semanticbible.org/ns/2006/NTNames#Christianity"/>
        <residentPlace rdf:resource="http://semanticbible.org/ns/2006/NTNames#Rome"/>
        <hasOnlyGenealogyMention rdf:datatype="http://www.w3.org/2001/XMLSchema#boolean">false</hasOnlyGenealogyMention>
        <rdfs:comment rdf:datatype="http://www.w3.org/2001/XMLSchema#string">Paul&apos;s description of Herodian as &quot;my kinsman&quot; is taken in the general snese (e.g. coming from the same region), rather than literally. </rdfs:comment>
        <rdfs:label xml:lang="en">Herodion</rdfs:label>
    </owl:NamedIndividual>
    


    <!-- http://semanticbible.org/ns/2006/NTNames#Hezekiah -->

    <owl:NamedIndividual rdf:about="http://semanticbible.org/ns/2006/NTNames#Hezekiah">
        <rdf:type rdf:resource="http://semanticbible.org/ns/2006/NTNames#Man"/>
        <childOf rdf:resource="http://semanticbible.org/ns/2006/NTNames#Ahaz"/>
        <ethnicity rdf:resource="http://semanticbible.org/ns/2006/NTNames#Jewish"/>
        <parentOf rdf:resource="http://semanticbible.org/ns/2006/NTNames#Manasseh"/>
        <rdfs:label xml:lang="en">Hezekiah</rdfs:label>
    </owl:NamedIndividual>
    


    <!-- http://semanticbible.org/ns/2006/NTNames#Hezron -->

    <owl:NamedIndividual rdf:about="http://semanticbible.org/ns/2006/NTNames#Hezron">
        <rdf:type rdf:resource="http://semanticbible.org/ns/2006/NTNames#Man"/>
        <childOf rdf:resource="http://semanticbible.org/ns/2006/NTNames#Perez"/>
        <ethnicity rdf:resource="http://semanticbible.org/ns/2006/NTNames#Jewish"/>
        <parentOf rdf:resource="http://semanticbible.org/ns/2006/NTNames#Arni"/>
        <parentOf rdf:resource="http://semanticbible.org/ns/2006/NTNames#Ram"/>
        <description rdf:datatype="http://www.w3.org/2001/XMLSchema#string">One of the ancestors of Jesus mentioned in Matthew&apos;s geneaology</description>
        <hasOnlyGenealogyMention rdf:datatype="http://www.w3.org/2001/XMLSchema#boolean">true</hasOnlyGenealogyMention>
        <rdfs:label xml:lang="en">Hezron</rdfs:label>
    </owl:NamedIndividual>
    


    <!-- http://semanticbible.org/ns/2006/NTNames#Hierapolis -->

    <owl:NamedIndividual rdf:about="http://semanticbible.org/ns/2006/NTNames#Hierapolis">
        <rdf:type rdf:resource="http://semanticbible.org/ns/2006/NTNames#City"/>
        <rdfs:label xml:lang="en">Hierapolis</rdfs:label>
    </owl:NamedIndividual>
    


    <!-- http://semanticbible.org/ns/2006/NTNames#Hosea -->

    <owl:NamedIndividual rdf:about="http://semanticbible.org/ns/2006/NTNames#Hosea">
        <rdf:type rdf:resource="http://semanticbible.org/ns/2006/NTNames#Man"/>
        <rdfs:label xml:lang="en">Hosea</rdfs:label>
    </owl:NamedIndividual>
    


    <!-- http://semanticbible.org/ns/2006/NTNames#Hymenaeus -->

    <owl:NamedIndividual rdf:about="http://semanticbible.org/ns/2006/NTNames#Hymenaeus">
        <rdf:type rdf:resource="http://semanticbible.org/ns/2006/NTNames#Man"/>
        <collaboratesWith rdf:resource="http://semanticbible.org/ns/2006/NTNames#AlexanderTheHeretic"/>
        <collaboratesWith rdf:resource="http://semanticbible.org/ns/2006/NTNames#Philetus"/>
        <rdfs:label xml:lang="en">Hymenaeus</rdfs:label>
    </owl:NamedIndividual>
    


    <!-- http://semanticbible.org/ns/2006/NTNames#Iconium -->

    <owl:NamedIndividual rdf:about="http://semanticbible.org/ns/2006/NTNames#Iconium">
        <rdf:type rdf:resource="http://semanticbible.org/ns/2006/NTNames#City"/>
        <location rdf:resource="http://semanticbible.org/ns/2006/NTNames#IconiumGeodata"/>
        <rdfs:label xml:lang="en">Iconium</rdfs:label>
    </owl:NamedIndividual>
    


    <!-- http://semanticbible.org/ns/2006/NTNames#IconiumGeodata -->

    <owl:NamedIndividual rdf:about="http://semanticbible.org/ns/2006/NTNames#IconiumGeodata">
        <rdf:type rdf:resource="http://semanticbible.org/ns/2006/NTNames#GeographicLocation"/>
        <altitude rdf:datatype="http://www.w3.org/2001/XMLSchema#int">0</altitude>
        <latitude rdf:datatype="http://www.w3.org/2001/XMLSchema#double">37.88182317434359</latitude>
        <longitude rdf:datatype="http://www.w3.org/2001/XMLSchema#double">32.48788166833032</longitude>
        <rdfs:label xml:lang="en">geodata for Iconium</rdfs:label>
    </owl:NamedIndividual>
    


    <!-- http://semanticbible.org/ns/2006/NTNames#Idumea -->

    <owl:NamedIndividual rdf:about="http://semanticbible.org/ns/2006/NTNames#Idumea">
        <rdf:type rdf:resource="http://semanticbible.org/ns/2006/NTNames#Region"/>
        <rdfs:label xml:lang="en">Idumea</rdfs:label>
    </owl:NamedIndividual>
    


    <!-- http://semanticbible.org/ns/2006/NTNames#Illyricum -->

    <owl:NamedIndividual rdf:about="http://semanticbible.org/ns/2006/NTNames#Illyricum">
        <rdf:type rdf:resource="http://semanticbible.org/ns/2006/NTNames#StateOrProvince"/>
        <rdfs:label xml:lang="en">Illyricum</rdfs:label>
    </owl:NamedIndividual>
    


    <!-- http://semanticbible.org/ns/2006/NTNames#Immanuel -->

    <owl:NamedIndividual rdf:about="http://semanticbible.org/ns/2006/NTNames#Immanuel">
        <rdf:type rdf:resource="http://semanticbible.org/ns/2006/NTNames#Man"/>
        <rdfs:label xml:lang="en">Immanuel</rdfs:label>
    </owl:NamedIndividual>
    


    <!-- http://semanticbible.org/ns/2006/NTNames#Isaac -->

    <owl:NamedIndividual rdf:about="http://semanticbible.org/ns/2006/NTNames#Isaac">
        <rdf:type rdf:resource="http://semanticbible.org/ns/2006/NTNames#Man"/>
        <childOf rdf:resource="http://semanticbible.org/ns/2006/NTNames#Abraham"/>
        <childOf rdf:resource="http://semanticbible.org/ns/2006/NTNames#Sarah"/>
        <ethnicity rdf:resource="http://semanticbible.org/ns/2006/NTNames#Jewish"/>
        <parentOf rdf:resource="http://semanticbible.org/ns/2006/NTNames#Esau"/>
        <parentOf rdf:resource="http://semanticbible.org/ns/2006/NTNames#Jacob"/>
        <spouseOf rdf:resource="http://semanticbible.org/ns/2006/NTNames#Rebecca"/>
        <hasOnlyGenealogyMention rdf:datatype="http://www.w3.org/2001/XMLSchema#boolean">false</hasOnlyGenealogyMention>
        <rdfs:label xml:lang="en">Isaac</rdfs:label>
    </owl:NamedIndividual>
    


    <!-- http://semanticbible.org/ns/2006/NTNames#Isaiah -->

    <owl:NamedIndividual rdf:about="http://semanticbible.org/ns/2006/NTNames#Isaiah">
        <rdf:type rdf:resource="http://semanticbible.org/ns/2006/NTNames#Man"/>
        <rdfs:label xml:lang="en">Isaiah</rdfs:label>
    </owl:NamedIndividual>
    


    <!-- http://semanticbible.org/ns/2006/NTNames#Iscariot -->

    <owl:NamedIndividual rdf:about="http://semanticbible.org/ns/2006/NTNames#Iscariot">
        <rdf:type rdf:resource="http://semanticbible.org/ns/2006/NTNames#Man"/>
        <rdfs:label xml:lang="en">Iscariot</rdfs:label>
    </owl:NamedIndividual>
    


    <!-- http://semanticbible.org/ns/2006/NTNames#Israel -->

    <owl:NamedIndividual rdf:about="http://semanticbible.org/ns/2006/NTNames#Israel">
        <rdf:type rdf:resource="http://semanticbible.org/ns/2006/NTNames#Nation"/>
        <nativePlaceOf rdf:resource="http://semanticbible.org/ns/2006/NTNames#Gamaliel"/>
        <subregion rdf:resource="http://semanticbible.org/ns/2006/NTNames#Galilee"/>
        <subregion rdf:resource="http://semanticbible.org/ns/2006/NTNames#Judea"/>
        <subregion rdf:resource="http://semanticbible.org/ns/2006/NTNames#Samaria"/>
        <rdfs:comment xml:lang="en">This name designates the nation inhabited by the descendants of Jacob&apos;s twelve sons. For Israel the patriarch, see Jacob. For the inhabitants of this nation, see Israelites. </rdfs:comment>
        <rdfs:label xml:lang="en">Israel</rdfs:label>
    </owl:NamedIndividual>
    


    <!-- http://semanticbible.org/ns/2006/NTNames#Israelites -->

    <owl:NamedIndividual rdf:about="http://semanticbible.org/ns/2006/NTNames#Israelites">
        <rdf:type rdf:resource="http://semanticbible.org/ns/2006/NTNames#EthnicGroup"/>
        <rdfs:label xml:lang="en">Israelites</rdfs:label>
    </owl:NamedIndividual>
    


    <!-- http://semanticbible.org/ns/2006/NTNames#Issachar -->

    <owl:NamedIndividual rdf:about="http://semanticbible.org/ns/2006/NTNames#Issachar">
        <rdf:type rdf:resource="http://semanticbible.org/ns/2006/NTNames#Man"/>
        <siblingOf rdf:resource="http://semanticbible.org/ns/2006/NTNames#Gad"/>
        <rdfs:label xml:lang="en">Issachar</rdfs:label>
    </owl:NamedIndividual>
    


    <!-- http://semanticbible.org/ns/2006/NTNames#ItalianCohort -->

    <owl:NamedIndividual rdf:about="http://semanticbible.org/ns/2006/NTNames#ItalianCohort">
        <rdf:type rdf:resource="http://semanticbible.org/ns/2006/NTNames#PoliticalOrganization"/>
        <rdfs:comment xml:lang="en">A Roman legion</rdfs:comment>
        <rdfs:label xml:lang="en">Italian Cohort</rdfs:label>
    </owl:NamedIndividual>
    


    <!-- http://semanticbible.org/ns/2006/NTNames#Italy -->

    <owl:NamedIndividual rdf:about="http://semanticbible.org/ns/2006/NTNames#Italy">
        <rdf:type rdf:resource="http://semanticbible.org/ns/2006/NTNames#GeopoliticalArea"/>
        <rdfs:label xml:lang="en">Italy</rdfs:label>
    </owl:NamedIndividual>
    


    <!-- http://semanticbible.org/ns/2006/NTNames#Ituraea -->

    <owl:NamedIndividual rdf:about="http://semanticbible.org/ns/2006/NTNames#Ituraea">
        <rdf:type rdf:resource="http://semanticbible.org/ns/2006/NTNames#StateOrProvince"/>
        <subregion rdf:resource="http://semanticbible.org/ns/2006/NTNames#CaesareaPhilippi"/>
        <rdfs:comment xml:lang="en">An area to the NW of the Sea of Galilee. It&apos;s unclear whether this refers to a definite region or an undefined general area occupied by the Ituraeans, a migratory tribe.</rdfs:comment>
        <rdfs:label xml:lang="en">Ituraea</rdfs:label>
    </owl:NamedIndividual>
    


    <!-- http://semanticbible.org/ns/2006/NTNames#Jacob -->

    <owl:NamedIndividual rdf:about="http://semanticbible.org/ns/2006/NTNames#Jacob">
        <rdf:type rdf:resource="http://semanticbible.org/ns/2006/NTNames#Man"/>
        <childOf rdf:resource="http://semanticbible.org/ns/2006/NTNames#Isaac"/>
        <childOf rdf:resource="http://semanticbible.org/ns/2006/NTNames#Rebecca"/>
        <ethnicity rdf:resource="http://semanticbible.org/ns/2006/NTNames#Jewish"/>
        <parentOf rdf:resource="http://semanticbible.org/ns/2006/NTNames#Asher"/>
        <parentOf rdf:resource="http://semanticbible.org/ns/2006/NTNames#Benjamin"/>
        <parentOf rdf:resource="http://semanticbible.org/ns/2006/NTNames#Gad"/>
        <parentOf rdf:resource="http://semanticbible.org/ns/2006/NTNames#JosephThePatriarch"/>
        <parentOf rdf:resource="http://semanticbible.org/ns/2006/NTNames#Judah"/>
        <parentOf rdf:resource="http://semanticbible.org/ns/2006/NTNames#ManassehThePatriarch"/>
        <parentOf rdf:resource="http://semanticbible.org/ns/2006/NTNames#SimeonThePatriarch"/>
        <siblingOf rdf:resource="http://semanticbible.org/ns/2006/NTNames#Esau"/>
        <spouseOf rdf:resource="http://semanticbible.org/ns/2006/NTNames#Rachel"/>
        <description rdf:datatype="http://www.w3.org/2001/XMLSchema#string">The patriarch of the nation of Israel, son of Isaac and Abraham</description>
        <hasOnlyGenealogyMention rdf:datatype="http://www.w3.org/2001/XMLSchema#boolean">false</hasOnlyGenealogyMention>
        <rdfs:comment rdf:datatype="http://www.w3.org/2001/XMLSchema#string">Israel becomes a metonym describing the nation of descendants from Jacob, so it is used both for a individual, a nation, and the members of that nation. </rdfs:comment>
        <rdfs:label xml:lang="en">Israel</rdfs:label>
        <rdfs:label xml:lang="en">Jacob</rdfs:label>
    </owl:NamedIndividual>
    


    <!-- http://semanticbible.org/ns/2006/NTNames#JacobSonOfMatthan -->

    <owl:NamedIndividual rdf:about="http://semanticbible.org/ns/2006/NTNames#JacobSonOfMatthan">
        <rdf:type rdf:resource="http://semanticbible.org/ns/2006/NTNames#Man"/>
        <childOf rdf:resource="http://semanticbible.org/ns/2006/NTNames#Matthan"/>
        <parentOf rdf:resource="http://semanticbible.org/ns/2006/NTNames#Joseph"/>
        <description rdf:datatype="http://www.w3.org/2001/XMLSchema#string">One of the ancestors of Jesus mentioned in Matthew&apos;s geneaology</description>
        <rdfs:comment xml:lang="en">Grandfather of Joseph, the husband of Mary, the mother of Jesus</rdfs:comment>
        <rdfs:label xml:lang="en">Jacob</rdfs:label>
    </owl:NamedIndividual>
    


    <!-- http://semanticbible.org/ns/2006/NTNames#Jairus -->

    <owl:NamedIndividual rdf:about="http://semanticbible.org/ns/2006/NTNames#Jairus">
        <rdf:type rdf:resource="http://semanticbible.org/ns/2006/NTNames#Man"/>
        <rdfs:label xml:lang="en">Jairus</rdfs:label>
    </owl:NamedIndividual>
    


    <!-- http://semanticbible.org/ns/2006/NTNames#Jambres -->

    <owl:NamedIndividual rdf:about="http://semanticbible.org/ns/2006/NTNames#Jambres">
        <rdf:type rdf:resource="http://semanticbible.org/ns/2006/NTNames#Man"/>
        <rdfs:label xml:lang="en">Jambres</rdfs:label>
    </owl:NamedIndividual>
    


    <!-- http://semanticbible.org/ns/2006/NTNames#James -->

    <owl:NamedIndividual rdf:about="http://semanticbible.org/ns/2006/NTNames#James">
        <rdf:type rdf:resource="http://semanticbible.org/ns/2006/NTNames#Man"/>
        <rdfs:label xml:lang="en">James</rdfs:label>
    </owl:NamedIndividual>
    


    <!-- http://semanticbible.org/ns/2006/NTNames#JamesSonOfAlphaeus -->

    <owl:NamedIndividual rdf:about="http://semanticbible.org/ns/2006/NTNames#JamesSonOfAlphaeus">
        <rdf:type rdf:resource="http://semanticbible.org/ns/2006/NTNames#Man"/>
        <childOf rdf:resource="http://semanticbible.org/ns/2006/NTNames#Alphaeus"/>
        <collaboratesWith rdf:resource="http://semanticbible.org/ns/2006/NTNames#Andrew"/>
        <ethnicity rdf:resource="http://semanticbible.org/ns/2006/NTNames#Galilean"/>
        <siblingOf rdf:resource="http://semanticbible.org/ns/2006/NTNames#Joses"/>
        <rdfs:label xml:lang="en">James</rdfs:label>
    </owl:NamedIndividual>
    


    <!-- http://semanticbible.org/ns/2006/NTNames#JamesSonOfZebedee -->

    <owl:NamedIndividual rdf:about="http://semanticbible.org/ns/2006/NTNames#JamesSonOfZebedee">
        <rdf:type rdf:resource="http://semanticbible.org/ns/2006/NTNames#Man"/>
        <childOf rdf:resource="http://semanticbible.org/ns/2006/NTNames#Salome"/>
        <childOf rdf:resource="http://semanticbible.org/ns/2006/NTNames#Zebedee"/>
        <collaboratesWith rdf:resource="http://semanticbible.org/ns/2006/NTNames#Andrew"/>
        <siblingOf rdf:resource="http://semanticbible.org/ns/2006/NTNames#JohnSonOfZebedee"/>
        <description rdf:datatype="http://www.w3.org/2001/XMLSchema#string">One of Jesus&apos; twelve apostles</description>
        <rdfs:label xml:lang="en">James</rdfs:label>
    </owl:NamedIndividual>
    


    <!-- http://semanticbible.org/ns/2006/NTNames#Jannai -->

    <owl:NamedIndividual rdf:about="http://semanticbible.org/ns/2006/NTNames#Jannai">
        <rdf:type rdf:resource="http://semanticbible.org/ns/2006/NTNames#Man"/>
        <childOf rdf:resource="http://semanticbible.org/ns/2006/NTNames#JosephSonOfMattathias"/>
        <ethnicity rdf:resource="http://semanticbible.org/ns/2006/NTNames#Jewish"/>
        <parentOf rdf:resource="http://semanticbible.org/ns/2006/NTNames#MelchiSonOfJannai"/>
        <description rdf:datatype="http://www.w3.org/2001/XMLSchema#string">One of the ancestors of Jesus mentioned in Luke&apos;s geneaology</description>
        <hasOnlyGenealogyMention rdf:datatype="http://www.w3.org/2001/XMLSchema#boolean">true</hasOnlyGenealogyMention>
        <rdfs:label xml:lang="en">Jannai</rdfs:label>
    </owl:NamedIndividual>
    


    <!-- http://semanticbible.org/ns/2006/NTNames#Jannes -->

    <owl:NamedIndividual rdf:about="http://semanticbible.org/ns/2006/NTNames#Jannes">
        <rdf:type rdf:resource="http://semanticbible.org/ns/2006/NTNames#Man"/>
        <rdfs:label xml:lang="en">Jannes</rdfs:label>
    </owl:NamedIndividual>
    


    <!-- http://semanticbible.org/ns/2006/NTNames#Jared -->

    <owl:NamedIndividual rdf:about="http://semanticbible.org/ns/2006/NTNames#Jared">
        <rdf:type rdf:resource="http://semanticbible.org/ns/2006/NTNames#Man"/>
        <childOf rdf:resource="http://semanticbible.org/ns/2006/NTNames#Mahalaleel"/>
        <parentOf rdf:resource="http://semanticbible.org/ns/2006/NTNames#Enoch"/>
        <hasOnlyGenealogyMention rdf:datatype="http://www.w3.org/2001/XMLSchema#boolean">true</hasOnlyGenealogyMention>
        <rdfs:label xml:lang="en">Jared</rdfs:label>
    </owl:NamedIndividual>
    


    <!-- http://semanticbible.org/ns/2006/NTNames#Jason -->

    <owl:NamedIndividual rdf:about="http://semanticbible.org/ns/2006/NTNames#Jason">
        <rdf:type rdf:resource="http://semanticbible.org/ns/2006/NTNames#Man"/>
        <knows rdf:resource="http://semanticbible.org/ns/2006/NTNames#Lucius"/>
        <knows rdf:resource="http://semanticbible.org/ns/2006/NTNames#Paul"/>
        <knows rdf:resource="http://semanticbible.org/ns/2006/NTNames#Sosipater"/>
        <knows rdf:resource="http://semanticbible.org/ns/2006/NTNames#Timothy"/>
        <religiousBelief rdf:resource="http://semanticbible.org/ns/2006/NTNames#Christianity"/>
        <residentPlace rdf:resource="http://semanticbible.org/ns/2006/NTNames#Corinth"/>
        <description rdf:datatype="http://www.w3.org/2001/XMLSchema#string"> a companion of Paul&apos;s who sent greetings to the Roman church</description>
        <hasOnlyGenealogyMention rdf:datatype="http://www.w3.org/2001/XMLSchema#boolean">false</hasOnlyGenealogyMention>
        <rdfs:comment rdf:datatype="http://www.w3.org/2001/XMLSchema#string">His residence in Corinth follows from the inference that Paul resided there when he wrote the letter to the Roman church.  &quot;kinsman&quot; here probably means that that he is a Jew, rather than an actual relative, given the number of people so designated in Romans 16. </rdfs:comment>
        <rdfs:label xml:lang="en">Jason</rdfs:label>
    </owl:NamedIndividual>
    


    <!-- http://semanticbible.org/ns/2006/NTNames#Jechoniah -->

    <owl:NamedIndividual rdf:about="http://semanticbible.org/ns/2006/NTNames#Jechoniah">
        <rdf:type rdf:resource="http://semanticbible.org/ns/2006/NTNames#Man"/>
        <childOf rdf:resource="http://semanticbible.org/ns/2006/NTNames#Josiah"/>
        <ethnicity rdf:resource="http://semanticbible.org/ns/2006/NTNames#Jewish"/>
        <parentOf rdf:resource="http://semanticbible.org/ns/2006/NTNames#Shealtiel"/>
        <rdfs:label xml:lang="en">Jechoniah</rdfs:label>
    </owl:NamedIndividual>
    


    <!-- http://semanticbible.org/ns/2006/NTNames#Jehoshaphat -->

    <owl:NamedIndividual rdf:about="http://semanticbible.org/ns/2006/NTNames#Jehoshaphat">
        <rdf:type rdf:resource="http://semanticbible.org/ns/2006/NTNames#Man"/>
        <childOf rdf:resource="http://semanticbible.org/ns/2006/NTNames#Asaph"/>
        <ethnicity rdf:resource="http://semanticbible.org/ns/2006/NTNames#Jewish"/>
        <parentOf rdf:resource="http://semanticbible.org/ns/2006/NTNames#Joram"/>
        <description rdf:datatype="http://www.w3.org/2001/XMLSchema#string">One of the ancestors of Jesus mentioned in Matthew&apos;s geneaology</description>
        <hasOnlyGenealogyMention rdf:datatype="http://www.w3.org/2001/XMLSchema#boolean">true</hasOnlyGenealogyMention>
        <occupation rdf:datatype="http://www.w3.org/2001/XMLSchema#string">king of Judah</occupation>
        <rdfs:label xml:lang="en">Jehoshaphat</rdfs:label>
    </owl:NamedIndividual>
    


    <!-- http://semanticbible.org/ns/2006/NTNames#Jephthah -->

    <owl:NamedIndividual rdf:about="http://semanticbible.org/ns/2006/NTNames#Jephthah">
        <rdf:type rdf:resource="http://semanticbible.org/ns/2006/NTNames#Man"/>
        <rdfs:label xml:lang="en">Jephthah</rdfs:label>
    </owl:NamedIndividual>
    


    <!-- http://semanticbible.org/ns/2006/NTNames#Jeremiah -->

    <owl:NamedIndividual rdf:about="http://semanticbible.org/ns/2006/NTNames#Jeremiah">
        <rdf:type rdf:resource="http://semanticbible.org/ns/2006/NTNames#Man"/>
        <rdfs:label xml:lang="en">Jeremiah</rdfs:label>
    </owl:NamedIndividual>
    


    <!-- http://semanticbible.org/ns/2006/NTNames#Jericho -->

    <owl:NamedIndividual rdf:about="http://semanticbible.org/ns/2006/NTNames#Jericho">
        <rdf:type rdf:resource="http://semanticbible.org/ns/2006/NTNames#City"/>
        <location rdf:resource="http://semanticbible.org/ns/2006/NTNames#JerichoGeodata"/>
        <subregionOf rdf:resource="http://semanticbible.org/ns/2006/NTNames#Judea"/>
        <rdfs:label xml:lang="en">Jericho</rdfs:label>
    </owl:NamedIndividual>
    


    <!-- http://semanticbible.org/ns/2006/NTNames#JerichoGeodata -->

    <owl:NamedIndividual rdf:about="http://semanticbible.org/ns/2006/NTNames#JerichoGeodata">
        <rdf:type rdf:resource="http://semanticbible.org/ns/2006/NTNames#GeographicLocation"/>
        <altitude rdf:datatype="http://www.w3.org/2001/XMLSchema#int">0</altitude>
        <latitude rdf:datatype="http://www.w3.org/2001/XMLSchema#double">31.87121832852874</latitude>
        <longitude rdf:datatype="http://www.w3.org/2001/XMLSchema#double">35.45194277611154</longitude>
        <rdfs:label xml:lang="en">geodata for Jericho</rdfs:label>
    </owl:NamedIndividual>
    


    <!-- http://semanticbible.org/ns/2006/NTNames#Jerusalem -->

    <owl:NamedIndividual rdf:about="http://semanticbible.org/ns/2006/NTNames#Jerusalem">
        <rdf:type rdf:resource="http://semanticbible.org/ns/2006/NTNames#City"/>
        <location rdf:resource="http://semanticbible.org/ns/2006/NTNames#JerusalemGeodata"/>
        <residentPlaceOf rdf:resource="http://semanticbible.org/ns/2006/NTNames#ClaudiusLysias"/>
        <residentPlaceOf rdf:resource="http://semanticbible.org/ns/2006/NTNames#Gamaliel"/>
        <residentPlaceOf rdf:resource="http://semanticbible.org/ns/2006/NTNames#MaryMotherOfJohnMark"/>
        <residentPlaceOf rdf:resource="http://semanticbible.org/ns/2006/NTNames#Rhoda"/>
        <residentPlaceOf rdf:resource="http://semanticbible.org/ns/2006/NTNames#Sapphira"/>
        <subregion rdf:resource="http://semanticbible.org/ns/2006/NTNames#Bethesda"/>
        <subregion rdf:resource="http://semanticbible.org/ns/2006/NTNames#Siloam"/>
        <subregionOf rdf:resource="http://semanticbible.org/ns/2006/NTNames#Judea"/>
        <visitedPlaceOf rdf:resource="http://semanticbible.org/ns/2006/NTNames#Cleopas"/>
        <visitedPlaceOf rdf:resource="http://semanticbible.org/ns/2006/NTNames#Festus"/>
        <visitedPlaceOf rdf:resource="http://semanticbible.org/ns/2006/NTNames#HerodAntipas"/>
        <visitedPlaceOf rdf:resource="http://semanticbible.org/ns/2006/NTNames#Joanna"/>
        <visitedPlaceOf rdf:resource="http://semanticbible.org/ns/2006/NTNames#Mary"/>
        <rdfs:label xml:lang="en">Jerusalem</rdfs:label>
    </owl:NamedIndividual>
    


    <!-- http://semanticbible.org/ns/2006/NTNames#JerusalemGeodata -->

    <owl:NamedIndividual rdf:about="http://semanticbible.org/ns/2006/NTNames#JerusalemGeodata">
        <rdf:type rdf:resource="http://semanticbible.org/ns/2006/NTNames#GeographicLocation"/>
        <altitude rdf:datatype="http://www.w3.org/2001/XMLSchema#int">0</altitude>
        <latitude rdf:datatype="http://www.w3.org/2001/XMLSchema#double">31.77451070780678</latitude>
        <longitude rdf:datatype="http://www.w3.org/2001/XMLSchema#double">35.22395850823153</longitude>
        <rdfs:label xml:lang="en">geodata for Jerusalem</rdfs:label>
    </owl:NamedIndividual>
    


    <!-- http://semanticbible.org/ns/2006/NTNames#Jesse -->

    <owl:NamedIndividual rdf:about="http://semanticbible.org/ns/2006/NTNames#Jesse">
        <rdf:type rdf:resource="http://semanticbible.org/ns/2006/NTNames#Man"/>
        <childOf rdf:resource="http://semanticbible.org/ns/2006/NTNames#Obed"/>
        <ethnicity rdf:resource="http://semanticbible.org/ns/2006/NTNames#Jewish"/>
        <parentOf rdf:resource="http://semanticbible.org/ns/2006/NTNames#David"/>
        <description rdf:datatype="http://www.w3.org/2001/XMLSchema#string">the father of King David</description>
        <hasOnlyGenealogyMention rdf:datatype="http://www.w3.org/2001/XMLSchema#boolean">true</hasOnlyGenealogyMention>
        <rdfs:label xml:lang="en">Jesse</rdfs:label>
    </owl:NamedIndividual>
    


    <!-- http://semanticbible.org/ns/2006/NTNames#Jesus -->

    <owl:NamedIndividual rdf:about="http://semanticbible.org/ns/2006/NTNames#Jesus">
        <rdf:type rdf:resource="http://semanticbible.org/ns/2006/NTNames#SonOfGod"/>
        <childOf rdf:resource="http://semanticbible.org/ns/2006/NTNames#Joseph"/>
        <childOf rdf:resource="http://semanticbible.org/ns/2006/NTNames#Mary"/>
        <collaboratesWith rdf:resource="http://semanticbible.org/ns/2006/NTNames#Andrew"/>
        <collaboratesWith rdf:resource="http://semanticbible.org/ns/2006/NTNames#Cleopas"/>
        <collaboratesWith rdf:resource="http://semanticbible.org/ns/2006/NTNames#Joanna"/>
        <collaboratesWith rdf:resource="http://semanticbible.org/ns/2006/NTNames#MaryMagdalene"/>
        <collaboratesWith rdf:resource="http://semanticbible.org/ns/2006/NTNames#MaryWifeOfClopas"/>
        <collaboratesWith rdf:resource="http://semanticbible.org/ns/2006/NTNames#Salome"/>
        <collaboratesWith rdf:resource="http://semanticbible.org/ns/2006/NTNames#Susanna"/>
        <hasEnemy rdf:resource="http://semanticbible.org/ns/2006/NTNames#HerodAntipas"/>
        <description rdf:datatype="http://www.w3.org/2001/XMLSchema#string">Jesus Christ, the Messiah and Son of God</description>
        <rdfs:comment xml:lang="en">As the central figure of the New Testament, it is impossible to incorporate all the information about Jesus in this limited framework. </rdfs:comment>
        <rdfs:label xml:lang="en">Jesus</rdfs:label>
    </owl:NamedIndividual>
    


    <!-- http://semanticbible.org/ns/2006/NTNames#Jew -->

    <owl:NamedIndividual rdf:about="http://semanticbible.org/ns/2006/NTNames#Jew">
        <rdf:type rdf:resource="http://semanticbible.org/ns/2006/NTNames#ReligiousBelief"/>
        <rdfs:label xml:lang="en">Jew</rdfs:label>
    </owl:NamedIndividual>
    


    <!-- http://semanticbible.org/ns/2006/NTNames#Jewish -->

    <owl:NamedIndividual rdf:about="http://semanticbible.org/ns/2006/NTNames#Jewish">
        <rdf:type rdf:resource="http://semanticbible.org/ns/2006/NTNames#EthnicityAttribute"/>
        <ethnicityOf rdf:resource="http://semanticbible.org/ns/2006/NTNames#Aaron"/>
        <ethnicityOf rdf:resource="http://semanticbible.org/ns/2006/NTNames#AbijahSonOfRehoboam"/>
        <ethnicityOf rdf:resource="http://semanticbible.org/ns/2006/NTNames#Abiud"/>
        <ethnicityOf rdf:resource="http://semanticbible.org/ns/2006/NTNames#Abraham"/>
        <ethnicityOf rdf:resource="http://semanticbible.org/ns/2006/NTNames#Achim"/>
        <ethnicityOf rdf:resource="http://semanticbible.org/ns/2006/NTNames#Addi"/>
        <ethnicityOf rdf:resource="http://semanticbible.org/ns/2006/NTNames#Admin"/>
        <ethnicityOf rdf:resource="http://semanticbible.org/ns/2006/NTNames#Ahaz"/>
        <ethnicityOf rdf:resource="http://semanticbible.org/ns/2006/NTNames#AlexanderOfEphesus"/>
        <ethnicityOf rdf:resource="http://semanticbible.org/ns/2006/NTNames#Amminadab"/>
        <ethnicityOf rdf:resource="http://semanticbible.org/ns/2006/NTNames#Amos"/>
        <ethnicityOf rdf:resource="http://semanticbible.org/ns/2006/NTNames#AmosSonOfNahum"/>
        <ethnicityOf rdf:resource="http://semanticbible.org/ns/2006/NTNames#Ananias"/>
        <ethnicityOf rdf:resource="http://semanticbible.org/ns/2006/NTNames#AnaniasOfDamascus"/>
        <ethnicityOf rdf:resource="http://semanticbible.org/ns/2006/NTNames#Anna"/>
        <ethnicityOf rdf:resource="http://semanticbible.org/ns/2006/NTNames#Aquila"/>
        <ethnicityOf rdf:resource="http://semanticbible.org/ns/2006/NTNames#Arni"/>
        <ethnicityOf rdf:resource="http://semanticbible.org/ns/2006/NTNames#Asaph"/>
        <ethnicityOf rdf:resource="http://semanticbible.org/ns/2006/NTNames#Asher"/>
        <ethnicityOf rdf:resource="http://semanticbible.org/ns/2006/NTNames#Azor"/>
        <ethnicityOf rdf:resource="http://semanticbible.org/ns/2006/NTNames#Bar-Jesus"/>
        <ethnicityOf rdf:resource="http://semanticbible.org/ns/2006/NTNames#Barabbas"/>
        <ethnicityOf rdf:resource="http://semanticbible.org/ns/2006/NTNames#Barachiah"/>
        <ethnicityOf rdf:resource="http://semanticbible.org/ns/2006/NTNames#Bathsheba"/>
        <ethnicityOf rdf:resource="http://semanticbible.org/ns/2006/NTNames#Benjamin"/>
        <ethnicityOf rdf:resource="http://semanticbible.org/ns/2006/NTNames#Bernice"/>
        <ethnicityOf rdf:resource="http://semanticbible.org/ns/2006/NTNames#Boaz"/>
        <ethnicityOf rdf:resource="http://semanticbible.org/ns/2006/NTNames#Caiaphas"/>
        <ethnicityOf rdf:resource="http://semanticbible.org/ns/2006/NTNames#Cosam"/>
        <ethnicityOf rdf:resource="http://semanticbible.org/ns/2006/NTNames#David"/>
        <ethnicityOf rdf:resource="http://semanticbible.org/ns/2006/NTNames#Drusilla"/>
        <ethnicityOf rdf:resource="http://semanticbible.org/ns/2006/NTNames#Eber"/>
        <ethnicityOf rdf:resource="http://semanticbible.org/ns/2006/NTNames#Eleazar"/>
        <ethnicityOf rdf:resource="http://semanticbible.org/ns/2006/NTNames#EliakimSonOfAbiud"/>
        <ethnicityOf rdf:resource="http://semanticbible.org/ns/2006/NTNames#EliakimSonOfMelea"/>
        <ethnicityOf rdf:resource="http://semanticbible.org/ns/2006/NTNames#Eliezer"/>
        <ethnicityOf rdf:resource="http://semanticbible.org/ns/2006/NTNames#Elijah"/>
        <ethnicityOf rdf:resource="http://semanticbible.org/ns/2006/NTNames#Elisha"/>
        <ethnicityOf rdf:resource="http://semanticbible.org/ns/2006/NTNames#Eliud"/>
        <ethnicityOf rdf:resource="http://semanticbible.org/ns/2006/NTNames#Elizabeth"/>
        <ethnicityOf rdf:resource="http://semanticbible.org/ns/2006/NTNames#Elmadam"/>
        <ethnicityOf rdf:resource="http://semanticbible.org/ns/2006/NTNames#Er"/>
        <ethnicityOf rdf:resource="http://semanticbible.org/ns/2006/NTNames#Esau"/>
        <ethnicityOf rdf:resource="http://semanticbible.org/ns/2006/NTNames#Esli"/>
        <ethnicityOf rdf:resource="http://semanticbible.org/ns/2006/NTNames#Eunice"/>
        <ethnicityOf rdf:resource="http://semanticbible.org/ns/2006/NTNames#Gad"/>
        <ethnicityOf rdf:resource="http://semanticbible.org/ns/2006/NTNames#Gamaliel"/>
        <ethnicityOf rdf:resource="http://semanticbible.org/ns/2006/NTNames#Gideon"/>
        <ethnicityOf rdf:resource="http://semanticbible.org/ns/2006/NTNames#Heli"/>
        <ethnicityOf rdf:resource="http://semanticbible.org/ns/2006/NTNames#Hezekiah"/>
        <ethnicityOf rdf:resource="http://semanticbible.org/ns/2006/NTNames#Hezron"/>
        <ethnicityOf rdf:resource="http://semanticbible.org/ns/2006/NTNames#Isaac"/>
        <ethnicityOf rdf:resource="http://semanticbible.org/ns/2006/NTNames#Jacob"/>
        <ethnicityOf rdf:resource="http://semanticbible.org/ns/2006/NTNames#Jannai"/>
        <ethnicityOf rdf:resource="http://semanticbible.org/ns/2006/NTNames#Jechoniah"/>
        <ethnicityOf rdf:resource="http://semanticbible.org/ns/2006/NTNames#Jehoshaphat"/>
        <ethnicityOf rdf:resource="http://semanticbible.org/ns/2006/NTNames#Jesse"/>
        <ethnicityOf rdf:resource="http://semanticbible.org/ns/2006/NTNames#Joanan"/>
        <ethnicityOf rdf:resource="http://semanticbible.org/ns/2006/NTNames#JohnOfTheSanhedrin"/>
        <ethnicityOf rdf:resource="http://semanticbible.org/ns/2006/NTNames#Jonam"/>
        <ethnicityOf rdf:resource="http://semanticbible.org/ns/2006/NTNames#Joram"/>
        <ethnicityOf rdf:resource="http://semanticbible.org/ns/2006/NTNames#Jorim"/>
        <ethnicityOf rdf:resource="http://semanticbible.org/ns/2006/NTNames#Josech"/>
        <ethnicityOf rdf:resource="http://semanticbible.org/ns/2006/NTNames#JosephBarsabbas"/>
        <ethnicityOf rdf:resource="http://semanticbible.org/ns/2006/NTNames#JosephSonOfJonam"/>
        <ethnicityOf rdf:resource="http://semanticbible.org/ns/2006/NTNames#JosephSonOfMattathias"/>
        <ethnicityOf rdf:resource="http://semanticbible.org/ns/2006/NTNames#JosephThePatriarch"/>
        <ethnicityOf rdf:resource="http://semanticbible.org/ns/2006/NTNames#JoshuaSonOfEliezer"/>
        <ethnicityOf rdf:resource="http://semanticbible.org/ns/2006/NTNames#Josiah"/>
        <ethnicityOf rdf:resource="http://semanticbible.org/ns/2006/NTNames#Jotham"/>
        <ethnicityOf rdf:resource="http://semanticbible.org/ns/2006/NTNames#Judah"/>
        <ethnicityOf rdf:resource="http://semanticbible.org/ns/2006/NTNames#JudahSonOfJoseph"/>
        <ethnicityOf rdf:resource="http://semanticbible.org/ns/2006/NTNames#LeviSonOfMelki"/>
        <ethnicityOf rdf:resource="http://semanticbible.org/ns/2006/NTNames#LeviSonOfSimeon"/>
        <ethnicityOf rdf:resource="http://semanticbible.org/ns/2006/NTNames#Lois"/>
        <ethnicityOf rdf:resource="http://semanticbible.org/ns/2006/NTNames#Maath"/>
        <ethnicityOf rdf:resource="http://semanticbible.org/ns/2006/NTNames#Manasseh"/>
        <ethnicityOf rdf:resource="http://semanticbible.org/ns/2006/NTNames#ManassehThePatriarch"/>
        <ethnicityOf rdf:resource="http://semanticbible.org/ns/2006/NTNames#Martha"/>
        <ethnicityOf rdf:resource="http://semanticbible.org/ns/2006/NTNames#Mary"/>
        <ethnicityOf rdf:resource="http://semanticbible.org/ns/2006/NTNames#MaryMagdalene"/>
        <ethnicityOf rdf:resource="http://semanticbible.org/ns/2006/NTNames#MaryMotherOfJohnMark"/>
        <ethnicityOf rdf:resource="http://semanticbible.org/ns/2006/NTNames#MaryOfBethany"/>
        <ethnicityOf rdf:resource="http://semanticbible.org/ns/2006/NTNames#MaryWifeOfClopas"/>
        <ethnicityOf rdf:resource="http://semanticbible.org/ns/2006/NTNames#Mattatha"/>
        <ethnicityOf rdf:resource="http://semanticbible.org/ns/2006/NTNames#MattathaisSonOfAmos"/>
        <ethnicityOf rdf:resource="http://semanticbible.org/ns/2006/NTNames#MattathiasSonOfSemein"/>
        <ethnicityOf rdf:resource="http://semanticbible.org/ns/2006/NTNames#MatthatSonOfLeviSonOfMelki"/>
        <ethnicityOf rdf:resource="http://semanticbible.org/ns/2006/NTNames#MatthatSonOfLeviSonOfSimeon"/>
        <ethnicityOf rdf:resource="http://semanticbible.org/ns/2006/NTNames#MelchiSonOfAddi"/>
        <ethnicityOf rdf:resource="http://semanticbible.org/ns/2006/NTNames#MelchiSonOfJannai"/>
        <ethnicityOf rdf:resource="http://semanticbible.org/ns/2006/NTNames#Melea"/>
        <ethnicityOf rdf:resource="http://semanticbible.org/ns/2006/NTNames#Menna"/>
        <ethnicityOf rdf:resource="http://semanticbible.org/ns/2006/NTNames#Naggai"/>
        <ethnicityOf rdf:resource="http://semanticbible.org/ns/2006/NTNames#Nahshon"/>
        <ethnicityOf rdf:resource="http://semanticbible.org/ns/2006/NTNames#Nahum"/>
        <ethnicityOf rdf:resource="http://semanticbible.org/ns/2006/NTNames#Nathan"/>
        <ethnicityOf rdf:resource="http://semanticbible.org/ns/2006/NTNames#Neri"/>
        <ethnicityOf rdf:resource="http://semanticbible.org/ns/2006/NTNames#Obed"/>
        <ethnicityOf rdf:resource="http://semanticbible.org/ns/2006/NTNames#Perez"/>
        <ethnicityOf rdf:resource="http://semanticbible.org/ns/2006/NTNames#Priscilla"/>
        <ethnicityOf rdf:resource="http://semanticbible.org/ns/2006/NTNames#Rachel"/>
        <ethnicityOf rdf:resource="http://semanticbible.org/ns/2006/NTNames#Ram"/>
        <ethnicityOf rdf:resource="http://semanticbible.org/ns/2006/NTNames#Rebecca"/>
        <ethnicityOf rdf:resource="http://semanticbible.org/ns/2006/NTNames#Rehoboam"/>
        <ethnicityOf rdf:resource="http://semanticbible.org/ns/2006/NTNames#Rhesa"/>
        <ethnicityOf rdf:resource="http://semanticbible.org/ns/2006/NTNames#Salmon"/>
        <ethnicityOf rdf:resource="http://semanticbible.org/ns/2006/NTNames#Sapphira"/>
        <ethnicityOf rdf:resource="http://semanticbible.org/ns/2006/NTNames#Sarah"/>
        <ethnicityOf rdf:resource="http://semanticbible.org/ns/2006/NTNames#Semein"/>
        <ethnicityOf rdf:resource="http://semanticbible.org/ns/2006/NTNames#Shealtiel"/>
        <ethnicityOf rdf:resource="http://semanticbible.org/ns/2006/NTNames#ShealtielSonOfNeri"/>
        <ethnicityOf rdf:resource="http://semanticbible.org/ns/2006/NTNames#SimeonSonOfJudah"/>
        <ethnicityOf rdf:resource="http://semanticbible.org/ns/2006/NTNames#SimeonThePatriarch"/>
        <ethnicityOf rdf:resource="http://semanticbible.org/ns/2006/NTNames#SimonOfCyrene"/>
        <ethnicityOf rdf:resource="http://semanticbible.org/ns/2006/NTNames#Solomon"/>
        <ethnicityOf rdf:resource="http://semanticbible.org/ns/2006/NTNames#Susanna"/>
        <ethnicityOf rdf:resource="http://semanticbible.org/ns/2006/NTNames#Tamar"/>
        <ethnicityOf rdf:resource="http://semanticbible.org/ns/2006/NTNames#Timothy"/>
        <ethnicityOf rdf:resource="http://semanticbible.org/ns/2006/NTNames#Uzziah"/>
        <ethnicityOf rdf:resource="http://semanticbible.org/ns/2006/NTNames#Zadok"/>
        <ethnicityOf rdf:resource="http://semanticbible.org/ns/2006/NTNames#ZechariahSonOfBarachiah"/>
        <ethnicityOf rdf:resource="http://semanticbible.org/ns/2006/NTNames#Zerah"/>
        <ethnicityOf rdf:resource="http://semanticbible.org/ns/2006/NTNames#Zerubbabel"/>
        <rdfs:comment xml:lang="en">The notion of &apos;Jewish&apos; as an ethnicity is problematic given the long history of God&apos;s chosen people and their many circumstances. Here it refers broadly to the Jewish identity, and is applied to all those from Abraham through Peter and Paul who would designate themselves as Jewish. In particular, no attempt is made to distinguish pre-Mosaic Jewish ethnicity from later forms. Israelite is only used a few times in the New Testament, and in those instances, it is treated synonymously with Jewish. </rdfs:comment>
        <rdfs:label xml:lang="en">Jewish</rdfs:label>
    </owl:NamedIndividual>
    


    <!-- http://semanticbible.org/ns/2006/NTNames#Jews -->

    <owl:NamedIndividual rdf:about="http://semanticbible.org/ns/2006/NTNames#Jews">
        <rdf:type rdf:resource="http://semanticbible.org/ns/2006/NTNames#BeliefGroup"/>
        <rdfs:label xml:lang="en">Jews</rdfs:label>
    </owl:NamedIndividual>
    


    <!-- http://semanticbible.org/ns/2006/NTNames#Jezebel -->

    <owl:NamedIndividual rdf:about="http://semanticbible.org/ns/2006/NTNames#Jezebel">
        <rdf:type rdf:resource="http://semanticbible.org/ns/2006/NTNames#Woman"/>
        <description rdf:datatype="http://www.w3.org/2001/XMLSchema#string">the pagan wife of Ahab in the Old Testament</description>
        <hasOnlyGenealogyMention rdf:datatype="http://www.w3.org/2001/XMLSchema#boolean">false</hasOnlyGenealogyMention>
        <rdfs:comment xml:lang="en">This may be a figurative reference based on the pagan wife of Ahab in the Old Testament, rather than the actual name of a contemporary person.</rdfs:comment>
        <rdfs:label xml:lang="en">Jezebel</rdfs:label>
    </owl:NamedIndividual>
    


    <!-- http://semanticbible.org/ns/2006/NTNames#Joanan -->

    <owl:NamedIndividual rdf:about="http://semanticbible.org/ns/2006/NTNames#Joanan">
        <rdf:type rdf:resource="http://semanticbible.org/ns/2006/NTNames#Man"/>
        <childOf rdf:resource="http://semanticbible.org/ns/2006/NTNames#Rhesa"/>
        <ethnicity rdf:resource="http://semanticbible.org/ns/2006/NTNames#Jewish"/>
        <parentOf rdf:resource="http://semanticbible.org/ns/2006/NTNames#Joda"/>
        <description rdf:datatype="http://www.w3.org/2001/XMLSchema#string">One of the ancestors of Jesus mentioned in Luke&apos;s geneaology</description>
        <hasOnlyGenealogyMention rdf:datatype="http://www.w3.org/2001/XMLSchema#boolean">true</hasOnlyGenealogyMention>
        <rdfs:label xml:lang="en">Joanan</rdfs:label>
    </owl:NamedIndividual>
    


    <!-- http://semanticbible.org/ns/2006/NTNames#Joanna -->

    <owl:NamedIndividual rdf:about="http://semanticbible.org/ns/2006/NTNames#Joanna">
        <rdf:type rdf:resource="http://semanticbible.org/ns/2006/NTNames#Woman"/>
        <collaboratesWith rdf:resource="http://semanticbible.org/ns/2006/NTNames#Jesus"/>
        <knows rdf:resource="http://semanticbible.org/ns/2006/NTNames#Susanna"/>
        <religiousBelief rdf:resource="http://semanticbible.org/ns/2006/NTNames#Christianity"/>
        <spouseOf rdf:resource="http://semanticbible.org/ns/2006/NTNames#Chuza"/>
        <visitedPlace rdf:resource="http://semanticbible.org/ns/2006/NTNames#Jerusalem"/>
        <description rdf:datatype="http://www.w3.org/2001/XMLSchema#string">a woman wno contributed to Jesus&apos; support</description>
        <hasOnlyGenealogyMention rdf:datatype="http://www.w3.org/2001/XMLSchema#boolean">false</hasOnlyGenealogyMention>
        <rdfs:comment xml:lang="en">Probably of Jewish ethnicity</rdfs:comment>
        <rdfs:label xml:lang="en">Joanna</rdfs:label>
    </owl:NamedIndividual>
    


    <!-- http://semanticbible.org/ns/2006/NTNames#Job -->

    <owl:NamedIndividual rdf:about="http://semanticbible.org/ns/2006/NTNames#Job">
        <rdf:type rdf:resource="http://semanticbible.org/ns/2006/NTNames#Man"/>
        <rdfs:label xml:lang="en">Job</rdfs:label>
    </owl:NamedIndividual>
    


    <!-- http://semanticbible.org/ns/2006/NTNames#Joda -->

    <owl:NamedIndividual rdf:about="http://semanticbible.org/ns/2006/NTNames#Joda">
        <rdf:type rdf:resource="http://semanticbible.org/ns/2006/NTNames#Man"/>
        <childOf rdf:resource="http://semanticbible.org/ns/2006/NTNames#Joanan"/>
        <parentOf rdf:resource="http://semanticbible.org/ns/2006/NTNames#Josech"/>
        <description rdf:datatype="http://www.w3.org/2001/XMLSchema#string">One of the ancestors of Jesus mentioned in Luke&apos;s geneaology</description>
        <hasOnlyGenealogyMention rdf:datatype="http://www.w3.org/2001/XMLSchema#boolean">true</hasOnlyGenealogyMention>
        <rdfs:label xml:lang="en">Joda</rdfs:label>
    </owl:NamedIndividual>
    


    <!-- http://semanticbible.org/ns/2006/NTNames#Joel -->

    <owl:NamedIndividual rdf:about="http://semanticbible.org/ns/2006/NTNames#Joel">
        <rdf:type rdf:resource="http://semanticbible.org/ns/2006/NTNames#Man"/>
        <rdfs:label xml:lang="en">Joel</rdfs:label>
    </owl:NamedIndividual>
    


    <!-- http://semanticbible.org/ns/2006/NTNames#JohnMark -->

    <owl:NamedIndividual rdf:about="http://semanticbible.org/ns/2006/NTNames#JohnMark">
        <rdf:type rdf:resource="http://semanticbible.org/ns/2006/NTNames#Man"/>
        <childOf rdf:resource="http://semanticbible.org/ns/2006/NTNames#MaryMotherOfJohnMark"/>
        <collaboratesWith rdf:resource="http://semanticbible.org/ns/2006/NTNames#Barnabas"/>
        <relativeOf rdf:resource="http://semanticbible.org/ns/2006/NTNames#Barnabas"/>
        <rdfs:comment xml:lang="en">One of Paul&apos;s companions</rdfs:comment>
        <rdfs:label xml:lang="en">John Mark</rdfs:label>
    </owl:NamedIndividual>
    


    <!-- http://semanticbible.org/ns/2006/NTNames#JohnOfTheSanhedrin -->

    <owl:NamedIndividual rdf:about="http://semanticbible.org/ns/2006/NTNames#JohnOfTheSanhedrin">
        <rdf:type rdf:resource="http://semanticbible.org/ns/2006/NTNames#Man"/>
        <collaboratesWith rdf:resource="http://semanticbible.org/ns/2006/NTNames#AlexanderOfTheSanhedrin"/>
        <collaboratesWith rdf:resource="http://semanticbible.org/ns/2006/NTNames#Annas"/>
        <enemyOf rdf:resource="http://semanticbible.org/ns/2006/NTNames#JohnSonOfZebedee"/>
        <enemyOf rdf:resource="http://semanticbible.org/ns/2006/NTNames#SimonPeter"/>
        <ethnicity rdf:resource="http://semanticbible.org/ns/2006/NTNames#Jewish"/>
        <memberOf rdf:resource="http://semanticbible.org/ns/2006/NTNames#Sanhedrin"/>
        <relativeOf rdf:resource="http://semanticbible.org/ns/2006/NTNames#AlexanderOfTheSanhedrin"/>
        <relativeOf rdf:resource="http://semanticbible.org/ns/2006/NTNames#Annas"/>
        <description rdf:datatype="http://www.w3.org/2001/XMLSchema#string">A relative of Annas the High Priest who was present when Peter and John were questioned about healing a lame man</description>
        <rdfs:label xml:lang="en">John</rdfs:label>
    </owl:NamedIndividual>
    


    <!-- http://semanticbible.org/ns/2006/NTNames#JohnSonOfZebedee -->

    <owl:NamedIndividual rdf:about="http://semanticbible.org/ns/2006/NTNames#JohnSonOfZebedee">
        <rdf:type rdf:resource="http://semanticbible.org/ns/2006/NTNames#Man"/>
        <childOf rdf:resource="http://semanticbible.org/ns/2006/NTNames#Salome"/>
        <childOf rdf:resource="http://semanticbible.org/ns/2006/NTNames#Zebedee"/>
        <collaboratesWith rdf:resource="http://semanticbible.org/ns/2006/NTNames#Andrew"/>
        <collaboratesWith rdf:resource="http://semanticbible.org/ns/2006/NTNames#Demetrius"/>
        <collaboratesWith rdf:resource="http://semanticbible.org/ns/2006/NTNames#GaiusTheBeloved"/>
        <collaboratesWith rdf:resource="http://semanticbible.org/ns/2006/NTNames#MaryMagdalene"/>
        <hasAntagonist rdf:resource="http://semanticbible.org/ns/2006/NTNames#Diotrephes"/>
        <hasEnemy rdf:resource="http://semanticbible.org/ns/2006/NTNames#AlexanderOfTheSanhedrin"/>
        <hasEnemy rdf:resource="http://semanticbible.org/ns/2006/NTNames#Annas"/>
        <hasEnemy rdf:resource="http://semanticbible.org/ns/2006/NTNames#JohnOfTheSanhedrin"/>
        <siblingOf rdf:resource="http://semanticbible.org/ns/2006/NTNames#JamesSonOfZebedee"/>
        <description rdf:datatype="http://www.w3.org/2001/XMLSchema#string">One of Jesus&apos; twelve apostles</description>
        <rdfs:label xml:lang="en">John</rdfs:label>
    </owl:NamedIndividual>
    


    <!-- http://semanticbible.org/ns/2006/NTNames#JohntheBaptist -->

    <owl:NamedIndividual rdf:about="http://semanticbible.org/ns/2006/NTNames#JohntheBaptist">
        <rdf:type rdf:resource="http://semanticbible.org/ns/2006/NTNames#Man"/>
        <childOf rdf:resource="http://semanticbible.org/ns/2006/NTNames#Elizabeth"/>
        <childOf rdf:resource="http://semanticbible.org/ns/2006/NTNames#Zechariah"/>
        <collaboratesWith rdf:resource="http://semanticbible.org/ns/2006/NTNames#Andrew"/>
        <collaboratesWith rdf:resource="http://semanticbible.org/ns/2006/NTNames#SimonPeter"/>
        <ethnicity rdf:resource="http://semanticbible.org/ns/2006/NTNames#Levite"/>
        <rdfs:comment rdf:datatype="http://www.w3.org/2001/XMLSchema#string">John certainly understood Jesus to be the Messiah and was a person of faith, but he cannot be accounted a Christian since Jesus&apos; ministry was not yet accomplished when he was beheaded. 
The use of the name Elijah to refer to John the Baptist is figurative.</rdfs:comment>
        <rdfs:label xml:lang="en">John</rdfs:label>
        <rdfs:label xml:lang="en">John the Baptist</rdfs:label>
    </owl:NamedIndividual>
    


    <!-- http://semanticbible.org/ns/2006/NTNames#JonahOfBethsaida -->

    <owl:NamedIndividual rdf:about="http://semanticbible.org/ns/2006/NTNames#JonahOfBethsaida">
        <rdf:type rdf:resource="http://semanticbible.org/ns/2006/NTNames#Man"/>
        <parentOf rdf:resource="http://semanticbible.org/ns/2006/NTNames#Andrew"/>
        <parentOf rdf:resource="http://semanticbible.org/ns/2006/NTNames#SimonPeter"/>
        <description rdf:datatype="http://www.w3.org/2001/XMLSchema#string">Father of Peter and Andrew, two of Jesus&apos; 12 disciples</description>
        <rdfs:comment rdf:datatype="http://www.w3.org/2001/XMLSchema#string">Bethsaide is assumed as his place of residence because his sons were from there. He was probably a fisherman, though nothing else is said of him in the New Testament.</rdfs:comment>
        <rdfs:label xml:lang="en">Jonah</rdfs:label>
    </owl:NamedIndividual>
    


    <!-- http://semanticbible.org/ns/2006/NTNames#JonahTheProphet -->

    <owl:NamedIndividual rdf:about="http://semanticbible.org/ns/2006/NTNames#JonahTheProphet">
        <rdf:type rdf:resource="http://semanticbible.org/ns/2006/NTNames#Man"/>
        <description rdf:datatype="http://www.w3.org/2001/XMLSchema#string">A prophet from the Old Testmanent</description>
        <rdfs:label xml:lang="en">Jonah</rdfs:label>
    </owl:NamedIndividual>
    


    <!-- http://semanticbible.org/ns/2006/NTNames#Jonam -->

    <owl:NamedIndividual rdf:about="http://semanticbible.org/ns/2006/NTNames#Jonam">
        <rdf:type rdf:resource="http://semanticbible.org/ns/2006/NTNames#Man"/>
        <childOf rdf:resource="http://semanticbible.org/ns/2006/NTNames#EliakimSonOfMelea"/>
        <ethnicity rdf:resource="http://semanticbible.org/ns/2006/NTNames#Jewish"/>
        <parentOf rdf:resource="http://semanticbible.org/ns/2006/NTNames#JosephSonOfJonam"/>
        <description rdf:datatype="http://www.w3.org/2001/XMLSchema#string">One of the ancestors of Jesus mentioned in Luke&apos;s geneaology</description>
        <hasOnlyGenealogyMention rdf:datatype="http://www.w3.org/2001/XMLSchema#boolean">true</hasOnlyGenealogyMention>
        <rdfs:label xml:lang="en">Jonam</rdfs:label>
    </owl:NamedIndividual>
    


    <!-- http://semanticbible.org/ns/2006/NTNames#Joppa -->

    <owl:NamedIndividual rdf:about="http://semanticbible.org/ns/2006/NTNames#Joppa">
        <rdf:type rdf:resource="http://semanticbible.org/ns/2006/NTNames#City"/>
        <location rdf:resource="http://semanticbible.org/ns/2006/NTNames#JoppaGeodata"/>
        <residentPlaceOf rdf:resource="http://semanticbible.org/ns/2006/NTNames#SimonTheTanner"/>
        <residentPlaceOf rdf:resource="http://semanticbible.org/ns/2006/NTNames#Tabitha"/>
        <subregionOf rdf:resource="http://semanticbible.org/ns/2006/NTNames#Judea"/>
        <rdfs:comment xml:lang="en">In Joppa, Peter raised the woman Tabitha from the dead. Later, he had a vision while praying there that prepared him for the coming of the Holy Spirit to the first Gentiles.</rdfs:comment>
        <rdfs:label xml:lang="en">Joppa</rdfs:label>
    </owl:NamedIndividual>
    


    <!-- http://semanticbible.org/ns/2006/NTNames#JoppaGeodata -->

    <owl:NamedIndividual rdf:about="http://semanticbible.org/ns/2006/NTNames#JoppaGeodata">
        <rdf:type rdf:resource="http://semanticbible.org/ns/2006/NTNames#GeographicLocation"/>
        <altitude rdf:datatype="http://www.w3.org/2001/XMLSchema#int">0</altitude>
        <latitude rdf:datatype="http://www.w3.org/2001/XMLSchema#double">32.05528613849865</latitude>
        <longitude rdf:datatype="http://www.w3.org/2001/XMLSchema#double">34.7494008586598</longitude>
        <rdfs:label xml:lang="en">geodata for Joppa</rdfs:label>
    </owl:NamedIndividual>
    


    <!-- http://semanticbible.org/ns/2006/NTNames#Joram -->

    <owl:NamedIndividual rdf:about="http://semanticbible.org/ns/2006/NTNames#Joram">
        <rdf:type rdf:resource="http://semanticbible.org/ns/2006/NTNames#Man"/>
        <childOf rdf:resource="http://semanticbible.org/ns/2006/NTNames#Jehoshaphat"/>
        <ethnicity rdf:resource="http://semanticbible.org/ns/2006/NTNames#Jewish"/>
        <parentOf rdf:resource="http://semanticbible.org/ns/2006/NTNames#Uzziah"/>
        <description rdf:datatype="http://www.w3.org/2001/XMLSchema#string">One of the ancestors of Jesus mentioned in Matthew&apos;s geneaology</description>
        <hasOnlyGenealogyMention rdf:datatype="http://www.w3.org/2001/XMLSchema#boolean">true</hasOnlyGenealogyMention>
        <occupation rdf:datatype="http://www.w3.org/2001/XMLSchema#string">king of Judah</occupation>
        <rdfs:comment rdf:datatype="http://www.w3.org/2001/XMLSchema#string">His occupation as King comes from Old Testament sources. </rdfs:comment>
        <rdfs:label xml:lang="en">Joram</rdfs:label>
    </owl:NamedIndividual>
    


    <!-- http://semanticbible.org/ns/2006/NTNames#Jordan -->

    <owl:NamedIndividual rdf:about="http://semanticbible.org/ns/2006/NTNames#Jordan">
        <rdf:type rdf:resource="http://semanticbible.org/ns/2006/NTNames#FreshWaterArea"/>
        <rdfs:label xml:lang="en">Jordan</rdfs:label>
    </owl:NamedIndividual>
    


    <!-- http://semanticbible.org/ns/2006/NTNames#Jorim -->

    <owl:NamedIndividual rdf:about="http://semanticbible.org/ns/2006/NTNames#Jorim">
        <rdf:type rdf:resource="http://semanticbible.org/ns/2006/NTNames#Man"/>
        <childOf rdf:resource="http://semanticbible.org/ns/2006/NTNames#MatthatSonOfLeviSonOfSimeon"/>
        <ethnicity rdf:resource="http://semanticbible.org/ns/2006/NTNames#Jewish"/>
        <parentOf rdf:resource="http://semanticbible.org/ns/2006/NTNames#Eliezer"/>
        <hasOnlyGenealogyMention rdf:datatype="http://www.w3.org/2001/XMLSchema#boolean">true</hasOnlyGenealogyMention>
        <rdfs:label xml:lang="en">Jorim</rdfs:label>
    </owl:NamedIndividual>
    


    <!-- http://semanticbible.org/ns/2006/NTNames#Josech -->

    <owl:NamedIndividual rdf:about="http://semanticbible.org/ns/2006/NTNames#Josech">
        <rdf:type rdf:resource="http://semanticbible.org/ns/2006/NTNames#Man"/>
        <childOf rdf:resource="http://semanticbible.org/ns/2006/NTNames#Joda"/>
        <ethnicity rdf:resource="http://semanticbible.org/ns/2006/NTNames#Jewish"/>
        <parentOf rdf:resource="http://semanticbible.org/ns/2006/NTNames#Semein"/>
        <description rdf:datatype="http://www.w3.org/2001/XMLSchema#string">One of the ancestors of Jesus mentioned in Luke&apos;s geneaology</description>
        <hasOnlyGenealogyMention rdf:datatype="http://www.w3.org/2001/XMLSchema#boolean">true</hasOnlyGenealogyMention>
        <rdfs:label xml:lang="en">Josech</rdfs:label>
    </owl:NamedIndividual>
    


    <!-- http://semanticbible.org/ns/2006/NTNames#Joseph -->

    <owl:NamedIndividual rdf:about="http://semanticbible.org/ns/2006/NTNames#Joseph">
        <rdf:type rdf:resource="http://semanticbible.org/ns/2006/NTNames#Man"/>
        <childOf rdf:resource="http://semanticbible.org/ns/2006/NTNames#Heli"/>
        <childOf rdf:resource="http://semanticbible.org/ns/2006/NTNames#JacobSonOfMatthan"/>
        <parentOf rdf:resource="http://semanticbible.org/ns/2006/NTNames#Jesus"/>
        <spouseOf rdf:resource="http://semanticbible.org/ns/2006/NTNames#Mary"/>
        <description rdf:datatype="http://www.w3.org/2001/XMLSchema#string">the earthly father of Jesus</description>
        <occupation rdf:datatype="http://www.w3.org/2001/XMLSchema#string">carpenter</occupation>
        <rdfs:comment xml:lang="en">Joseph was Jesus&apos; parent in the normal sense, even though not his biological father.
Luke 3:23 has &quot;Joseph, son of Heli&quot;, though Matthew has Joseph&apos;s father named Jacob. Here I&apos;ve represented the opinion that Joseph was actually son-in-law of Heli, and that Luke&apos;s geneaology describes Mary&apos;s lineage rather than Joseph&apos;s. </rdfs:comment>
        <rdfs:label xml:lang="en">Joseph</rdfs:label>
    </owl:NamedIndividual>
    


    <!-- http://semanticbible.org/ns/2006/NTNames#JosephBarsabbas -->

    <owl:NamedIndividual rdf:about="http://semanticbible.org/ns/2006/NTNames#JosephBarsabbas">
        <rdf:type rdf:resource="http://semanticbible.org/ns/2006/NTNames#Man"/>
        <collaboratesWith rdf:resource="http://semanticbible.org/ns/2006/NTNames#SimonPeter"/>
        <ethnicity rdf:resource="http://semanticbible.org/ns/2006/NTNames#Jewish"/>
        <description rdf:datatype="http://www.w3.org/2001/XMLSchema#string">an early Christian who was put forward (but not chosen) as a replacement for Judas Iscariot</description>
        <rdfs:label xml:lang="en">Joseph Barsabbas</rdfs:label>
    </owl:NamedIndividual>
    


    <!-- http://semanticbible.org/ns/2006/NTNames#JosephOfArimathea -->

    <owl:NamedIndividual rdf:about="http://semanticbible.org/ns/2006/NTNames#JosephOfArimathea">
        <rdf:type rdf:resource="http://semanticbible.org/ns/2006/NTNames#Man"/>
        <rdfs:comment xml:lang="en">Joseph was a member of the Jewish ruling council, and a follower of Jesus. He put Jesus&apos; body in his own tomb after the crucifixion. {en}</rdfs:comment>
        <rdfs:label xml:lang="en">Joseph of Arimathea</rdfs:label>
    </owl:NamedIndividual>
    


    <!-- http://semanticbible.org/ns/2006/NTNames#JosephSonOfJonam -->

    <owl:NamedIndividual rdf:about="http://semanticbible.org/ns/2006/NTNames#JosephSonOfJonam">
        <rdf:type rdf:resource="http://semanticbible.org/ns/2006/NTNames#Man"/>
        <childOf rdf:resource="http://semanticbible.org/ns/2006/NTNames#Jonam"/>
        <ethnicity rdf:resource="http://semanticbible.org/ns/2006/NTNames#Jewish"/>
        <parentOf rdf:resource="http://semanticbible.org/ns/2006/NTNames#JudahSonOfJoseph"/>
        <description rdf:datatype="http://www.w3.org/2001/XMLSchema#string">One of the ancestors of Jesus mentioned in Luke&apos;s geneaology</description>
        <hasOnlyGenealogyMention rdf:datatype="http://www.w3.org/2001/XMLSchema#boolean">true</hasOnlyGenealogyMention>
        <rdfs:label xml:lang="en">Joseph</rdfs:label>
    </owl:NamedIndividual>
    


    <!-- http://semanticbible.org/ns/2006/NTNames#JosephSonOfMattathias -->

    <owl:NamedIndividual rdf:about="http://semanticbible.org/ns/2006/NTNames#JosephSonOfMattathias">
        <rdf:type rdf:resource="http://semanticbible.org/ns/2006/NTNames#Man"/>
        <childOf rdf:resource="http://semanticbible.org/ns/2006/NTNames#MattathaisSonOfAmos"/>
        <ethnicity rdf:resource="http://semanticbible.org/ns/2006/NTNames#Jewish"/>
        <parentOf rdf:resource="http://semanticbible.org/ns/2006/NTNames#Jannai"/>
        <description rdf:datatype="http://www.w3.org/2001/XMLSchema#string">One of the ancestors of Jesus mentioned in Luke&apos;s geneaology</description>
        <hasOnlyGenealogyMention rdf:datatype="http://www.w3.org/2001/XMLSchema#boolean">true</hasOnlyGenealogyMention>
        <rdfs:label xml:lang="en">Joseph</rdfs:label>
    </owl:NamedIndividual>
    


    <!-- http://semanticbible.org/ns/2006/NTNames#JosephThePatriarch -->

    <owl:NamedIndividual rdf:about="http://semanticbible.org/ns/2006/NTNames#JosephThePatriarch">
        <rdf:type rdf:resource="http://semanticbible.org/ns/2006/NTNames#Man"/>
        <childOf rdf:resource="http://semanticbible.org/ns/2006/NTNames#Jacob"/>
        <childOf rdf:resource="http://semanticbible.org/ns/2006/NTNames#Rachel"/>
        <ethnicity rdf:resource="http://semanticbible.org/ns/2006/NTNames#Jewish"/>
        <siblingOf rdf:resource="http://semanticbible.org/ns/2006/NTNames#Gad"/>
        <rdfs:label xml:lang="en">Joseph</rdfs:label>
    </owl:NamedIndividual>
    


    <!-- http://semanticbible.org/ns/2006/NTNames#Joses -->

    <owl:NamedIndividual rdf:about="http://semanticbible.org/ns/2006/NTNames#Joses">
        <rdf:type rdf:resource="http://semanticbible.org/ns/2006/NTNames#Man"/>
        <siblingOf rdf:resource="http://semanticbible.org/ns/2006/NTNames#JamesSonOfAlphaeus"/>
        <rdfs:label xml:lang="en">Joses</rdfs:label>
    </owl:NamedIndividual>
    


    <!-- http://semanticbible.org/ns/2006/NTNames#Joshua -->

    <owl:NamedIndividual rdf:about="http://semanticbible.org/ns/2006/NTNames#Joshua">
        <rdf:type rdf:resource="http://semanticbible.org/ns/2006/NTNames#Man"/>
        <rdfs:label xml:lang="en">Joshua</rdfs:label>
    </owl:NamedIndividual>
    


    <!-- http://semanticbible.org/ns/2006/NTNames#JoshuaSonOfEliezer -->

    <owl:NamedIndividual rdf:about="http://semanticbible.org/ns/2006/NTNames#JoshuaSonOfEliezer">
        <rdf:type rdf:resource="http://semanticbible.org/ns/2006/NTNames#Man"/>
        <childOf rdf:resource="http://semanticbible.org/ns/2006/NTNames#Eliezer"/>
        <ethnicity rdf:resource="http://semanticbible.org/ns/2006/NTNames#Jewish"/>
        <parentOf rdf:resource="http://semanticbible.org/ns/2006/NTNames#Er"/>
        <description rdf:datatype="http://www.w3.org/2001/XMLSchema#string">One of the ancestors of Jesus mentioned in Luke&apos;s geneaology</description>
        <hasOnlyGenealogyMention rdf:datatype="http://www.w3.org/2001/XMLSchema#boolean">true</hasOnlyGenealogyMention>
        <rdfs:label xml:lang="en">Joshua</rdfs:label>
    </owl:NamedIndividual>
    


    <!-- http://semanticbible.org/ns/2006/NTNames#Josiah -->

    <owl:NamedIndividual rdf:about="http://semanticbible.org/ns/2006/NTNames#Josiah">
        <rdf:type rdf:resource="http://semanticbible.org/ns/2006/NTNames#Man"/>
        <childOf rdf:resource="http://semanticbible.org/ns/2006/NTNames#Amos"/>
        <ethnicity rdf:resource="http://semanticbible.org/ns/2006/NTNames#Jewish"/>
        <parentOf rdf:resource="http://semanticbible.org/ns/2006/NTNames#Jechoniah"/>
        <rdfs:label xml:lang="en">Josiah</rdfs:label>
    </owl:NamedIndividual>
    


    <!-- http://semanticbible.org/ns/2006/NTNames#Jotham -->

    <owl:NamedIndividual rdf:about="http://semanticbible.org/ns/2006/NTNames#Jotham">
        <rdf:type rdf:resource="http://semanticbible.org/ns/2006/NTNames#Man"/>
        <childOf rdf:resource="http://semanticbible.org/ns/2006/NTNames#Uzziah"/>
        <ethnicity rdf:resource="http://semanticbible.org/ns/2006/NTNames#Jewish"/>
        <parentOf rdf:resource="http://semanticbible.org/ns/2006/NTNames#Ahaz"/>
        <description rdf:datatype="http://www.w3.org/2001/XMLSchema#string">One of the ancestors of Jesus mentioned in Matthew&apos;s geneaology</description>
        <hasOnlyGenealogyMention rdf:datatype="http://www.w3.org/2001/XMLSchema#boolean">true</hasOnlyGenealogyMention>
        <occupation rdf:datatype="http://www.w3.org/2001/XMLSchema#string">king of Judah</occupation>
        <rdfs:comment rdf:datatype="http://www.w3.org/2001/XMLSchema#string">His occupation as King comes from Old Testament sources, 2Chron.26-27. </rdfs:comment>
        <rdfs:label xml:lang="en">Jotham</rdfs:label>
    </owl:NamedIndividual>
    


    <!-- http://semanticbible.org/ns/2006/NTNames#Judah -->

    <owl:NamedIndividual rdf:about="http://semanticbible.org/ns/2006/NTNames#Judah">
        <rdf:type rdf:resource="http://semanticbible.org/ns/2006/NTNames#Man"/>
        <childOf rdf:resource="http://semanticbible.org/ns/2006/NTNames#Jacob"/>
        <ethnicity rdf:resource="http://semanticbible.org/ns/2006/NTNames#Jewish"/>
        <parentOf rdf:resource="http://semanticbible.org/ns/2006/NTNames#Perez"/>
        <parentOf rdf:resource="http://semanticbible.org/ns/2006/NTNames#Zerah"/>
        <siblingOf rdf:resource="http://semanticbible.org/ns/2006/NTNames#Gad"/>
        <description rdf:datatype="http://www.w3.org/2001/XMLSchema#string">One of the 12 Patriarchs of Israel, after whom the land of Judea took its name.</description>
        <hasOnlyGenealogyMention rdf:datatype="http://www.w3.org/2001/XMLSchema#boolean">false</hasOnlyGenealogyMention>
        <rdfs:comment rdf:datatype="http://www.w3.org/2001/XMLSchema#string">Tamar was not actually his spouse, but his daughter-in-law (Gen 38).
</rdfs:comment>
        <rdfs:label xml:lang="en">Judah</rdfs:label>
    </owl:NamedIndividual>
    


    <!-- http://semanticbible.org/ns/2006/NTNames#JudahSonOfJoseph -->

    <owl:NamedIndividual rdf:about="http://semanticbible.org/ns/2006/NTNames#JudahSonOfJoseph">
        <rdf:type rdf:resource="http://semanticbible.org/ns/2006/NTNames#Man"/>
        <childOf rdf:resource="http://semanticbible.org/ns/2006/NTNames#JosephSonOfJonam"/>
        <ethnicity rdf:resource="http://semanticbible.org/ns/2006/NTNames#Jewish"/>
        <parentOf rdf:resource="http://semanticbible.org/ns/2006/NTNames#SimeonSonOfJudah"/>
        <description rdf:datatype="http://www.w3.org/2001/XMLSchema#string">One of the ancestors of Jesus mentioned in Luke&apos;s geneaology</description>
        <hasOnlyGenealogyMention rdf:datatype="http://www.w3.org/2001/XMLSchema#boolean">true</hasOnlyGenealogyMention>
        <rdfs:label xml:lang="en">Judah</rdfs:label>
    </owl:NamedIndividual>
    


    <!-- http://semanticbible.org/ns/2006/NTNames#Judaism -->

    <owl:NamedIndividual rdf:about="http://semanticbible.org/ns/2006/NTNames#Judaism">
        <rdf:type rdf:resource="http://semanticbible.org/ns/2006/NTNames#ReligiousBeliefSystem"/>
        <rdfs:comment xml:lang="en">This is distinct from Jewish as an ethnic heritage, which implies birth: one can have a ReligiousBelief of Judaism through conversion, despite not having Jewish ethnicity. Those who convert to other beliefs (most notably for the New Testament, Christianity) are typically designated as having Jewish ethnicity, but Christianity as a ReligiousBelief. There is no implication of faithful devotion to the Jewish faith. </rdfs:comment>
        <rdfs:label xml:lang="en">Judaism</rdfs:label>
    </owl:NamedIndividual>
    


    <!-- http://semanticbible.org/ns/2006/NTNames#Judas -->

    <owl:NamedIndividual rdf:about="http://semanticbible.org/ns/2006/NTNames#Judas">
        <rdf:type rdf:resource="http://semanticbible.org/ns/2006/NTNames#Man"/>
        <rdfs:label xml:lang="en">Judas</rdfs:label>
    </owl:NamedIndividual>
    


    <!-- http://semanticbible.org/ns/2006/NTNames#JudasOfAntioch -->

    <owl:NamedIndividual rdf:about="http://semanticbible.org/ns/2006/NTNames#JudasOfAntioch">
        <rdf:type rdf:resource="http://semanticbible.org/ns/2006/NTNames#Man"/>
        <collaboratesWith rdf:resource="http://semanticbible.org/ns/2006/NTNames#Barnabas"/>
        <collaboratesWith rdf:resource="http://semanticbible.org/ns/2006/NTNames#Paul"/>
        <description rdf:datatype="http://www.w3.org/2001/XMLSchema#string">a prophet in the church at Antioch</description>
        <rdfs:label xml:lang="en">Judas</rdfs:label>
    </owl:NamedIndividual>
    


    <!-- http://semanticbible.org/ns/2006/NTNames#Jude -->

    <owl:NamedIndividual rdf:about="http://semanticbible.org/ns/2006/NTNames#Jude">
        <rdf:type rdf:resource="http://semanticbible.org/ns/2006/NTNames#Man"/>
        <rdfs:label xml:lang="en">Jude</rdfs:label>
    </owl:NamedIndividual>
    


    <!-- http://semanticbible.org/ns/2006/NTNames#Judea -->

    <owl:NamedIndividual rdf:about="http://semanticbible.org/ns/2006/NTNames#Judea">
        <rdf:type rdf:resource="http://semanticbible.org/ns/2006/NTNames#StateOrProvince"/>
        <nativePlaceOf rdf:resource="http://semanticbible.org/ns/2006/NTNames#Elizabeth"/>
        <residentPlaceOf rdf:resource="http://semanticbible.org/ns/2006/NTNames#Elizabeth"/>
        <subregion rdf:resource="http://semanticbible.org/ns/2006/NTNames#Antipatris"/>
        <subregion rdf:resource="http://semanticbible.org/ns/2006/NTNames#Arimathea"/>
        <subregion rdf:resource="http://semanticbible.org/ns/2006/NTNames#Azotus"/>
        <subregion rdf:resource="http://semanticbible.org/ns/2006/NTNames#Bethany"/>
        <subregion rdf:resource="http://semanticbible.org/ns/2006/NTNames#Bethlehem"/>
        <subregion rdf:resource="http://semanticbible.org/ns/2006/NTNames#Bethphage"/>
        <subregion rdf:resource="http://semanticbible.org/ns/2006/NTNames#Emmaus"/>
        <subregion rdf:resource="http://semanticbible.org/ns/2006/NTNames#Ephraim"/>
        <subregion rdf:resource="http://semanticbible.org/ns/2006/NTNames#Gaza"/>
        <subregion rdf:resource="http://semanticbible.org/ns/2006/NTNames#Jericho"/>
        <subregion rdf:resource="http://semanticbible.org/ns/2006/NTNames#Jerusalem"/>
        <subregion rdf:resource="http://semanticbible.org/ns/2006/NTNames#Joppa"/>
        <subregion rdf:resource="http://semanticbible.org/ns/2006/NTNames#Lydda"/>
        <subregion rdf:resource="http://semanticbible.org/ns/2006/NTNames#Ramah"/>
        <subregion rdf:resource="http://semanticbible.org/ns/2006/NTNames#Sharon"/>
        <subregionOf rdf:resource="http://semanticbible.org/ns/2006/NTNames#Israel"/>
        <rdfs:label xml:lang="en">Judea</rdfs:label>
    </owl:NamedIndividual>
    


    <!-- http://semanticbible.org/ns/2006/NTNames#Judean -->

    <owl:NamedIndividual rdf:about="http://semanticbible.org/ns/2006/NTNames#Judean">
        <rdf:type rdf:resource="http://semanticbible.org/ns/2006/NTNames#EthnicityAttribute"/>
        <ethnicityOf rdf:resource="http://semanticbible.org/ns/2006/NTNames#AlexanderOfTheSanhedrin"/>
        <ethnicityOf rdf:resource="http://semanticbible.org/ns/2006/NTNames#AnaniasTheHighPriest"/>
        <rdfs:comment xml:lang="en">The main subgroup of Jewish Palestine at the time of Christ: to be Judean therefore implies being Jewish as well. This is distinct from describing those of the tribe and lineage of Judah.</rdfs:comment>
        <rdfs:label xml:lang="en">Judean</rdfs:label>
    </owl:NamedIndividual>
    


    <!-- http://semanticbible.org/ns/2006/NTNames#Julia -->

    <owl:NamedIndividual rdf:about="http://semanticbible.org/ns/2006/NTNames#Julia">
        <rdf:type rdf:resource="http://semanticbible.org/ns/2006/NTNames#Woman"/>
        <knows rdf:resource="http://semanticbible.org/ns/2006/NTNames#Paul"/>
        <knows rdf:resource="http://semanticbible.org/ns/2006/NTNames#Priscilla"/>
        <religiousBelief rdf:resource="http://semanticbible.org/ns/2006/NTNames#Christianity"/>
        <residentPlace rdf:resource="http://semanticbible.org/ns/2006/NTNames#Rome"/>
        <description rdf:datatype="http://www.w3.org/2001/XMLSchema#string">a Roman to whom Paul sent greetings</description>
        <hasOnlyGenealogyMention rdf:datatype="http://www.w3.org/2001/XMLSchema#boolean">false</hasOnlyGenealogyMention>
        <rdfs:comment rdf:datatype="http://www.w3.org/2001/XMLSchema#string">Julia may be the spouse or sister of Philologus, given their mention together in Rom.16.15</rdfs:comment>
        <rdfs:label xml:lang="en">Julia</rdfs:label>
    </owl:NamedIndividual>
    


    <!-- http://semanticbible.org/ns/2006/NTNames#Julius -->

    <owl:NamedIndividual rdf:about="http://semanticbible.org/ns/2006/NTNames#Julius">
        <rdf:type rdf:resource="http://semanticbible.org/ns/2006/NTNames#Man"/>
        <rdfs:label xml:lang="en">Julius</rdfs:label>
    </owl:NamedIndividual>
    


    <!-- http://semanticbible.org/ns/2006/NTNames#Junia -->

    <owl:NamedIndividual rdf:about="http://semanticbible.org/ns/2006/NTNames#Junia">
        <rdf:type rdf:resource="http://semanticbible.org/ns/2006/NTNames#Woman"/>
        <collaboratesWith rdf:resource="http://semanticbible.org/ns/2006/NTNames#Andronicus"/>
        <knows rdf:resource="http://semanticbible.org/ns/2006/NTNames#Priscilla"/>
        <religiousBelief rdf:resource="http://semanticbible.org/ns/2006/NTNames#Christianity"/>
        <residentPlace rdf:resource="http://semanticbible.org/ns/2006/NTNames#Rome"/>
        <description rdf:datatype="http://www.w3.org/2001/XMLSchema#string">a &quot;kinsman&quot; and fellow prisoner of Paul</description>
        <hasOnlyGenealogyMention rdf:datatype="http://www.w3.org/2001/XMLSchema#boolean">false</hasOnlyGenealogyMention>
        <rdfs:comment xml:lang="en">Given their joint mention by Paul, it seems likely that Junia was Andronicus&apos; spouse, though this is not explicitly stated. Paul&apos;s description of Andronicus and Junia as &quot;my kinsmen&quot; is taken in the general sense (e.g. coming from the same region), rather than literally. 
Given they were Christians before Paul, their conversion must have been relatively early in the history of the church, and so it is quite likely they also visited Jerusalem (though this is nowhere stated). 
Much controversy rests on whether this description means they were well-known _to_ the apostles, or well-known _as_ apostles. </rdfs:comment>
        <rdfs:label xml:lang="en">Junia</rdfs:label>
    </owl:NamedIndividual>
    


    <!-- http://semanticbible.org/ns/2006/NTNames#Kidron -->

    <owl:NamedIndividual rdf:about="http://semanticbible.org/ns/2006/NTNames#Kidron">
        <rdf:type rdf:resource="http://semanticbible.org/ns/2006/NTNames#FreshWaterArea"/>
        <rdfs:comment xml:lang="en">The Kidron Brook/Valley is just outside the walls of Jerusalem</rdfs:comment>
        <rdfs:label xml:lang="en">Kidron</rdfs:label>
    </owl:NamedIndividual>
    


    <!-- http://semanticbible.org/ns/2006/NTNames#Kish -->

    <owl:NamedIndividual rdf:about="http://semanticbible.org/ns/2006/NTNames#Kish">
        <rdf:type rdf:resource="http://semanticbible.org/ns/2006/NTNames#Man"/>
        <parentOf rdf:resource="http://semanticbible.org/ns/2006/NTNames#SaulSonOfKish"/>
        <rdfs:label xml:lang="en">Kish</rdfs:label>
    </owl:NamedIndividual>
    


    <!-- http://semanticbible.org/ns/2006/NTNames#Korah -->

    <owl:NamedIndividual rdf:about="http://semanticbible.org/ns/2006/NTNames#Korah">
        <rdf:type rdf:resource="http://semanticbible.org/ns/2006/NTNames#Man"/>
        <rdfs:label xml:lang="en">Korah</rdfs:label>
    </owl:NamedIndividual>
    


    <!-- http://semanticbible.org/ns/2006/NTNames#Lamech -->

    <owl:NamedIndividual rdf:about="http://semanticbible.org/ns/2006/NTNames#Lamech">
        <rdf:type rdf:resource="http://semanticbible.org/ns/2006/NTNames#Man"/>
        <childOf rdf:resource="http://semanticbible.org/ns/2006/NTNames#Methuselah"/>
        <parentOf rdf:resource="http://semanticbible.org/ns/2006/NTNames#Noah"/>
        <hasOnlyGenealogyMention rdf:datatype="http://www.w3.org/2001/XMLSchema#boolean">true</hasOnlyGenealogyMention>
        <rdfs:label xml:lang="en">Lamech</rdfs:label>
    </owl:NamedIndividual>
    


    <!-- http://semanticbible.org/ns/2006/NTNames#Laodicea -->

    <owl:NamedIndividual rdf:about="http://semanticbible.org/ns/2006/NTNames#Laodicea">
        <rdf:type rdf:resource="http://semanticbible.org/ns/2006/NTNames#City"/>
        <location rdf:resource="http://semanticbible.org/ns/2006/NTNames#LaodiceaGeodata"/>
        <residentPlaceOf rdf:resource="http://semanticbible.org/ns/2006/NTNames#Nympha"/>
        <rdfs:label xml:lang="en">Laodicea</rdfs:label>
    </owl:NamedIndividual>
    


    <!-- http://semanticbible.org/ns/2006/NTNames#LaodiceaGeodata -->

    <owl:NamedIndividual rdf:about="http://semanticbible.org/ns/2006/NTNames#LaodiceaGeodata">
        <rdf:type rdf:resource="http://semanticbible.org/ns/2006/NTNames#GeographicLocation"/>
        <altitude rdf:datatype="http://www.w3.org/2001/XMLSchema#int">0</altitude>
        <latitude rdf:datatype="http://www.w3.org/2001/XMLSchema#double">37.77464665610933</latitude>
        <longitude rdf:datatype="http://www.w3.org/2001/XMLSchema#double">29.09677098362944</longitude>
        <rdfs:label xml:lang="en">geodata for Laodicea</rdfs:label>
    </owl:NamedIndividual>
    


    <!-- http://semanticbible.org/ns/2006/NTNames#Laodiceans -->

    <owl:NamedIndividual rdf:about="http://semanticbible.org/ns/2006/NTNames#Laodiceans">
        <rdf:type rdf:resource="http://semanticbible.org/ns/2006/NTNames#ResidenceGroup"/>
        <rdfs:label xml:lang="en">Laodiceans</rdfs:label>
    </owl:NamedIndividual>
    


    <!-- http://semanticbible.org/ns/2006/NTNames#Lasea -->

    <owl:NamedIndividual rdf:about="http://semanticbible.org/ns/2006/NTNames#Lasea">
        <rdf:type rdf:resource="http://semanticbible.org/ns/2006/NTNames#City"/>
        <location rdf:resource="http://semanticbible.org/ns/2006/NTNames#LaseaGeodata"/>
        <rdfs:label xml:lang="en">Lasea</rdfs:label>
    </owl:NamedIndividual>
    


    <!-- http://semanticbible.org/ns/2006/NTNames#LaseaGeodata -->

    <owl:NamedIndividual rdf:about="http://semanticbible.org/ns/2006/NTNames#LaseaGeodata">
        <rdf:type rdf:resource="http://semanticbible.org/ns/2006/NTNames#GeographicLocation"/>
        <altitude rdf:datatype="http://www.w3.org/2001/XMLSchema#int">0</altitude>
        <latitude rdf:datatype="http://www.w3.org/2001/XMLSchema#double">34.93102546484152</latitude>
        <longitude rdf:datatype="http://www.w3.org/2001/XMLSchema#double">24.8056554464516</longitude>
        <rdfs:label xml:lang="en">geodata for Lasea</rdfs:label>
    </owl:NamedIndividual>
    


    <!-- http://semanticbible.org/ns/2006/NTNames#Latin -->

    <owl:NamedIndividual rdf:about="http://semanticbible.org/ns/2006/NTNames#Latin">
        <rdf:type rdf:resource="http://semanticbible.org/ns/2006/NTNames#NaturalLanguage"/>
        <rdfs:label xml:lang="en">Latin</rdfs:label>
    </owl:NamedIndividual>
    


    <!-- http://semanticbible.org/ns/2006/NTNames#Lazarus -->

    <owl:NamedIndividual rdf:about="http://semanticbible.org/ns/2006/NTNames#Lazarus">
        <rdf:type rdf:resource="http://semanticbible.org/ns/2006/NTNames#Man"/>
        <knows rdf:resource="http://semanticbible.org/ns/2006/NTNames#Jesus"/>
        <religiousBelief rdf:resource="http://semanticbible.org/ns/2006/NTNames#Christianity"/>
        <residentPlace rdf:resource="http://semanticbible.org/ns/2006/NTNames#Bethany"/>
        <siblingOf rdf:resource="http://semanticbible.org/ns/2006/NTNames#Martha"/>
        <siblingOf rdf:resource="http://semanticbible.org/ns/2006/NTNames#MaryOfBethany"/>
        <description rdf:datatype="http://www.w3.org/2001/XMLSchema#string">a man Jesus brought back to life</description>
        <rdfs:comment xml:lang="en">There&apos;s no evidence to suggest a connection between Lazarus of Bethany and the same-named subject of Jesus&apos; parable.</rdfs:comment>
        <rdfs:label xml:lang="en">Lazarus</rdfs:label>
    </owl:NamedIndividual>
    


    <!-- http://semanticbible.org/ns/2006/NTNames#Levi -->

    <owl:NamedIndividual rdf:about="http://semanticbible.org/ns/2006/NTNames#Levi">
        <rdf:type rdf:resource="http://semanticbible.org/ns/2006/NTNames#Man"/>
        <childOf rdf:resource="http://semanticbible.org/ns/2006/NTNames#AlphaeusFatherOfLevi"/>
        <collaboratesWith rdf:resource="http://semanticbible.org/ns/2006/NTNames#Andrew"/>
        <ethnicity rdf:resource="http://semanticbible.org/ns/2006/NTNames#Galilean"/>
        <siblingOf rdf:resource="http://semanticbible.org/ns/2006/NTNames#Gad"/>
        <description rdf:datatype="http://www.w3.org/2001/XMLSchema#string">One of Jesus&apos; twelve apostles</description>
        <occupation rdf:datatype="http://www.w3.org/2001/XMLSchema#string">tax collector</occupation>
        <rdfs:comment xml:lang="en">One of the Twelve, also known as Matthew. </rdfs:comment>
        <rdfs:label xml:lang="en">Levi</rdfs:label>
    </owl:NamedIndividual>
    


    <!-- http://semanticbible.org/ns/2006/NTNames#LeviSonOfMelki -->

    <owl:NamedIndividual rdf:about="http://semanticbible.org/ns/2006/NTNames#LeviSonOfMelki">
        <rdf:type rdf:resource="http://semanticbible.org/ns/2006/NTNames#Man"/>
        <childOf rdf:resource="http://semanticbible.org/ns/2006/NTNames#MelchiSonOfJannai"/>
        <ethnicity rdf:resource="http://semanticbible.org/ns/2006/NTNames#Jewish"/>
        <parentOf rdf:resource="http://semanticbible.org/ns/2006/NTNames#MatthatSonOfLeviSonOfMelki"/>
        <description rdf:datatype="http://www.w3.org/2001/XMLSchema#string">One of the ancestors of Jesus mentioned in Luke&apos;s geneaology</description>
        <hasOnlyGenealogyMention rdf:datatype="http://www.w3.org/2001/XMLSchema#boolean">true</hasOnlyGenealogyMention>
        <rdfs:label xml:lang="en">Levi</rdfs:label>
    </owl:NamedIndividual>
    


    <!-- http://semanticbible.org/ns/2006/NTNames#LeviSonOfSimeon -->

    <owl:NamedIndividual rdf:about="http://semanticbible.org/ns/2006/NTNames#LeviSonOfSimeon">
        <rdf:type rdf:resource="http://semanticbible.org/ns/2006/NTNames#Man"/>
        <childOf rdf:resource="http://semanticbible.org/ns/2006/NTNames#SimeonSonOfJudah"/>
        <ethnicity rdf:resource="http://semanticbible.org/ns/2006/NTNames#Jewish"/>
        <parentOf rdf:resource="http://semanticbible.org/ns/2006/NTNames#MatthatSonOfLeviSonOfSimeon"/>
        <description rdf:datatype="http://www.w3.org/2001/XMLSchema#string">One of the ancestors of Jesus mentioned in Luke&apos;s geneaology</description>
        <hasOnlyGenealogyMention rdf:datatype="http://www.w3.org/2001/XMLSchema#boolean">true</hasOnlyGenealogyMention>
        <rdfs:label xml:lang="en">Levi</rdfs:label>
    </owl:NamedIndividual>
    


    <!-- http://semanticbible.org/ns/2006/NTNames#Levite -->

    <owl:NamedIndividual rdf:about="http://semanticbible.org/ns/2006/NTNames#Levite">
        <rdf:type rdf:resource="http://semanticbible.org/ns/2006/NTNames#EthnicityAttribute"/>
        <ethnicityOf rdf:resource="http://semanticbible.org/ns/2006/NTNames#Abiathar"/>
        <ethnicityOf rdf:resource="http://semanticbible.org/ns/2006/NTNames#AbijahthePriest"/>
        <ethnicityOf rdf:resource="http://semanticbible.org/ns/2006/NTNames#AnaniasTheHighPriest"/>
        <ethnicityOf rdf:resource="http://semanticbible.org/ns/2006/NTNames#Barnabas"/>
        <ethnicityOf rdf:resource="http://semanticbible.org/ns/2006/NTNames#JohntheBaptist"/>
        <rdfs:comment xml:lang="en">All Levites are Jewish by definition.</rdfs:comment>
        <rdfs:label xml:lang="en">Levite</rdfs:label>
    </owl:NamedIndividual>
    


    <!-- http://semanticbible.org/ns/2006/NTNames#Levites -->

    <owl:NamedIndividual rdf:about="http://semanticbible.org/ns/2006/NTNames#Levites">
        <rdf:type rdf:resource="http://semanticbible.org/ns/2006/NTNames#ReligiousOrganization"/>
        <rdfs:comment xml:lang="en">Distinguished from Jews not by different beliefs, but by special roles related to observation of temple worship.</rdfs:comment>
        <rdfs:label xml:lang="en">Levites</rdfs:label>
    </owl:NamedIndividual>
    


    <!-- http://semanticbible.org/ns/2006/NTNames#Libya -->

    <owl:NamedIndividual rdf:about="http://semanticbible.org/ns/2006/NTNames#Libya">
        <rdf:type rdf:resource="http://semanticbible.org/ns/2006/NTNames#Region"/>
        <rdfs:label xml:lang="en">Libya</rdfs:label>
    </owl:NamedIndividual>
    


    <!-- http://semanticbible.org/ns/2006/NTNames#Linus -->

    <owl:NamedIndividual rdf:about="http://semanticbible.org/ns/2006/NTNames#Linus">
        <rdf:type rdf:resource="http://semanticbible.org/ns/2006/NTNames#Man"/>
        <rdfs:label xml:lang="en">Linus</rdfs:label>
    </owl:NamedIndividual>
    


    <!-- http://semanticbible.org/ns/2006/NTNames#Lois -->

    <owl:NamedIndividual rdf:about="http://semanticbible.org/ns/2006/NTNames#Lois">
        <rdf:type rdf:resource="http://semanticbible.org/ns/2006/NTNames#Woman"/>
        <ethnicity rdf:resource="http://semanticbible.org/ns/2006/NTNames#Jewish"/>
        <parentOf rdf:resource="http://semanticbible.org/ns/2006/NTNames#Eunice"/>
        <religiousBelief rdf:resource="http://semanticbible.org/ns/2006/NTNames#Christianity"/>
        <description rdf:datatype="http://www.w3.org/2001/XMLSchema#string">the grandmother of Timothy</description>
        <hasOnlyGenealogyMention rdf:datatype="http://www.w3.org/2001/XMLSchema#boolean">false</hasOnlyGenealogyMention>
        <rdfs:comment rdf:datatype="http://www.w3.org/2001/XMLSchema#string">Her Christian belief is implied by Paul&apos;s commendation of her faith. Her daughter Eunice lived in Lystra, but her residence is unknown. </rdfs:comment>
        <rdfs:label xml:lang="en">Lois</rdfs:label>
    </owl:NamedIndividual>
    


    <!-- http://semanticbible.org/ns/2006/NTNames#Lot -->

    <owl:NamedIndividual rdf:about="http://semanticbible.org/ns/2006/NTNames#Lot">
        <rdf:type rdf:resource="http://semanticbible.org/ns/2006/NTNames#Man"/>
        <rdfs:label xml:lang="en">Lot</rdfs:label>
    </owl:NamedIndividual>
    


    <!-- http://semanticbible.org/ns/2006/NTNames#Lucius -->

    <owl:NamedIndividual rdf:about="http://semanticbible.org/ns/2006/NTNames#Lucius">
        <rdf:type rdf:resource="http://semanticbible.org/ns/2006/NTNames#Man"/>
        <knows rdf:resource="http://semanticbible.org/ns/2006/NTNames#Jason"/>
        <knows rdf:resource="http://semanticbible.org/ns/2006/NTNames#Sosipater"/>
        <knows rdf:resource="http://semanticbible.org/ns/2006/NTNames#Timothy"/>
        <religiousBelief rdf:resource="http://semanticbible.org/ns/2006/NTNames#Christianity"/>
        <residentPlace rdf:resource="http://semanticbible.org/ns/2006/NTNames#Corinth"/>
        <description rdf:datatype="http://www.w3.org/2001/XMLSchema#string">a companion of Paul&apos;s who sent greetings to the Roman church</description>
        <hasOnlyGenealogyMention rdf:datatype="http://www.w3.org/2001/XMLSchema#boolean">false</hasOnlyGenealogyMention>
        <rdfs:comment rdf:datatype="http://www.w3.org/2001/XMLSchema#string">This person may be the same as Lucius of Cyrene, but there&apos;s no clear evidence other than the name. His residence in Corinth follows from the inference that Paul resided there when he wrote the letter to the Roman church.  &quot;kinsman&quot; here probably means that that he is a Jew, rather than an actual relation, given the number of people so designated in Romans 16. </rdfs:comment>
        <rdfs:label xml:lang="en">Lucius</rdfs:label>
    </owl:NamedIndividual>
    


    <!-- http://semanticbible.org/ns/2006/NTNames#LuciusOfCyrene -->

    <owl:NamedIndividual rdf:about="http://semanticbible.org/ns/2006/NTNames#LuciusOfCyrene">
        <rdf:type rdf:resource="http://semanticbible.org/ns/2006/NTNames#Man"/>
        <collaboratesWith rdf:resource="http://semanticbible.org/ns/2006/NTNames#Barnabas"/>
        <collaboratesWith rdf:resource="http://semanticbible.org/ns/2006/NTNames#Manaen"/>
        <collaboratesWith rdf:resource="http://semanticbible.org/ns/2006/NTNames#Paul"/>
        <collaboratesWith rdf:resource="http://semanticbible.org/ns/2006/NTNames#SimeonNiger"/>
        <description rdf:datatype="http://www.w3.org/2001/XMLSchema#string">a Christian leader in Antioch</description>
        <rdfs:comment rdf:datatype="http://www.w3.org/2001/XMLSchema#string">This person may be the same as the Lucius in Rome, but there&apos;s no clear evidence other than the name.</rdfs:comment>
        <rdfs:label xml:lang="en">Lucius</rdfs:label>
    </owl:NamedIndividual>
    


    <!-- http://semanticbible.org/ns/2006/NTNames#Luke -->

    <owl:NamedIndividual rdf:about="http://semanticbible.org/ns/2006/NTNames#Luke">
        <rdf:type rdf:resource="http://semanticbible.org/ns/2006/NTNames#Man"/>
        <rdfs:label xml:lang="en">Luke</rdfs:label>
    </owl:NamedIndividual>
    


    <!-- http://semanticbible.org/ns/2006/NTNames#Lycaonia -->

    <owl:NamedIndividual rdf:about="http://semanticbible.org/ns/2006/NTNames#Lycaonia">
        <rdf:type rdf:resource="http://semanticbible.org/ns/2006/NTNames#StateOrProvince"/>
        <rdfs:label xml:lang="en">Lycaonia</rdfs:label>
    </owl:NamedIndividual>
    


    <!-- http://semanticbible.org/ns/2006/NTNames#Lycaonian -->

    <owl:NamedIndividual rdf:about="http://semanticbible.org/ns/2006/NTNames#Lycaonian">
        <rdf:type rdf:resource="http://semanticbible.org/ns/2006/NTNames#NaturalLanguage"/>
        <rdfs:label xml:lang="en">Lycaonian</rdfs:label>
    </owl:NamedIndividual>
    


    <!-- http://semanticbible.org/ns/2006/NTNames#Lycia -->

    <owl:NamedIndividual rdf:about="http://semanticbible.org/ns/2006/NTNames#Lycia">
        <rdf:type rdf:resource="http://semanticbible.org/ns/2006/NTNames#StateOrProvince"/>
        <rdfs:label xml:lang="en">Lycia</rdfs:label>
    </owl:NamedIndividual>
    


    <!-- http://semanticbible.org/ns/2006/NTNames#Lydda -->

    <owl:NamedIndividual rdf:about="http://semanticbible.org/ns/2006/NTNames#Lydda">
        <rdf:type rdf:resource="http://semanticbible.org/ns/2006/NTNames#City"/>
        <location rdf:resource="http://semanticbible.org/ns/2006/NTNames#LyddaGeodata"/>
        <subregionOf rdf:resource="http://semanticbible.org/ns/2006/NTNames#Judea"/>
        <rdfs:label xml:lang="en">Lydda</rdfs:label>
    </owl:NamedIndividual>
    


    <!-- http://semanticbible.org/ns/2006/NTNames#LyddaGeodata -->

    <owl:NamedIndividual rdf:about="http://semanticbible.org/ns/2006/NTNames#LyddaGeodata">
        <rdf:type rdf:resource="http://semanticbible.org/ns/2006/NTNames#GeographicLocation"/>
        <altitude rdf:datatype="http://www.w3.org/2001/XMLSchema#int">0</altitude>
        <latitude rdf:datatype="http://www.w3.org/2001/XMLSchema#double">31.98583717588782</latitude>
        <longitude rdf:datatype="http://www.w3.org/2001/XMLSchema#double">34.89443039056358</longitude>
        <rdfs:label xml:lang="en">geodata for Lydda</rdfs:label>
    </owl:NamedIndividual>
    


    <!-- http://semanticbible.org/ns/2006/NTNames#Lydia -->

    <owl:NamedIndividual rdf:about="http://semanticbible.org/ns/2006/NTNames#Lydia">
        <rdf:type rdf:resource="http://semanticbible.org/ns/2006/NTNames#Woman"/>
        <collaboratesWith rdf:resource="http://semanticbible.org/ns/2006/NTNames#Paul"/>
        <nativePlace rdf:resource="http://semanticbible.org/ns/2006/NTNames#Thyatira"/>
        <religiousBelief rdf:resource="http://semanticbible.org/ns/2006/NTNames#Christianity"/>
        <visitedPlace rdf:resource="http://semanticbible.org/ns/2006/NTNames#Philippi"/>
        <description rdf:datatype="http://www.w3.org/2001/XMLSchema#string">a convert from Paul&apos;s preaching in Philippi</description>
        <hasOnlyGenealogyMention rdf:datatype="http://www.w3.org/2001/XMLSchema#boolean">false</hasOnlyGenealogyMention>
        <occupation rdf:datatype="http://www.w3.org/2001/XMLSchema#string">seller of purple goods</occupation>
        <rdfs:label xml:lang="en">Lydia</rdfs:label>
    </owl:NamedIndividual>
    


    <!-- http://semanticbible.org/ns/2006/NTNames#Lysanias -->

    <owl:NamedIndividual rdf:about="http://semanticbible.org/ns/2006/NTNames#Lysanias">
        <rdf:type rdf:resource="http://semanticbible.org/ns/2006/NTNames#Man"/>
        <rdfs:label xml:lang="en">Lysanias</rdfs:label>
    </owl:NamedIndividual>
    


    <!-- http://semanticbible.org/ns/2006/NTNames#Lysias -->

    <owl:NamedIndividual rdf:about="http://semanticbible.org/ns/2006/NTNames#Lysias">
        <rdf:type rdf:resource="http://semanticbible.org/ns/2006/NTNames#Man"/>
        <rdfs:label xml:lang="en">Lysias</rdfs:label>
    </owl:NamedIndividual>
    


    <!-- http://semanticbible.org/ns/2006/NTNames#Lystra -->

    <owl:NamedIndividual rdf:about="http://semanticbible.org/ns/2006/NTNames#Lystra">
        <rdf:type rdf:resource="http://semanticbible.org/ns/2006/NTNames#City"/>
        <location rdf:resource="http://semanticbible.org/ns/2006/NTNames#LystraGeodata"/>
        <residentPlaceOf rdf:resource="http://semanticbible.org/ns/2006/NTNames#Eunice"/>
        <rdfs:label xml:lang="en">Lystra</rdfs:label>
    </owl:NamedIndividual>
    


    <!-- http://semanticbible.org/ns/2006/NTNames#LystraGeodata -->

    <owl:NamedIndividual rdf:about="http://semanticbible.org/ns/2006/NTNames#LystraGeodata">
        <rdf:type rdf:resource="http://semanticbible.org/ns/2006/NTNames#GeographicLocation"/>
        <altitude rdf:datatype="http://www.w3.org/2001/XMLSchema#int">0</altitude>
        <latitude rdf:datatype="http://www.w3.org/2001/XMLSchema#double">37.60127988966087</latitude>
        <longitude rdf:datatype="http://www.w3.org/2001/XMLSchema#double">32.44677760633329</longitude>
        <rdfs:label xml:lang="en">geodata for Lystra</rdfs:label>
    </owl:NamedIndividual>
    


    <!-- http://semanticbible.org/ns/2006/NTNames#Maath -->

    <owl:NamedIndividual rdf:about="http://semanticbible.org/ns/2006/NTNames#Maath">
        <rdf:type rdf:resource="http://semanticbible.org/ns/2006/NTNames#Man"/>
        <childOf rdf:resource="http://semanticbible.org/ns/2006/NTNames#MattathiasSonOfSemein"/>
        <ethnicity rdf:resource="http://semanticbible.org/ns/2006/NTNames#Jewish"/>
        <parentOf rdf:resource="http://semanticbible.org/ns/2006/NTNames#Naggai"/>
        <description rdf:datatype="http://www.w3.org/2001/XMLSchema#string">One of the ancestors of Jesus mentioned in Luke&apos;s geneaology</description>
        <hasOnlyGenealogyMention rdf:datatype="http://www.w3.org/2001/XMLSchema#boolean">true</hasOnlyGenealogyMention>
        <rdfs:label xml:lang="en">Maath</rdfs:label>
    </owl:NamedIndividual>
    


    <!-- http://semanticbible.org/ns/2006/NTNames#Macedonia -->

    <owl:NamedIndividual rdf:about="http://semanticbible.org/ns/2006/NTNames#Macedonia">
        <rdf:type rdf:resource="http://semanticbible.org/ns/2006/NTNames#StateOrProvince"/>
        <subregion rdf:resource="http://semanticbible.org/ns/2006/NTNames#Amphipolis"/>
        <subregion rdf:resource="http://semanticbible.org/ns/2006/NTNames#Apollonia"/>
        <subregion rdf:resource="http://semanticbible.org/ns/2006/NTNames#Berea"/>
        <subregion rdf:resource="http://semanticbible.org/ns/2006/NTNames#Thessalonica"/>
        <visitedPlaceOf rdf:resource="http://semanticbible.org/ns/2006/NTNames#Erastus"/>
        <rdfs:label xml:lang="en">Macedonia</rdfs:label>
    </owl:NamedIndividual>
    


    <!-- http://semanticbible.org/ns/2006/NTNames#Macedonian -->

    <owl:NamedIndividual rdf:about="http://semanticbible.org/ns/2006/NTNames#Macedonian">
        <rdf:type rdf:resource="http://semanticbible.org/ns/2006/NTNames#EthnicityAttribute"/>
        <ethnicityOf rdf:resource="http://semanticbible.org/ns/2006/NTNames#Aristarchus"/>
        <ethnicityOf rdf:resource="http://semanticbible.org/ns/2006/NTNames#GaiusOfMacedonia"/>
        <rdfs:comment xml:lang="en">Of the region of Macedonia (and therefore also Greek).</rdfs:comment>
        <rdfs:label xml:lang="en">Macedonian</rdfs:label>
    </owl:NamedIndividual>
    


    <!-- http://semanticbible.org/ns/2006/NTNames#Macedonians -->

    <owl:NamedIndividual rdf:about="http://semanticbible.org/ns/2006/NTNames#Macedonians">
        <rdf:type rdf:resource="http://semanticbible.org/ns/2006/NTNames#ResidenceGroup"/>
        <rdfs:label xml:lang="en">Macedonians</rdfs:label>
    </owl:NamedIndividual>
    


    <!-- http://semanticbible.org/ns/2006/NTNames#Magadan -->

    <owl:NamedIndividual rdf:about="http://semanticbible.org/ns/2006/NTNames#Magadan">
        <rdf:type rdf:resource="http://semanticbible.org/ns/2006/NTNames#City"/>
        <rdfs:label xml:lang="en">Magadan</rdfs:label>
    </owl:NamedIndividual>
    


    <!-- http://semanticbible.org/ns/2006/NTNames#Magog -->

    <owl:NamedIndividual rdf:about="http://semanticbible.org/ns/2006/NTNames#Magog">
        <rdf:type rdf:resource="http://semanticbible.org/ns/2006/NTNames#GroupOfPeople"/>
        <description rdf:datatype="http://www.w3.org/2001/XMLSchema#string">an apocalyptic opponent of God&apos;s people</description>
        <hasOnlyGenealogyMention rdf:datatype="http://www.w3.org/2001/XMLSchema#boolean">false</hasOnlyGenealogyMention>
        <rdfs:comment rdf:datatype="http://www.w3.org/2001/XMLSchema#string">Though in its original Old Testament context Magog  referred to a region, its New Testament usage seems to describe a group of people. </rdfs:comment>
        <rdfs:label xml:lang="en">Magog</rdfs:label>
    </owl:NamedIndividual>
    


    <!-- http://semanticbible.org/ns/2006/NTNames#Mahalaleel -->

    <owl:NamedIndividual rdf:about="http://semanticbible.org/ns/2006/NTNames#Mahalaleel">
        <rdf:type rdf:resource="http://semanticbible.org/ns/2006/NTNames#Man"/>
        <childOf rdf:resource="http://semanticbible.org/ns/2006/NTNames#CainanSonOfEnosh"/>
        <parentOf rdf:resource="http://semanticbible.org/ns/2006/NTNames#Jared"/>
        <description rdf:datatype="http://www.w3.org/2001/XMLSchema#string">One of the ancestors of Jesus mentioned in Luke&apos;s geneaology</description>
        <hasOnlyGenealogyMention rdf:datatype="http://www.w3.org/2001/XMLSchema#boolean">true</hasOnlyGenealogyMention>
        <rdfs:label xml:lang="en">Mahalaleel</rdfs:label>
    </owl:NamedIndividual>
    


    <!-- http://semanticbible.org/ns/2006/NTNames#Malchus -->

    <owl:NamedIndividual rdf:about="http://semanticbible.org/ns/2006/NTNames#Malchus">
        <rdf:type rdf:resource="http://semanticbible.org/ns/2006/NTNames#Man"/>
        <rdfs:label xml:lang="en">Malchus</rdfs:label>
    </owl:NamedIndividual>
    


    <!-- http://semanticbible.org/ns/2006/NTNames#Malta -->

    <owl:NamedIndividual rdf:about="http://semanticbible.org/ns/2006/NTNames#Malta">
        <rdf:type rdf:resource="http://semanticbible.org/ns/2006/NTNames#Island"/>
        <location rdf:resource="http://semanticbible.org/ns/2006/NTNames#MaltaGeodata"/>
        <rdfs:label xml:lang="en">Malta</rdfs:label>
    </owl:NamedIndividual>
    


    <!-- http://semanticbible.org/ns/2006/NTNames#MaltaGeodata -->

    <owl:NamedIndividual rdf:about="http://semanticbible.org/ns/2006/NTNames#MaltaGeodata">
        <rdf:type rdf:resource="http://semanticbible.org/ns/2006/NTNames#GeographicLocation"/>
        <altitude rdf:datatype="http://www.w3.org/2001/XMLSchema#int">0</altitude>
        <latitude rdf:datatype="http://www.w3.org/2001/XMLSchema#double">35.85282675242785</latitude>
        <longitude rdf:datatype="http://www.w3.org/2001/XMLSchema#double">14.53243601407711</longitude>
        <rdfs:label xml:lang="en">geodata for Malta</rdfs:label>
    </owl:NamedIndividual>
    


    <!-- http://semanticbible.org/ns/2006/NTNames#Manaen -->

    <owl:NamedIndividual rdf:about="http://semanticbible.org/ns/2006/NTNames#Manaen">
        <rdf:type rdf:resource="http://semanticbible.org/ns/2006/NTNames#Man"/>
        <collaboratesWith rdf:resource="http://semanticbible.org/ns/2006/NTNames#Barnabas"/>
        <collaboratesWith rdf:resource="http://semanticbible.org/ns/2006/NTNames#LuciusOfCyrene"/>
        <collaboratesWith rdf:resource="http://semanticbible.org/ns/2006/NTNames#Paul"/>
        <collaboratesWith rdf:resource="http://semanticbible.org/ns/2006/NTNames#SimeonNiger"/>
        <knows rdf:resource="http://semanticbible.org/ns/2006/NTNames#HerodAntipas"/>
        <description rdf:datatype="http://www.w3.org/2001/XMLSchema#string">a Christian leader at Antioch</description>
        <rdfs:comment rdf:datatype="http://www.w3.org/2001/XMLSchema#string">The term translated &quot;foster-brother&quot; means Manaen and Herod Antipas were raised together, though not literally relatives.</rdfs:comment>
        <rdfs:label xml:lang="en">Manaen</rdfs:label>
    </owl:NamedIndividual>
    


    <!-- http://semanticbible.org/ns/2006/NTNames#Manasseh -->

    <owl:NamedIndividual rdf:about="http://semanticbible.org/ns/2006/NTNames#Manasseh">
        <rdf:type rdf:resource="http://semanticbible.org/ns/2006/NTNames#Man"/>
        <childOf rdf:resource="http://semanticbible.org/ns/2006/NTNames#Hezekiah"/>
        <ethnicity rdf:resource="http://semanticbible.org/ns/2006/NTNames#Jewish"/>
        <parentOf rdf:resource="http://semanticbible.org/ns/2006/NTNames#Amos"/>
        <rdfs:label xml:lang="en">Manasseh</rdfs:label>
    </owl:NamedIndividual>
    


    <!-- http://semanticbible.org/ns/2006/NTNames#ManassehThePatriarch -->

    <owl:NamedIndividual rdf:about="http://semanticbible.org/ns/2006/NTNames#ManassehThePatriarch">
        <rdf:type rdf:resource="http://semanticbible.org/ns/2006/NTNames#Man"/>
        <childOf rdf:resource="http://semanticbible.org/ns/2006/NTNames#Jacob"/>
        <ethnicity rdf:resource="http://semanticbible.org/ns/2006/NTNames#Jewish"/>
        <siblingOf rdf:resource="http://semanticbible.org/ns/2006/NTNames#Gad"/>
        <rdfs:label xml:lang="en">Manasseh</rdfs:label>
    </owl:NamedIndividual>
    


    <!-- http://semanticbible.org/ns/2006/NTNames#Martha -->

    <owl:NamedIndividual rdf:about="http://semanticbible.org/ns/2006/NTNames#Martha">
        <rdf:type rdf:resource="http://semanticbible.org/ns/2006/NTNames#Woman"/>
        <ethnicity rdf:resource="http://semanticbible.org/ns/2006/NTNames#Jewish"/>
        <knows rdf:resource="http://semanticbible.org/ns/2006/NTNames#Jesus"/>
        <religiousBelief rdf:resource="http://semanticbible.org/ns/2006/NTNames#Christianity"/>
        <residentPlace rdf:resource="http://semanticbible.org/ns/2006/NTNames#Bethany"/>
        <siblingOf rdf:resource="http://semanticbible.org/ns/2006/NTNames#Lazarus"/>
        <siblingOf rdf:resource="http://semanticbible.org/ns/2006/NTNames#MaryOfBethany"/>
        <description rdf:datatype="http://www.w3.org/2001/XMLSchema#string">the sister of Lazarus and Mary who annointed Jesus before his death</description>
        <hasOnlyGenealogyMention rdf:datatype="http://www.w3.org/2001/XMLSchema#boolean">false</hasOnlyGenealogyMention>
        <rdfs:label xml:lang="en">Martha</rdfs:label>
    </owl:NamedIndividual>
    


    <!-- http://semanticbible.org/ns/2006/NTNames#Mary -->

    <owl:NamedIndividual rdf:about="http://semanticbible.org/ns/2006/NTNames#Mary">
        <rdf:type rdf:resource="http://semanticbible.org/ns/2006/NTNames#Woman"/>
        <ethnicity rdf:resource="http://semanticbible.org/ns/2006/NTNames#Jewish"/>
        <knows rdf:resource="http://semanticbible.org/ns/2006/NTNames#JohnSonOfZebedee"/>
        <knows rdf:resource="http://semanticbible.org/ns/2006/NTNames#MaryMagdalene"/>
        <parentOf rdf:resource="http://semanticbible.org/ns/2006/NTNames#Jesus"/>
        <relativeOf rdf:resource="http://semanticbible.org/ns/2006/NTNames#Elizabeth"/>
        <religiousBelief rdf:resource="http://semanticbible.org/ns/2006/NTNames#Christianity"/>
        <residentPlace rdf:resource="http://semanticbible.org/ns/2006/NTNames#Egypt"/>
        <residentPlace rdf:resource="http://semanticbible.org/ns/2006/NTNames#Nazareth"/>
        <siblingOf rdf:resource="http://semanticbible.org/ns/2006/NTNames#MaryWifeOfClopas"/>
        <spouseOf rdf:resource="http://semanticbible.org/ns/2006/NTNames#Joseph"/>
        <visitedPlace rdf:resource="http://semanticbible.org/ns/2006/NTNames#Bethlehem"/>
        <visitedPlace rdf:resource="http://semanticbible.org/ns/2006/NTNames#Cana"/>
        <visitedPlace rdf:resource="http://semanticbible.org/ns/2006/NTNames#Jerusalem"/>
        <description rdf:datatype="http://www.w3.org/2001/XMLSchema#string">the mother of Jesus</description>
        <hasOnlyGenealogyMention rdf:datatype="http://www.w3.org/2001/XMLSchema#boolean">false</hasOnlyGenealogyMention>
        <rdfs:comment xml:lang="en">See the note on Joseph for why Mary is childOf Heli. She is described by John as standing at the foot of Jesus&apos; cross with two other Marys. Her relationship to John assumes he is the &quot;beloved discipled&quot; described in John&apos;s gospel. </rdfs:comment>
        <rdfs:label xml:lang="en">Mary</rdfs:label>
    </owl:NamedIndividual>
    


    <!-- http://semanticbible.org/ns/2006/NTNames#MaryMagdalene -->

    <owl:NamedIndividual rdf:about="http://semanticbible.org/ns/2006/NTNames#MaryMagdalene">
        <rdf:type rdf:resource="http://semanticbible.org/ns/2006/NTNames#Woman"/>
        <collaboratesWith rdf:resource="http://semanticbible.org/ns/2006/NTNames#Jesus"/>
        <collaboratesWith rdf:resource="http://semanticbible.org/ns/2006/NTNames#JohnSonOfZebedee"/>
        <collaboratesWith rdf:resource="http://semanticbible.org/ns/2006/NTNames#SimonPeter"/>
        <ethnicity rdf:resource="http://semanticbible.org/ns/2006/NTNames#Jewish"/>
        <knows rdf:resource="http://semanticbible.org/ns/2006/NTNames#Mary"/>
        <knows rdf:resource="http://semanticbible.org/ns/2006/NTNames#MaryWifeOfClopas"/>
        <knows rdf:resource="http://semanticbible.org/ns/2006/NTNames#Salome"/>
        <knows rdf:resource="http://semanticbible.org/ns/2006/NTNames#Susanna"/>
        <religiousBelief rdf:resource="http://semanticbible.org/ns/2006/NTNames#Christianity"/>
        <residentPlace rdf:resource="http://semanticbible.org/ns/2006/NTNames#Galilee"/>
        <description rdf:datatype="http://www.w3.org/2001/XMLSchema#string">A woman from whom seven demons had been exorcised</description>
        <hasOnlyGenealogyMention rdf:datatype="http://www.w3.org/2001/XMLSchema#boolean">false</hasOnlyGenealogyMention>
        <rdfs:comment xml:lang="en">From Magdala, a town in Galilee not mentioned in the New Testament</rdfs:comment>
        <rdfs:label xml:lang="en">Mary Magdalene</rdfs:label>
    </owl:NamedIndividual>
    


    <!-- http://semanticbible.org/ns/2006/NTNames#MaryMotherOfJohnMark -->

    <owl:NamedIndividual rdf:about="http://semanticbible.org/ns/2006/NTNames#MaryMotherOfJohnMark">
        <rdf:type rdf:resource="http://semanticbible.org/ns/2006/NTNames#Woman"/>
        <ethnicity rdf:resource="http://semanticbible.org/ns/2006/NTNames#Jewish"/>
        <knows rdf:resource="http://semanticbible.org/ns/2006/NTNames#Rhoda"/>
        <parentOf rdf:resource="http://semanticbible.org/ns/2006/NTNames#JohnMark"/>
        <religiousBelief rdf:resource="http://semanticbible.org/ns/2006/NTNames#Christianity"/>
        <residentPlace rdf:resource="http://semanticbible.org/ns/2006/NTNames#Jerusalem"/>
        <siblingOf rdf:resource="http://semanticbible.org/ns/2006/NTNames#Barnabas"/>
        <description rdf:datatype="http://www.w3.org/2001/XMLSchema#string">a woman to whose house Peter came after his release from prison</description>
        <hasOnlyGenealogyMention rdf:datatype="http://www.w3.org/2001/XMLSchema#boolean">false</hasOnlyGenealogyMention>
        <rdfs:label xml:lang="en">Mary</rdfs:label>
    </owl:NamedIndividual>
    


    <!-- http://semanticbible.org/ns/2006/NTNames#MaryOfBethany -->

    <owl:NamedIndividual rdf:about="http://semanticbible.org/ns/2006/NTNames#MaryOfBethany">
        <rdf:type rdf:resource="http://semanticbible.org/ns/2006/NTNames#Woman"/>
        <ethnicity rdf:resource="http://semanticbible.org/ns/2006/NTNames#Jewish"/>
        <knows rdf:resource="http://semanticbible.org/ns/2006/NTNames#Jesus"/>
        <religiousBelief rdf:resource="http://semanticbible.org/ns/2006/NTNames#Christianity"/>
        <residentPlace rdf:resource="http://semanticbible.org/ns/2006/NTNames#Bethany"/>
        <siblingOf rdf:resource="http://semanticbible.org/ns/2006/NTNames#Lazarus"/>
        <siblingOf rdf:resource="http://semanticbible.org/ns/2006/NTNames#Martha"/>
        <description rdf:datatype="http://www.w3.org/2001/XMLSchema#string">a follower of Jesus who annointed him late in his ministry</description>
        <hasOnlyGenealogyMention rdf:datatype="http://www.w3.org/2001/XMLSchema#boolean">false</hasOnlyGenealogyMention>
        <rdfs:comment rdf:datatype="http://www.w3.org/2001/XMLSchema#string">There are other accounts of an unnamed woman annointing Jesus with oil, and various arguments about whether these were the same or different women. </rdfs:comment>
        <rdfs:label xml:lang="en">Mary</rdfs:label>
    </owl:NamedIndividual>
    


    <!-- http://semanticbible.org/ns/2006/NTNames#MaryOfRome -->

    <owl:NamedIndividual rdf:about="http://semanticbible.org/ns/2006/NTNames#MaryOfRome">
        <rdf:type rdf:resource="http://semanticbible.org/ns/2006/NTNames#Woman"/>
        <knows rdf:resource="http://semanticbible.org/ns/2006/NTNames#Paul"/>
        <knows rdf:resource="http://semanticbible.org/ns/2006/NTNames#Priscilla"/>
        <religiousBelief rdf:resource="http://semanticbible.org/ns/2006/NTNames#Christianity"/>
        <residentPlace rdf:resource="http://semanticbible.org/ns/2006/NTNames#Rome"/>
        <description rdf:datatype="http://www.w3.org/2001/XMLSchema#string">a woman to whom Paul sent greetings in his letter to the Romans</description>
        <hasOnlyGenealogyMention rdf:datatype="http://www.w3.org/2001/XMLSchema#boolean">false</hasOnlyGenealogyMention>
        <rdfs:label xml:lang="en">Mary</rdfs:label>
    </owl:NamedIndividual>
    


    <!-- http://semanticbible.org/ns/2006/NTNames#MaryWifeOfClopas -->

    <owl:NamedIndividual rdf:about="http://semanticbible.org/ns/2006/NTNames#MaryWifeOfClopas">
        <rdf:type rdf:resource="http://semanticbible.org/ns/2006/NTNames#Woman"/>
        <collaboratesWith rdf:resource="http://semanticbible.org/ns/2006/NTNames#Jesus"/>
        <ethnicity rdf:resource="http://semanticbible.org/ns/2006/NTNames#Jewish"/>
        <knows rdf:resource="http://semanticbible.org/ns/2006/NTNames#MaryMagdalene"/>
        <knows rdf:resource="http://semanticbible.org/ns/2006/NTNames#Salome"/>
        <religiousBelief rdf:resource="http://semanticbible.org/ns/2006/NTNames#Christianity"/>
        <siblingOf rdf:resource="http://semanticbible.org/ns/2006/NTNames#Mary"/>
        <spouseOf rdf:resource="http://semanticbible.org/ns/2006/NTNames#Alphaeus"/>
        <description rdf:datatype="http://www.w3.org/2001/XMLSchema#string">A follower of Jesus who was present at the crucifixion</description>
        <hasOnlyGenealogyMention rdf:datatype="http://www.w3.org/2001/XMLSchema#boolean">false</hasOnlyGenealogyMention>
        <rdfs:comment xml:lang="en">Comparing the Gospel accounts in John.19.25 and Mark.15.40, this Mary appears to be the same woman as the mother of James and Joseph/Joses, and therefore sister of Mary the mother of Jesus.</rdfs:comment>
        <rdfs:label xml:lang="en">Mary</rdfs:label>
    </owl:NamedIndividual>
    


    <!-- http://semanticbible.org/ns/2006/NTNames#Mattatha -->

    <owl:NamedIndividual rdf:about="http://semanticbible.org/ns/2006/NTNames#Mattatha">
        <rdf:type rdf:resource="http://semanticbible.org/ns/2006/NTNames#Man"/>
        <childOf rdf:resource="http://semanticbible.org/ns/2006/NTNames#Nathan"/>
        <ethnicity rdf:resource="http://semanticbible.org/ns/2006/NTNames#Jewish"/>
        <parentOf rdf:resource="http://semanticbible.org/ns/2006/NTNames#Menna"/>
        <description rdf:datatype="http://www.w3.org/2001/XMLSchema#string">One of the ancestors of Jesus mentioned in Luke&apos;s geneaology</description>
        <hasOnlyGenealogyMention rdf:datatype="http://www.w3.org/2001/XMLSchema#boolean">true</hasOnlyGenealogyMention>
        <rdfs:label xml:lang="en">Mattatha</rdfs:label>
    </owl:NamedIndividual>
    


    <!-- http://semanticbible.org/ns/2006/NTNames#MattathaisSonOfAmos -->

    <owl:NamedIndividual rdf:about="http://semanticbible.org/ns/2006/NTNames#MattathaisSonOfAmos">
        <rdf:type rdf:resource="http://semanticbible.org/ns/2006/NTNames#Man"/>
        <childOf rdf:resource="http://semanticbible.org/ns/2006/NTNames#AmosSonOfNahum"/>
        <ethnicity rdf:resource="http://semanticbible.org/ns/2006/NTNames#Jewish"/>
        <parentOf rdf:resource="http://semanticbible.org/ns/2006/NTNames#JosephSonOfMattathias"/>
        <description rdf:datatype="http://www.w3.org/2001/XMLSchema#string">One of the ancestors of Jesus mentioned in Luke&apos;s geneaology</description>
        <hasOnlyGenealogyMention rdf:datatype="http://www.w3.org/2001/XMLSchema#boolean">true</hasOnlyGenealogyMention>
        <rdfs:label xml:lang="en">Mattathias</rdfs:label>
    </owl:NamedIndividual>
    


    <!-- http://semanticbible.org/ns/2006/NTNames#MattathiasSonOfSemein -->

    <owl:NamedIndividual rdf:about="http://semanticbible.org/ns/2006/NTNames#MattathiasSonOfSemein">
        <rdf:type rdf:resource="http://semanticbible.org/ns/2006/NTNames#Man"/>
        <childOf rdf:resource="http://semanticbible.org/ns/2006/NTNames#Semein"/>
        <ethnicity rdf:resource="http://semanticbible.org/ns/2006/NTNames#Jewish"/>
        <parentOf rdf:resource="http://semanticbible.org/ns/2006/NTNames#Maath"/>
        <description rdf:datatype="http://www.w3.org/2001/XMLSchema#string">One of the ancestors of Jesus mentioned in Luke&apos;s geneaology</description>
        <hasOnlyGenealogyMention rdf:datatype="http://www.w3.org/2001/XMLSchema#boolean">true</hasOnlyGenealogyMention>
        <rdfs:label xml:lang="en">Mattathias</rdfs:label>
    </owl:NamedIndividual>
    


    <!-- http://semanticbible.org/ns/2006/NTNames#Matthan -->

    <owl:NamedIndividual rdf:about="http://semanticbible.org/ns/2006/NTNames#Matthan">
        <rdf:type rdf:resource="http://semanticbible.org/ns/2006/NTNames#Man"/>
        <childOf rdf:resource="http://semanticbible.org/ns/2006/NTNames#Eleazar"/>
        <parentOf rdf:resource="http://semanticbible.org/ns/2006/NTNames#JacobSonOfMatthan"/>
        <description rdf:datatype="http://www.w3.org/2001/XMLSchema#string">One of the ancestors of Jesus mentioned in Matthew&apos;s geneaology</description>
        <rdfs:label xml:lang="en">Matthan</rdfs:label>
    </owl:NamedIndividual>
    


    <!-- http://semanticbible.org/ns/2006/NTNames#MatthatSonOfLeviSonOfMelki -->

    <owl:NamedIndividual rdf:about="http://semanticbible.org/ns/2006/NTNames#MatthatSonOfLeviSonOfMelki">
        <rdf:type rdf:resource="http://semanticbible.org/ns/2006/NTNames#Man"/>
        <childOf rdf:resource="http://semanticbible.org/ns/2006/NTNames#LeviSonOfMelki"/>
        <ethnicity rdf:resource="http://semanticbible.org/ns/2006/NTNames#Jewish"/>
        <parentOf rdf:resource="http://semanticbible.org/ns/2006/NTNames#Heli"/>
        <hasOnlyGenealogyMention rdf:datatype="http://www.w3.org/2001/XMLSchema#boolean">true</hasOnlyGenealogyMention>
        <rdfs:label xml:lang="en">Matthat</rdfs:label>
    </owl:NamedIndividual>
    


    <!-- http://semanticbible.org/ns/2006/NTNames#MatthatSonOfLeviSonOfSimeon -->

    <owl:NamedIndividual rdf:about="http://semanticbible.org/ns/2006/NTNames#MatthatSonOfLeviSonOfSimeon">
        <rdf:type rdf:resource="http://semanticbible.org/ns/2006/NTNames#Man"/>
        <childOf rdf:resource="http://semanticbible.org/ns/2006/NTNames#LeviSonOfSimeon"/>
        <ethnicity rdf:resource="http://semanticbible.org/ns/2006/NTNames#Jewish"/>
        <parentOf rdf:resource="http://semanticbible.org/ns/2006/NTNames#Jorim"/>
        <hasOnlyGenealogyMention rdf:datatype="http://www.w3.org/2001/XMLSchema#boolean">true</hasOnlyGenealogyMention>
        <rdfs:label xml:lang="en">Matthat</rdfs:label>
    </owl:NamedIndividual>
    


    <!-- http://semanticbible.org/ns/2006/NTNames#Matthias -->

    <owl:NamedIndividual rdf:about="http://semanticbible.org/ns/2006/NTNames#Matthias">
        <rdf:type rdf:resource="http://semanticbible.org/ns/2006/NTNames#Man"/>
        <rdfs:label xml:lang="en">Matthias</rdfs:label>
    </owl:NamedIndividual>
    


    <!-- http://semanticbible.org/ns/2006/NTNames#Medes -->

    <owl:NamedIndividual rdf:about="http://semanticbible.org/ns/2006/NTNames#Medes">
        <rdf:type rdf:resource="http://semanticbible.org/ns/2006/NTNames#EthnicGroup"/>
        <rdfs:label xml:lang="en">Medes</rdfs:label>
    </owl:NamedIndividual>
    


    <!-- http://semanticbible.org/ns/2006/NTNames#MelchiSonOfAddi -->

    <owl:NamedIndividual rdf:about="http://semanticbible.org/ns/2006/NTNames#MelchiSonOfAddi">
        <rdf:type rdf:resource="http://semanticbible.org/ns/2006/NTNames#Man"/>
        <childOf rdf:resource="http://semanticbible.org/ns/2006/NTNames#Addi"/>
        <ethnicity rdf:resource="http://semanticbible.org/ns/2006/NTNames#Jewish"/>
        <parentOf rdf:resource="http://semanticbible.org/ns/2006/NTNames#Neri"/>
        <description rdf:datatype="http://www.w3.org/2001/XMLSchema#string">One of the ancestors of Jesus mentioned in Luke&apos;s geneaology</description>
        <hasOnlyGenealogyMention rdf:datatype="http://www.w3.org/2001/XMLSchema#boolean">true</hasOnlyGenealogyMention>
        <rdfs:label xml:lang="en">Melchi</rdfs:label>
    </owl:NamedIndividual>
    


    <!-- http://semanticbible.org/ns/2006/NTNames#MelchiSonOfJannai -->

    <owl:NamedIndividual rdf:about="http://semanticbible.org/ns/2006/NTNames#MelchiSonOfJannai">
        <rdf:type rdf:resource="http://semanticbible.org/ns/2006/NTNames#Man"/>
        <childOf rdf:resource="http://semanticbible.org/ns/2006/NTNames#Jannai"/>
        <ethnicity rdf:resource="http://semanticbible.org/ns/2006/NTNames#Jewish"/>
        <parentOf rdf:resource="http://semanticbible.org/ns/2006/NTNames#LeviSonOfMelki"/>
        <description rdf:datatype="http://www.w3.org/2001/XMLSchema#string">One of the ancestors of Jesus mentioned in Luke&apos;s geneaology</description>
        <hasOnlyGenealogyMention rdf:datatype="http://www.w3.org/2001/XMLSchema#boolean">true</hasOnlyGenealogyMention>
        <rdfs:label xml:lang="en">Melchi</rdfs:label>
    </owl:NamedIndividual>
    


    <!-- http://semanticbible.org/ns/2006/NTNames#Melchizedek -->

    <owl:NamedIndividual rdf:about="http://semanticbible.org/ns/2006/NTNames#Melchizedek">
        <rdf:type rdf:resource="http://semanticbible.org/ns/2006/NTNames#Man"/>
        <rdfs:label xml:lang="en">Melchizedek</rdfs:label>
    </owl:NamedIndividual>
    


    <!-- http://semanticbible.org/ns/2006/NTNames#Melea -->

    <owl:NamedIndividual rdf:about="http://semanticbible.org/ns/2006/NTNames#Melea">
        <rdf:type rdf:resource="http://semanticbible.org/ns/2006/NTNames#Man"/>
        <childOf rdf:resource="http://semanticbible.org/ns/2006/NTNames#Menna"/>
        <ethnicity rdf:resource="http://semanticbible.org/ns/2006/NTNames#Jewish"/>
        <parentOf rdf:resource="http://semanticbible.org/ns/2006/NTNames#EliakimSonOfMelea"/>
        <hasOnlyGenealogyMention rdf:datatype="http://www.w3.org/2001/XMLSchema#boolean">true</hasOnlyGenealogyMention>
        <rdfs:label xml:lang="en">Melea</rdfs:label>
    </owl:NamedIndividual>
    


    <!-- http://semanticbible.org/ns/2006/NTNames#Menna -->

    <owl:NamedIndividual rdf:about="http://semanticbible.org/ns/2006/NTNames#Menna">
        <rdf:type rdf:resource="http://semanticbible.org/ns/2006/NTNames#Man"/>
        <childOf rdf:resource="http://semanticbible.org/ns/2006/NTNames#Mattatha"/>
        <ethnicity rdf:resource="http://semanticbible.org/ns/2006/NTNames#Jewish"/>
        <parentOf rdf:resource="http://semanticbible.org/ns/2006/NTNames#Melea"/>
        <hasOnlyGenealogyMention rdf:datatype="http://www.w3.org/2001/XMLSchema#boolean">true</hasOnlyGenealogyMention>
        <rdfs:label xml:lang="en">Menna</rdfs:label>
    </owl:NamedIndividual>
    


    <!-- http://semanticbible.org/ns/2006/NTNames#Mesopotamia -->

    <owl:NamedIndividual rdf:about="http://semanticbible.org/ns/2006/NTNames#Mesopotamia">
        <rdf:type rdf:resource="http://semanticbible.org/ns/2006/NTNames#Region"/>
        <rdfs:label xml:lang="en">Mesopotamia</rdfs:label>
    </owl:NamedIndividual>
    


    <!-- http://semanticbible.org/ns/2006/NTNames#Methuselah -->

    <owl:NamedIndividual rdf:about="http://semanticbible.org/ns/2006/NTNames#Methuselah">
        <rdf:type rdf:resource="http://semanticbible.org/ns/2006/NTNames#Man"/>
        <childOf rdf:resource="http://semanticbible.org/ns/2006/NTNames#Enoch"/>
        <parentOf rdf:resource="http://semanticbible.org/ns/2006/NTNames#Lamech"/>
        <hasOnlyGenealogyMention rdf:datatype="http://www.w3.org/2001/XMLSchema#boolean">true</hasOnlyGenealogyMention>
        <rdfs:label xml:lang="en">Methuselah</rdfs:label>
    </owl:NamedIndividual>
    


    <!-- http://semanticbible.org/ns/2006/NTNames#Michael -->

    <owl:NamedIndividual rdf:about="http://semanticbible.org/ns/2006/NTNames#Michael">
        <rdf:type rdf:resource="http://semanticbible.org/ns/2006/NTNames#Angel"/>
        <rdfs:label xml:lang="en">Michael</rdfs:label>
    </owl:NamedIndividual>
    


    <!-- http://semanticbible.org/ns/2006/NTNames#Midian -->

    <owl:NamedIndividual rdf:about="http://semanticbible.org/ns/2006/NTNames#Midian">
        <rdf:type rdf:resource="http://semanticbible.org/ns/2006/NTNames#Man"/>
        <rdfs:label xml:lang="en">Midian</rdfs:label>
    </owl:NamedIndividual>
    


    <!-- http://semanticbible.org/ns/2006/NTNames#Miletus -->

    <owl:NamedIndividual rdf:about="http://semanticbible.org/ns/2006/NTNames#Miletus">
        <rdf:type rdf:resource="http://semanticbible.org/ns/2006/NTNames#City"/>
        <location rdf:resource="http://semanticbible.org/ns/2006/NTNames#MiletusGeodata"/>
        <rdfs:label xml:lang="en">Miletus</rdfs:label>
    </owl:NamedIndividual>
    


    <!-- http://semanticbible.org/ns/2006/NTNames#MiletusGeodata -->

    <owl:NamedIndividual rdf:about="http://semanticbible.org/ns/2006/NTNames#MiletusGeodata">
        <rdf:type rdf:resource="http://semanticbible.org/ns/2006/NTNames#GeographicLocation"/>
        <altitude rdf:datatype="http://www.w3.org/2001/XMLSchema#int">0</altitude>
        <latitude rdf:datatype="http://www.w3.org/2001/XMLSchema#double">37.59280951286878</latitude>
        <longitude rdf:datatype="http://www.w3.org/2001/XMLSchema#double">27.30704421298264</longitude>
        <rdfs:label xml:lang="en">geodata for Miletus</rdfs:label>
    </owl:NamedIndividual>
    


    <!-- http://semanticbible.org/ns/2006/NTNames#Mitylene -->

    <owl:NamedIndividual rdf:about="http://semanticbible.org/ns/2006/NTNames#Mitylene">
        <rdf:type rdf:resource="http://semanticbible.org/ns/2006/NTNames#City"/>
        <location rdf:resource="http://semanticbible.org/ns/2006/NTNames#MityleneGeodata"/>
        <rdfs:label xml:lang="en">Mitylene</rdfs:label>
    </owl:NamedIndividual>
    


    <!-- http://semanticbible.org/ns/2006/NTNames#MityleneGeodata -->

    <owl:NamedIndividual rdf:about="http://semanticbible.org/ns/2006/NTNames#MityleneGeodata">
        <rdf:type rdf:resource="http://semanticbible.org/ns/2006/NTNames#GeographicLocation"/>
        <altitude rdf:datatype="http://www.w3.org/2001/XMLSchema#int">0</altitude>
        <latitude rdf:datatype="http://www.w3.org/2001/XMLSchema#double">39.09884068878018</latitude>
        <longitude rdf:datatype="http://www.w3.org/2001/XMLSchema#double">26.55789095333027</longitude>
        <rdfs:label xml:lang="en">geodata for Mitylene</rdfs:label>
    </owl:NamedIndividual>
    


    <!-- http://semanticbible.org/ns/2006/NTNames#Mnason -->

    <owl:NamedIndividual rdf:about="http://semanticbible.org/ns/2006/NTNames#Mnason">
        <rdf:type rdf:resource="http://semanticbible.org/ns/2006/NTNames#Man"/>
        <rdfs:label xml:lang="en">Mnason</rdfs:label>
    </owl:NamedIndividual>
    


    <!-- http://semanticbible.org/ns/2006/NTNames#Moabite -->

    <owl:NamedIndividual rdf:about="http://semanticbible.org/ns/2006/NTNames#Moabite">
        <rdf:type rdf:resource="http://semanticbible.org/ns/2006/NTNames#EthnicityAttribute"/>
        <ethnicityOf rdf:resource="http://semanticbible.org/ns/2006/NTNames#Balak"/>
        <ethnicityOf rdf:resource="http://semanticbible.org/ns/2006/NTNames#Ruth"/>
        <rdfs:comment xml:lang="en">Not mentioned in the New Testament: of the people of Moab, a non-Jewish group.</rdfs:comment>
        <rdfs:label xml:lang="en">Moabite</rdfs:label>
    </owl:NamedIndividual>
    


    <!-- http://semanticbible.org/ns/2006/NTNames#Moloch -->

    <owl:NamedIndividual rdf:about="http://semanticbible.org/ns/2006/NTNames#Moloch">
        <rdf:type rdf:resource="http://semanticbible.org/ns/2006/NTNames#SupernaturalBeing"/>
        <rdfs:label xml:lang="en">Moloch</rdfs:label>
    </owl:NamedIndividual>
    


    <!-- http://semanticbible.org/ns/2006/NTNames#Moses -->

    <owl:NamedIndividual rdf:about="http://semanticbible.org/ns/2006/NTNames#Moses">
        <rdf:type rdf:resource="http://semanticbible.org/ns/2006/NTNames#Man"/>
        <siblingOf rdf:resource="http://semanticbible.org/ns/2006/NTNames#Aaron"/>
        <rdfs:label xml:lang="en">Moses</rdfs:label>
    </owl:NamedIndividual>
    


    <!-- http://semanticbible.org/ns/2006/NTNames#MountofOlivesGeodata -->

    <owl:NamedIndividual rdf:about="http://semanticbible.org/ns/2006/NTNames#MountofOlivesGeodata">
        <rdf:type rdf:resource="http://semanticbible.org/ns/2006/NTNames#GeographicLocation"/>
        <altitude rdf:datatype="http://www.w3.org/2001/XMLSchema#int">0</altitude>
        <latitude rdf:datatype="http://www.w3.org/2001/XMLSchema#double">31.77646075162188</latitude>
        <longitude rdf:datatype="http://www.w3.org/2001/XMLSchema#double">35.24256973151253</longitude>
        <rdfs:label xml:lang="en">geodata for Mount of Olives</rdfs:label>
    </owl:NamedIndividual>
    


    <!-- http://semanticbible.org/ns/2006/NTNames#Myra -->

    <owl:NamedIndividual rdf:about="http://semanticbible.org/ns/2006/NTNames#Myra">
        <rdf:type rdf:resource="http://semanticbible.org/ns/2006/NTNames#City"/>
        <location rdf:resource="http://semanticbible.org/ns/2006/NTNames#MyraGeodata"/>
        <rdfs:label xml:lang="en">Myra</rdfs:label>
    </owl:NamedIndividual>
    


    <!-- http://semanticbible.org/ns/2006/NTNames#MyraGeodata -->

    <owl:NamedIndividual rdf:about="http://semanticbible.org/ns/2006/NTNames#MyraGeodata">
        <rdf:type rdf:resource="http://semanticbible.org/ns/2006/NTNames#GeographicLocation"/>
        <altitude rdf:datatype="http://www.w3.org/2001/XMLSchema#int">0</altitude>
        <latitude rdf:datatype="http://www.w3.org/2001/XMLSchema#double">36.26320556210278</latitude>
        <longitude rdf:datatype="http://www.w3.org/2001/XMLSchema#double">30.06643253716855</longitude>
        <rdfs:label xml:lang="en">geodata for Myra</rdfs:label>
    </owl:NamedIndividual>
    


    <!-- http://semanticbible.org/ns/2006/NTNames#Mysia -->

    <owl:NamedIndividual rdf:about="http://semanticbible.org/ns/2006/NTNames#Mysia">
        <rdf:type rdf:resource="http://semanticbible.org/ns/2006/NTNames#StateOrProvince"/>
        <rdfs:label xml:lang="en">Mysia</rdfs:label>
    </owl:NamedIndividual>
    


    <!-- http://semanticbible.org/ns/2006/NTNames#Naaman -->

    <owl:NamedIndividual rdf:about="http://semanticbible.org/ns/2006/NTNames#Naaman">
        <rdf:type rdf:resource="http://semanticbible.org/ns/2006/NTNames#Man"/>
        <ethnicity rdf:resource="http://semanticbible.org/ns/2006/NTNames#Syrian"/>
        <rdfs:label xml:lang="en">Naaman</rdfs:label>
    </owl:NamedIndividual>
    


    <!-- http://semanticbible.org/ns/2006/NTNames#Naggai -->

    <owl:NamedIndividual rdf:about="http://semanticbible.org/ns/2006/NTNames#Naggai">
        <rdf:type rdf:resource="http://semanticbible.org/ns/2006/NTNames#Man"/>
        <childOf rdf:resource="http://semanticbible.org/ns/2006/NTNames#Maath"/>
        <ethnicity rdf:resource="http://semanticbible.org/ns/2006/NTNames#Jewish"/>
        <parentOf rdf:resource="http://semanticbible.org/ns/2006/NTNames#Esli"/>
        <description rdf:datatype="http://www.w3.org/2001/XMLSchema#string">One of the ancestors of Jesus mentioned in Luke&apos;s geneaology</description>
        <hasOnlyGenealogyMention rdf:datatype="http://www.w3.org/2001/XMLSchema#boolean">true</hasOnlyGenealogyMention>
        <rdfs:label xml:lang="en">Naggai</rdfs:label>
    </owl:NamedIndividual>
    


    <!-- http://semanticbible.org/ns/2006/NTNames#Nahor -->

    <owl:NamedIndividual rdf:about="http://semanticbible.org/ns/2006/NTNames#Nahor">
        <rdf:type rdf:resource="http://semanticbible.org/ns/2006/NTNames#Man"/>
        <childOf rdf:resource="http://semanticbible.org/ns/2006/NTNames#Serug"/>
        <parentOf rdf:resource="http://semanticbible.org/ns/2006/NTNames#Terah"/>
        <description rdf:datatype="http://www.w3.org/2001/XMLSchema#string">One of the ancestors of Jesus mentioned in Luke&apos;s geneaology</description>
        <hasOnlyGenealogyMention rdf:datatype="http://www.w3.org/2001/XMLSchema#boolean">true</hasOnlyGenealogyMention>
        <rdfs:label xml:lang="en">Nahor</rdfs:label>
    </owl:NamedIndividual>
    


    <!-- http://semanticbible.org/ns/2006/NTNames#Nahshon -->

    <owl:NamedIndividual rdf:about="http://semanticbible.org/ns/2006/NTNames#Nahshon">
        <rdf:type rdf:resource="http://semanticbible.org/ns/2006/NTNames#Man"/>
        <childOf rdf:resource="http://semanticbible.org/ns/2006/NTNames#Amminadab"/>
        <ethnicity rdf:resource="http://semanticbible.org/ns/2006/NTNames#Jewish"/>
        <parentOf rdf:resource="http://semanticbible.org/ns/2006/NTNames#Salmon"/>
        <description rdf:datatype="http://www.w3.org/2001/XMLSchema#string">One of the ancestors of Jesus mentioned in Matthew&apos;s geneaology</description>
        <hasOnlyGenealogyMention rdf:datatype="http://www.w3.org/2001/XMLSchema#boolean">true</hasOnlyGenealogyMention>
        <rdfs:label xml:lang="en">Nahshon</rdfs:label>
    </owl:NamedIndividual>
    


    <!-- http://semanticbible.org/ns/2006/NTNames#Nahum -->

    <owl:NamedIndividual rdf:about="http://semanticbible.org/ns/2006/NTNames#Nahum">
        <rdf:type rdf:resource="http://semanticbible.org/ns/2006/NTNames#Man"/>
        <childOf rdf:resource="http://semanticbible.org/ns/2006/NTNames#Esli"/>
        <ethnicity rdf:resource="http://semanticbible.org/ns/2006/NTNames#Jewish"/>
        <parentOf rdf:resource="http://semanticbible.org/ns/2006/NTNames#AmosSonOfNahum"/>
        <description rdf:datatype="http://www.w3.org/2001/XMLSchema#string">One of the ancestors of Jesus mentioned in Luke&apos;s geneaology</description>
        <hasOnlyGenealogyMention rdf:datatype="http://www.w3.org/2001/XMLSchema#boolean">true</hasOnlyGenealogyMention>
        <rdfs:label xml:lang="en">Nahum</rdfs:label>
    </owl:NamedIndividual>
    


    <!-- http://semanticbible.org/ns/2006/NTNames#Nain -->

    <owl:NamedIndividual rdf:about="http://semanticbible.org/ns/2006/NTNames#Nain">
        <rdf:type rdf:resource="http://semanticbible.org/ns/2006/NTNames#City"/>
        <location rdf:resource="http://semanticbible.org/ns/2006/NTNames#NainGeodata"/>
        <subregionOf rdf:resource="http://semanticbible.org/ns/2006/NTNames#Galilee"/>
        <rdfs:label xml:lang="en">Nain</rdfs:label>
    </owl:NamedIndividual>
    


    <!-- http://semanticbible.org/ns/2006/NTNames#NainGeodata -->

    <owl:NamedIndividual rdf:about="http://semanticbible.org/ns/2006/NTNames#NainGeodata">
        <rdf:type rdf:resource="http://semanticbible.org/ns/2006/NTNames#GeographicLocation"/>
        <altitude rdf:datatype="http://www.w3.org/2001/XMLSchema#int">0</altitude>
        <latitude rdf:datatype="http://www.w3.org/2001/XMLSchema#double">32.62729319536898</latitude>
        <longitude rdf:datatype="http://www.w3.org/2001/XMLSchema#double">35.35011627032325</longitude>
        <rdfs:label xml:lang="en">geodata for Nain</rdfs:label>
    </owl:NamedIndividual>
    


    <!-- http://semanticbible.org/ns/2006/NTNames#Naphtali -->

    <owl:NamedIndividual rdf:about="http://semanticbible.org/ns/2006/NTNames#Naphtali">
        <rdf:type rdf:resource="http://semanticbible.org/ns/2006/NTNames#Man"/>
        <siblingOf rdf:resource="http://semanticbible.org/ns/2006/NTNames#Gad"/>
        <rdfs:label xml:lang="en">Naphtali</rdfs:label>
    </owl:NamedIndividual>
    


    <!-- http://semanticbible.org/ns/2006/NTNames#Narcissus -->

    <owl:NamedIndividual rdf:about="http://semanticbible.org/ns/2006/NTNames#Narcissus">
        <rdf:type rdf:resource="http://semanticbible.org/ns/2006/NTNames#Man"/>
        <residentPlace rdf:resource="http://semanticbible.org/ns/2006/NTNames#Rome"/>
        <hasOnlyGenealogyMention rdf:datatype="http://www.w3.org/2001/XMLSchema#boolean">false</hasOnlyGenealogyMention>
        <rdfs:comment rdf:datatype="http://www.w3.org/2001/XMLSchema#string">Paul addresses &quot;the family/household of Narcissus&quot;, which may refer to slaves: so we have no evidence about the beliefs or other attributes of Narcissus himself, other than his residence in Rome. </rdfs:comment>
        <rdfs:label xml:lang="en">Narcissus</rdfs:label>
    </owl:NamedIndividual>
    


    <!-- http://semanticbible.org/ns/2006/NTNames#Nathan -->

    <owl:NamedIndividual rdf:about="http://semanticbible.org/ns/2006/NTNames#Nathan">
        <rdf:type rdf:resource="http://semanticbible.org/ns/2006/NTNames#Man"/>
        <childOf rdf:resource="http://semanticbible.org/ns/2006/NTNames#David"/>
        <ethnicity rdf:resource="http://semanticbible.org/ns/2006/NTNames#Jewish"/>
        <parentOf rdf:resource="http://semanticbible.org/ns/2006/NTNames#Mattatha"/>
        <description rdf:datatype="http://www.w3.org/2001/XMLSchema#string">One of the ancestors of Jesus mentioned in Luke&apos;s geneaology</description>
        <hasOnlyGenealogyMention rdf:datatype="http://www.w3.org/2001/XMLSchema#boolean">true</hasOnlyGenealogyMention>
        <rdfs:comment xml:lang="en">This is not the prophet contemporary with King David, but David&apos;s son.</rdfs:comment>
        <rdfs:label xml:lang="en">Nathan</rdfs:label>
    </owl:NamedIndividual>
    


    <!-- http://semanticbible.org/ns/2006/NTNames#Nazarene -->

    <owl:NamedIndividual rdf:about="http://semanticbible.org/ns/2006/NTNames#Nazarene">
        <rdf:type rdf:resource="http://semanticbible.org/ns/2006/NTNames#ResidencyAttribute"/>
        <rdfs:label xml:lang="en">Nazarene</rdfs:label>
    </owl:NamedIndividual>
    


    <!-- http://semanticbible.org/ns/2006/NTNames#Nazarenes -->

    <owl:NamedIndividual rdf:about="http://semanticbible.org/ns/2006/NTNames#Nazarenes">
        <rdf:type rdf:resource="http://semanticbible.org/ns/2006/NTNames#ResidenceGroup"/>
        <rdfs:label xml:lang="en">Nazarenes</rdfs:label>
    </owl:NamedIndividual>
    


    <!-- http://semanticbible.org/ns/2006/NTNames#Nazareth -->

    <owl:NamedIndividual rdf:about="http://semanticbible.org/ns/2006/NTNames#Nazareth">
        <rdf:type rdf:resource="http://semanticbible.org/ns/2006/NTNames#City"/>
        <location rdf:resource="http://semanticbible.org/ns/2006/NTNames#NazarethGeodata"/>
        <residentPlaceOf rdf:resource="http://semanticbible.org/ns/2006/NTNames#Mary"/>
        <subregionOf rdf:resource="http://semanticbible.org/ns/2006/NTNames#Galilee"/>
        <rdfs:label xml:lang="en">Nazareth</rdfs:label>
    </owl:NamedIndividual>
    


    <!-- http://semanticbible.org/ns/2006/NTNames#NazarethGeodata -->

    <owl:NamedIndividual rdf:about="http://semanticbible.org/ns/2006/NTNames#NazarethGeodata">
        <rdf:type rdf:resource="http://semanticbible.org/ns/2006/NTNames#GeographicLocation"/>
        <altitude rdf:datatype="http://www.w3.org/2001/XMLSchema#int">0</altitude>
        <latitude rdf:datatype="http://www.w3.org/2001/XMLSchema#double">32.706884652966</latitude>
        <longitude rdf:datatype="http://www.w3.org/2001/XMLSchema#double">35.30169055809072</longitude>
        <rdfs:label xml:lang="en">geodata for Nazareth</rdfs:label>
    </owl:NamedIndividual>
    


    <!-- http://semanticbible.org/ns/2006/NTNames#Neapolis -->

    <owl:NamedIndividual rdf:about="http://semanticbible.org/ns/2006/NTNames#Neapolis">
        <rdf:type rdf:resource="http://semanticbible.org/ns/2006/NTNames#City"/>
        <location rdf:resource="http://semanticbible.org/ns/2006/NTNames#NeapolisGeodata"/>
        <rdfs:label xml:lang="en">Neapolis</rdfs:label>
    </owl:NamedIndividual>
    


    <!-- http://semanticbible.org/ns/2006/NTNames#NeapolisGeodata -->

    <owl:NamedIndividual rdf:about="http://semanticbible.org/ns/2006/NTNames#NeapolisGeodata">
        <rdf:type rdf:resource="http://semanticbible.org/ns/2006/NTNames#GeographicLocation"/>
        <altitude rdf:datatype="http://www.w3.org/2001/XMLSchema#int">0</altitude>
        <latitude rdf:datatype="http://www.w3.org/2001/XMLSchema#double">40.94505979070409</latitude>
        <longitude rdf:datatype="http://www.w3.org/2001/XMLSchema#double">24.43247892824545</longitude>
        <rdfs:label xml:lang="en">geodata for Neapolis</rdfs:label>
    </owl:NamedIndividual>
    


    <!-- http://semanticbible.org/ns/2006/NTNames#Nereus -->

    <owl:NamedIndividual rdf:about="http://semanticbible.org/ns/2006/NTNames#Nereus">
        <rdf:type rdf:resource="http://semanticbible.org/ns/2006/NTNames#Man"/>
        <knows rdf:resource="http://semanticbible.org/ns/2006/NTNames#Paul"/>
        <knows rdf:resource="http://semanticbible.org/ns/2006/NTNames#Priscilla"/>
        <religiousBelief rdf:resource="http://semanticbible.org/ns/2006/NTNames#Christianity"/>
        <residentPlace rdf:resource="http://semanticbible.org/ns/2006/NTNames#Rome"/>
        <description rdf:datatype="http://www.w3.org/2001/XMLSchema#string">a Roman to whom Paul sent greetings</description>
        <hasOnlyGenealogyMention rdf:datatype="http://www.w3.org/2001/XMLSchema#boolean">false</hasOnlyGenealogyMention>
        <rdfs:label xml:lang="en">Nereus</rdfs:label>
    </owl:NamedIndividual>
    


    <!-- http://semanticbible.org/ns/2006/NTNames#Neri -->

    <owl:NamedIndividual rdf:about="http://semanticbible.org/ns/2006/NTNames#Neri">
        <rdf:type rdf:resource="http://semanticbible.org/ns/2006/NTNames#Man"/>
        <childOf rdf:resource="http://semanticbible.org/ns/2006/NTNames#MelchiSonOfAddi"/>
        <ethnicity rdf:resource="http://semanticbible.org/ns/2006/NTNames#Jewish"/>
        <parentOf rdf:resource="http://semanticbible.org/ns/2006/NTNames#ShealtielSonOfNeri"/>
        <description rdf:datatype="http://www.w3.org/2001/XMLSchema#string">One of the ancestors of Jesus mentioned in Luke&apos;s geneaology</description>
        <hasOnlyGenealogyMention rdf:datatype="http://www.w3.org/2001/XMLSchema#boolean">true</hasOnlyGenealogyMention>
        <rdfs:label xml:lang="en">Neri</rdfs:label>
    </owl:NamedIndividual>
    


    <!-- http://semanticbible.org/ns/2006/NTNames#Nicanor -->

    <owl:NamedIndividual rdf:about="http://semanticbible.org/ns/2006/NTNames#Nicanor">
        <rdf:type rdf:resource="http://semanticbible.org/ns/2006/NTNames#Man"/>
        <rdfs:label xml:lang="en">Nicanor</rdfs:label>
    </owl:NamedIndividual>
    


    <!-- http://semanticbible.org/ns/2006/NTNames#Nicodemus -->

    <owl:NamedIndividual rdf:about="http://semanticbible.org/ns/2006/NTNames#Nicodemus">
        <rdf:type rdf:resource="http://semanticbible.org/ns/2006/NTNames#Man"/>
        <rdfs:label xml:lang="en">Nicodemus</rdfs:label>
    </owl:NamedIndividual>
    


    <!-- http://semanticbible.org/ns/2006/NTNames#Nicolaitans -->

    <owl:NamedIndividual rdf:about="http://semanticbible.org/ns/2006/NTNames#Nicolaitans">
        <rdf:type rdf:resource="http://semanticbible.org/ns/2006/NTNames#BeliefGroup"/>
        <rdfs:label xml:lang="en">Nicolaitans</rdfs:label>
    </owl:NamedIndividual>
    


    <!-- http://semanticbible.org/ns/2006/NTNames#Nicolatianism -->

    <owl:NamedIndividual rdf:about="http://semanticbible.org/ns/2006/NTNames#Nicolatianism">
        <rdf:type rdf:resource="http://semanticbible.org/ns/2006/NTNames#ReligiousBeliefSystem"/>
        <rdfs:comment xml:lang="en">Not referenced as a belief system in the New Testament.</rdfs:comment>
        <rdfs:label xml:lang="en">Nicolatianism</rdfs:label>
    </owl:NamedIndividual>
    


    <!-- http://semanticbible.org/ns/2006/NTNames#Nicolaus -->

    <owl:NamedIndividual rdf:about="http://semanticbible.org/ns/2006/NTNames#Nicolaus">
        <rdf:type rdf:resource="http://semanticbible.org/ns/2006/NTNames#Man"/>
        <rdfs:label xml:lang="en">Nicolaus</rdfs:label>
    </owl:NamedIndividual>
    


    <!-- http://semanticbible.org/ns/2006/NTNames#Nicopolis -->

    <owl:NamedIndividual rdf:about="http://semanticbible.org/ns/2006/NTNames#Nicopolis">
        <rdf:type rdf:resource="http://semanticbible.org/ns/2006/NTNames#City"/>
        <rdfs:label xml:lang="en">Nicopolis</rdfs:label>
    </owl:NamedIndividual>
    


    <!-- http://semanticbible.org/ns/2006/NTNames#Niger -->

    <owl:NamedIndividual rdf:about="http://semanticbible.org/ns/2006/NTNames#Niger">
        <rdf:type rdf:resource="http://semanticbible.org/ns/2006/NTNames#Man"/>
        <rdfs:label xml:lang="en">Niger</rdfs:label>
    </owl:NamedIndividual>
    


    <!-- http://semanticbible.org/ns/2006/NTNames#Nineveh -->

    <owl:NamedIndividual rdf:about="http://semanticbible.org/ns/2006/NTNames#Nineveh">
        <rdf:type rdf:resource="http://semanticbible.org/ns/2006/NTNames#City"/>
        <location rdf:resource="http://semanticbible.org/ns/2006/NTNames#NinevehGeodata"/>
        <rdfs:label xml:lang="en">Nineveh</rdfs:label>
    </owl:NamedIndividual>
    


    <!-- http://semanticbible.org/ns/2006/NTNames#NinevehGeodata -->

    <owl:NamedIndividual rdf:about="http://semanticbible.org/ns/2006/NTNames#NinevehGeodata">
        <rdf:type rdf:resource="http://semanticbible.org/ns/2006/NTNames#GeographicLocation"/>
        <altitude rdf:datatype="http://www.w3.org/2001/XMLSchema#int">0</altitude>
        <latitude rdf:datatype="http://www.w3.org/2001/XMLSchema#double">36.37255383798249</latitude>
        <longitude rdf:datatype="http://www.w3.org/2001/XMLSchema#double">43.13289767782624</longitude>
        <rdfs:label xml:lang="en">geodata for Nineveh</rdfs:label>
    </owl:NamedIndividual>
    


    <!-- http://semanticbible.org/ns/2006/NTNames#Noah -->

    <owl:NamedIndividual rdf:about="http://semanticbible.org/ns/2006/NTNames#Noah">
        <rdf:type rdf:resource="http://semanticbible.org/ns/2006/NTNames#Man"/>
        <childOf rdf:resource="http://semanticbible.org/ns/2006/NTNames#Lamech"/>
        <parentOf rdf:resource="http://semanticbible.org/ns/2006/NTNames#Shem"/>
        <hasOnlyGenealogyMention rdf:datatype="http://www.w3.org/2001/XMLSchema#boolean">false</hasOnlyGenealogyMention>
        <rdfs:label xml:lang="en">Noah</rdfs:label>
    </owl:NamedIndividual>
    


    <!-- http://semanticbible.org/ns/2006/NTNames#Nympha -->

    <owl:NamedIndividual rdf:about="http://semanticbible.org/ns/2006/NTNames#Nympha">
        <rdf:type rdf:resource="http://semanticbible.org/ns/2006/NTNames#Woman"/>
        <collaboratesWith rdf:resource="http://semanticbible.org/ns/2006/NTNames#Paul"/>
        <religiousBelief rdf:resource="http://semanticbible.org/ns/2006/NTNames#Christianity"/>
        <residentPlace rdf:resource="http://semanticbible.org/ns/2006/NTNames#Laodicea"/>
        <description rdf:datatype="http://www.w3.org/2001/XMLSchema#string">the church in Laodicea met in her house</description>
        <hasOnlyGenealogyMention rdf:datatype="http://www.w3.org/2001/XMLSchema#boolean">false</hasOnlyGenealogyMention>
        <rdfs:comment rdf:datatype="http://www.w3.org/2001/XMLSchema#string">The Church in Laodicea met in her house. Some manuscript variants indicate a man rather than a woman. </rdfs:comment>
        <rdfs:label xml:lang="en">Nympha</rdfs:label>
    </owl:NamedIndividual>
    


    <!-- http://semanticbible.org/ns/2006/NTNames#Obed -->

    <owl:NamedIndividual rdf:about="http://semanticbible.org/ns/2006/NTNames#Obed">
        <rdf:type rdf:resource="http://semanticbible.org/ns/2006/NTNames#Man"/>
        <childOf rdf:resource="http://semanticbible.org/ns/2006/NTNames#Boaz"/>
        <childOf rdf:resource="http://semanticbible.org/ns/2006/NTNames#Ruth"/>
        <ethnicity rdf:resource="http://semanticbible.org/ns/2006/NTNames#Jewish"/>
        <parentOf rdf:resource="http://semanticbible.org/ns/2006/NTNames#Jesse"/>
        <description rdf:datatype="http://www.w3.org/2001/XMLSchema#string">One of the ancestors of Jesus mentioned in Matthew and Luke&apos;s geneaologies</description>
        <hasOnlyGenealogyMention rdf:datatype="http://www.w3.org/2001/XMLSchema#boolean">true</hasOnlyGenealogyMention>
        <rdfs:label xml:lang="en">Obed</rdfs:label>
    </owl:NamedIndividual>
    


    <!-- http://semanticbible.org/ns/2006/NTNames#Olivet -->

    <owl:NamedIndividual rdf:about="http://semanticbible.org/ns/2006/NTNames#Olivet">
        <rdf:type rdf:resource="http://semanticbible.org/ns/2006/NTNames#Mountain"/>
        <location rdf:resource="http://semanticbible.org/ns/2006/NTNames#MountofOlivesGeodata"/>
        <rdfs:label xml:lang="en">Mount of Olives</rdfs:label>
        <rdfs:label xml:lang="en">Olivet</rdfs:label>
    </owl:NamedIndividual>
    


    <!-- http://semanticbible.org/ns/2006/NTNames#Olympas -->

    <owl:NamedIndividual rdf:about="http://semanticbible.org/ns/2006/NTNames#Olympas">
        <rdf:type rdf:resource="http://semanticbible.org/ns/2006/NTNames#Man"/>
        <knows rdf:resource="http://semanticbible.org/ns/2006/NTNames#Paul"/>
        <knows rdf:resource="http://semanticbible.org/ns/2006/NTNames#Priscilla"/>
        <religiousBelief rdf:resource="http://semanticbible.org/ns/2006/NTNames#Christianity"/>
        <residentPlace rdf:resource="http://semanticbible.org/ns/2006/NTNames#Rome"/>
        <description rdf:datatype="http://www.w3.org/2001/XMLSchema#string">a Roman to whom Paul sent greetings</description>
        <hasOnlyGenealogyMention rdf:datatype="http://www.w3.org/2001/XMLSchema#boolean">false</hasOnlyGenealogyMention>
        <rdfs:label xml:lang="en">Olympas</rdfs:label>
    </owl:NamedIndividual>
    


    <!-- http://semanticbible.org/ns/2006/NTNames#Omega -->

    <owl:NamedIndividual rdf:about="http://semanticbible.org/ns/2006/NTNames#Omega">
        <rdf:type rdf:resource="http://semanticbible.org/ns/2006/NTNames#Character"/>
        <rdfs:label xml:lang="en">Omega</rdfs:label>
    </owl:NamedIndividual>
    


    <!-- http://semanticbible.org/ns/2006/NTNames#Onesimus -->

    <owl:NamedIndividual rdf:about="http://semanticbible.org/ns/2006/NTNames#Onesimus">
        <rdf:type rdf:resource="http://semanticbible.org/ns/2006/NTNames#Man"/>
        <rdfs:label xml:lang="en">Onesimus</rdfs:label>
    </owl:NamedIndividual>
    


    <!-- http://semanticbible.org/ns/2006/NTNames#Onesiphorus -->

    <owl:NamedIndividual rdf:about="http://semanticbible.org/ns/2006/NTNames#Onesiphorus">
        <rdf:type rdf:resource="http://semanticbible.org/ns/2006/NTNames#Man"/>
        <rdfs:label xml:lang="en">Onesiphorus</rdfs:label>
    </owl:NamedIndividual>
    


    <!-- http://semanticbible.org/ns/2006/NTNames#Pamphylia -->

    <owl:NamedIndividual rdf:about="http://semanticbible.org/ns/2006/NTNames#Pamphylia">
        <rdf:type rdf:resource="http://semanticbible.org/ns/2006/NTNames#StateOrProvince"/>
        <rdfs:label xml:lang="en">Pamphylia</rdfs:label>
    </owl:NamedIndividual>
    


    <!-- http://semanticbible.org/ns/2006/NTNames#Paphos -->

    <owl:NamedIndividual rdf:about="http://semanticbible.org/ns/2006/NTNames#Paphos">
        <rdf:type rdf:resource="http://semanticbible.org/ns/2006/NTNames#City"/>
        <location rdf:resource="http://semanticbible.org/ns/2006/NTNames#PaphosGeodata"/>
        <rdfs:label xml:lang="en">Paphos</rdfs:label>
    </owl:NamedIndividual>
    


    <!-- http://semanticbible.org/ns/2006/NTNames#PaphosGeodata -->

    <owl:NamedIndividual rdf:about="http://semanticbible.org/ns/2006/NTNames#PaphosGeodata">
        <rdf:type rdf:resource="http://semanticbible.org/ns/2006/NTNames#GeographicLocation"/>
        <altitude rdf:datatype="http://www.w3.org/2001/XMLSchema#int">0</altitude>
        <latitude rdf:datatype="http://www.w3.org/2001/XMLSchema#double">34.77011113075128</latitude>
        <longitude rdf:datatype="http://www.w3.org/2001/XMLSchema#double">32.42822722601693</longitude>
        <rdfs:label xml:lang="en">geodata for Paphos</rdfs:label>
    </owl:NamedIndividual>
    


    <!-- http://semanticbible.org/ns/2006/NTNames#Parmenas -->

    <owl:NamedIndividual rdf:about="http://semanticbible.org/ns/2006/NTNames#Parmenas">
        <rdf:type rdf:resource="http://semanticbible.org/ns/2006/NTNames#Man"/>
        <rdfs:label xml:lang="en">Parmenas</rdfs:label>
    </owl:NamedIndividual>
    


    <!-- http://semanticbible.org/ns/2006/NTNames#Parthia -->

    <owl:NamedIndividual rdf:about="http://semanticbible.org/ns/2006/NTNames#Parthia">
        <rdf:type rdf:resource="http://semanticbible.org/ns/2006/NTNames#StateOrProvince"/>
        <rdfs:comment rdf:datatype="http://www.w3.org/2001/XMLSchema#string">Part of the ancient empire of Persia, though under Roman domination in New Testmament times.</rdfs:comment>
    </owl:NamedIndividual>
    


    <!-- http://semanticbible.org/ns/2006/NTNames#Parthians -->

    <owl:NamedIndividual rdf:about="http://semanticbible.org/ns/2006/NTNames#Parthians">
        <rdf:type rdf:resource="http://semanticbible.org/ns/2006/NTNames#ResidenceGroup"/>
        <rdfs:label xml:lang="en">Parthians</rdfs:label>
    </owl:NamedIndividual>
    


    <!-- http://semanticbible.org/ns/2006/NTNames#PartyOfZealots -->

    <owl:NamedIndividual rdf:about="http://semanticbible.org/ns/2006/NTNames#PartyOfZealots">
        <rdf:type rdf:resource="http://semanticbible.org/ns/2006/NTNames#PoliticalBeliefSystem"/>
        <rdfs:label xml:lang="en">Party of Zealots</rdfs:label>
    </owl:NamedIndividual>
    


    <!-- http://semanticbible.org/ns/2006/NTNames#Passover -->

    <owl:NamedIndividual rdf:about="http://semanticbible.org/ns/2006/NTNames#Passover">
        <rdf:type rdf:resource="http://semanticbible.org/ns/2006/NTNames#FixedHoliday"/>
        <rdfs:label xml:lang="en">Passover</rdfs:label>
    </owl:NamedIndividual>
    


    <!-- http://semanticbible.org/ns/2006/NTNames#Patara -->

    <owl:NamedIndividual rdf:about="http://semanticbible.org/ns/2006/NTNames#Patara">
        <rdf:type rdf:resource="http://semanticbible.org/ns/2006/NTNames#City"/>
        <location rdf:resource="http://semanticbible.org/ns/2006/NTNames#PataraGeodata"/>
        <rdfs:label xml:lang="en">Patara</rdfs:label>
    </owl:NamedIndividual>
    


    <!-- http://semanticbible.org/ns/2006/NTNames#PataraGeodata -->

    <owl:NamedIndividual rdf:about="http://semanticbible.org/ns/2006/NTNames#PataraGeodata">
        <rdf:type rdf:resource="http://semanticbible.org/ns/2006/NTNames#GeographicLocation"/>
        <altitude rdf:datatype="http://www.w3.org/2001/XMLSchema#int">0</altitude>
        <latitude rdf:datatype="http://www.w3.org/2001/XMLSchema#double">36.27516973857826</latitude>
        <longitude rdf:datatype="http://www.w3.org/2001/XMLSchema#double">29.31849755912533</longitude>
        <rdfs:label xml:lang="en">geodata for Patara</rdfs:label>
    </owl:NamedIndividual>
    


    <!-- http://semanticbible.org/ns/2006/NTNames#Patmos -->

    <owl:NamedIndividual rdf:about="http://semanticbible.org/ns/2006/NTNames#Patmos">
        <rdf:type rdf:resource="http://semanticbible.org/ns/2006/NTNames#Island"/>
        <rdfs:label xml:lang="en">Patmos</rdfs:label>
    </owl:NamedIndividual>
    


    <!-- http://semanticbible.org/ns/2006/NTNames#Patrobas -->

    <owl:NamedIndividual rdf:about="http://semanticbible.org/ns/2006/NTNames#Patrobas">
        <rdf:type rdf:resource="http://semanticbible.org/ns/2006/NTNames#Man"/>
        <knows rdf:resource="http://semanticbible.org/ns/2006/NTNames#Paul"/>
        <knows rdf:resource="http://semanticbible.org/ns/2006/NTNames#Priscilla"/>
        <religiousBelief rdf:resource="http://semanticbible.org/ns/2006/NTNames#Christianity"/>
        <residentPlace rdf:resource="http://semanticbible.org/ns/2006/NTNames#Rome"/>
        <description rdf:datatype="http://www.w3.org/2001/XMLSchema#string">a Roman to whom Paul sent greetings</description>
        <hasOnlyGenealogyMention rdf:datatype="http://www.w3.org/2001/XMLSchema#boolean">false</hasOnlyGenealogyMention>
        <rdfs:label xml:lang="en">Patrobas</rdfs:label>
    </owl:NamedIndividual>
    


    <!-- http://semanticbible.org/ns/2006/NTNames#Paul -->

    <owl:NamedIndividual rdf:about="http://semanticbible.org/ns/2006/NTNames#Paul">
        <rdf:type rdf:resource="http://semanticbible.org/ns/2006/NTNames#Man"/>
        <collaboratesWith rdf:resource="http://semanticbible.org/ns/2006/NTNames#Achaicus"/>
        <collaboratesWith rdf:resource="http://semanticbible.org/ns/2006/NTNames#Agabus"/>
        <collaboratesWith rdf:resource="http://semanticbible.org/ns/2006/NTNames#AnaniasOfDamascus"/>
        <collaboratesWith rdf:resource="http://semanticbible.org/ns/2006/NTNames#Andronicus"/>
        <collaboratesWith rdf:resource="http://semanticbible.org/ns/2006/NTNames#Apollos"/>
        <collaboratesWith rdf:resource="http://semanticbible.org/ns/2006/NTNames#Aquila"/>
        <collaboratesWith rdf:resource="http://semanticbible.org/ns/2006/NTNames#Aristarchus"/>
        <collaboratesWith rdf:resource="http://semanticbible.org/ns/2006/NTNames#Artemas"/>
        <collaboratesWith rdf:resource="http://semanticbible.org/ns/2006/NTNames#Barnabas"/>
        <collaboratesWith rdf:resource="http://semanticbible.org/ns/2006/NTNames#Carpus"/>
        <collaboratesWith rdf:resource="http://semanticbible.org/ns/2006/NTNames#Clement"/>
        <collaboratesWith rdf:resource="http://semanticbible.org/ns/2006/NTNames#Crescens"/>
        <collaboratesWith rdf:resource="http://semanticbible.org/ns/2006/NTNames#Demas"/>
        <collaboratesWith rdf:resource="http://semanticbible.org/ns/2006/NTNames#Epaphras"/>
        <collaboratesWith rdf:resource="http://semanticbible.org/ns/2006/NTNames#Epaphroditus"/>
        <collaboratesWith rdf:resource="http://semanticbible.org/ns/2006/NTNames#Erastus"/>
        <collaboratesWith rdf:resource="http://semanticbible.org/ns/2006/NTNames#Eubulus"/>
        <collaboratesWith rdf:resource="http://semanticbible.org/ns/2006/NTNames#Eunice"/>
        <collaboratesWith rdf:resource="http://semanticbible.org/ns/2006/NTNames#Euodia"/>
        <collaboratesWith rdf:resource="http://semanticbible.org/ns/2006/NTNames#Fortunatus"/>
        <collaboratesWith rdf:resource="http://semanticbible.org/ns/2006/NTNames#GaiusOfCorinth"/>
        <collaboratesWith rdf:resource="http://semanticbible.org/ns/2006/NTNames#GaiusOfDerbe"/>
        <collaboratesWith rdf:resource="http://semanticbible.org/ns/2006/NTNames#GaiusOfMacedonia"/>
        <collaboratesWith rdf:resource="http://semanticbible.org/ns/2006/NTNames#JudasOfAntioch"/>
        <collaboratesWith rdf:resource="http://semanticbible.org/ns/2006/NTNames#LuciusOfCyrene"/>
        <collaboratesWith rdf:resource="http://semanticbible.org/ns/2006/NTNames#Lydia"/>
        <collaboratesWith rdf:resource="http://semanticbible.org/ns/2006/NTNames#Manaen"/>
        <collaboratesWith rdf:resource="http://semanticbible.org/ns/2006/NTNames#Nympha"/>
        <collaboratesWith rdf:resource="http://semanticbible.org/ns/2006/NTNames#Phoebe"/>
        <collaboratesWith rdf:resource="http://semanticbible.org/ns/2006/NTNames#Priscilla"/>
        <collaboratesWith rdf:resource="http://semanticbible.org/ns/2006/NTNames#Secundus"/>
        <collaboratesWith rdf:resource="http://semanticbible.org/ns/2006/NTNames#SimeonNiger"/>
        <collaboratesWith rdf:resource="http://semanticbible.org/ns/2006/NTNames#Stephanas"/>
        <collaboratesWith rdf:resource="http://semanticbible.org/ns/2006/NTNames#Syntyche"/>
        <collaboratesWith rdf:resource="http://semanticbible.org/ns/2006/NTNames#Tertius"/>
        <collaboratesWith rdf:resource="http://semanticbible.org/ns/2006/NTNames#Timothy"/>
        <collaboratesWith rdf:resource="http://semanticbible.org/ns/2006/NTNames#Urbanus"/>
        <hasAntagonist rdf:resource="http://semanticbible.org/ns/2006/NTNames#Bar-Jesus"/>
        <hasEnemy rdf:resource="http://semanticbible.org/ns/2006/NTNames#AlexanderTheCoppersmith"/>
        <hasEnemy rdf:resource="http://semanticbible.org/ns/2006/NTNames#AnaniasTheHighPriest"/>
        <hasEnemy rdf:resource="http://semanticbible.org/ns/2006/NTNames#DemetriusTheSilversmith"/>
        <hasEnemy rdf:resource="http://semanticbible.org/ns/2006/NTNames#Felix"/>
        <hasEnemy rdf:resource="http://semanticbible.org/ns/2006/NTNames#Tertullus"/>
        <knows rdf:resource="http://semanticbible.org/ns/2006/NTNames#Ampliatus"/>
        <knows rdf:resource="http://semanticbible.org/ns/2006/NTNames#Apelles"/>
        <knows rdf:resource="http://semanticbible.org/ns/2006/NTNames#Asyncritus"/>
        <knows rdf:resource="http://semanticbible.org/ns/2006/NTNames#Epaenetus"/>
        <knows rdf:resource="http://semanticbible.org/ns/2006/NTNames#Hermas"/>
        <knows rdf:resource="http://semanticbible.org/ns/2006/NTNames#Hermes"/>
        <knows rdf:resource="http://semanticbible.org/ns/2006/NTNames#Hermogenes"/>
        <knows rdf:resource="http://semanticbible.org/ns/2006/NTNames#Herodion"/>
        <knows rdf:resource="http://semanticbible.org/ns/2006/NTNames#Julia"/>
        <knows rdf:resource="http://semanticbible.org/ns/2006/NTNames#MaryOfRome"/>
        <knows rdf:resource="http://semanticbible.org/ns/2006/NTNames#Nereus"/>
        <knows rdf:resource="http://semanticbible.org/ns/2006/NTNames#Olympas"/>
        <knows rdf:resource="http://semanticbible.org/ns/2006/NTNames#Patrobas"/>
        <knows rdf:resource="http://semanticbible.org/ns/2006/NTNames#Persis"/>
        <knows rdf:resource="http://semanticbible.org/ns/2006/NTNames#Philologus"/>
        <knows rdf:resource="http://semanticbible.org/ns/2006/NTNames#Phlegon"/>
        <knows rdf:resource="http://semanticbible.org/ns/2006/NTNames#Phygelus"/>
        <knows rdf:resource="http://semanticbible.org/ns/2006/NTNames#Stachys"/>
        <knows rdf:resource="http://semanticbible.org/ns/2006/NTNames#Tryphaena"/>
        <knows rdf:resource="http://semanticbible.org/ns/2006/NTNames#Tryphosa"/>
        <religiousBelief rdf:resource="http://semanticbible.org/ns/2006/NTNames#Christianity"/>
        <residentPlace rdf:resource="http://semanticbible.org/ns/2006/NTNames#Ephesus"/>
        <hasOnlyGenealogyMention rdf:datatype="http://www.w3.org/2001/XMLSchema#boolean">false</hasOnlyGenealogyMention>
        <occupation rdf:datatype="http://www.w3.org/2001/XMLSchema#string">apostle</occupation>
        <occupation rdf:datatype="http://www.w3.org/2001/XMLSchema#string">tentmaker</occupation>
        <rdfs:comment xml:lang="en">The Apostle Paul was known earlier as Saul: he was given the name Paul when he was converted.</rdfs:comment>
        <rdfs:label xml:lang="en">Paul</rdfs:label>
    </owl:NamedIndividual>
    


    <!-- http://semanticbible.org/ns/2006/NTNames#Peleg -->

    <owl:NamedIndividual rdf:about="http://semanticbible.org/ns/2006/NTNames#Peleg">
        <rdf:type rdf:resource="http://semanticbible.org/ns/2006/NTNames#Man"/>
        <childOf rdf:resource="http://semanticbible.org/ns/2006/NTNames#Eber"/>
        <parentOf rdf:resource="http://semanticbible.org/ns/2006/NTNames#Reu"/>
        <description rdf:datatype="http://www.w3.org/2001/XMLSchema#string">One of the ancestors of Jesus mentioned in Luke&apos;s geneaology</description>
        <hasOnlyGenealogyMention rdf:datatype="http://www.w3.org/2001/XMLSchema#boolean">true</hasOnlyGenealogyMention>
        <rdfs:label xml:lang="en">Peleg</rdfs:label>
    </owl:NamedIndividual>
    


    <!-- http://semanticbible.org/ns/2006/NTNames#Pentecost -->

    <owl:NamedIndividual rdf:about="http://semanticbible.org/ns/2006/NTNames#Pentecost">
        <rdf:type rdf:resource="http://semanticbible.org/ns/2006/NTNames#FixedHoliday"/>
        <rdfs:label xml:lang="en">Pentecost</rdfs:label>
    </owl:NamedIndividual>
    


    <!-- http://semanticbible.org/ns/2006/NTNames#Perez -->

    <owl:NamedIndividual rdf:about="http://semanticbible.org/ns/2006/NTNames#Perez">
        <rdf:type rdf:resource="http://semanticbible.org/ns/2006/NTNames#Man"/>
        <childOf rdf:resource="http://semanticbible.org/ns/2006/NTNames#Judah"/>
        <childOf rdf:resource="http://semanticbible.org/ns/2006/NTNames#Tamar"/>
        <ethnicity rdf:resource="http://semanticbible.org/ns/2006/NTNames#Jewish"/>
        <parentOf rdf:resource="http://semanticbible.org/ns/2006/NTNames#Hezron"/>
        <siblingOf rdf:resource="http://semanticbible.org/ns/2006/NTNames#Zerah"/>
        <description rdf:datatype="http://www.w3.org/2001/XMLSchema#string">One of the ancestors of Jesus mentioned in Matthew&apos;s geneaology</description>
        <hasOnlyGenealogyMention rdf:datatype="http://www.w3.org/2001/XMLSchema#boolean">true</hasOnlyGenealogyMention>
        <rdfs:label xml:lang="en">Perez</rdfs:label>
    </owl:NamedIndividual>
    


    <!-- http://semanticbible.org/ns/2006/NTNames#Perga -->

    <owl:NamedIndividual rdf:about="http://semanticbible.org/ns/2006/NTNames#Perga">
        <rdf:type rdf:resource="http://semanticbible.org/ns/2006/NTNames#City"/>
        <location rdf:resource="http://semanticbible.org/ns/2006/NTNames#PergaGeodata"/>
        <rdfs:label xml:lang="en">Perga</rdfs:label>
    </owl:NamedIndividual>
    


    <!-- http://semanticbible.org/ns/2006/NTNames#PergaGeodata -->

    <owl:NamedIndividual rdf:about="http://semanticbible.org/ns/2006/NTNames#PergaGeodata">
        <rdf:type rdf:resource="http://semanticbible.org/ns/2006/NTNames#GeographicLocation"/>
        <altitude rdf:datatype="http://www.w3.org/2001/XMLSchema#int">0</altitude>
        <latitude rdf:datatype="http://www.w3.org/2001/XMLSchema#double">36.99887690087876</latitude>
        <longitude rdf:datatype="http://www.w3.org/2001/XMLSchema#double">30.91083478573943</longitude>
        <rdfs:label xml:lang="en">geodata for Perga</rdfs:label>
    </owl:NamedIndividual>
    


    <!-- http://semanticbible.org/ns/2006/NTNames#Pergamum -->

    <owl:NamedIndividual rdf:about="http://semanticbible.org/ns/2006/NTNames#Pergamum">
        <rdf:type rdf:resource="http://semanticbible.org/ns/2006/NTNames#City"/>
        <rdfs:label xml:lang="en">Pergamum</rdfs:label>
    </owl:NamedIndividual>
    


    <!-- http://semanticbible.org/ns/2006/NTNames#Persis -->

    <owl:NamedIndividual rdf:about="http://semanticbible.org/ns/2006/NTNames#Persis">
        <rdf:type rdf:resource="http://semanticbible.org/ns/2006/NTNames#Woman"/>
        <knows rdf:resource="http://semanticbible.org/ns/2006/NTNames#Paul"/>
        <knows rdf:resource="http://semanticbible.org/ns/2006/NTNames#Priscilla"/>
        <religiousBelief rdf:resource="http://semanticbible.org/ns/2006/NTNames#Christianity"/>
        <residentPlace rdf:resource="http://semanticbible.org/ns/2006/NTNames#Rome"/>
        <description rdf:datatype="http://www.w3.org/2001/XMLSchema#string">One who worked hard in the Lord among the Roman Christians</description>
        <hasOnlyGenealogyMention rdf:datatype="http://www.w3.org/2001/XMLSchema#boolean">false</hasOnlyGenealogyMention>
        <rdfs:label xml:lang="en">Persis</rdfs:label>
    </owl:NamedIndividual>
    


    <!-- http://semanticbible.org/ns/2006/NTNames#Phanuel -->

    <owl:NamedIndividual rdf:about="http://semanticbible.org/ns/2006/NTNames#Phanuel">
        <rdf:type rdf:resource="http://semanticbible.org/ns/2006/NTNames#Man"/>
        <parentOf rdf:resource="http://semanticbible.org/ns/2006/NTNames#Anna"/>
        <rdfs:label xml:lang="en">Phanuel</rdfs:label>
    </owl:NamedIndividual>
    


    <!-- http://semanticbible.org/ns/2006/NTNames#Pharaoh -->

    <owl:NamedIndividual rdf:about="http://semanticbible.org/ns/2006/NTNames#Pharaoh">
        <rdf:type rdf:resource="http://semanticbible.org/ns/2006/NTNames#Man"/>
        <occupation rdf:datatype="http://www.w3.org/2001/XMLSchema#string">king</occupation>
        <rdfs:comment xml:lang="en">Pharaoh is actually a title rather than a personal name, but in the New Testament it refers to a single individual.</rdfs:comment>
        <rdfs:label xml:lang="en">Pharaoh</rdfs:label>
    </owl:NamedIndividual>
    


    <!-- http://semanticbible.org/ns/2006/NTNames#Pharisee -->

    <owl:NamedIndividual rdf:about="http://semanticbible.org/ns/2006/NTNames#Pharisee">
        <rdf:type rdf:resource="http://semanticbible.org/ns/2006/NTNames#ReligiousBelief"/>
        <rdfs:comment rdf:datatype="http://www.w3.org/2001/XMLSchema#string">Having a ReligiousBelief of Pharisee implies the belief of Jew as well. </rdfs:comment>
        <rdfs:label xml:lang="en">Pharisee</rdfs:label>
    </owl:NamedIndividual>
    


    <!-- http://semanticbible.org/ns/2006/NTNames#Phariseeism -->

    <owl:NamedIndividual rdf:about="http://semanticbible.org/ns/2006/NTNames#Phariseeism">
        <rdf:type rdf:resource="http://semanticbible.org/ns/2006/NTNames#ReligiousBeliefSystem"/>
        <rdfs:comment xml:lang="en">The beliefs of one of the main Jewish sects during the life of Jesus. In the New Testament the name of the sect is used, though not the belief system per se.</rdfs:comment>
        <rdfs:label xml:lang="en">Phariseeism</rdfs:label>
    </owl:NamedIndividual>
    


    <!-- http://semanticbible.org/ns/2006/NTNames#Pharisees -->

    <owl:NamedIndividual rdf:about="http://semanticbible.org/ns/2006/NTNames#Pharisees">
        <rdf:type rdf:resource="http://semanticbible.org/ns/2006/NTNames#ReligiousOrganization"/>
        <member rdf:resource="http://semanticbible.org/ns/2006/NTNames#Gamaliel"/>
        <rdfs:label xml:lang="en">Pharisees</rdfs:label>
    </owl:NamedIndividual>
    


    <!-- http://semanticbible.org/ns/2006/NTNames#Philadelphia -->

    <owl:NamedIndividual rdf:about="http://semanticbible.org/ns/2006/NTNames#Philadelphia">
        <rdf:type rdf:resource="http://semanticbible.org/ns/2006/NTNames#City"/>
        <location rdf:resource="http://semanticbible.org/ns/2006/NTNames#PhiladelphiaGeodata"/>
        <rdfs:label xml:lang="en">Philadelphia</rdfs:label>
    </owl:NamedIndividual>
    


    <!-- http://semanticbible.org/ns/2006/NTNames#PhiladelphiaGeodata -->

    <owl:NamedIndividual rdf:about="http://semanticbible.org/ns/2006/NTNames#PhiladelphiaGeodata">
        <rdf:type rdf:resource="http://semanticbible.org/ns/2006/NTNames#GeographicLocation"/>
        <altitude rdf:datatype="http://www.w3.org/2001/XMLSchema#int">0</altitude>
        <latitude rdf:datatype="http://www.w3.org/2001/XMLSchema#double">38.35785882454039</latitude>
        <longitude rdf:datatype="http://www.w3.org/2001/XMLSchema#double">28.52643605613694</longitude>
        <rdfs:label xml:lang="en">geodata for Philadelphia</rdfs:label>
    </owl:NamedIndividual>
    


    <!-- http://semanticbible.org/ns/2006/NTNames#Philemon -->

    <owl:NamedIndividual rdf:about="http://semanticbible.org/ns/2006/NTNames#Philemon">
        <rdf:type rdf:resource="http://semanticbible.org/ns/2006/NTNames#Man"/>
        <collaboratesWith rdf:resource="http://semanticbible.org/ns/2006/NTNames#Archippus"/>
        <spouseOf rdf:resource="http://semanticbible.org/ns/2006/NTNames#Apphia"/>
        <rdfs:comment xml:lang="en">His residence in Colossae is implied from his relationship to Archippus and Onesimus (Col.4.9; Col.4.17). He may have been been a native as well. 
Paul describes him as &quot;our beloved fellow worker&quot;.</rdfs:comment>
        <rdfs:label xml:lang="en">Philemon</rdfs:label>
    </owl:NamedIndividual>
    


    <!-- http://semanticbible.org/ns/2006/NTNames#Philetus -->

    <owl:NamedIndividual rdf:about="http://semanticbible.org/ns/2006/NTNames#Philetus">
        <rdf:type rdf:resource="http://semanticbible.org/ns/2006/NTNames#Man"/>
        <collaboratesWith rdf:resource="http://semanticbible.org/ns/2006/NTNames#Hymenaeus"/>
        <rdfs:label xml:lang="en">Philetus</rdfs:label>
    </owl:NamedIndividual>
    


    <!-- http://semanticbible.org/ns/2006/NTNames#Philip -->

    <owl:NamedIndividual rdf:about="http://semanticbible.org/ns/2006/NTNames#Philip">
        <rdf:type rdf:resource="http://semanticbible.org/ns/2006/NTNames#Man"/>
        <collaboratesWith rdf:resource="http://semanticbible.org/ns/2006/NTNames#Andrew"/>
        <ethnicity rdf:resource="http://semanticbible.org/ns/2006/NTNames#Galilean"/>
        <description rdf:datatype="http://www.w3.org/2001/XMLSchema#string">One of Jesus&apos; twelve apostles</description>
        <rdfs:label xml:lang="en">Philip</rdfs:label>
    </owl:NamedIndividual>
    


    <!-- http://semanticbible.org/ns/2006/NTNames#PhilipSonOfHerod -->

    <owl:NamedIndividual rdf:about="http://semanticbible.org/ns/2006/NTNames#PhilipSonOfHerod">
        <rdf:type rdf:resource="http://semanticbible.org/ns/2006/NTNames#Man"/>
        <childOf rdf:resource="http://semanticbible.org/ns/2006/NTNames#HerodTheGreat"/>
        <siblingOf rdf:resource="http://semanticbible.org/ns/2006/NTNames#Archelaus"/>
        <siblingOf rdf:resource="http://semanticbible.org/ns/2006/NTNames#HerodAntipas"/>
        <spouseOf rdf:resource="http://semanticbible.org/ns/2006/NTNames#Herodias"/>
        <description rdf:datatype="http://www.w3.org/2001/XMLSchema#string">King of the land east of the Jordan</description>
        <rdfs:label xml:lang="en">Philip</rdfs:label>
    </owl:NamedIndividual>
    


    <!-- http://semanticbible.org/ns/2006/NTNames#Philippi -->

    <owl:NamedIndividual rdf:about="http://semanticbible.org/ns/2006/NTNames#Philippi">
        <rdf:type rdf:resource="http://semanticbible.org/ns/2006/NTNames#City"/>
        <location rdf:resource="http://semanticbible.org/ns/2006/NTNames#PhilippiGeodata"/>
        <residentPlaceOf rdf:resource="http://semanticbible.org/ns/2006/NTNames#Euodia"/>
        <residentPlaceOf rdf:resource="http://semanticbible.org/ns/2006/NTNames#Syntyche"/>
        <visitedPlaceOf rdf:resource="http://semanticbible.org/ns/2006/NTNames#Lydia"/>
        <rdfs:label xml:lang="en">Philippi</rdfs:label>
    </owl:NamedIndividual>
    


    <!-- http://semanticbible.org/ns/2006/NTNames#PhilippiGeodata -->

    <owl:NamedIndividual rdf:about="http://semanticbible.org/ns/2006/NTNames#PhilippiGeodata">
        <rdf:type rdf:resource="http://semanticbible.org/ns/2006/NTNames#GeographicLocation"/>
        <altitude rdf:datatype="http://www.w3.org/2001/XMLSchema#int">0</altitude>
        <latitude rdf:datatype="http://www.w3.org/2001/XMLSchema#double">41.01329092166473</latitude>
        <longitude rdf:datatype="http://www.w3.org/2001/XMLSchema#double">24.28828605219695</longitude>
        <rdfs:label xml:lang="en">geodata for Philippi</rdfs:label>
    </owl:NamedIndividual>
    


    <!-- http://semanticbible.org/ns/2006/NTNames#Philippians -->

    <owl:NamedIndividual rdf:about="http://semanticbible.org/ns/2006/NTNames#Philippians">
        <rdf:type rdf:resource="http://semanticbible.org/ns/2006/NTNames#ResidenceGroup"/>
        <rdfs:label xml:lang="en">Philippians</rdfs:label>
    </owl:NamedIndividual>
    


    <!-- http://semanticbible.org/ns/2006/NTNames#Philologus -->

    <owl:NamedIndividual rdf:about="http://semanticbible.org/ns/2006/NTNames#Philologus">
        <rdf:type rdf:resource="http://semanticbible.org/ns/2006/NTNames#Man"/>
        <knows rdf:resource="http://semanticbible.org/ns/2006/NTNames#Paul"/>
        <knows rdf:resource="http://semanticbible.org/ns/2006/NTNames#Priscilla"/>
        <religiousBelief rdf:resource="http://semanticbible.org/ns/2006/NTNames#Christianity"/>
        <residentPlace rdf:resource="http://semanticbible.org/ns/2006/NTNames#Rome"/>
        <description rdf:datatype="http://www.w3.org/2001/XMLSchema#string">a Roman to whom Paul sent greetings</description>
        <hasOnlyGenealogyMention rdf:datatype="http://www.w3.org/2001/XMLSchema#boolean">false</hasOnlyGenealogyMention>
        <rdfs:label xml:lang="en">Philologus</rdfs:label>
    </owl:NamedIndividual>
    


    <!-- http://semanticbible.org/ns/2006/NTNames#Phlegon -->

    <owl:NamedIndividual rdf:about="http://semanticbible.org/ns/2006/NTNames#Phlegon">
        <rdf:type rdf:resource="http://semanticbible.org/ns/2006/NTNames#Man"/>
        <knows rdf:resource="http://semanticbible.org/ns/2006/NTNames#Paul"/>
        <knows rdf:resource="http://semanticbible.org/ns/2006/NTNames#Priscilla"/>
        <religiousBelief rdf:resource="http://semanticbible.org/ns/2006/NTNames#Christianity"/>
        <residentPlace rdf:resource="http://semanticbible.org/ns/2006/NTNames#Rome"/>
        <description rdf:datatype="http://www.w3.org/2001/XMLSchema#string">a Roman to whom Paul sent greetings</description>
        <hasOnlyGenealogyMention rdf:datatype="http://www.w3.org/2001/XMLSchema#boolean">false</hasOnlyGenealogyMention>
        <rdfs:label xml:lang="en">Phlegon</rdfs:label>
    </owl:NamedIndividual>
    


    <!-- http://semanticbible.org/ns/2006/NTNames#Phoebe -->

    <owl:NamedIndividual rdf:about="http://semanticbible.org/ns/2006/NTNames#Phoebe">
        <rdf:type rdf:resource="http://semanticbible.org/ns/2006/NTNames#Woman"/>
        <collaboratesWith rdf:resource="http://semanticbible.org/ns/2006/NTNames#Paul"/>
        <religiousBelief rdf:resource="http://semanticbible.org/ns/2006/NTNames#Christianity"/>
        <residentPlace rdf:resource="http://semanticbible.org/ns/2006/NTNames#Cenchreae"/>
        <description rdf:datatype="http://www.w3.org/2001/XMLSchema#string">Deaconess of the Church of Cenchreae</description>
        <hasOnlyGenealogyMention rdf:datatype="http://www.w3.org/2001/XMLSchema#boolean">false</hasOnlyGenealogyMention>
        <rdfs:comment xml:lang="en">Paul&apos;s commendation of Phoebe in Romans strongly suggests she delivered the letter</rdfs:comment>
        <rdfs:label xml:lang="en">Phoebe</rdfs:label>
    </owl:NamedIndividual>
    


    <!-- http://semanticbible.org/ns/2006/NTNames#Phoenicia -->

    <owl:NamedIndividual rdf:about="http://semanticbible.org/ns/2006/NTNames#Phoenicia">
        <rdf:type rdf:resource="http://semanticbible.org/ns/2006/NTNames#Region"/>
        <rdfs:label xml:lang="en">Phoenicia</rdfs:label>
    </owl:NamedIndividual>
    


    <!-- http://semanticbible.org/ns/2006/NTNames#Phoenix -->

    <owl:NamedIndividual rdf:about="http://semanticbible.org/ns/2006/NTNames#Phoenix">
        <rdf:type rdf:resource="http://semanticbible.org/ns/2006/NTNames#City"/>
        <location rdf:resource="http://semanticbible.org/ns/2006/NTNames#PhoenixGeodata"/>
        <rdfs:label xml:lang="en">Phoenix</rdfs:label>
    </owl:NamedIndividual>
    


    <!-- http://semanticbible.org/ns/2006/NTNames#PhoenixGeodata -->

    <owl:NamedIndividual rdf:about="http://semanticbible.org/ns/2006/NTNames#PhoenixGeodata">
        <rdf:type rdf:resource="http://semanticbible.org/ns/2006/NTNames#GeographicLocation"/>
        <altitude rdf:datatype="http://www.w3.org/2001/XMLSchema#int">0</altitude>
        <latitude rdf:datatype="http://www.w3.org/2001/XMLSchema#double">35.26650579704394</latitude>
        <longitude rdf:datatype="http://www.w3.org/2001/XMLSchema#double">24.01414490625663</longitude>
        <rdfs:label xml:lang="en">geodata for Phoenix</rdfs:label>
    </owl:NamedIndividual>
    


    <!-- http://semanticbible.org/ns/2006/NTNames#Phrygia -->

    <owl:NamedIndividual rdf:about="http://semanticbible.org/ns/2006/NTNames#Phrygia">
        <rdf:type rdf:resource="http://semanticbible.org/ns/2006/NTNames#Region"/>
        <rdfs:label xml:lang="en">Phrygia</rdfs:label>
    </owl:NamedIndividual>
    


    <!-- http://semanticbible.org/ns/2006/NTNames#Phygelus -->

    <owl:NamedIndividual rdf:about="http://semanticbible.org/ns/2006/NTNames#Phygelus">
        <rdf:type rdf:resource="http://semanticbible.org/ns/2006/NTNames#Man"/>
        <knows rdf:resource="http://semanticbible.org/ns/2006/NTNames#Hermogenes"/>
        <knows rdf:resource="http://semanticbible.org/ns/2006/NTNames#Paul"/>
        <religiousBelief rdf:resource="http://semanticbible.org/ns/2006/NTNames#Christianity"/>
        <description rdf:datatype="http://www.w3.org/2001/XMLSchema#string">a Christian who refused to help Paul during his Roman imprisonment</description>
        <hasOnlyGenealogyMention rdf:datatype="http://www.w3.org/2001/XMLSchema#boolean">false</hasOnlyGenealogyMention>
        <rdfs:comment xml:lang="en">The circumstances behind his &quot;turning away&quot; from Paul are unknown. Likewise, Paul&apos;s description of him as being &quot;is Asia&quot; isn&apos;t specific enough to assign a place. </rdfs:comment>
        <rdfs:label xml:lang="en">Phygelus</rdfs:label>
    </owl:NamedIndividual>
    


    <!-- http://semanticbible.org/ns/2006/NTNames#Pilate -->

    <owl:NamedIndividual rdf:about="http://semanticbible.org/ns/2006/NTNames#Pilate">
        <rdf:type rdf:resource="http://semanticbible.org/ns/2006/NTNames#Man"/>
        <rdfs:label xml:lang="en">Pilate</rdfs:label>
    </owl:NamedIndividual>
    


    <!-- http://semanticbible.org/ns/2006/NTNames#Pisidia -->

    <owl:NamedIndividual rdf:about="http://semanticbible.org/ns/2006/NTNames#Pisidia">
        <rdf:type rdf:resource="http://semanticbible.org/ns/2006/NTNames#StateOrProvince"/>
        <rdfs:label xml:lang="en">Pisidia</rdfs:label>
    </owl:NamedIndividual>
    


    <!-- http://semanticbible.org/ns/2006/NTNames#PontiusPilate -->

    <owl:NamedIndividual rdf:about="http://semanticbible.org/ns/2006/NTNames#PontiusPilate">
        <rdf:type rdf:resource="http://semanticbible.org/ns/2006/NTNames#Man"/>
        <collaboratesWith rdf:resource="http://semanticbible.org/ns/2006/NTNames#Archelaus"/>
        <collaboratesWith rdf:resource="http://semanticbible.org/ns/2006/NTNames#HerodAntipas"/>
        <rdfs:label xml:lang="en">Pontius Pilate</rdfs:label>
    </owl:NamedIndividual>
    


    <!-- http://semanticbible.org/ns/2006/NTNames#Pontus -->

    <owl:NamedIndividual rdf:about="http://semanticbible.org/ns/2006/NTNames#Pontus">
        <rdf:type rdf:resource="http://semanticbible.org/ns/2006/NTNames#Region"/>
        <rdfs:label xml:lang="en">Pontus</rdfs:label>
    </owl:NamedIndividual>
    


    <!-- http://semanticbible.org/ns/2006/NTNames#Porcius -->

    <owl:NamedIndividual rdf:about="http://semanticbible.org/ns/2006/NTNames#Porcius">
        <rdf:type rdf:resource="http://semanticbible.org/ns/2006/NTNames#Man"/>
        <rdfs:label xml:lang="en">Porcius</rdfs:label>
    </owl:NamedIndividual>
    


    <!-- http://semanticbible.org/ns/2006/NTNames#Priscilla -->

    <owl:NamedIndividual rdf:about="http://semanticbible.org/ns/2006/NTNames#Priscilla">
        <rdf:type rdf:resource="http://semanticbible.org/ns/2006/NTNames#Woman"/>
        <collaboratesWith rdf:resource="http://semanticbible.org/ns/2006/NTNames#Apollos"/>
        <collaboratesWith rdf:resource="http://semanticbible.org/ns/2006/NTNames#Paul"/>
        <ethnicity rdf:resource="http://semanticbible.org/ns/2006/NTNames#Jewish"/>
        <knows rdf:resource="http://semanticbible.org/ns/2006/NTNames#Ampliatus"/>
        <knows rdf:resource="http://semanticbible.org/ns/2006/NTNames#Andronicus"/>
        <knows rdf:resource="http://semanticbible.org/ns/2006/NTNames#Apelles"/>
        <knows rdf:resource="http://semanticbible.org/ns/2006/NTNames#Asyncritus"/>
        <knows rdf:resource="http://semanticbible.org/ns/2006/NTNames#Epaenetus"/>
        <knows rdf:resource="http://semanticbible.org/ns/2006/NTNames#Hermas"/>
        <knows rdf:resource="http://semanticbible.org/ns/2006/NTNames#Hermes"/>
        <knows rdf:resource="http://semanticbible.org/ns/2006/NTNames#Herodion"/>
        <knows rdf:resource="http://semanticbible.org/ns/2006/NTNames#Julia"/>
        <knows rdf:resource="http://semanticbible.org/ns/2006/NTNames#Junia"/>
        <knows rdf:resource="http://semanticbible.org/ns/2006/NTNames#MaryOfRome"/>
        <knows rdf:resource="http://semanticbible.org/ns/2006/NTNames#Nereus"/>
        <knows rdf:resource="http://semanticbible.org/ns/2006/NTNames#Olympas"/>
        <knows rdf:resource="http://semanticbible.org/ns/2006/NTNames#Patrobas"/>
        <knows rdf:resource="http://semanticbible.org/ns/2006/NTNames#Persis"/>
        <knows rdf:resource="http://semanticbible.org/ns/2006/NTNames#Philologus"/>
        <knows rdf:resource="http://semanticbible.org/ns/2006/NTNames#Phlegon"/>
        <knows rdf:resource="http://semanticbible.org/ns/2006/NTNames#Rufus"/>
        <knows rdf:resource="http://semanticbible.org/ns/2006/NTNames#Stachys"/>
        <knows rdf:resource="http://semanticbible.org/ns/2006/NTNames#Tryphaena"/>
        <knows rdf:resource="http://semanticbible.org/ns/2006/NTNames#Tryphosa"/>
        <knows rdf:resource="http://semanticbible.org/ns/2006/NTNames#Urbanus"/>
        <religiousBelief rdf:resource="http://semanticbible.org/ns/2006/NTNames#Christianity"/>
        <residentPlace rdf:resource="http://semanticbible.org/ns/2006/NTNames#Corinth"/>
        <residentPlace rdf:resource="http://semanticbible.org/ns/2006/NTNames#Ephesus"/>
        <residentPlace rdf:resource="http://semanticbible.org/ns/2006/NTNames#Rome"/>
        <spouseOf rdf:resource="http://semanticbible.org/ns/2006/NTNames#Aquila"/>
        <hasOnlyGenealogyMention rdf:datatype="http://www.w3.org/2001/XMLSchema#boolean">false</hasOnlyGenealogyMention>
        <rdfs:comment rdf:datatype="http://www.w3.org/2001/XMLSchema#string">Prisca is the diminutive form of Priscilla. Brownrigg notes that Paul always uses this form.</rdfs:comment>
        <rdfs:label xml:lang="en">Prisca</rdfs:label>
        <rdfs:label xml:lang="en">Priscilla</rdfs:label>
    </owl:NamedIndividual>
    


    <!-- http://semanticbible.org/ns/2006/NTNames#Prochorus -->

    <owl:NamedIndividual rdf:about="http://semanticbible.org/ns/2006/NTNames#Prochorus">
        <rdf:type rdf:resource="http://semanticbible.org/ns/2006/NTNames#Man"/>
        <rdfs:label xml:lang="en">Prochorus</rdfs:label>
    </owl:NamedIndividual>
    


    <!-- http://semanticbible.org/ns/2006/NTNames#Ptolemais -->

    <owl:NamedIndividual rdf:about="http://semanticbible.org/ns/2006/NTNames#Ptolemais">
        <rdf:type rdf:resource="http://semanticbible.org/ns/2006/NTNames#Man"/>
        <rdfs:label xml:lang="en">Ptolemais</rdfs:label>
    </owl:NamedIndividual>
    


    <!-- http://semanticbible.org/ns/2006/NTNames#Publius -->

    <owl:NamedIndividual rdf:about="http://semanticbible.org/ns/2006/NTNames#Publius">
        <rdf:type rdf:resource="http://semanticbible.org/ns/2006/NTNames#Man"/>
        <rdfs:label xml:lang="en">Publius</rdfs:label>
    </owl:NamedIndividual>
    


    <!-- http://semanticbible.org/ns/2006/NTNames#Pudens -->

    <owl:NamedIndividual rdf:about="http://semanticbible.org/ns/2006/NTNames#Pudens">
        <rdf:type rdf:resource="http://semanticbible.org/ns/2006/NTNames#Man"/>
        <rdfs:label xml:lang="en">Pudens</rdfs:label>
    </owl:NamedIndividual>
    


    <!-- http://semanticbible.org/ns/2006/NTNames#Puteoli -->

    <owl:NamedIndividual rdf:about="http://semanticbible.org/ns/2006/NTNames#Puteoli">
        <rdf:type rdf:resource="http://semanticbible.org/ns/2006/NTNames#City"/>
        <location rdf:resource="http://semanticbible.org/ns/2006/NTNames#PuteoliGeodata"/>
        <rdfs:label xml:lang="en">Puteoli</rdfs:label>
    </owl:NamedIndividual>
    


    <!-- http://semanticbible.org/ns/2006/NTNames#PuteoliGeodata -->

    <owl:NamedIndividual rdf:about="http://semanticbible.org/ns/2006/NTNames#PuteoliGeodata">
        <rdf:type rdf:resource="http://semanticbible.org/ns/2006/NTNames#GeographicLocation"/>
        <altitude rdf:datatype="http://www.w3.org/2001/XMLSchema#int">0</altitude>
        <latitude rdf:datatype="http://www.w3.org/2001/XMLSchema#double">40.83850773167724</latitude>
        <longitude rdf:datatype="http://www.w3.org/2001/XMLSchema#double">14.24733299483093</longitude>
        <rdfs:label xml:lang="en">geodata for Puteoli</rdfs:label>
    </owl:NamedIndividual>
    


    <!-- http://semanticbible.org/ns/2006/NTNames#Pyrrhus -->

    <owl:NamedIndividual rdf:about="http://semanticbible.org/ns/2006/NTNames#Pyrrhus">
        <rdf:type rdf:resource="http://semanticbible.org/ns/2006/NTNames#Man"/>
        <parentOf rdf:resource="http://semanticbible.org/ns/2006/NTNames#Sopater"/>
        <rdfs:label xml:lang="en">Pyrrhus</rdfs:label>
    </owl:NamedIndividual>
    


    <!-- http://semanticbible.org/ns/2006/NTNames#Quartus -->

    <owl:NamedIndividual rdf:about="http://semanticbible.org/ns/2006/NTNames#Quartus">
        <rdf:type rdf:resource="http://semanticbible.org/ns/2006/NTNames#Man"/>
        <rdfs:label xml:lang="en">Quartus</rdfs:label>
    </owl:NamedIndividual>
    


    <!-- http://semanticbible.org/ns/2006/NTNames#Quirinius -->

    <owl:NamedIndividual rdf:about="http://semanticbible.org/ns/2006/NTNames#Quirinius">
        <rdf:type rdf:resource="http://semanticbible.org/ns/2006/NTNames#Man"/>
        <rdfs:label xml:lang="en">Quirinius</rdfs:label>
    </owl:NamedIndividual>
    


    <!-- http://semanticbible.org/ns/2006/NTNames#Rachel -->

    <owl:NamedIndividual rdf:about="http://semanticbible.org/ns/2006/NTNames#Rachel">
        <rdf:type rdf:resource="http://semanticbible.org/ns/2006/NTNames#Woman"/>
        <ethnicity rdf:resource="http://semanticbible.org/ns/2006/NTNames#Jewish"/>
        <parentOf rdf:resource="http://semanticbible.org/ns/2006/NTNames#Benjamin"/>
        <parentOf rdf:resource="http://semanticbible.org/ns/2006/NTNames#JosephThePatriarch"/>
        <religiousBelief rdf:resource="http://semanticbible.org/ns/2006/NTNames#Judaism"/>
        <spouseOf rdf:resource="http://semanticbible.org/ns/2006/NTNames#Jacob"/>
        <description rdf:datatype="http://www.w3.org/2001/XMLSchema#string">one of Jacob&apos;s wives</description>
        <hasOnlyGenealogyMention rdf:datatype="http://www.w3.org/2001/XMLSchema#boolean">false</hasOnlyGenealogyMention>
        <rdfs:comment xml:lang="en">Daughter of Laban and sister of Leah, who are not named in the New Testament. </rdfs:comment>
        <rdfs:label xml:lang="en">Rachel</rdfs:label>
    </owl:NamedIndividual>
    


    <!-- http://semanticbible.org/ns/2006/NTNames#Rahab -->

    <owl:NamedIndividual rdf:about="http://semanticbible.org/ns/2006/NTNames#Rahab">
        <rdf:type rdf:resource="http://semanticbible.org/ns/2006/NTNames#Woman"/>
        <parentOf rdf:resource="http://semanticbible.org/ns/2006/NTNames#Boaz"/>
        <spouseOf rdf:resource="http://semanticbible.org/ns/2006/NTNames#Salmon"/>
        <description rdf:datatype="http://www.w3.org/2001/XMLSchema#string">An Old Testament example of faith who hid Joshua&apos;s spies</description>
        <hasOnlyGenealogyMention rdf:datatype="http://www.w3.org/2001/XMLSchema#boolean">false</hasOnlyGenealogyMention>
        <occupation rdf:datatype="http://www.w3.org/2001/XMLSchema#string">prostitute</occupation>
        <rdfs:label xml:lang="en">Rahab</rdfs:label>
    </owl:NamedIndividual>
    


    <!-- http://semanticbible.org/ns/2006/NTNames#Ram -->

    <owl:NamedIndividual rdf:about="http://semanticbible.org/ns/2006/NTNames#Ram">
        <rdf:type rdf:resource="http://semanticbible.org/ns/2006/NTNames#Man"/>
        <childOf rdf:resource="http://semanticbible.org/ns/2006/NTNames#Hezron"/>
        <ethnicity rdf:resource="http://semanticbible.org/ns/2006/NTNames#Jewish"/>
        <parentOf rdf:resource="http://semanticbible.org/ns/2006/NTNames#Amminadab"/>
        <possiblySamePersonAs rdf:resource="http://semanticbible.org/ns/2006/NTNames#Arni"/>
        <description rdf:datatype="http://www.w3.org/2001/XMLSchema#string">One of the ancestors of Jesus mentioned in Matthew&apos;s geneaology</description>
        <hasOnlyGenealogyMention rdf:datatype="http://www.w3.org/2001/XMLSchema#boolean">true</hasOnlyGenealogyMention>
        <rdfs:label xml:lang="en">Ram</rdfs:label>
    </owl:NamedIndividual>
    


    <!-- http://semanticbible.org/ns/2006/NTNames#Ramah -->

    <owl:NamedIndividual rdf:about="http://semanticbible.org/ns/2006/NTNames#Ramah">
        <rdf:type rdf:resource="http://semanticbible.org/ns/2006/NTNames#City"/>
        <location rdf:resource="http://semanticbible.org/ns/2006/NTNames#RamahGeodata"/>
        <subregionOf rdf:resource="http://semanticbible.org/ns/2006/NTNames#Judea"/>
        <rdfs:comment rdf:datatype="http://www.w3.org/2001/XMLSchema#string">The only NT reference is a quotation from Jer 31:15: this presumably refers to Ramah near Bethel. </rdfs:comment>
        <rdfs:label xml:lang="en">Ramah</rdfs:label>
    </owl:NamedIndividual>
    


    <!-- http://semanticbible.org/ns/2006/NTNames#RamahGeodata -->

    <owl:NamedIndividual rdf:about="http://semanticbible.org/ns/2006/NTNames#RamahGeodata">
        <rdf:type rdf:resource="http://semanticbible.org/ns/2006/NTNames#GeographicLocation"/>
        <altitude rdf:datatype="http://www.w3.org/2001/XMLSchema#int">0</altitude>
        <latitude rdf:datatype="http://www.w3.org/2001/XMLSchema#double">31.90463130995243</latitude>
        <longitude rdf:datatype="http://www.w3.org/2001/XMLSchema#double">35.23965156684373</longitude>
        <rdfs:label xml:lang="en">geodata for Ramah</rdfs:label>
    </owl:NamedIndividual>
    


    <!-- http://semanticbible.org/ns/2006/NTNames#Rebecca -->

    <owl:NamedIndividual rdf:about="http://semanticbible.org/ns/2006/NTNames#Rebecca">
        <rdf:type rdf:resource="http://semanticbible.org/ns/2006/NTNames#Woman"/>
        <ethnicity rdf:resource="http://semanticbible.org/ns/2006/NTNames#Jewish"/>
        <parentOf rdf:resource="http://semanticbible.org/ns/2006/NTNames#Esau"/>
        <parentOf rdf:resource="http://semanticbible.org/ns/2006/NTNames#Jacob"/>
        <spouseOf rdf:resource="http://semanticbible.org/ns/2006/NTNames#Isaac"/>
        <description rdf:datatype="http://www.w3.org/2001/XMLSchema#string">husband of Isaac</description>
        <hasOnlyGenealogyMention rdf:datatype="http://www.w3.org/2001/XMLSchema#boolean">false</hasOnlyGenealogyMention>
        <rdfs:comment rdf:datatype="http://www.w3.org/2001/XMLSchema#string">Brother of Laban, who is not named in the New Testament. </rdfs:comment>
        <rdfs:label xml:lang="en">Rebecca</rdfs:label>
    </owl:NamedIndividual>
    


    <!-- http://semanticbible.org/ns/2006/NTNames#Rehoboam -->

    <owl:NamedIndividual rdf:about="http://semanticbible.org/ns/2006/NTNames#Rehoboam">
        <rdf:type rdf:resource="http://semanticbible.org/ns/2006/NTNames#Man"/>
        <childOf rdf:resource="http://semanticbible.org/ns/2006/NTNames#Solomon"/>
        <ethnicity rdf:resource="http://semanticbible.org/ns/2006/NTNames#Jewish"/>
        <parentOf rdf:resource="http://semanticbible.org/ns/2006/NTNames#AbijahSonOfRehoboam"/>
        <relativeOf rdf:resource="http://semanticbible.org/ns/2006/NTNames#AbijahSonOfRehoboam"/>
        <description rdf:datatype="http://www.w3.org/2001/XMLSchema#string">A king of Israel, and one of the ancestors of Jesus mentioned in Matthew&apos;s geneaology</description>
        <hasOnlyGenealogyMention rdf:datatype="http://www.w3.org/2001/XMLSchema#boolean">true</hasOnlyGenealogyMention>
        <occupation rdf:datatype="http://www.w3.org/2001/XMLSchema#string">king</occupation>
        <rdfs:comment rdf:datatype="http://www.w3.org/2001/XMLSchema#string">His occupation as king comes from the Old Testament, 1Kgs.12-14</rdfs:comment>
        <rdfs:label xml:lang="en">Rehoboam</rdfs:label>
    </owl:NamedIndividual>
    


    <!-- http://semanticbible.org/ns/2006/NTNames#Rephan -->

    <owl:NamedIndividual rdf:about="http://semanticbible.org/ns/2006/NTNames#Rephan">
        <rdf:type rdf:resource="http://semanticbible.org/ns/2006/NTNames#SupernaturalBeing"/>
        <rdfs:label xml:lang="en">Rephan</rdfs:label>
    </owl:NamedIndividual>
    


    <!-- http://semanticbible.org/ns/2006/NTNames#Reu -->

    <owl:NamedIndividual rdf:about="http://semanticbible.org/ns/2006/NTNames#Reu">
        <rdf:type rdf:resource="http://semanticbible.org/ns/2006/NTNames#Man"/>
        <childOf rdf:resource="http://semanticbible.org/ns/2006/NTNames#Peleg"/>
        <parentOf rdf:resource="http://semanticbible.org/ns/2006/NTNames#Serug"/>
        <description rdf:datatype="http://www.w3.org/2001/XMLSchema#string">One of the ancestors of Jesus mentioned in Luke&apos;s geneaology</description>
        <hasOnlyGenealogyMention rdf:datatype="http://www.w3.org/2001/XMLSchema#boolean">true</hasOnlyGenealogyMention>
        <rdfs:label xml:lang="en">Reu</rdfs:label>
    </owl:NamedIndividual>
    


    <!-- http://semanticbible.org/ns/2006/NTNames#Reuben -->

    <owl:NamedIndividual rdf:about="http://semanticbible.org/ns/2006/NTNames#Reuben">
        <rdf:type rdf:resource="http://semanticbible.org/ns/2006/NTNames#Man"/>
        <siblingOf rdf:resource="http://semanticbible.org/ns/2006/NTNames#Gad"/>
        <rdfs:label xml:lang="en">Reuben</rdfs:label>
    </owl:NamedIndividual>
    


    <!-- http://semanticbible.org/ns/2006/NTNames#Rhegium -->

    <owl:NamedIndividual rdf:about="http://semanticbible.org/ns/2006/NTNames#Rhegium">
        <rdf:type rdf:resource="http://semanticbible.org/ns/2006/NTNames#City"/>
        <location rdf:resource="http://semanticbible.org/ns/2006/NTNames#RhegiumGeodata"/>
        <rdfs:label xml:lang="en">Rhegium</rdfs:label>
    </owl:NamedIndividual>
    


    <!-- http://semanticbible.org/ns/2006/NTNames#RhegiumGeodata -->

    <owl:NamedIndividual rdf:about="http://semanticbible.org/ns/2006/NTNames#RhegiumGeodata">
        <rdf:type rdf:resource="http://semanticbible.org/ns/2006/NTNames#GeographicLocation"/>
        <altitude rdf:datatype="http://www.w3.org/2001/XMLSchema#int">0</altitude>
        <latitude rdf:datatype="http://www.w3.org/2001/XMLSchema#double">38.11332514500865</latitude>
        <longitude rdf:datatype="http://www.w3.org/2001/XMLSchema#double">15.64606604911537</longitude>
        <rdfs:label xml:lang="en">geodata for Rhegium</rdfs:label>
    </owl:NamedIndividual>
    


    <!-- http://semanticbible.org/ns/2006/NTNames#Rhesa -->

    <owl:NamedIndividual rdf:about="http://semanticbible.org/ns/2006/NTNames#Rhesa">
        <rdf:type rdf:resource="http://semanticbible.org/ns/2006/NTNames#Man"/>
        <childOf rdf:resource="http://semanticbible.org/ns/2006/NTNames#Zerubbabel"/>
        <ethnicity rdf:resource="http://semanticbible.org/ns/2006/NTNames#Jewish"/>
        <parentOf rdf:resource="http://semanticbible.org/ns/2006/NTNames#Joanan"/>
        <description rdf:datatype="http://www.w3.org/2001/XMLSchema#string">One of the ancestors of Jesus mentioned in Luke&apos;s geneaology</description>
        <hasOnlyGenealogyMention rdf:datatype="http://www.w3.org/2001/XMLSchema#boolean">true</hasOnlyGenealogyMention>
        <rdfs:label xml:lang="en">Rhesa</rdfs:label>
    </owl:NamedIndividual>
    


    <!-- http://semanticbible.org/ns/2006/NTNames#Rhoda -->

    <owl:NamedIndividual rdf:about="http://semanticbible.org/ns/2006/NTNames#Rhoda">
        <rdf:type rdf:resource="http://semanticbible.org/ns/2006/NTNames#Woman"/>
        <knows rdf:resource="http://semanticbible.org/ns/2006/NTNames#MaryMotherOfJohnMark"/>
        <residentPlace rdf:resource="http://semanticbible.org/ns/2006/NTNames#Jerusalem"/>
        <description rdf:datatype="http://www.w3.org/2001/XMLSchema#string">a maid in the house of Mary, mother of John Mark</description>
        <hasOnlyGenealogyMention rdf:datatype="http://www.w3.org/2001/XMLSchema#boolean">false</hasOnlyGenealogyMention>
        <occupation rdf:datatype="http://www.w3.org/2001/XMLSchema#string">maid</occupation>
        <rdfs:comment rdf:datatype="http://www.w3.org/2001/XMLSchema#string">One might infer Rhoda was a Christian because of her mistress&apos; faith, and her joy in seeing Peter after his release.</rdfs:comment>
        <rdfs:label xml:lang="en">Rhoda</rdfs:label>
    </owl:NamedIndividual>
    


    <!-- http://semanticbible.org/ns/2006/NTNames#Rhodes -->

    <owl:NamedIndividual rdf:about="http://semanticbible.org/ns/2006/NTNames#Rhodes">
        <rdf:type rdf:resource="http://semanticbible.org/ns/2006/NTNames#Island"/>
        <location rdf:resource="http://semanticbible.org/ns/2006/NTNames#RhodesGeodata"/>
        <rdfs:label xml:lang="en">Rhodes</rdfs:label>
    </owl:NamedIndividual>
    


    <!-- http://semanticbible.org/ns/2006/NTNames#RhodesGeodata -->

    <owl:NamedIndividual rdf:about="http://semanticbible.org/ns/2006/NTNames#RhodesGeodata">
        <rdf:type rdf:resource="http://semanticbible.org/ns/2006/NTNames#GeographicLocation"/>
        <altitude rdf:datatype="http://www.w3.org/2001/XMLSchema#int">0</altitude>
        <latitude rdf:datatype="http://www.w3.org/2001/XMLSchema#double">36.43927573777137</latitude>
        <longitude rdf:datatype="http://www.w3.org/2001/XMLSchema#double">28.22852638439881</longitude>
        <rdfs:label xml:lang="en">geodata for Rhodes</rdfs:label>
    </owl:NamedIndividual>
    


    <!-- http://semanticbible.org/ns/2006/NTNames#Roman -->

    <owl:NamedIndividual rdf:about="http://semanticbible.org/ns/2006/NTNames#Roman">
        <rdf:type rdf:resource="http://semanticbible.org/ns/2006/NTNames#EthnicityAttribute"/>
        <ethnicityOf rdf:resource="http://semanticbible.org/ns/2006/NTNames#CaesarAugustus"/>
        <ethnicityOf rdf:resource="http://semanticbible.org/ns/2006/NTNames#CaesarNero"/>
        <ethnicityOf rdf:resource="http://semanticbible.org/ns/2006/NTNames#Cornelius"/>
        <ethnicityOf rdf:resource="http://semanticbible.org/ns/2006/NTNames#Felix"/>
        <ethnicityOf rdf:resource="http://semanticbible.org/ns/2006/NTNames#Festus"/>
        <ethnicityOf rdf:resource="http://semanticbible.org/ns/2006/NTNames#Gallio"/>
        <ethnicityOf rdf:resource="http://semanticbible.org/ns/2006/NTNames#TiberiusCaesar"/>
        <rdfs:label xml:lang="en">Roman</rdfs:label>
    </owl:NamedIndividual>
    


    <!-- http://semanticbible.org/ns/2006/NTNames#RomanCitizenship -->

    <owl:NamedIndividual rdf:about="http://semanticbible.org/ns/2006/NTNames#RomanCitizenship">
        <rdf:type rdf:resource="http://semanticbible.org/ns/2006/NTNames#CitizenshipAttribute"/>
        <rdfs:label xml:lang="en">Roman</rdfs:label>
    </owl:NamedIndividual>
    


    <!-- http://semanticbible.org/ns/2006/NTNames#Romans -->

    <owl:NamedIndividual rdf:about="http://semanticbible.org/ns/2006/NTNames#Romans">
        <rdf:type rdf:resource="http://semanticbible.org/ns/2006/NTNames#EthnicGroup"/>
        <rdfs:label xml:lang="en">Romans</rdfs:label>
    </owl:NamedIndividual>
    


    <!-- http://semanticbible.org/ns/2006/NTNames#Rome -->

    <owl:NamedIndividual rdf:about="http://semanticbible.org/ns/2006/NTNames#Rome">
        <rdf:type rdf:resource="http://semanticbible.org/ns/2006/NTNames#City"/>
        <residentPlaceOf rdf:resource="http://semanticbible.org/ns/2006/NTNames#Ampliatus"/>
        <residentPlaceOf rdf:resource="http://semanticbible.org/ns/2006/NTNames#Andronicus"/>
        <residentPlaceOf rdf:resource="http://semanticbible.org/ns/2006/NTNames#Apelles"/>
        <residentPlaceOf rdf:resource="http://semanticbible.org/ns/2006/NTNames#Aquila"/>
        <residentPlaceOf rdf:resource="http://semanticbible.org/ns/2006/NTNames#Aristobulus"/>
        <residentPlaceOf rdf:resource="http://semanticbible.org/ns/2006/NTNames#Asyncritus"/>
        <residentPlaceOf rdf:resource="http://semanticbible.org/ns/2006/NTNames#Claudia"/>
        <residentPlaceOf rdf:resource="http://semanticbible.org/ns/2006/NTNames#Epaenetus"/>
        <residentPlaceOf rdf:resource="http://semanticbible.org/ns/2006/NTNames#Eubulus"/>
        <residentPlaceOf rdf:resource="http://semanticbible.org/ns/2006/NTNames#Hermas"/>
        <residentPlaceOf rdf:resource="http://semanticbible.org/ns/2006/NTNames#Hermes"/>
        <residentPlaceOf rdf:resource="http://semanticbible.org/ns/2006/NTNames#Herodion"/>
        <residentPlaceOf rdf:resource="http://semanticbible.org/ns/2006/NTNames#Julia"/>
        <residentPlaceOf rdf:resource="http://semanticbible.org/ns/2006/NTNames#Junia"/>
        <residentPlaceOf rdf:resource="http://semanticbible.org/ns/2006/NTNames#MaryOfRome"/>
        <residentPlaceOf rdf:resource="http://semanticbible.org/ns/2006/NTNames#Narcissus"/>
        <residentPlaceOf rdf:resource="http://semanticbible.org/ns/2006/NTNames#Nereus"/>
        <residentPlaceOf rdf:resource="http://semanticbible.org/ns/2006/NTNames#Olympas"/>
        <residentPlaceOf rdf:resource="http://semanticbible.org/ns/2006/NTNames#Patrobas"/>
        <residentPlaceOf rdf:resource="http://semanticbible.org/ns/2006/NTNames#Persis"/>
        <residentPlaceOf rdf:resource="http://semanticbible.org/ns/2006/NTNames#Philologus"/>
        <residentPlaceOf rdf:resource="http://semanticbible.org/ns/2006/NTNames#Phlegon"/>
        <residentPlaceOf rdf:resource="http://semanticbible.org/ns/2006/NTNames#Priscilla"/>
        <residentPlaceOf rdf:resource="http://semanticbible.org/ns/2006/NTNames#RufusOfRome"/>
        <residentPlaceOf rdf:resource="http://semanticbible.org/ns/2006/NTNames#Stachys"/>
        <residentPlaceOf rdf:resource="http://semanticbible.org/ns/2006/NTNames#Tryphaena"/>
        <residentPlaceOf rdf:resource="http://semanticbible.org/ns/2006/NTNames#Tryphosa"/>
        <residentPlaceOf rdf:resource="http://semanticbible.org/ns/2006/NTNames#Urbanus"/>
        <rdfs:label xml:lang="en">Rome</rdfs:label>
    </owl:NamedIndividual>
    


    <!-- http://semanticbible.org/ns/2006/NTNames#Rufus -->

    <owl:NamedIndividual rdf:about="http://semanticbible.org/ns/2006/NTNames#Rufus">
        <rdf:type rdf:resource="http://semanticbible.org/ns/2006/NTNames#Man"/>
        <childOf rdf:resource="http://semanticbible.org/ns/2006/NTNames#SimonOfCyrene"/>
        <knows rdf:resource="http://semanticbible.org/ns/2006/NTNames#Priscilla"/>
        <possiblySamePersonAs rdf:resource="http://semanticbible.org/ns/2006/NTNames#RufusOfRome"/>
        <siblingOf rdf:resource="http://semanticbible.org/ns/2006/NTNames#Alexander"/>
        <rdfs:label xml:lang="en">Rufus</rdfs:label>
    </owl:NamedIndividual>
    


    <!-- http://semanticbible.org/ns/2006/NTNames#RufusOfRome -->

    <owl:NamedIndividual rdf:about="http://semanticbible.org/ns/2006/NTNames#RufusOfRome">
        <rdf:type rdf:resource="http://semanticbible.org/ns/2006/NTNames#Man"/>
        <knows rdf:resource="http://semanticbible.org/ns/2006/NTNames#Paul"/>
        <possiblySamePersonAs rdf:resource="http://semanticbible.org/ns/2006/NTNames#Rufus"/>
        <religiousBelief rdf:resource="http://semanticbible.org/ns/2006/NTNames#Christianity"/>
        <residentPlace rdf:resource="http://semanticbible.org/ns/2006/NTNames#Rome"/>
        <hasOnlyGenealogyMention rdf:datatype="http://www.w3.org/2001/XMLSchema#boolean">false</hasOnlyGenealogyMention>
        <rdfs:comment rdf:datatype="http://www.w3.org/2001/XMLSchema#string">There are no firm grounds for identifying this Rufus as the same person as the son of Simon of Cyrene mentioned in Mark 15 (though the tradition that Mark&apos;s Gospel was written in Rome makes this an intriguing possibility). </rdfs:comment>
    </owl:NamedIndividual>
    


    <!-- http://semanticbible.org/ns/2006/NTNames#Ruth -->

    <owl:NamedIndividual rdf:about="http://semanticbible.org/ns/2006/NTNames#Ruth">
        <rdf:type rdf:resource="http://semanticbible.org/ns/2006/NTNames#Woman"/>
        <ethnicity rdf:resource="http://semanticbible.org/ns/2006/NTNames#Moabite"/>
        <parentOf rdf:resource="http://semanticbible.org/ns/2006/NTNames#Obed"/>
        <spouseOf rdf:resource="http://semanticbible.org/ns/2006/NTNames#Boaz"/>
        <description rdf:datatype="http://www.w3.org/2001/XMLSchema#string">an ancestor of King David in Matthew&apos;s genealogy of Jesus</description>
        <hasOnlyGenealogyMention rdf:datatype="http://www.w3.org/2001/XMLSchema#boolean">true</hasOnlyGenealogyMention>
        <rdfs:comment xml:lang="en">An Old Testament figure</rdfs:comment>
        <rdfs:label xml:lang="en">Ruth</rdfs:label>
    </owl:NamedIndividual>
    


    <!-- http://semanticbible.org/ns/2006/NTNames#Sabbath -->

    <owl:NamedIndividual rdf:about="http://semanticbible.org/ns/2006/NTNames#Sabbath">
        <rdf:type rdf:resource="http://semanticbible.org/ns/2006/NTNames#FixedHoliday"/>
        <rdfs:label xml:lang="en">Sabbath</rdfs:label>
    </owl:NamedIndividual>
    


    <!-- http://semanticbible.org/ns/2006/NTNames#Sadduceanism -->

    <owl:NamedIndividual rdf:about="http://semanticbible.org/ns/2006/NTNames#Sadduceanism">
        <rdf:type rdf:resource="http://semanticbible.org/ns/2006/NTNames#ReligiousBeliefSystem"/>
        <rdfs:comment xml:lang="en">The beliefs of one of the main Jewish sects during the life of Jesus. In the New Testament the name of the sect is used, though not the belief system per se.</rdfs:comment>
        <rdfs:label xml:lang="en">Sadduceanism</rdfs:label>
    </owl:NamedIndividual>
    


    <!-- http://semanticbible.org/ns/2006/NTNames#Sadducees -->

    <owl:NamedIndividual rdf:about="http://semanticbible.org/ns/2006/NTNames#Sadducees">
        <rdf:type rdf:resource="http://semanticbible.org/ns/2006/NTNames#ReligiousOrganization"/>
        <rdfs:label xml:lang="en">Sadducees</rdfs:label>
    </owl:NamedIndividual>
    


    <!-- http://semanticbible.org/ns/2006/NTNames#Salamis -->

    <owl:NamedIndividual rdf:about="http://semanticbible.org/ns/2006/NTNames#Salamis">
        <rdf:type rdf:resource="http://semanticbible.org/ns/2006/NTNames#City"/>
        <location rdf:resource="http://semanticbible.org/ns/2006/NTNames#SalamisGeodata"/>
        <rdfs:label xml:lang="en">Salamis</rdfs:label>
    </owl:NamedIndividual>
    


    <!-- http://semanticbible.org/ns/2006/NTNames#SalamisGeodata -->

    <owl:NamedIndividual rdf:about="http://semanticbible.org/ns/2006/NTNames#SalamisGeodata">
        <rdf:type rdf:resource="http://semanticbible.org/ns/2006/NTNames#GeographicLocation"/>
        <altitude rdf:datatype="http://www.w3.org/2001/XMLSchema#int">0</altitude>
        <latitude rdf:datatype="http://www.w3.org/2001/XMLSchema#double">35.14774697653193</latitude>
        <longitude rdf:datatype="http://www.w3.org/2001/XMLSchema#double">33.85186619255565</longitude>
        <rdfs:label xml:lang="en">geodata for Salamis</rdfs:label>
    </owl:NamedIndividual>
    


    <!-- http://semanticbible.org/ns/2006/NTNames#Salem -->

    <owl:NamedIndividual rdf:about="http://semanticbible.org/ns/2006/NTNames#Salem">
        <rdf:type rdf:resource="http://semanticbible.org/ns/2006/NTNames#City"/>
        <location rdf:resource="http://semanticbible.org/ns/2006/NTNames#SalemGeodata"/>
        <rdfs:comment rdf:datatype="http://www.w3.org/2001/XMLSchema#string">Geodata assumes this is an earlier name for Jerusalem, though this is not certain. </rdfs:comment>
        <rdfs:label xml:lang="en">Salem</rdfs:label>
    </owl:NamedIndividual>
    


    <!-- http://semanticbible.org/ns/2006/NTNames#SalemGeodata -->

    <owl:NamedIndividual rdf:about="http://semanticbible.org/ns/2006/NTNames#SalemGeodata">
        <rdf:type rdf:resource="http://semanticbible.org/ns/2006/NTNames#GeographicLocation"/>
        <altitude rdf:datatype="http://www.w3.org/2001/XMLSchema#int">0</altitude>
        <latitude rdf:datatype="http://www.w3.org/2001/XMLSchema#double">31.77451070780678</latitude>
        <longitude rdf:datatype="http://www.w3.org/2001/XMLSchema#double">35.22395850823153</longitude>
        <rdfs:label xml:lang="en">geodata for Salem</rdfs:label>
    </owl:NamedIndividual>
    


    <!-- http://semanticbible.org/ns/2006/NTNames#Salim -->

    <owl:NamedIndividual rdf:about="http://semanticbible.org/ns/2006/NTNames#Salim">
        <rdf:type rdf:resource="http://semanticbible.org/ns/2006/NTNames#City"/>
        <location rdf:resource="http://semanticbible.org/ns/2006/NTNames#SalimGeodata"/>
        <rdfs:label xml:lang="en">Salim</rdfs:label>
    </owl:NamedIndividual>
    


    <!-- http://semanticbible.org/ns/2006/NTNames#SalimGeodata -->

    <owl:NamedIndividual rdf:about="http://semanticbible.org/ns/2006/NTNames#SalimGeodata">
        <rdf:type rdf:resource="http://semanticbible.org/ns/2006/NTNames#GeographicLocation"/>
        <altitude rdf:datatype="http://www.w3.org/2001/XMLSchema#int">0</altitude>
        <latitude rdf:datatype="http://www.w3.org/2001/XMLSchema#double">32.39607055991332</latitude>
        <longitude rdf:datatype="http://www.w3.org/2001/XMLSchema#double">35.53870968584208</longitude>
        <rdfs:label xml:lang="en">geodata for Salim</rdfs:label>
    </owl:NamedIndividual>
    


    <!-- http://semanticbible.org/ns/2006/NTNames#Salmon -->

    <owl:NamedIndividual rdf:about="http://semanticbible.org/ns/2006/NTNames#Salmon">
        <rdf:type rdf:resource="http://semanticbible.org/ns/2006/NTNames#Man"/>
        <childOf rdf:resource="http://semanticbible.org/ns/2006/NTNames#Nahshon"/>
        <ethnicity rdf:resource="http://semanticbible.org/ns/2006/NTNames#Jewish"/>
        <parentOf rdf:resource="http://semanticbible.org/ns/2006/NTNames#Boaz"/>
        <spouseOf rdf:resource="http://semanticbible.org/ns/2006/NTNames#Rahab"/>
        <description rdf:datatype="http://www.w3.org/2001/XMLSchema#string">One of the ancestors of Jesus mentioned in Matthew and Luke&apos;s geneaologies</description>
        <hasOnlyGenealogyMention rdf:datatype="http://www.w3.org/2001/XMLSchema#boolean">true</hasOnlyGenealogyMention>
        <rdfs:comment rdf:datatype="http://www.w3.org/2001/XMLSchema#string">Luke&apos;s genealogy has Sala, a minor variant, but the relationships make clear it is the same person.</rdfs:comment>
        <rdfs:label xml:lang="en">Salmon</rdfs:label>
    </owl:NamedIndividual>
    


    <!-- http://semanticbible.org/ns/2006/NTNames#Salmone -->

    <owl:NamedIndividual rdf:about="http://semanticbible.org/ns/2006/NTNames#Salmone">
        <rdf:type rdf:resource="http://semanticbible.org/ns/2006/NTNames#LandArea"/>
        <location rdf:resource="http://semanticbible.org/ns/2006/NTNames#SalmoneGeodata"/>
        <rdfs:label xml:lang="en">Salmone</rdfs:label>
    </owl:NamedIndividual>
    


    <!-- http://semanticbible.org/ns/2006/NTNames#SalmoneGeodata -->

    <owl:NamedIndividual rdf:about="http://semanticbible.org/ns/2006/NTNames#SalmoneGeodata">
        <rdf:type rdf:resource="http://semanticbible.org/ns/2006/NTNames#GeographicLocation"/>
        <altitude rdf:datatype="http://www.w3.org/2001/XMLSchema#int">0</altitude>
        <latitude rdf:datatype="http://www.w3.org/2001/XMLSchema#double">35.20497664329137</latitude>
        <longitude rdf:datatype="http://www.w3.org/2001/XMLSchema#double">25.98384834966224</longitude>
        <rdfs:label xml:lang="en">geodata for Salmone</rdfs:label>
    </owl:NamedIndividual>
    


    <!-- http://semanticbible.org/ns/2006/NTNames#Salome -->

    <owl:NamedIndividual rdf:about="http://semanticbible.org/ns/2006/NTNames#Salome">
        <rdf:type rdf:resource="http://semanticbible.org/ns/2006/NTNames#Woman"/>
        <collaboratesWith rdf:resource="http://semanticbible.org/ns/2006/NTNames#Jesus"/>
        <knows rdf:resource="http://semanticbible.org/ns/2006/NTNames#MaryMagdalene"/>
        <knows rdf:resource="http://semanticbible.org/ns/2006/NTNames#MaryWifeOfClopas"/>
        <parentOf rdf:resource="http://semanticbible.org/ns/2006/NTNames#JamesSonOfZebedee"/>
        <parentOf rdf:resource="http://semanticbible.org/ns/2006/NTNames#JohnSonOfZebedee"/>
        <religiousBelief rdf:resource="http://semanticbible.org/ns/2006/NTNames#Christianity"/>
        <spouseOf rdf:resource="http://semanticbible.org/ns/2006/NTNames#Zebedee"/>
        <description rdf:datatype="http://www.w3.org/2001/XMLSchema#string">one of the woman who came to annoint Jesus&apos; body after his crucifixion</description>
        <hasOnlyGenealogyMention rdf:datatype="http://www.w3.org/2001/XMLSchema#boolean">false</hasOnlyGenealogyMention>
        <rdfs:comment xml:lang="en">Matthew and Mark&apos;s accounts of the crucifixion together identify Salome as the mother of the sons of Zebedee. 
This is also the traditional name of the daughter of Herodias, whose dance before King Herod led to the beheading of John the Baptist. But this woman is not named in the New Testament. </rdfs:comment>
        <rdfs:label xml:lang="en">Salome</rdfs:label>
    </owl:NamedIndividual>
    


    <!-- http://semanticbible.org/ns/2006/NTNames#Samaria -->

    <owl:NamedIndividual rdf:about="http://semanticbible.org/ns/2006/NTNames#Samaria">
        <rdf:type rdf:resource="http://semanticbible.org/ns/2006/NTNames#StateOrProvince"/>
        <location rdf:resource="http://semanticbible.org/ns/2006/NTNames#SamariaGeodata"/>
        <subregion rdf:resource="http://semanticbible.org/ns/2006/NTNames#Caesarea"/>
        <subregion rdf:resource="http://semanticbible.org/ns/2006/NTNames#SamariaTheCity"/>
        <subregion rdf:resource="http://semanticbible.org/ns/2006/NTNames#Sychar"/>
        <subregionOf rdf:resource="http://semanticbible.org/ns/2006/NTNames#Israel"/>
        <rdfs:label xml:lang="en">Samaria</rdfs:label>
    </owl:NamedIndividual>
    


    <!-- http://semanticbible.org/ns/2006/NTNames#SamariaGeodata -->

    <owl:NamedIndividual rdf:about="http://semanticbible.org/ns/2006/NTNames#SamariaGeodata">
        <rdf:type rdf:resource="http://semanticbible.org/ns/2006/NTNames#GeographicLocation"/>
        <altitude rdf:datatype="http://www.w3.org/2001/XMLSchema#int">0</altitude>
        <latitude rdf:datatype="http://www.w3.org/2001/XMLSchema#double">32.27767116198458</latitude>
        <longitude rdf:datatype="http://www.w3.org/2001/XMLSchema#double">35.1986186525302</longitude>
        <rdfs:comment xml:lang="en">This may be overly precise positioning for a region</rdfs:comment>
        <rdfs:label xml:lang="en">geodata for Samaria</rdfs:label>
    </owl:NamedIndividual>
    


    <!-- http://semanticbible.org/ns/2006/NTNames#SamariaTheCity -->

    <owl:NamedIndividual rdf:about="http://semanticbible.org/ns/2006/NTNames#SamariaTheCity">
        <rdf:type rdf:resource="http://semanticbible.org/ns/2006/NTNames#City"/>
        <subregionOf rdf:resource="http://semanticbible.org/ns/2006/NTNames#Samaria"/>
        <rdfs:comment xml:lang="en">Samaria was both a province in Palestine and a city of the same name.</rdfs:comment>
        <rdfs:label xml:lang="en">Samaria</rdfs:label>
    </owl:NamedIndividual>
    


    <!-- http://semanticbible.org/ns/2006/NTNames#Samaritan -->

    <owl:NamedIndividual rdf:about="http://semanticbible.org/ns/2006/NTNames#Samaritan">
        <rdf:type rdf:resource="http://semanticbible.org/ns/2006/NTNames#EthnicityAttribute"/>
        <ethnicityOf rdf:resource="http://semanticbible.org/ns/2006/NTNames#HerodAntipas"/>
        <rdfs:comment xml:lang="en">A Jewish sect centered around the city of Samaria: in New Testament times, there was great emnity between Samaritans and Jews.</rdfs:comment>
        <rdfs:label xml:lang="en">Samaritan</rdfs:label>
    </owl:NamedIndividual>
    


    <!-- http://semanticbible.org/ns/2006/NTNames#Samaritans -->

    <owl:NamedIndividual rdf:about="http://semanticbible.org/ns/2006/NTNames#Samaritans">
        <rdf:type rdf:resource="http://semanticbible.org/ns/2006/NTNames#EthnicGroup"/>
        <rdfs:label xml:lang="en">Samaritans</rdfs:label>
    </owl:NamedIndividual>
    


    <!-- http://semanticbible.org/ns/2006/NTNames#Samos -->

    <owl:NamedIndividual rdf:about="http://semanticbible.org/ns/2006/NTNames#Samos">
        <rdf:type rdf:resource="http://semanticbible.org/ns/2006/NTNames#Island"/>
        <rdfs:label xml:lang="en">Samos</rdfs:label>
    </owl:NamedIndividual>
    


    <!-- http://semanticbible.org/ns/2006/NTNames#Samothrace -->

    <owl:NamedIndividual rdf:about="http://semanticbible.org/ns/2006/NTNames#Samothrace">
        <rdf:type rdf:resource="http://semanticbible.org/ns/2006/NTNames#Island"/>
        <rdfs:label xml:lang="en">Samothrace</rdfs:label>
    </owl:NamedIndividual>
    


    <!-- http://semanticbible.org/ns/2006/NTNames#Samson -->

    <owl:NamedIndividual rdf:about="http://semanticbible.org/ns/2006/NTNames#Samson">
        <rdf:type rdf:resource="http://semanticbible.org/ns/2006/NTNames#Man"/>
        <rdfs:label xml:lang="en">Samson</rdfs:label>
    </owl:NamedIndividual>
    


    <!-- http://semanticbible.org/ns/2006/NTNames#Samuel -->

    <owl:NamedIndividual rdf:about="http://semanticbible.org/ns/2006/NTNames#Samuel">
        <rdf:type rdf:resource="http://semanticbible.org/ns/2006/NTNames#Man"/>
        <rdfs:label xml:lang="en">Samuel</rdfs:label>
    </owl:NamedIndividual>
    


    <!-- http://semanticbible.org/ns/2006/NTNames#Sanhedrin -->

    <owl:NamedIndividual rdf:about="http://semanticbible.org/ns/2006/NTNames#Sanhedrin">
        <rdf:type rdf:resource="http://semanticbible.org/ns/2006/NTNames#ReligiousOrganization"/>
        <member rdf:resource="http://semanticbible.org/ns/2006/NTNames#AlexanderOfTheSanhedrin"/>
        <member rdf:resource="http://semanticbible.org/ns/2006/NTNames#AnaniasTheHighPriest"/>
        <member rdf:resource="http://semanticbible.org/ns/2006/NTNames#Annas"/>
        <member rdf:resource="http://semanticbible.org/ns/2006/NTNames#Gamaliel"/>
        <member rdf:resource="http://semanticbible.org/ns/2006/NTNames#JohnOfTheSanhedrin"/>
        <rdfs:comment xml:lang="en">The Jewish supreme council</rdfs:comment>
        <rdfs:label xml:lang="en">Sanhedrin</rdfs:label>
    </owl:NamedIndividual>
    


    <!-- http://semanticbible.org/ns/2006/NTNames#Sapphira -->

    <owl:NamedIndividual rdf:about="http://semanticbible.org/ns/2006/NTNames#Sapphira">
        <rdf:type rdf:resource="http://semanticbible.org/ns/2006/NTNames#Woman"/>
        <ethnicity rdf:resource="http://semanticbible.org/ns/2006/NTNames#Jewish"/>
        <hasAntagonist rdf:resource="http://semanticbible.org/ns/2006/NTNames#SimonPeter"/>
        <knows rdf:resource="http://semanticbible.org/ns/2006/NTNames#SimonPeter"/>
        <religiousBelief rdf:resource="http://semanticbible.org/ns/2006/NTNames#Christianity"/>
        <residentPlace rdf:resource="http://semanticbible.org/ns/2006/NTNames#Jerusalem"/>
        <spouseOf rdf:resource="http://semanticbible.org/ns/2006/NTNames#Ananias"/>
        <description rdf:datatype="http://www.w3.org/2001/XMLSchema#string">a member of the early church who misrepresented a gift and died as a 
    consequence</description>
        <hasOnlyGenealogyMention rdf:datatype="http://www.w3.org/2001/XMLSchema#boolean">false</hasOnlyGenealogyMention>
        <rdfs:label xml:lang="en">Sapphira</rdfs:label>
    </owl:NamedIndividual>
    


    <!-- http://semanticbible.org/ns/2006/NTNames#Sarah -->

    <owl:NamedIndividual rdf:about="http://semanticbible.org/ns/2006/NTNames#Sarah">
        <rdf:type rdf:resource="http://semanticbible.org/ns/2006/NTNames#Woman"/>
        <antagonistOf rdf:resource="http://semanticbible.org/ns/2006/NTNames#Hagar"/>
        <childOf rdf:resource="http://semanticbible.org/ns/2006/NTNames#Terah"/>
        <ethnicity rdf:resource="http://semanticbible.org/ns/2006/NTNames#Jewish"/>
        <hasAntagonist rdf:resource="http://semanticbible.org/ns/2006/NTNames#Hagar"/>
        <parentOf rdf:resource="http://semanticbible.org/ns/2006/NTNames#Isaac"/>
        <residentPlace rdf:resource="http://semanticbible.org/ns/2006/NTNames#Canaan"/>
        <spouseOf rdf:resource="http://semanticbible.org/ns/2006/NTNames#Abraham"/>
        <description rdf:datatype="http://www.w3.org/2001/XMLSchema#string">the wife of Abraham and an example of faith</description>
        <hasOnlyGenealogyMention rdf:datatype="http://www.w3.org/2001/XMLSchema#boolean">false</hasOnlyGenealogyMention>
        <rdfs:comment xml:lang="en">An important Old Testament figure. Curiously enough, both Abraham and Sarah are described as having Terah as father, presumably by different mothers. </rdfs:comment>
        <rdfs:label xml:lang="en">Sarah</rdfs:label>
    </owl:NamedIndividual>
    


    <!-- http://semanticbible.org/ns/2006/NTNames#Sardis -->

    <owl:NamedIndividual rdf:about="http://semanticbible.org/ns/2006/NTNames#Sardis">
        <rdf:type rdf:resource="http://semanticbible.org/ns/2006/NTNames#City"/>
        <location rdf:resource="http://semanticbible.org/ns/2006/NTNames#SardisGeodata"/>
        <rdfs:label xml:lang="en">Sardis</rdfs:label>
    </owl:NamedIndividual>
    


    <!-- http://semanticbible.org/ns/2006/NTNames#SardisGeodata -->

    <owl:NamedIndividual rdf:about="http://semanticbible.org/ns/2006/NTNames#SardisGeodata">
        <rdf:type rdf:resource="http://semanticbible.org/ns/2006/NTNames#GeographicLocation"/>
        <altitude rdf:datatype="http://www.w3.org/2001/XMLSchema#int">0</altitude>
        <latitude rdf:datatype="http://www.w3.org/2001/XMLSchema#double">38.48410261177621</latitude>
        <longitude rdf:datatype="http://www.w3.org/2001/XMLSchema#double">28.11569681314403</longitude>
        <rdfs:label xml:lang="en">geodata for Sardis</rdfs:label>
    </owl:NamedIndividual>
    


    <!-- http://semanticbible.org/ns/2006/NTNames#Satan -->

    <owl:NamedIndividual rdf:about="http://semanticbible.org/ns/2006/NTNames#Satan">
        <rdf:type rdf:resource="http://semanticbible.org/ns/2006/NTNames#EvilSupernaturalBeing"/>
        <rdfs:label xml:lang="en">Satan</rdfs:label>
    </owl:NamedIndividual>
    


    <!-- http://semanticbible.org/ns/2006/NTNames#SaulSonOfKish -->

    <owl:NamedIndividual rdf:about="http://semanticbible.org/ns/2006/NTNames#SaulSonOfKish">
        <rdf:type rdf:resource="http://semanticbible.org/ns/2006/NTNames#Man"/>
        <childOf rdf:resource="http://semanticbible.org/ns/2006/NTNames#Kish"/>
        <memberOf rdf:resource="http://semanticbible.org/ns/2006/NTNames#TribeOfBenjamin"/>
        <occupation rdf:datatype="http://www.w3.org/2001/XMLSchema#string">King of Israel</occupation>
        <rdfs:label xml:lang="en">Saul</rdfs:label>
    </owl:NamedIndividual>
    


    <!-- http://semanticbible.org/ns/2006/NTNames#Sceva -->

    <owl:NamedIndividual rdf:about="http://semanticbible.org/ns/2006/NTNames#Sceva">
        <rdf:type rdf:resource="http://semanticbible.org/ns/2006/NTNames#Man"/>
        <rdfs:label xml:lang="en">Sceva</rdfs:label>
    </owl:NamedIndividual>
    


    <!-- http://semanticbible.org/ns/2006/NTNames#Scripture -->

    <owl:NamedIndividual rdf:about="http://semanticbible.org/ns/2006/NTNames#Scripture">
        <rdf:type rdf:resource="http://semanticbible.org/ns/2006/NTNames#Series"/>
        <rdfs:label xml:lang="en">Scripture</rdfs:label>
    </owl:NamedIndividual>
    


    <!-- http://semanticbible.org/ns/2006/NTNames#Scriptures -->

    <owl:NamedIndividual rdf:about="http://semanticbible.org/ns/2006/NTNames#Scriptures">
        <rdf:type rdf:resource="http://semanticbible.org/ns/2006/NTNames#Series"/>
        <rdfs:label xml:lang="en">Scriptures</rdfs:label>
    </owl:NamedIndividual>
    


    <!-- http://semanticbible.org/ns/2006/NTNames#Scythian -->

    <owl:NamedIndividual rdf:about="http://semanticbible.org/ns/2006/NTNames#Scythian">
        <rdf:type rdf:resource="http://semanticbible.org/ns/2006/NTNames#EthnicityAttribute"/>
        <rdfs:comment xml:lang="en">Herodotus describes the Scythians as a savage race of nomads, living generally north of the Black and Caspain Seas. Paul&apos;s single use of the term seems largely synonymous with them as a type of barbarians. </rdfs:comment>
        <rdfs:label xml:lang="en">Scythian</rdfs:label>
    </owl:NamedIndividual>
    


    <!-- http://semanticbible.org/ns/2006/NTNames#SeaOfGalilee -->

    <owl:NamedIndividual rdf:about="http://semanticbible.org/ns/2006/NTNames#SeaOfGalilee">
        <rdf:type rdf:resource="http://semanticbible.org/ns/2006/NTNames#FreshWaterArea"/>
        <location rdf:resource="http://semanticbible.org/ns/2006/NTNames#SeaofGalileeGeodata"/>
        <subregionOf rdf:resource="http://semanticbible.org/ns/2006/NTNames#Galilee"/>
        <rdfs:label xml:lang="en">Sea of Galilee</rdfs:label>
    </owl:NamedIndividual>
    


    <!-- http://semanticbible.org/ns/2006/NTNames#SeaofGalileeGeodata -->

    <owl:NamedIndividual rdf:about="http://semanticbible.org/ns/2006/NTNames#SeaofGalileeGeodata">
        <rdf:type rdf:resource="http://semanticbible.org/ns/2006/NTNames#GeographicLocation"/>
        <altitude rdf:datatype="http://www.w3.org/2001/XMLSchema#int">0</altitude>
        <latitude rdf:datatype="http://www.w3.org/2001/XMLSchema#double">32.77589768765405</latitude>
        <longitude rdf:datatype="http://www.w3.org/2001/XMLSchema#double">35.59041519244655</longitude>
        <rdfs:label xml:lang="en">geodata for Sea of Galilee</rdfs:label>
    </owl:NamedIndividual>
    


    <!-- http://semanticbible.org/ns/2006/NTNames#Secundus -->

    <owl:NamedIndividual rdf:about="http://semanticbible.org/ns/2006/NTNames#Secundus">
        <rdf:type rdf:resource="http://semanticbible.org/ns/2006/NTNames#Man"/>
        <collaboratesWith rdf:resource="http://semanticbible.org/ns/2006/NTNames#Aristarchus"/>
        <collaboratesWith rdf:resource="http://semanticbible.org/ns/2006/NTNames#GaiusOfDerbe"/>
        <collaboratesWith rdf:resource="http://semanticbible.org/ns/2006/NTNames#Paul"/>
        <collaboratesWith rdf:resource="http://semanticbible.org/ns/2006/NTNames#Sopater"/>
        <collaboratesWith rdf:resource="http://semanticbible.org/ns/2006/NTNames#Timothy"/>
        <collaboratesWith rdf:resource="http://semanticbible.org/ns/2006/NTNames#Trophimus"/>
        <collaboratesWith rdf:resource="http://semanticbible.org/ns/2006/NTNames#Tychicus"/>
        <religiousBelief rdf:resource="http://semanticbible.org/ns/2006/NTNames#Christianity"/>
        <residentPlace rdf:resource="http://semanticbible.org/ns/2006/NTNames#Thessalonica"/>
        <description rdf:datatype="http://www.w3.org/2001/XMLSchema#string">a Thessalonian companion of Paul&apos;s</description>
        <hasOnlyGenealogyMention rdf:datatype="http://www.w3.org/2001/XMLSchema#boolean">false</hasOnlyGenealogyMention>
        <rdfs:comment rdf:datatype="http://www.w3.org/2001/XMLSchema#string">Luke describes him as &quot;of the Thessalonians&quot;, which could mean either his residence or his origin. </rdfs:comment>
        <rdfs:label xml:lang="en">Secundus</rdfs:label>
    </owl:NamedIndividual>
    


    <!-- http://semanticbible.org/ns/2006/NTNames#Seleucia -->

    <owl:NamedIndividual rdf:about="http://semanticbible.org/ns/2006/NTNames#Seleucia">
        <rdf:type rdf:resource="http://semanticbible.org/ns/2006/NTNames#City"/>
        <location rdf:resource="http://semanticbible.org/ns/2006/NTNames#SeleuciaGeodata"/>
        <rdfs:label xml:lang="en">Seleucia</rdfs:label>
    </owl:NamedIndividual>
    


    <!-- http://semanticbible.org/ns/2006/NTNames#SeleuciaGeodata -->

    <owl:NamedIndividual rdf:about="http://semanticbible.org/ns/2006/NTNames#SeleuciaGeodata">
        <rdf:type rdf:resource="http://semanticbible.org/ns/2006/NTNames#GeographicLocation"/>
        <altitude rdf:datatype="http://www.w3.org/2001/XMLSchema#int">0</altitude>
        <latitude rdf:datatype="http://www.w3.org/2001/XMLSchema#double">36.12957722548538</latitude>
        <longitude rdf:datatype="http://www.w3.org/2001/XMLSchema#double">35.93980304207995</longitude>
        <rdfs:label xml:lang="en">geodata for Seleucia</rdfs:label>
    </owl:NamedIndividual>
    


    <!-- http://semanticbible.org/ns/2006/NTNames#Semein -->

    <owl:NamedIndividual rdf:about="http://semanticbible.org/ns/2006/NTNames#Semein">
        <rdf:type rdf:resource="http://semanticbible.org/ns/2006/NTNames#Man"/>
        <childOf rdf:resource="http://semanticbible.org/ns/2006/NTNames#Josech"/>
        <ethnicity rdf:resource="http://semanticbible.org/ns/2006/NTNames#Jewish"/>
        <parentOf rdf:resource="http://semanticbible.org/ns/2006/NTNames#MattathiasSonOfSemein"/>
        <description rdf:datatype="http://www.w3.org/2001/XMLSchema#string">One of the ancestors of Jesus mentioned in Luke&apos;s geneaology</description>
        <hasOnlyGenealogyMention rdf:datatype="http://www.w3.org/2001/XMLSchema#boolean">true</hasOnlyGenealogyMention>
        <rdfs:label xml:lang="en">Semein</rdfs:label>
    </owl:NamedIndividual>
    


    <!-- http://semanticbible.org/ns/2006/NTNames#SergiusPaulus -->

    <owl:NamedIndividual rdf:about="http://semanticbible.org/ns/2006/NTNames#SergiusPaulus">
        <rdf:type rdf:resource="http://semanticbible.org/ns/2006/NTNames#Man"/>
        <knows rdf:resource="http://semanticbible.org/ns/2006/NTNames#Bar-Jesus"/>
        <knows rdf:resource="http://semanticbible.org/ns/2006/NTNames#Paul"/>
        <knows rdf:resource="http://semanticbible.org/ns/2006/NTNames#Silas"/>
        <description rdf:datatype="http://www.w3.org/2001/XMLSchema#string">procounsul of Cyprus and &apos;a man of intelligence&apos;</description>
        <occupation rdf:datatype="http://www.w3.org/2001/XMLSchema#string">procounsul</occupation>
        <rdfs:label xml:lang="en">Sergius Paulus</rdfs:label>
    </owl:NamedIndividual>
    


    <!-- http://semanticbible.org/ns/2006/NTNames#Serug -->

    <owl:NamedIndividual rdf:about="http://semanticbible.org/ns/2006/NTNames#Serug">
        <rdf:type rdf:resource="http://semanticbible.org/ns/2006/NTNames#Man"/>
        <childOf rdf:resource="http://semanticbible.org/ns/2006/NTNames#Reu"/>
        <parentOf rdf:resource="http://semanticbible.org/ns/2006/NTNames#Nahor"/>
        <description rdf:datatype="http://www.w3.org/2001/XMLSchema#string">One of the ancestors of Jesus mentioned in Luke&apos;s geneaology</description>
        <hasOnlyGenealogyMention rdf:datatype="http://www.w3.org/2001/XMLSchema#boolean">true</hasOnlyGenealogyMention>
        <rdfs:label xml:lang="en">Serug</rdfs:label>
    </owl:NamedIndividual>
    


    <!-- http://semanticbible.org/ns/2006/NTNames#Seth -->

    <owl:NamedIndividual rdf:about="http://semanticbible.org/ns/2006/NTNames#Seth">
        <rdf:type rdf:resource="http://semanticbible.org/ns/2006/NTNames#Man"/>
        <childOf rdf:resource="http://semanticbible.org/ns/2006/NTNames#Adam"/>
        <parentOf rdf:resource="http://semanticbible.org/ns/2006/NTNames#Enos"/>
        <hasOnlyGenealogyMention rdf:datatype="http://www.w3.org/2001/XMLSchema#boolean">true</hasOnlyGenealogyMention>
        <rdfs:label xml:lang="en">Seth</rdfs:label>
    </owl:NamedIndividual>
    


    <!-- http://semanticbible.org/ns/2006/NTNames#Sharon -->

    <owl:NamedIndividual rdf:about="http://semanticbible.org/ns/2006/NTNames#Sharon">
        <rdf:type rdf:resource="http://semanticbible.org/ns/2006/NTNames#LandArea"/>
        <subregionOf rdf:resource="http://semanticbible.org/ns/2006/NTNames#Judea"/>
        <rdfs:label xml:lang="en">Sharon</rdfs:label>
    </owl:NamedIndividual>
    


    <!-- http://semanticbible.org/ns/2006/NTNames#Shealtiel -->

    <owl:NamedIndividual rdf:about="http://semanticbible.org/ns/2006/NTNames#Shealtiel">
        <rdf:type rdf:resource="http://semanticbible.org/ns/2006/NTNames#Man"/>
        <childOf rdf:resource="http://semanticbible.org/ns/2006/NTNames#Jechoniah"/>
        <ethnicity rdf:resource="http://semanticbible.org/ns/2006/NTNames#Jewish"/>
        <parentOf rdf:resource="http://semanticbible.org/ns/2006/NTNames#Zerubbabel"/>
        <hasOnlyGenealogyMention rdf:datatype="http://www.w3.org/2001/XMLSchema#boolean">true</hasOnlyGenealogyMention>
        <rdfs:label xml:lang="en">Shealtiel</rdfs:label>
    </owl:NamedIndividual>
    


    <!-- http://semanticbible.org/ns/2006/NTNames#ShealtielSonOfNeri -->

    <owl:NamedIndividual rdf:about="http://semanticbible.org/ns/2006/NTNames#ShealtielSonOfNeri">
        <rdf:type rdf:resource="http://semanticbible.org/ns/2006/NTNames#Man"/>
        <childOf rdf:resource="http://semanticbible.org/ns/2006/NTNames#Neri"/>
        <ethnicity rdf:resource="http://semanticbible.org/ns/2006/NTNames#Jewish"/>
        <description rdf:datatype="http://www.w3.org/2001/XMLSchema#string">One of the ancestors of Jesus mentioned in Luke&apos;s geneaology</description>
        <rdfs:label xml:lang="en">Shealtiel</rdfs:label>
    </owl:NamedIndividual>
    


    <!-- http://semanticbible.org/ns/2006/NTNames#Shechem -->

    <owl:NamedIndividual rdf:about="http://semanticbible.org/ns/2006/NTNames#Shechem">
        <rdf:type rdf:resource="http://semanticbible.org/ns/2006/NTNames#City"/>
        <location rdf:resource="http://semanticbible.org/ns/2006/NTNames#ShechemGeodata"/>
        <nativePlaceOf rdf:resource="http://semanticbible.org/ns/2006/NTNames#Hamor"/>
        <rdfs:comment rdf:datatype="http://www.w3.org/2001/XMLSchema#string">A subregion of Canaan.</rdfs:comment>
        <rdfs:label xml:lang="en">Shechem</rdfs:label>
    </owl:NamedIndividual>
    


    <!-- http://semanticbible.org/ns/2006/NTNames#ShechemGeodata -->

    <owl:NamedIndividual rdf:about="http://semanticbible.org/ns/2006/NTNames#ShechemGeodata">
        <rdf:type rdf:resource="http://semanticbible.org/ns/2006/NTNames#GeographicLocation"/>
        <altitude rdf:datatype="http://www.w3.org/2001/XMLSchema#int">0</altitude>
        <latitude rdf:datatype="http://www.w3.org/2001/XMLSchema#double">32.21495259430149</latitude>
        <longitude rdf:datatype="http://www.w3.org/2001/XMLSchema#double">35.27651098164232</longitude>
        <rdfs:label xml:lang="en">geodata for Shechem</rdfs:label>
    </owl:NamedIndividual>
    


    <!-- http://semanticbible.org/ns/2006/NTNames#Shelah -->

    <owl:NamedIndividual rdf:about="http://semanticbible.org/ns/2006/NTNames#Shelah">
        <rdf:type rdf:resource="http://semanticbible.org/ns/2006/NTNames#Man"/>
        <childOf rdf:resource="http://semanticbible.org/ns/2006/NTNames#CainanSonOfArphaxad"/>
        <parentOf rdf:resource="http://semanticbible.org/ns/2006/NTNames#Eber"/>
        <description rdf:datatype="http://www.w3.org/2001/XMLSchema#string">One of the ancestors of Jesus mentioned in Luke&apos;s geneaology</description>
        <hasOnlyGenealogyMention rdf:datatype="http://www.w3.org/2001/XMLSchema#boolean">true</hasOnlyGenealogyMention>
        <rdfs:label xml:lang="en">Shelah</rdfs:label>
    </owl:NamedIndividual>
    


    <!-- http://semanticbible.org/ns/2006/NTNames#Shem -->

    <owl:NamedIndividual rdf:about="http://semanticbible.org/ns/2006/NTNames#Shem">
        <rdf:type rdf:resource="http://semanticbible.org/ns/2006/NTNames#Man"/>
        <childOf rdf:resource="http://semanticbible.org/ns/2006/NTNames#Noah"/>
        <parentOf rdf:resource="http://semanticbible.org/ns/2006/NTNames#Arphaxad"/>
        <description rdf:datatype="http://www.w3.org/2001/XMLSchema#string">One of the ancestors of Jesus mentioned in Luke&apos;s geneaology</description>
        <hasOnlyGenealogyMention rdf:datatype="http://www.w3.org/2001/XMLSchema#boolean">true</hasOnlyGenealogyMention>
        <rdfs:label xml:lang="en">Shem</rdfs:label>
    </owl:NamedIndividual>
    


    <!-- http://semanticbible.org/ns/2006/NTNames#Sidon -->

    <owl:NamedIndividual rdf:about="http://semanticbible.org/ns/2006/NTNames#Sidon">
        <rdf:type rdf:resource="http://semanticbible.org/ns/2006/NTNames#City"/>
        <location rdf:resource="http://semanticbible.org/ns/2006/NTNames#SidonGeodata"/>
        <subregionOf rdf:resource="http://semanticbible.org/ns/2006/NTNames#Phoenicia"/>
        <rdfs:label xml:lang="en">Sidon</rdfs:label>
    </owl:NamedIndividual>
    


    <!-- http://semanticbible.org/ns/2006/NTNames#SidonGeodata -->

    <owl:NamedIndividual rdf:about="http://semanticbible.org/ns/2006/NTNames#SidonGeodata">
        <rdf:type rdf:resource="http://semanticbible.org/ns/2006/NTNames#GeographicLocation"/>
        <altitude rdf:datatype="http://www.w3.org/2001/XMLSchema#int">0</altitude>
        <latitude rdf:datatype="http://www.w3.org/2001/XMLSchema#double">33.5571694642368</latitude>
        <longitude rdf:datatype="http://www.w3.org/2001/XMLSchema#double">35.35565736166527</longitude>
        <rdfs:label xml:lang="en">geodata for Sidon</rdfs:label>
    </owl:NamedIndividual>
    


    <!-- http://semanticbible.org/ns/2006/NTNames#Silas -->

    <owl:NamedIndividual rdf:about="http://semanticbible.org/ns/2006/NTNames#Silas">
        <rdf:type rdf:resource="http://semanticbible.org/ns/2006/NTNames#Man"/>
        <collaboratesWith rdf:resource="http://semanticbible.org/ns/2006/NTNames#Barnabas"/>
        <hasAntagonist rdf:resource="http://semanticbible.org/ns/2006/NTNames#Bar-Jesus"/>
        <rdfs:label xml:lang="en">Silas</rdfs:label>
    </owl:NamedIndividual>
    


    <!-- http://semanticbible.org/ns/2006/NTNames#Siloam -->

    <owl:NamedIndividual rdf:about="http://semanticbible.org/ns/2006/NTNames#Siloam">
        <rdf:type rdf:resource="http://semanticbible.org/ns/2006/NTNames#FreshWaterArea"/>
        <subregionOf rdf:resource="http://semanticbible.org/ns/2006/NTNames#Jerusalem"/>
        <rdfs:comment xml:lang="en">A pool outside the walls of Jerusalem.</rdfs:comment>
        <rdfs:label xml:lang="en">Siloam</rdfs:label>
    </owl:NamedIndividual>
    


    <!-- http://semanticbible.org/ns/2006/NTNames#Silvanus -->

    <owl:NamedIndividual rdf:about="http://semanticbible.org/ns/2006/NTNames#Silvanus">
        <rdf:type rdf:resource="http://semanticbible.org/ns/2006/NTNames#Man"/>
        <rdfs:label xml:lang="en">Silvanus</rdfs:label>
    </owl:NamedIndividual>
    


    <!-- http://semanticbible.org/ns/2006/NTNames#SimeonNiger -->

    <owl:NamedIndividual rdf:about="http://semanticbible.org/ns/2006/NTNames#SimeonNiger">
        <rdf:type rdf:resource="http://semanticbible.org/ns/2006/NTNames#Man"/>
        <collaboratesWith rdf:resource="http://semanticbible.org/ns/2006/NTNames#Barnabas"/>
        <collaboratesWith rdf:resource="http://semanticbible.org/ns/2006/NTNames#LuciusOfCyrene"/>
        <collaboratesWith rdf:resource="http://semanticbible.org/ns/2006/NTNames#Manaen"/>
        <collaboratesWith rdf:resource="http://semanticbible.org/ns/2006/NTNames#Paul"/>
        <description rdf:datatype="http://www.w3.org/2001/XMLSchema#string">A leader in the church of Antioch</description>
        <rdfs:label xml:lang="en">Simeon</rdfs:label>
    </owl:NamedIndividual>
    


    <!-- http://semanticbible.org/ns/2006/NTNames#SimeonSonOfJudah -->

    <owl:NamedIndividual rdf:about="http://semanticbible.org/ns/2006/NTNames#SimeonSonOfJudah">
        <rdf:type rdf:resource="http://semanticbible.org/ns/2006/NTNames#Man"/>
        <childOf rdf:resource="http://semanticbible.org/ns/2006/NTNames#JudahSonOfJoseph"/>
        <ethnicity rdf:resource="http://semanticbible.org/ns/2006/NTNames#Jewish"/>
        <parentOf rdf:resource="http://semanticbible.org/ns/2006/NTNames#LeviSonOfSimeon"/>
        <description rdf:datatype="http://www.w3.org/2001/XMLSchema#string">One of the ancestors of Jesus mentioned in Luke&apos;s geneaology</description>
        <hasOnlyGenealogyMention rdf:datatype="http://www.w3.org/2001/XMLSchema#boolean">true</hasOnlyGenealogyMention>
        <rdfs:label xml:lang="en">Simeon</rdfs:label>
    </owl:NamedIndividual>
    


    <!-- http://semanticbible.org/ns/2006/NTNames#SimeonThePatriarch -->

    <owl:NamedIndividual rdf:about="http://semanticbible.org/ns/2006/NTNames#SimeonThePatriarch">
        <rdf:type rdf:resource="http://semanticbible.org/ns/2006/NTNames#Man"/>
        <childOf rdf:resource="http://semanticbible.org/ns/2006/NTNames#Jacob"/>
        <ethnicity rdf:resource="http://semanticbible.org/ns/2006/NTNames#Jewish"/>
        <siblingOf rdf:resource="http://semanticbible.org/ns/2006/NTNames#Gad"/>
        <description rdf:datatype="http://www.w3.org/2001/XMLSchema#string">One of the twelve sons of Jacob, whose name is adopted for one of the Twelve Tribes of Israel.</description>
        <rdfs:label xml:lang="en">Simeon</rdfs:label>
    </owl:NamedIndividual>
    


    <!-- http://semanticbible.org/ns/2006/NTNames#SimeonTheProphet -->

    <owl:NamedIndividual rdf:about="http://semanticbible.org/ns/2006/NTNames#SimeonTheProphet">
        <rdf:type rdf:resource="http://semanticbible.org/ns/2006/NTNames#Man"/>
        <description rdf:datatype="http://www.w3.org/2001/XMLSchema#string">A righteous man present in the temple when Jesus was presented as a baby</description>
        <rdfs:label xml:lang="en">Simeon</rdfs:label>
    </owl:NamedIndividual>
    


    <!-- http://semanticbible.org/ns/2006/NTNames#SimonOfCyrene -->

    <owl:NamedIndividual rdf:about="http://semanticbible.org/ns/2006/NTNames#SimonOfCyrene">
        <rdf:type rdf:resource="http://semanticbible.org/ns/2006/NTNames#Man"/>
        <ethnicity rdf:resource="http://semanticbible.org/ns/2006/NTNames#Jewish"/>
        <parentOf rdf:resource="http://semanticbible.org/ns/2006/NTNames#Alexander"/>
        <parentOf rdf:resource="http://semanticbible.org/ns/2006/NTNames#Rufus"/>
        <description rdf:datatype="http://www.w3.org/2001/XMLSchema#string">Simon was forced to carry Jesus&apos; cross by the Romans who were taking him to be cruficied</description>
        <rdfs:comment xml:lang="en">Identified as a Jew because, though a foreigner, he was in Jerusalem at the time of Passover</rdfs:comment>
        <rdfs:label xml:lang="en">Simon</rdfs:label>
    </owl:NamedIndividual>
    


    <!-- http://semanticbible.org/ns/2006/NTNames#SimonPeter -->

    <owl:NamedIndividual rdf:about="http://semanticbible.org/ns/2006/NTNames#SimonPeter">
        <rdf:type rdf:resource="http://semanticbible.org/ns/2006/NTNames#Man"/>
        <antagonistOf rdf:resource="http://semanticbible.org/ns/2006/NTNames#Ananias"/>
        <antagonistOf rdf:resource="http://semanticbible.org/ns/2006/NTNames#Sapphira"/>
        <childOf rdf:resource="http://semanticbible.org/ns/2006/NTNames#JonahOfBethsaida"/>
        <collaboratesWith rdf:resource="http://semanticbible.org/ns/2006/NTNames#Andrew"/>
        <collaboratesWith rdf:resource="http://semanticbible.org/ns/2006/NTNames#Barnabas"/>
        <collaboratesWith rdf:resource="http://semanticbible.org/ns/2006/NTNames#JohntheBaptist"/>
        <collaboratesWith rdf:resource="http://semanticbible.org/ns/2006/NTNames#JosephBarsabbas"/>
        <collaboratesWith rdf:resource="http://semanticbible.org/ns/2006/NTNames#MaryMagdalene"/>
        <collaboratesWith rdf:resource="http://semanticbible.org/ns/2006/NTNames#SimonTheTanner"/>
        <ethnicity rdf:resource="http://semanticbible.org/ns/2006/NTNames#Galilean"/>
        <hasEnemy rdf:resource="http://semanticbible.org/ns/2006/NTNames#AlexanderOfTheSanhedrin"/>
        <hasEnemy rdf:resource="http://semanticbible.org/ns/2006/NTNames#Annas"/>
        <hasEnemy rdf:resource="http://semanticbible.org/ns/2006/NTNames#JohnOfTheSanhedrin"/>
        <knows rdf:resource="http://semanticbible.org/ns/2006/NTNames#Aeneas"/>
        <knows rdf:resource="http://semanticbible.org/ns/2006/NTNames#Ananias"/>
        <knows rdf:resource="http://semanticbible.org/ns/2006/NTNames#Sapphira"/>
        <knows rdf:resource="http://semanticbible.org/ns/2006/NTNames#Tabitha"/>
        <siblingOf rdf:resource="http://semanticbible.org/ns/2006/NTNames#Andrew"/>
        <description rdf:datatype="http://www.w3.org/2001/XMLSchema#string">one of Jesus&apos; twelve apostles</description>
        <occupation rdf:datatype="http://www.w3.org/2001/XMLSchema#string">apostle</occupation>
        <occupation rdf:datatype="http://www.w3.org/2001/XMLSchema#string">fisherman</occupation>
        <rdfs:comment rdf:datatype="http://www.w3.org/2001/XMLSchema#string">The main definition for the Apostle Peter.</rdfs:comment>
        <rdfs:label xml:lang="en">Simon Peter</rdfs:label>
    </owl:NamedIndividual>
    


    <!-- http://semanticbible.org/ns/2006/NTNames#SimonTheTanner -->

    <owl:NamedIndividual rdf:about="http://semanticbible.org/ns/2006/NTNames#SimonTheTanner">
        <rdf:type rdf:resource="http://semanticbible.org/ns/2006/NTNames#Man"/>
        <collaboratesWith rdf:resource="http://semanticbible.org/ns/2006/NTNames#SimonPeter"/>
        <religiousBelief rdf:resource="http://semanticbible.org/ns/2006/NTNames#Christianity"/>
        <residentPlace rdf:resource="http://semanticbible.org/ns/2006/NTNames#Joppa"/>
        <description rdf:datatype="http://www.w3.org/2001/XMLSchema#string">Simon Peter stayed at Simon the Tanner&apos;s house in Joppa</description>
        <hasOnlyGenealogyMention rdf:datatype="http://www.w3.org/2001/XMLSchema#boolean">false</hasOnlyGenealogyMention>
        <occupation rdf:datatype="http://www.w3.org/2001/XMLSchema#string">tanner</occupation>
        <rdfs:label xml:lang="en">Simon</rdfs:label>
    </owl:NamedIndividual>
    


    <!-- http://semanticbible.org/ns/2006/NTNames#SimonTheZealot -->

    <owl:NamedIndividual rdf:about="http://semanticbible.org/ns/2006/NTNames#SimonTheZealot">
        <rdf:type rdf:resource="http://semanticbible.org/ns/2006/NTNames#Man"/>
        <ethnicity rdf:resource="http://semanticbible.org/ns/2006/NTNames#Galilean"/>
        <relativeOf rdf:resource="http://semanticbible.org/ns/2006/NTNames#Andrew"/>
        <description rdf:datatype="http://www.w3.org/2001/XMLSchema#string">One of Jesus&apos; twelve apostles</description>
        <rdfs:comment xml:lang="en">Simon the Zealot was also known as Simon the Cananaean (but the term is one of political, not geographic, affiliation).</rdfs:comment>
        <rdfs:label xml:lang="en">Simon</rdfs:label>
    </owl:NamedIndividual>
    


    <!-- http://semanticbible.org/ns/2006/NTNames#Sinai -->

    <owl:NamedIndividual rdf:about="http://semanticbible.org/ns/2006/NTNames#Sinai">
        <rdf:type rdf:resource="http://semanticbible.org/ns/2006/NTNames#Mountain"/>
        <rdfs:label xml:lang="en">Sinai</rdfs:label>
    </owl:NamedIndividual>
    


    <!-- http://semanticbible.org/ns/2006/NTNames#Smyrna -->

    <owl:NamedIndividual rdf:about="http://semanticbible.org/ns/2006/NTNames#Smyrna">
        <rdf:type rdf:resource="http://semanticbible.org/ns/2006/NTNames#City"/>
        <location rdf:resource="http://semanticbible.org/ns/2006/NTNames#SmyrnaGeodata"/>
        <rdfs:label xml:lang="en">Smyrna</rdfs:label>
    </owl:NamedIndividual>
    


    <!-- http://semanticbible.org/ns/2006/NTNames#SmyrnaGeodata -->

    <owl:NamedIndividual rdf:about="http://semanticbible.org/ns/2006/NTNames#SmyrnaGeodata">
        <rdf:type rdf:resource="http://semanticbible.org/ns/2006/NTNames#GeographicLocation"/>
        <altitude rdf:datatype="http://www.w3.org/2001/XMLSchema#int">0</altitude>
        <latitude rdf:datatype="http://www.w3.org/2001/XMLSchema#double">38.32512200511864</latitude>
        <longitude rdf:datatype="http://www.w3.org/2001/XMLSchema#double">27.25625458305646</longitude>
        <rdfs:label xml:lang="en">geodata for Smyrna</rdfs:label>
    </owl:NamedIndividual>
    


    <!-- http://semanticbible.org/ns/2006/NTNames#Sodom -->

    <owl:NamedIndividual rdf:about="http://semanticbible.org/ns/2006/NTNames#Sodom">
        <rdf:type rdf:resource="http://semanticbible.org/ns/2006/NTNames#City"/>
        <location rdf:resource="http://semanticbible.org/ns/2006/NTNames#SodomGeodata"/>
        <rdfs:label xml:lang="en">Sodom</rdfs:label>
    </owl:NamedIndividual>
    


    <!-- http://semanticbible.org/ns/2006/NTNames#SodomGeodata -->

    <owl:NamedIndividual rdf:about="http://semanticbible.org/ns/2006/NTNames#SodomGeodata">
        <rdf:type rdf:resource="http://semanticbible.org/ns/2006/NTNames#GeographicLocation"/>
        <altitude rdf:datatype="http://www.w3.org/2001/XMLSchema#int">0</altitude>
        <latitude rdf:datatype="http://www.w3.org/2001/XMLSchema#double">31.42838121424862</latitude>
        <longitude rdf:datatype="http://www.w3.org/2001/XMLSchema#double">35.37152949677915</longitude>
        <rdfs:label xml:lang="en">geodata for Sodom</rdfs:label>
    </owl:NamedIndividual>
    


    <!-- http://semanticbible.org/ns/2006/NTNames#Solomon -->

    <owl:NamedIndividual rdf:about="http://semanticbible.org/ns/2006/NTNames#Solomon">
        <rdf:type rdf:resource="http://semanticbible.org/ns/2006/NTNames#Man"/>
        <childOf rdf:resource="http://semanticbible.org/ns/2006/NTNames#Bathsheba"/>
        <childOf rdf:resource="http://semanticbible.org/ns/2006/NTNames#David"/>
        <ethnicity rdf:resource="http://semanticbible.org/ns/2006/NTNames#Jewish"/>
        <parentOf rdf:resource="http://semanticbible.org/ns/2006/NTNames#Rehoboam"/>
        <description rdf:datatype="http://www.w3.org/2001/XMLSchema#string">King of Israel renowned for his wisdom</description>
        <occupation rdf:datatype="http://www.w3.org/2001/XMLSchema#string">king</occupation>
        <rdfs:label xml:lang="en">Solomon</rdfs:label>
    </owl:NamedIndividual>
    


    <!-- http://semanticbible.org/ns/2006/NTNames#Sopater -->

    <owl:NamedIndividual rdf:about="http://semanticbible.org/ns/2006/NTNames#Sopater">
        <rdf:type rdf:resource="http://semanticbible.org/ns/2006/NTNames#Man"/>
        <childOf rdf:resource="http://semanticbible.org/ns/2006/NTNames#Pyrrhus"/>
        <collaboratesWith rdf:resource="http://semanticbible.org/ns/2006/NTNames#Aristarchus"/>
        <collaboratesWith rdf:resource="http://semanticbible.org/ns/2006/NTNames#GaiusOfDerbe"/>
        <collaboratesWith rdf:resource="http://semanticbible.org/ns/2006/NTNames#Secundus"/>
        <collaboratesWith rdf:resource="http://semanticbible.org/ns/2006/NTNames#Timothy"/>
        <collaboratesWith rdf:resource="http://semanticbible.org/ns/2006/NTNames#Trophimus"/>
        <collaboratesWith rdf:resource="http://semanticbible.org/ns/2006/NTNames#Tychicus"/>
        <rdfs:label xml:lang="en">Sopater</rdfs:label>
    </owl:NamedIndividual>
    


    <!-- http://semanticbible.org/ns/2006/NTNames#Sosipater -->

    <owl:NamedIndividual rdf:about="http://semanticbible.org/ns/2006/NTNames#Sosipater">
        <rdf:type rdf:resource="http://semanticbible.org/ns/2006/NTNames#Man"/>
        <knows rdf:resource="http://semanticbible.org/ns/2006/NTNames#ErastusTheTreasurer"/>
        <knows rdf:resource="http://semanticbible.org/ns/2006/NTNames#GaiusOfCorinth"/>
        <knows rdf:resource="http://semanticbible.org/ns/2006/NTNames#Jason"/>
        <knows rdf:resource="http://semanticbible.org/ns/2006/NTNames#Lucius"/>
        <knows rdf:resource="http://semanticbible.org/ns/2006/NTNames#Quartus"/>
        <knows rdf:resource="http://semanticbible.org/ns/2006/NTNames#Tertius"/>
        <knows rdf:resource="http://semanticbible.org/ns/2006/NTNames#Timothy"/>
        <religiousBelief rdf:resource="http://semanticbible.org/ns/2006/NTNames#Christianity"/>
        <residentPlace rdf:resource="http://semanticbible.org/ns/2006/NTNames#Corinth"/>
        <description rdf:datatype="http://www.w3.org/2001/XMLSchema#string">a companion of Paul&apos;s who sent greetings to the Roman church</description>
        <hasOnlyGenealogyMention rdf:datatype="http://www.w3.org/2001/XMLSchema#boolean">false</hasOnlyGenealogyMention>
        <rdfs:comment xml:lang="en">&quot;kinsman&quot; here probably means that that he is a Jew, rather than an actual relation, given the number of people so designated in Romans 16. His residence in Corinth follows from the inference that Paul resided there when he wrote the letter to the Roman church.  </rdfs:comment>
        <rdfs:label xml:lang="en">Sosipater</rdfs:label>
    </owl:NamedIndividual>
    


    <!-- http://semanticbible.org/ns/2006/NTNames#Sosthenes -->

    <owl:NamedIndividual rdf:about="http://semanticbible.org/ns/2006/NTNames#Sosthenes">
        <rdf:type rdf:resource="http://semanticbible.org/ns/2006/NTNames#Man"/>
        <rdfs:label xml:lang="en">Sosthenes</rdfs:label>
    </owl:NamedIndividual>
    


    <!-- http://semanticbible.org/ns/2006/NTNames#Spain -->

    <owl:NamedIndividual rdf:about="http://semanticbible.org/ns/2006/NTNames#Spain">
        <rdf:type rdf:resource="http://semanticbible.org/ns/2006/NTNames#LandArea"/>
        <rdfs:label xml:lang="en">Spain</rdfs:label>
    </owl:NamedIndividual>
    


    <!-- http://semanticbible.org/ns/2006/NTNames#Stachys -->

    <owl:NamedIndividual rdf:about="http://semanticbible.org/ns/2006/NTNames#Stachys">
        <rdf:type rdf:resource="http://semanticbible.org/ns/2006/NTNames#Man"/>
        <knows rdf:resource="http://semanticbible.org/ns/2006/NTNames#Paul"/>
        <knows rdf:resource="http://semanticbible.org/ns/2006/NTNames#Priscilla"/>
        <religiousBelief rdf:resource="http://semanticbible.org/ns/2006/NTNames#Christianity"/>
        <residentPlace rdf:resource="http://semanticbible.org/ns/2006/NTNames#Rome"/>
        <description rdf:datatype="http://www.w3.org/2001/XMLSchema#string">a Christian in Rome to whom Paul sent greetings</description>
        <hasOnlyGenealogyMention rdf:datatype="http://www.w3.org/2001/XMLSchema#boolean">false</hasOnlyGenealogyMention>
        <rdfs:label xml:lang="en">Stachys</rdfs:label>
    </owl:NamedIndividual>
    


    <!-- http://semanticbible.org/ns/2006/NTNames#Stephanas -->

    <owl:NamedIndividual rdf:about="http://semanticbible.org/ns/2006/NTNames#Stephanas">
        <rdf:type rdf:resource="http://semanticbible.org/ns/2006/NTNames#Man"/>
        <collaboratesWith rdf:resource="http://semanticbible.org/ns/2006/NTNames#Achaicus"/>
        <collaboratesWith rdf:resource="http://semanticbible.org/ns/2006/NTNames#Fortunatus"/>
        <collaboratesWith rdf:resource="http://semanticbible.org/ns/2006/NTNames#Paul"/>
        <religiousBelief rdf:resource="http://semanticbible.org/ns/2006/NTNames#Christianity"/>
        <residentPlace rdf:resource="http://semanticbible.org/ns/2006/NTNames#Corinth"/>
        <visitedPlace rdf:resource="http://semanticbible.org/ns/2006/NTNames#Ephesus"/>
        <hasOnlyGenealogyMention rdf:datatype="http://www.w3.org/2001/XMLSchema#boolean">false</hasOnlyGenealogyMention>
        <rdfs:comment xml:lang="en">His residence in Corinth and visit to Ephesus follow from Paul&apos;s statement in 1Cor.16.17, and the assumption that Paul was in Ephesus when he wrote 1 Corinthians. </rdfs:comment>
        <rdfs:label xml:lang="en">Stephanas</rdfs:label>
    </owl:NamedIndividual>
    


    <!-- http://semanticbible.org/ns/2006/NTNames#Stephen -->

    <owl:NamedIndividual rdf:about="http://semanticbible.org/ns/2006/NTNames#Stephen">
        <rdf:type rdf:resource="http://semanticbible.org/ns/2006/NTNames#Man"/>
        <rdfs:label xml:lang="en">Stephen</rdfs:label>
    </owl:NamedIndividual>
    


    <!-- http://semanticbible.org/ns/2006/NTNames#Stoic -->

    <owl:NamedIndividual rdf:about="http://semanticbible.org/ns/2006/NTNames#Stoic">
        <rdf:type rdf:resource="http://semanticbible.org/ns/2006/NTNames#ReligiousBelief"/>
        <rdfs:label xml:lang="en">Stoic</rdfs:label>
    </owl:NamedIndividual>
    


    <!-- http://semanticbible.org/ns/2006/NTNames#Susanna -->

    <owl:NamedIndividual rdf:about="http://semanticbible.org/ns/2006/NTNames#Susanna">
        <rdf:type rdf:resource="http://semanticbible.org/ns/2006/NTNames#Woman"/>
        <collaboratesWith rdf:resource="http://semanticbible.org/ns/2006/NTNames#Jesus"/>
        <ethnicity rdf:resource="http://semanticbible.org/ns/2006/NTNames#Jewish"/>
        <knows rdf:resource="http://semanticbible.org/ns/2006/NTNames#Joanna"/>
        <knows rdf:resource="http://semanticbible.org/ns/2006/NTNames#MaryMagdalene"/>
        <religiousBelief rdf:resource="http://semanticbible.org/ns/2006/NTNames#Christianity"/>
        <description rdf:datatype="http://www.w3.org/2001/XMLSchema#string">a woman who contributed to Jesus&apos; support</description>
        <hasOnlyGenealogyMention rdf:datatype="http://www.w3.org/2001/XMLSchema#boolean">false</hasOnlyGenealogyMention>
        <rdfs:label xml:lang="en">Susanna</rdfs:label>
    </owl:NamedIndividual>
    


    <!-- http://semanticbible.org/ns/2006/NTNames#Sychar -->

    <owl:NamedIndividual rdf:about="http://semanticbible.org/ns/2006/NTNames#Sychar">
        <rdf:type rdf:resource="http://semanticbible.org/ns/2006/NTNames#City"/>
        <location rdf:resource="http://semanticbible.org/ns/2006/NTNames#SycharGeodata"/>
        <subregionOf rdf:resource="http://semanticbible.org/ns/2006/NTNames#Samaria"/>
        <rdfs:comment xml:lang="en">Jesus spoke here with a Samaritan woman about living water</rdfs:comment>
        <rdfs:label xml:lang="en">Sychar</rdfs:label>
    </owl:NamedIndividual>
    


    <!-- http://semanticbible.org/ns/2006/NTNames#SycharGeodata -->

    <owl:NamedIndividual rdf:about="http://semanticbible.org/ns/2006/NTNames#SycharGeodata">
        <rdf:type rdf:resource="http://semanticbible.org/ns/2006/NTNames#GeographicLocation"/>
        <altitude rdf:datatype="http://www.w3.org/2001/XMLSchema#int">0</altitude>
        <latitude rdf:datatype="http://www.w3.org/2001/XMLSchema#double">32.20570054376385</latitude>
        <longitude rdf:datatype="http://www.w3.org/2001/XMLSchema#double">35.30486456165939</longitude>
        <rdfs:label xml:lang="en">geodata for Sychar</rdfs:label>
    </owl:NamedIndividual>
    


    <!-- http://semanticbible.org/ns/2006/NTNames#Syntyche -->

    <owl:NamedIndividual rdf:about="http://semanticbible.org/ns/2006/NTNames#Syntyche">
        <rdf:type rdf:resource="http://semanticbible.org/ns/2006/NTNames#Woman"/>
        <collaboratesWith rdf:resource="http://semanticbible.org/ns/2006/NTNames#Clement"/>
        <collaboratesWith rdf:resource="http://semanticbible.org/ns/2006/NTNames#Euodia"/>
        <collaboratesWith rdf:resource="http://semanticbible.org/ns/2006/NTNames#Paul"/>
        <religiousBelief rdf:resource="http://semanticbible.org/ns/2006/NTNames#Christianity"/>
        <residentPlace rdf:resource="http://semanticbible.org/ns/2006/NTNames#Philippi"/>
        <description rdf:datatype="http://www.w3.org/2001/XMLSchema#string">a Philippian Christian who worked alongside Paul</description>
        <hasOnlyGenealogyMention rdf:datatype="http://www.w3.org/2001/XMLSchema#boolean">false</hasOnlyGenealogyMention>
        <rdfs:label xml:lang="en">Syntyche</rdfs:label>
    </owl:NamedIndividual>
    


    <!-- http://semanticbible.org/ns/2006/NTNames#Syracuse -->

    <owl:NamedIndividual rdf:about="http://semanticbible.org/ns/2006/NTNames#Syracuse">
        <rdf:type rdf:resource="http://semanticbible.org/ns/2006/NTNames#City"/>
        <location rdf:resource="http://semanticbible.org/ns/2006/NTNames#SyracuseGeodata"/>
        <rdfs:label xml:lang="en">Syracuse</rdfs:label>
    </owl:NamedIndividual>
    


    <!-- http://semanticbible.org/ns/2006/NTNames#SyracuseGeodata -->

    <owl:NamedIndividual rdf:about="http://semanticbible.org/ns/2006/NTNames#SyracuseGeodata">
        <rdf:type rdf:resource="http://semanticbible.org/ns/2006/NTNames#GeographicLocation"/>
        <altitude rdf:datatype="http://www.w3.org/2001/XMLSchema#int">0</altitude>
        <latitude rdf:datatype="http://www.w3.org/2001/XMLSchema#double">37.07082102418126</latitude>
        <longitude rdf:datatype="http://www.w3.org/2001/XMLSchema#double">15.29666086592392</longitude>
        <rdfs:label xml:lang="en">geodata for Syracuse</rdfs:label>
    </owl:NamedIndividual>
    


    <!-- http://semanticbible.org/ns/2006/NTNames#Syria -->

    <owl:NamedIndividual rdf:about="http://semanticbible.org/ns/2006/NTNames#Syria">
        <rdf:type rdf:resource="http://semanticbible.org/ns/2006/NTNames#StateOrProvince"/>
        <rdfs:label xml:lang="en">Syria</rdfs:label>
    </owl:NamedIndividual>
    


    <!-- http://semanticbible.org/ns/2006/NTNames#Syrian -->

    <owl:NamedIndividual rdf:about="http://semanticbible.org/ns/2006/NTNames#Syrian">
        <rdf:type rdf:resource="http://semanticbible.org/ns/2006/NTNames#EthnicityAttribute"/>
        <ethnicityOf rdf:resource="http://semanticbible.org/ns/2006/NTNames#Naaman"/>
        <rdfs:comment xml:lang="en">Of the country of Syria.</rdfs:comment>
        <rdfs:label xml:lang="en">Syrian</rdfs:label>
    </owl:NamedIndividual>
    


    <!-- http://semanticbible.org/ns/2006/NTNames#Syrophoenician -->

    <owl:NamedIndividual rdf:about="http://semanticbible.org/ns/2006/NTNames#Syrophoenician">
        <rdf:type rdf:resource="http://semanticbible.org/ns/2006/NTNames#EthnicityAttribute"/>
        <rdfs:comment xml:lang="en">Likely synonymous with Canaanite, and referring to those from the region of Syria and Phoenicia, and therefore a subgroup of Greek Gentiles.</rdfs:comment>
        <rdfs:label xml:lang="en">Syrophoenician</rdfs:label>
    </owl:NamedIndividual>
    


    <!-- http://semanticbible.org/ns/2006/NTNames#Syrtis -->

    <owl:NamedIndividual rdf:about="http://semanticbible.org/ns/2006/NTNames#Syrtis">
        <rdf:type rdf:resource="http://semanticbible.org/ns/2006/NTNames#SaltWaterArea"/>
        <rdfs:label xml:lang="en">Syrtis</rdfs:label>
    </owl:NamedIndividual>
    


    <!-- http://semanticbible.org/ns/2006/NTNames#Tabitha -->

    <owl:NamedIndividual rdf:about="http://semanticbible.org/ns/2006/NTNames#Tabitha">
        <rdf:type rdf:resource="http://semanticbible.org/ns/2006/NTNames#Woman"/>
        <knows rdf:resource="http://semanticbible.org/ns/2006/NTNames#SimonPeter"/>
        <religiousBelief rdf:resource="http://semanticbible.org/ns/2006/NTNames#Christianity"/>
        <residentPlace rdf:resource="http://semanticbible.org/ns/2006/NTNames#Joppa"/>
        <description rdf:datatype="http://www.w3.org/2001/XMLSchema#string">a Christian in Joppa known for her charity</description>
        <hasOnlyGenealogyMention rdf:datatype="http://www.w3.org/2001/XMLSchema#boolean">false</hasOnlyGenealogyMention>
        <rdfs:comment xml:lang="en">The Aramaic name Tabitha corresponds to the Greek form Dorcas. She probably also knew Simon the Tanner. </rdfs:comment>
        <rdfs:label xml:lang="en">Dorcas</rdfs:label>
        <rdfs:label xml:lang="en">Tabitha</rdfs:label>
    </owl:NamedIndividual>
    


    <!-- http://semanticbible.org/ns/2006/NTNames#Tamar -->

    <owl:NamedIndividual rdf:about="http://semanticbible.org/ns/2006/NTNames#Tamar">
        <rdf:type rdf:resource="http://semanticbible.org/ns/2006/NTNames#Woman"/>
        <ethnicity rdf:resource="http://semanticbible.org/ns/2006/NTNames#Jewish"/>
        <parentOf rdf:resource="http://semanticbible.org/ns/2006/NTNames#Perez"/>
        <parentOf rdf:resource="http://semanticbible.org/ns/2006/NTNames#Zerah"/>
        <description rdf:datatype="http://www.w3.org/2001/XMLSchema#string">One of the ancestors of Jesus mentioned in Matthew&apos;s geneaology</description>
        <hasOnlyGenealogyMention rdf:datatype="http://www.w3.org/2001/XMLSchema#boolean">true</hasOnlyGenealogyMention>
        <rdfs:label xml:lang="en">Tamar</rdfs:label>
    </owl:NamedIndividual>
    


    <!-- http://semanticbible.org/ns/2006/NTNames#Tarsus -->

    <owl:NamedIndividual rdf:about="http://semanticbible.org/ns/2006/NTNames#Tarsus">
        <rdf:type rdf:resource="http://semanticbible.org/ns/2006/NTNames#City"/>
        <location rdf:resource="http://semanticbible.org/ns/2006/NTNames#TarsusGeodata"/>
        <rdfs:label xml:lang="en">Tarsus</rdfs:label>
    </owl:NamedIndividual>
    


    <!-- http://semanticbible.org/ns/2006/NTNames#TarsusGeodata -->

    <owl:NamedIndividual rdf:about="http://semanticbible.org/ns/2006/NTNames#TarsusGeodata">
        <rdf:type rdf:resource="http://semanticbible.org/ns/2006/NTNames#GeographicLocation"/>
        <altitude rdf:datatype="http://www.w3.org/2001/XMLSchema#int">0</altitude>
        <latitude rdf:datatype="http://www.w3.org/2001/XMLSchema#double">36.91390164056132</latitude>
        <longitude rdf:datatype="http://www.w3.org/2001/XMLSchema#double">34.88339832154442</longitude>
        <rdfs:label xml:lang="en">geodata for Tarsus</rdfs:label>
    </owl:NamedIndividual>
    


    <!-- http://semanticbible.org/ns/2006/NTNames#Taverns -->

    <owl:NamedIndividual rdf:about="http://semanticbible.org/ns/2006/NTNames#Taverns">
        <rdf:type rdf:resource="http://semanticbible.org/ns/2006/NTNames#LandArea"/>
        <rdfs:label xml:lang="en">Taverns</rdfs:label>
    </owl:NamedIndividual>
    


    <!-- http://semanticbible.org/ns/2006/NTNames#Terah -->

    <owl:NamedIndividual rdf:about="http://semanticbible.org/ns/2006/NTNames#Terah">
        <rdf:type rdf:resource="http://semanticbible.org/ns/2006/NTNames#Man"/>
        <childOf rdf:resource="http://semanticbible.org/ns/2006/NTNames#Nahor"/>
        <parentOf rdf:resource="http://semanticbible.org/ns/2006/NTNames#Abraham"/>
        <parentOf rdf:resource="http://semanticbible.org/ns/2006/NTNames#Sarah"/>
        <hasOnlyGenealogyMention rdf:datatype="http://www.w3.org/2001/XMLSchema#boolean">true</hasOnlyGenealogyMention>
        <rdfs:label xml:lang="en">Terah</rdfs:label>
    </owl:NamedIndividual>
    


    <!-- http://semanticbible.org/ns/2006/NTNames#Tertius -->

    <owl:NamedIndividual rdf:about="http://semanticbible.org/ns/2006/NTNames#Tertius">
        <rdf:type rdf:resource="http://semanticbible.org/ns/2006/NTNames#Man"/>
        <collaboratesWith rdf:resource="http://semanticbible.org/ns/2006/NTNames#Paul"/>
        <religiousBelief rdf:resource="http://semanticbible.org/ns/2006/NTNames#Christianity"/>
        <residentPlace rdf:resource="http://semanticbible.org/ns/2006/NTNames#Corinth"/>
        <description rdf:datatype="http://www.w3.org/2001/XMLSchema#string">the scribe of Paul&apos;s letter to the Roman church</description>
        <hasOnlyGenealogyMention rdf:datatype="http://www.w3.org/2001/XMLSchema#boolean">false</hasOnlyGenealogyMention>
        <rdfs:comment rdf:datatype="http://www.w3.org/2001/XMLSchema#string">His residence in Corinth follows from the inference that Paul resided there when he wrote the letter to the Roman church.  </rdfs:comment>
        <rdfs:label xml:lang="en">Tertius</rdfs:label>
    </owl:NamedIndividual>
    


    <!-- http://semanticbible.org/ns/2006/NTNames#Tertullus -->

    <owl:NamedIndividual rdf:about="http://semanticbible.org/ns/2006/NTNames#Tertullus">
        <rdf:type rdf:resource="http://semanticbible.org/ns/2006/NTNames#Man"/>
        <collaboratesWith rdf:resource="http://semanticbible.org/ns/2006/NTNames#AnaniasTheHighPriest"/>
        <enemyOf rdf:resource="http://semanticbible.org/ns/2006/NTNames#Paul"/>
        <knows rdf:resource="http://semanticbible.org/ns/2006/NTNames#Felix"/>
        <description rdf:datatype="http://www.w3.org/2001/XMLSchema#string">an orator enlisted by Ananias the high priest to speak against Paul to Felix</description>
        <occupation rdf:datatype="http://www.w3.org/2001/XMLSchema#string">orator</occupation>
        <rdfs:comment xml:lang="en">Speaking on behalf of the Sanhedrin does not imply Tertullus was Jewish: more likely (but not certain), he was a Roman, hired for his familiarity with Roman law. But the account describes him as traveling from Jerusalem with the others.</rdfs:comment>
        <rdfs:label xml:lang="en">Tertullus</rdfs:label>
    </owl:NamedIndividual>
    


    <!-- http://semanticbible.org/ns/2006/NTNames#Thaddaeus -->

    <owl:NamedIndividual rdf:about="http://semanticbible.org/ns/2006/NTNames#Thaddaeus">
        <rdf:type rdf:resource="http://semanticbible.org/ns/2006/NTNames#Man"/>
        <collaboratesWith rdf:resource="http://semanticbible.org/ns/2006/NTNames#Andrew"/>
        <rdfs:label xml:lang="en">Thaddaeus</rdfs:label>
    </owl:NamedIndividual>
    


    <!-- http://semanticbible.org/ns/2006/NTNames#Theophilus -->

    <owl:NamedIndividual rdf:about="http://semanticbible.org/ns/2006/NTNames#Theophilus">
        <rdf:type rdf:resource="http://semanticbible.org/ns/2006/NTNames#Man"/>
        <rdfs:label xml:lang="en">Theophilus</rdfs:label>
    </owl:NamedIndividual>
    


    <!-- http://semanticbible.org/ns/2006/NTNames#Thessalonians -->

    <owl:NamedIndividual rdf:about="http://semanticbible.org/ns/2006/NTNames#Thessalonians">
        <rdf:type rdf:resource="http://semanticbible.org/ns/2006/NTNames#ResidenceGroup"/>
        <rdfs:label xml:lang="en">Thessalonians</rdfs:label>
    </owl:NamedIndividual>
    


    <!-- http://semanticbible.org/ns/2006/NTNames#Thessalonica -->

    <owl:NamedIndividual rdf:about="http://semanticbible.org/ns/2006/NTNames#Thessalonica">
        <rdf:type rdf:resource="http://semanticbible.org/ns/2006/NTNames#City"/>
        <location rdf:resource="http://semanticbible.org/ns/2006/NTNames#ThessalonicaGeodata"/>
        <residentPlaceOf rdf:resource="http://semanticbible.org/ns/2006/NTNames#Secundus"/>
        <subregionOf rdf:resource="http://semanticbible.org/ns/2006/NTNames#Macedonia"/>
        <rdfs:label xml:lang="en">Thessalonica</rdfs:label>
    </owl:NamedIndividual>
    


    <!-- http://semanticbible.org/ns/2006/NTNames#ThessalonicaGeodata -->

    <owl:NamedIndividual rdf:about="http://semanticbible.org/ns/2006/NTNames#ThessalonicaGeodata">
        <rdf:type rdf:resource="http://semanticbible.org/ns/2006/NTNames#GeographicLocation"/>
        <altitude rdf:datatype="http://www.w3.org/2001/XMLSchema#int">0</altitude>
        <latitude rdf:datatype="http://www.w3.org/2001/XMLSchema#double">40.64160894418217</latitude>
        <longitude rdf:datatype="http://www.w3.org/2001/XMLSchema#double">22.93594798656816</longitude>
        <rdfs:label xml:lang="en">geodata for Thessalonica</rdfs:label>
    </owl:NamedIndividual>
    


    <!-- http://semanticbible.org/ns/2006/NTNames#Theudas -->

    <owl:NamedIndividual rdf:about="http://semanticbible.org/ns/2006/NTNames#Theudas">
        <rdf:type rdf:resource="http://semanticbible.org/ns/2006/NTNames#Man"/>
        <rdfs:label xml:lang="en">Theudas</rdfs:label>
    </owl:NamedIndividual>
    


    <!-- http://semanticbible.org/ns/2006/NTNames#Thomas -->

    <owl:NamedIndividual rdf:about="http://semanticbible.org/ns/2006/NTNames#Thomas">
        <rdf:type rdf:resource="http://semanticbible.org/ns/2006/NTNames#Man"/>
        <collaboratesWith rdf:resource="http://semanticbible.org/ns/2006/NTNames#Andrew"/>
        <ethnicity rdf:resource="http://semanticbible.org/ns/2006/NTNames#Galilean"/>
        <description rdf:datatype="http://www.w3.org/2001/XMLSchema#string">One of Jesus&apos; twelve apostles</description>
        <rdfs:label xml:lang="en">Thomas</rdfs:label>
    </owl:NamedIndividual>
    


    <!-- http://semanticbible.org/ns/2006/NTNames#Thyatira -->

    <owl:NamedIndividual rdf:about="http://semanticbible.org/ns/2006/NTNames#Thyatira">
        <rdf:type rdf:resource="http://semanticbible.org/ns/2006/NTNames#City"/>
        <location rdf:resource="http://semanticbible.org/ns/2006/NTNames#ThyatiraGeodata"/>
        <nativePlaceOf rdf:resource="http://semanticbible.org/ns/2006/NTNames#Lydia"/>
        <rdfs:label xml:lang="en">Thyatira</rdfs:label>
    </owl:NamedIndividual>
    


    <!-- http://semanticbible.org/ns/2006/NTNames#ThyatiraGeodata -->

    <owl:NamedIndividual rdf:about="http://semanticbible.org/ns/2006/NTNames#ThyatiraGeodata">
        <rdf:type rdf:resource="http://semanticbible.org/ns/2006/NTNames#GeographicLocation"/>
        <altitude rdf:datatype="http://www.w3.org/2001/XMLSchema#int">0</altitude>
        <latitude rdf:datatype="http://www.w3.org/2001/XMLSchema#double">38.92574516366593</latitude>
        <longitude rdf:datatype="http://www.w3.org/2001/XMLSchema#double">27.85737139107431</longitude>
        <rdfs:label xml:lang="en">geodata for Thyatira</rdfs:label>
    </owl:NamedIndividual>
    


    <!-- http://semanticbible.org/ns/2006/NTNames#Tiberias -->

    <owl:NamedIndividual rdf:about="http://semanticbible.org/ns/2006/NTNames#Tiberias">
        <rdf:type rdf:resource="http://semanticbible.org/ns/2006/NTNames#City"/>
        <location rdf:resource="http://semanticbible.org/ns/2006/NTNames#TiberiasGeodata"/>
        <subregionOf rdf:resource="http://semanticbible.org/ns/2006/NTNames#Galilee"/>
        <rdfs:comment xml:lang="en">Tiberias was built by Herod Antipas, the tetrarch of Galilee, as his capital. </rdfs:comment>
        <rdfs:label xml:lang="en">Tiberias</rdfs:label>
    </owl:NamedIndividual>
    


    <!-- http://semanticbible.org/ns/2006/NTNames#TiberiasGeodata -->

    <owl:NamedIndividual rdf:about="http://semanticbible.org/ns/2006/NTNames#TiberiasGeodata">
        <rdf:type rdf:resource="http://semanticbible.org/ns/2006/NTNames#GeographicLocation"/>
        <altitude rdf:datatype="http://www.w3.org/2001/XMLSchema#int">0</altitude>
        <latitude rdf:datatype="http://www.w3.org/2001/XMLSchema#double">32.79687612684089</latitude>
        <longitude rdf:datatype="http://www.w3.org/2001/XMLSchema#double">35.52732984815425</longitude>
        <rdfs:label xml:lang="en">geodata for Tiberias</rdfs:label>
    </owl:NamedIndividual>
    


    <!-- http://semanticbible.org/ns/2006/NTNames#TiberiusCaesar -->

    <owl:NamedIndividual rdf:about="http://semanticbible.org/ns/2006/NTNames#TiberiusCaesar">
        <rdf:type rdf:resource="http://semanticbible.org/ns/2006/NTNames#Man"/>
        <ethnicity rdf:resource="http://semanticbible.org/ns/2006/NTNames#Roman"/>
        <description rdf:datatype="http://www.w3.org/2001/XMLSchema#string">Roman Emperor at the time of Jesus&apos; ministry</description>
        <occupation rdf:datatype="http://www.w3.org/2001/XMLSchema#string">emperor</occupation>
        <rdfs:comment xml:lang="en">Caesar is used as a name for several different individuals in the New Testament. This is the Caesar referred to by Jesus. </rdfs:comment>
        <rdfs:label xml:lang="en">Tiberius Caesar</rdfs:label>
    </owl:NamedIndividual>
    


    <!-- http://semanticbible.org/ns/2006/NTNames#Timaeus -->

    <owl:NamedIndividual rdf:about="http://semanticbible.org/ns/2006/NTNames#Timaeus">
        <rdf:type rdf:resource="http://semanticbible.org/ns/2006/NTNames#Man"/>
        <parentOf rdf:resource="http://semanticbible.org/ns/2006/NTNames#Bartimaeus"/>
        <rdfs:label xml:lang="en">Timaeus</rdfs:label>
    </owl:NamedIndividual>
    


    <!-- http://semanticbible.org/ns/2006/NTNames#Timon -->

    <owl:NamedIndividual rdf:about="http://semanticbible.org/ns/2006/NTNames#Timon">
        <rdf:type rdf:resource="http://semanticbible.org/ns/2006/NTNames#Man"/>
        <rdfs:label xml:lang="en">Timon</rdfs:label>
    </owl:NamedIndividual>
    


    <!-- http://semanticbible.org/ns/2006/NTNames#Timothy -->

    <owl:NamedIndividual rdf:about="http://semanticbible.org/ns/2006/NTNames#Timothy">
        <rdf:type rdf:resource="http://semanticbible.org/ns/2006/NTNames#Man"/>
        <childOf rdf:resource="http://semanticbible.org/ns/2006/NTNames#Eunice"/>
        <collaboratesWith rdf:resource="http://semanticbible.org/ns/2006/NTNames#Aristarchus"/>
        <collaboratesWith rdf:resource="http://semanticbible.org/ns/2006/NTNames#Erastus"/>
        <collaboratesWith rdf:resource="http://semanticbible.org/ns/2006/NTNames#GaiusOfDerbe"/>
        <collaboratesWith rdf:resource="http://semanticbible.org/ns/2006/NTNames#Paul"/>
        <collaboratesWith rdf:resource="http://semanticbible.org/ns/2006/NTNames#Secundus"/>
        <collaboratesWith rdf:resource="http://semanticbible.org/ns/2006/NTNames#Sopater"/>
        <ethnicity rdf:resource="http://semanticbible.org/ns/2006/NTNames#Greek"/>
        <ethnicity rdf:resource="http://semanticbible.org/ns/2006/NTNames#Jewish"/>
        <knows rdf:resource="http://semanticbible.org/ns/2006/NTNames#Jason"/>
        <knows rdf:resource="http://semanticbible.org/ns/2006/NTNames#Lucius"/>
        <knows rdf:resource="http://semanticbible.org/ns/2006/NTNames#Sosipater"/>
        <religiousBelief rdf:resource="http://semanticbible.org/ns/2006/NTNames#Christianity"/>
        <residentPlace rdf:resource="http://semanticbible.org/ns/2006/NTNames#Corinth"/>
        <hasOnlyGenealogyMention rdf:datatype="http://www.w3.org/2001/XMLSchema#boolean">false</hasOnlyGenealogyMention>
        <rdfs:comment xml:lang="en">Timothy&apos;s residence in Corinth follows from the close of Paul&apos;s letter to the Romans, assumed to have been written from Corinth. </rdfs:comment>
        <rdfs:label xml:lang="en">Timothy</rdfs:label>
    </owl:NamedIndividual>
    


    <!-- http://semanticbible.org/ns/2006/NTNames#Titius -->

    <owl:NamedIndividual rdf:about="http://semanticbible.org/ns/2006/NTNames#Titius">
        <rdf:type rdf:resource="http://semanticbible.org/ns/2006/NTNames#Man"/>
        <ethnicity rdf:resource="http://semanticbible.org/ns/2006/NTNames#Greek"/>
        <rdfs:label xml:lang="en">Titius</rdfs:label>
    </owl:NamedIndividual>
    


    <!-- http://semanticbible.org/ns/2006/NTNames#Titus -->

    <owl:NamedIndividual rdf:about="http://semanticbible.org/ns/2006/NTNames#Titus">
        <rdf:type rdf:resource="http://semanticbible.org/ns/2006/NTNames#Man"/>
        <rdfs:label xml:lang="en">Titus</rdfs:label>
    </owl:NamedIndividual>
    


    <!-- http://semanticbible.org/ns/2006/NTNames#Trachonitis -->

    <owl:NamedIndividual rdf:about="http://semanticbible.org/ns/2006/NTNames#Trachonitis">
        <rdf:type rdf:resource="http://semanticbible.org/ns/2006/NTNames#Man"/>
        <rdfs:label xml:lang="en">Trachonitis</rdfs:label>
    </owl:NamedIndividual>
    


    <!-- http://semanticbible.org/ns/2006/NTNames#TribeOfAsher -->

    <owl:NamedIndividual rdf:about="http://semanticbible.org/ns/2006/NTNames#TribeOfAsher">
        <rdf:type rdf:resource="http://semanticbible.org/ns/2006/NTNames#Tribe"/>
        <member rdf:resource="http://semanticbible.org/ns/2006/NTNames#Anna"/>
        <rdfs:label xml:lang="en">tribe of Asher</rdfs:label>
    </owl:NamedIndividual>
    


    <!-- http://semanticbible.org/ns/2006/NTNames#TribeOfBenjamin -->

    <owl:NamedIndividual rdf:about="http://semanticbible.org/ns/2006/NTNames#TribeOfBenjamin">
        <rdf:type rdf:resource="http://semanticbible.org/ns/2006/NTNames#Tribe"/>
        <member rdf:resource="http://semanticbible.org/ns/2006/NTNames#SaulSonOfKish"/>
        <rdfs:label xml:lang="en">tribe of Benjamin</rdfs:label>
    </owl:NamedIndividual>
    


    <!-- http://semanticbible.org/ns/2006/NTNames#TribeOfGad -->

    <owl:NamedIndividual rdf:about="http://semanticbible.org/ns/2006/NTNames#TribeOfGad">
        <rdf:type rdf:resource="http://semanticbible.org/ns/2006/NTNames#Tribe"/>
        <rdfs:label xml:lang="en">tribe of Gad</rdfs:label>
    </owl:NamedIndividual>
    


    <!-- http://semanticbible.org/ns/2006/NTNames#TribeOfIssachar -->

    <owl:NamedIndividual rdf:about="http://semanticbible.org/ns/2006/NTNames#TribeOfIssachar">
        <rdf:type rdf:resource="http://semanticbible.org/ns/2006/NTNames#Tribe"/>
        <rdfs:label xml:lang="en">tribe of Issachar</rdfs:label>
    </owl:NamedIndividual>
    


    <!-- http://semanticbible.org/ns/2006/NTNames#TribeOfJoseph -->

    <owl:NamedIndividual rdf:about="http://semanticbible.org/ns/2006/NTNames#TribeOfJoseph">
        <rdf:type rdf:resource="http://semanticbible.org/ns/2006/NTNames#Tribe"/>
        <rdfs:label xml:lang="en">tribe of Joseph</rdfs:label>
    </owl:NamedIndividual>
    


    <!-- http://semanticbible.org/ns/2006/NTNames#TribeOfJudah -->

    <owl:NamedIndividual rdf:about="http://semanticbible.org/ns/2006/NTNames#TribeOfJudah">
        <rdf:type rdf:resource="http://semanticbible.org/ns/2006/NTNames#Tribe"/>
        <rdfs:label xml:lang="en">tribe of Judah</rdfs:label>
    </owl:NamedIndividual>
    


    <!-- http://semanticbible.org/ns/2006/NTNames#TribeOfLevi -->

    <owl:NamedIndividual rdf:about="http://semanticbible.org/ns/2006/NTNames#TribeOfLevi">
        <rdf:type rdf:resource="http://semanticbible.org/ns/2006/NTNames#Tribe"/>
        <rdfs:label xml:lang="en">tribe of Levi</rdfs:label>
    </owl:NamedIndividual>
    


    <!-- http://semanticbible.org/ns/2006/NTNames#TribeOfManasseh -->

    <owl:NamedIndividual rdf:about="http://semanticbible.org/ns/2006/NTNames#TribeOfManasseh">
        <rdf:type rdf:resource="http://semanticbible.org/ns/2006/NTNames#Tribe"/>
        <rdfs:label xml:lang="en">tribe of Manasseh</rdfs:label>
    </owl:NamedIndividual>
    


    <!-- http://semanticbible.org/ns/2006/NTNames#TribeOfNaphtali -->

    <owl:NamedIndividual rdf:about="http://semanticbible.org/ns/2006/NTNames#TribeOfNaphtali">
        <rdf:type rdf:resource="http://semanticbible.org/ns/2006/NTNames#Tribe"/>
        <rdfs:label xml:lang="en">Naphtali</rdfs:label>
        <rdfs:label xml:lang="en">tribe of Naphtali</rdfs:label>
    </owl:NamedIndividual>
    


    <!-- http://semanticbible.org/ns/2006/NTNames#TribeOfReuben -->

    <owl:NamedIndividual rdf:about="http://semanticbible.org/ns/2006/NTNames#TribeOfReuben">
        <rdf:type rdf:resource="http://semanticbible.org/ns/2006/NTNames#Tribe"/>
        <rdfs:label xml:lang="en">tribe of Reuben</rdfs:label>
    </owl:NamedIndividual>
    


    <!-- http://semanticbible.org/ns/2006/NTNames#TribeOfSimeon -->

    <owl:NamedIndividual rdf:about="http://semanticbible.org/ns/2006/NTNames#TribeOfSimeon">
        <rdf:type rdf:resource="http://semanticbible.org/ns/2006/NTNames#Tribe"/>
        <rdfs:label xml:lang="en">tribe of Simeon</rdfs:label>
    </owl:NamedIndividual>
    


    <!-- http://semanticbible.org/ns/2006/NTNames#TribeOfZebulun -->

    <owl:NamedIndividual rdf:about="http://semanticbible.org/ns/2006/NTNames#TribeOfZebulun">
        <rdf:type rdf:resource="http://semanticbible.org/ns/2006/NTNames#Tribe"/>
        <rdfs:label xml:lang="en">Zebulun</rdfs:label>
        <rdfs:label xml:lang="en">tribe of Zebulun</rdfs:label>
    </owl:NamedIndividual>
    


    <!-- http://semanticbible.org/ns/2006/NTNames#Troas -->

    <owl:NamedIndividual rdf:about="http://semanticbible.org/ns/2006/NTNames#Troas">
        <rdf:type rdf:resource="http://semanticbible.org/ns/2006/NTNames#City"/>
        <location rdf:resource="http://semanticbible.org/ns/2006/NTNames#TroasGeodata"/>
        <residentPlaceOf rdf:resource="http://semanticbible.org/ns/2006/NTNames#Eutychus"/>
        <visitedPlaceOf rdf:resource="http://semanticbible.org/ns/2006/NTNames#GaiusOfDerbe"/>
        <rdfs:label xml:lang="en">Troas</rdfs:label>
    </owl:NamedIndividual>
    


    <!-- http://semanticbible.org/ns/2006/NTNames#TroasGeodata -->

    <owl:NamedIndividual rdf:about="http://semanticbible.org/ns/2006/NTNames#TroasGeodata">
        <rdf:type rdf:resource="http://semanticbible.org/ns/2006/NTNames#GeographicLocation"/>
        <altitude rdf:datatype="http://www.w3.org/2001/XMLSchema#int">0</altitude>
        <latitude rdf:datatype="http://www.w3.org/2001/XMLSchema#double">39.50181513585497</latitude>
        <longitude rdf:datatype="http://www.w3.org/2001/XMLSchema#double">26.08148842388431</longitude>
        <rdfs:label xml:lang="en">geodata for Troas</rdfs:label>
    </owl:NamedIndividual>
    


    <!-- http://semanticbible.org/ns/2006/NTNames#Trophimus -->

    <owl:NamedIndividual rdf:about="http://semanticbible.org/ns/2006/NTNames#Trophimus">
        <rdf:type rdf:resource="http://semanticbible.org/ns/2006/NTNames#Man"/>
        <collaboratesWith rdf:resource="http://semanticbible.org/ns/2006/NTNames#Aristarchus"/>
        <collaboratesWith rdf:resource="http://semanticbible.org/ns/2006/NTNames#GaiusOfDerbe"/>
        <collaboratesWith rdf:resource="http://semanticbible.org/ns/2006/NTNames#Secundus"/>
        <collaboratesWith rdf:resource="http://semanticbible.org/ns/2006/NTNames#Sopater"/>
        <rdfs:label xml:lang="en">Trophimus</rdfs:label>
    </owl:NamedIndividual>
    


    <!-- http://semanticbible.org/ns/2006/NTNames#Tryphaena -->

    <owl:NamedIndividual rdf:about="http://semanticbible.org/ns/2006/NTNames#Tryphaena">
        <rdf:type rdf:resource="http://semanticbible.org/ns/2006/NTNames#Woman"/>
        <knows rdf:resource="http://semanticbible.org/ns/2006/NTNames#Paul"/>
        <knows rdf:resource="http://semanticbible.org/ns/2006/NTNames#Priscilla"/>
        <knows rdf:resource="http://semanticbible.org/ns/2006/NTNames#Tryphosa"/>
        <religiousBelief rdf:resource="http://semanticbible.org/ns/2006/NTNames#Christianity"/>
        <residentPlace rdf:resource="http://semanticbible.org/ns/2006/NTNames#Rome"/>
        <description rdf:datatype="http://www.w3.org/2001/XMLSchema#string">a &quot;worker in the Lord&quot; in Rome</description>
        <hasOnlyGenealogyMention rdf:datatype="http://www.w3.org/2001/XMLSchema#boolean">false</hasOnlyGenealogyMention>
        <rdfs:label xml:lang="en">Tryphaena</rdfs:label>
    </owl:NamedIndividual>
    


    <!-- http://semanticbible.org/ns/2006/NTNames#Tryphosa -->

    <owl:NamedIndividual rdf:about="http://semanticbible.org/ns/2006/NTNames#Tryphosa">
        <rdf:type rdf:resource="http://semanticbible.org/ns/2006/NTNames#Woman"/>
        <knows rdf:resource="http://semanticbible.org/ns/2006/NTNames#Paul"/>
        <knows rdf:resource="http://semanticbible.org/ns/2006/NTNames#Priscilla"/>
        <knows rdf:resource="http://semanticbible.org/ns/2006/NTNames#Tryphaena"/>
        <religiousBelief rdf:resource="http://semanticbible.org/ns/2006/NTNames#Christianity"/>
        <residentPlace rdf:resource="http://semanticbible.org/ns/2006/NTNames#Rome"/>
        <description rdf:datatype="http://www.w3.org/2001/XMLSchema#string">a &quot;worker in the Lord&quot; in Rome</description>
        <hasOnlyGenealogyMention rdf:datatype="http://www.w3.org/2001/XMLSchema#boolean">false</hasOnlyGenealogyMention>
        <rdfs:label xml:lang="en">Tryphosa</rdfs:label>
    </owl:NamedIndividual>
    


    <!-- http://semanticbible.org/ns/2006/NTNames#Tychicus -->

    <owl:NamedIndividual rdf:about="http://semanticbible.org/ns/2006/NTNames#Tychicus">
        <rdf:type rdf:resource="http://semanticbible.org/ns/2006/NTNames#Man"/>
        <collaboratesWith rdf:resource="http://semanticbible.org/ns/2006/NTNames#Aristarchus"/>
        <collaboratesWith rdf:resource="http://semanticbible.org/ns/2006/NTNames#GaiusOfDerbe"/>
        <collaboratesWith rdf:resource="http://semanticbible.org/ns/2006/NTNames#Secundus"/>
        <collaboratesWith rdf:resource="http://semanticbible.org/ns/2006/NTNames#Sopater"/>
        <rdfs:label xml:lang="en">Tychicus</rdfs:label>
    </owl:NamedIndividual>
    


    <!-- http://semanticbible.org/ns/2006/NTNames#Tyrannus -->

    <owl:NamedIndividual rdf:about="http://semanticbible.org/ns/2006/NTNames#Tyrannus">
        <rdf:type rdf:resource="http://semanticbible.org/ns/2006/NTNames#Man"/>
        <rdfs:label xml:lang="en">Tyrannus</rdfs:label>
    </owl:NamedIndividual>
    


    <!-- http://semanticbible.org/ns/2006/NTNames#Tyre -->

    <owl:NamedIndividual rdf:about="http://semanticbible.org/ns/2006/NTNames#Tyre">
        <rdf:type rdf:resource="http://semanticbible.org/ns/2006/NTNames#City"/>
        <location rdf:resource="http://semanticbible.org/ns/2006/NTNames#TyreGeodata"/>
        <subregionOf rdf:resource="http://semanticbible.org/ns/2006/NTNames#Phoenicia"/>
        <rdfs:label xml:lang="en">Tyre</rdfs:label>
    </owl:NamedIndividual>
    


    <!-- http://semanticbible.org/ns/2006/NTNames#TyreGeodata -->

    <owl:NamedIndividual rdf:about="http://semanticbible.org/ns/2006/NTNames#TyreGeodata">
        <rdf:type rdf:resource="http://semanticbible.org/ns/2006/NTNames#GeographicLocation"/>
        <altitude rdf:datatype="http://www.w3.org/2001/XMLSchema#int">0</altitude>
        <latitude rdf:datatype="http://www.w3.org/2001/XMLSchema#double">33.2729182169202</latitude>
        <longitude rdf:datatype="http://www.w3.org/2001/XMLSchema#double">35.19877875091432</longitude>
        <rdfs:label xml:lang="en">geodata for Tyre</rdfs:label>
    </owl:NamedIndividual>
    


    <!-- http://semanticbible.org/ns/2006/NTNames#Urbanus -->

    <owl:NamedIndividual rdf:about="http://semanticbible.org/ns/2006/NTNames#Urbanus">
        <rdf:type rdf:resource="http://semanticbible.org/ns/2006/NTNames#Man"/>
        <collaboratesWith rdf:resource="http://semanticbible.org/ns/2006/NTNames#Paul"/>
        <knows rdf:resource="http://semanticbible.org/ns/2006/NTNames#Priscilla"/>
        <religiousBelief rdf:resource="http://semanticbible.org/ns/2006/NTNames#Christianity"/>
        <residentPlace rdf:resource="http://semanticbible.org/ns/2006/NTNames#Rome"/>
        <description rdf:datatype="http://www.w3.org/2001/XMLSchema#string">a Christian in Rome to whom Paul sent greetings</description>
        <hasOnlyGenealogyMention rdf:datatype="http://www.w3.org/2001/XMLSchema#boolean">false</hasOnlyGenealogyMention>
        <rdfs:label xml:lang="en">Urbanus</rdfs:label>
    </owl:NamedIndividual>
    


    <!-- http://semanticbible.org/ns/2006/NTNames#Uriah -->

    <owl:NamedIndividual rdf:about="http://semanticbible.org/ns/2006/NTNames#Uriah">
        <rdf:type rdf:resource="http://semanticbible.org/ns/2006/NTNames#Man"/>
        <collaboratesWith rdf:resource="http://semanticbible.org/ns/2006/NTNames#David"/>
        <hasEnemy rdf:resource="http://semanticbible.org/ns/2006/NTNames#David"/>
        <spouseOf rdf:resource="http://semanticbible.org/ns/2006/NTNames#Bathsheba"/>
        <description rdf:datatype="http://www.w3.org/2001/XMLSchema#string">One of the ancestors of Jesus mentioned in Matthew&apos;s geneaology</description>
        <hasOnlyGenealogyMention rdf:datatype="http://www.w3.org/2001/XMLSchema#boolean">true</hasOnlyGenealogyMention>
        <occupation rdf:datatype="http://www.w3.org/2001/XMLSchema#string">soldier</occupation>
        <rdfs:comment xml:lang="en">From OT sources, Uriah was a Hittite and a soldier in David&apos;s army (therefore having both collaboratesWith and hasEnemy relationships with David). </rdfs:comment>
        <rdfs:label xml:lang="en">Uriah</rdfs:label>
    </owl:NamedIndividual>
    


    <!-- http://semanticbible.org/ns/2006/NTNames#Uzziah -->

    <owl:NamedIndividual rdf:about="http://semanticbible.org/ns/2006/NTNames#Uzziah">
        <rdf:type rdf:resource="http://semanticbible.org/ns/2006/NTNames#Man"/>
        <childOf rdf:resource="http://semanticbible.org/ns/2006/NTNames#Joram"/>
        <ethnicity rdf:resource="http://semanticbible.org/ns/2006/NTNames#Jewish"/>
        <parentOf rdf:resource="http://semanticbible.org/ns/2006/NTNames#Jotham"/>
        <description rdf:datatype="http://www.w3.org/2001/XMLSchema#string">One of the ancestors of Jesus mentioned in Matthew&apos;s geneaology</description>
        <hasOnlyGenealogyMention rdf:datatype="http://www.w3.org/2001/XMLSchema#boolean">true</hasOnlyGenealogyMention>
        <occupation rdf:datatype="http://www.w3.org/2001/XMLSchema#string">king of Judah</occupation>
        <rdfs:comment rdf:datatype="http://www.w3.org/2001/XMLSchema#string">His occupation as King comes from Old Testament sources. </rdfs:comment>
        <rdfs:label xml:lang="en">Uzziah</rdfs:label>
    </owl:NamedIndividual>
    


    <!-- http://semanticbible.org/ns/2006/NTNames#Zacchaeus -->

    <owl:NamedIndividual rdf:about="http://semanticbible.org/ns/2006/NTNames#Zacchaeus">
        <rdf:type rdf:resource="http://semanticbible.org/ns/2006/NTNames#Man"/>
        <rdfs:label xml:lang="en">Zacchaeus</rdfs:label>
    </owl:NamedIndividual>
    


    <!-- http://semanticbible.org/ns/2006/NTNames#Zadok -->

    <owl:NamedIndividual rdf:about="http://semanticbible.org/ns/2006/NTNames#Zadok">
        <rdf:type rdf:resource="http://semanticbible.org/ns/2006/NTNames#Man"/>
        <childOf rdf:resource="http://semanticbible.org/ns/2006/NTNames#Azor"/>
        <ethnicity rdf:resource="http://semanticbible.org/ns/2006/NTNames#Jewish"/>
        <parentOf rdf:resource="http://semanticbible.org/ns/2006/NTNames#Achim"/>
        <rdfs:label xml:lang="en">Zadok</rdfs:label>
    </owl:NamedIndividual>
    


    <!-- http://semanticbible.org/ns/2006/NTNames#Zarephath -->

    <owl:NamedIndividual rdf:about="http://semanticbible.org/ns/2006/NTNames#Zarephath">
        <rdf:type rdf:resource="http://semanticbible.org/ns/2006/NTNames#City"/>
        <subregionOf rdf:resource="http://semanticbible.org/ns/2006/NTNames#Phoenicia"/>
        <rdfs:comment xml:lang="en">Jesus recounts the story of Elijah being sent to a widow of Zarephath as an example of God blessing those outside the nation of Israel.</rdfs:comment>
        <rdfs:label xml:lang="en">Zarephath</rdfs:label>
    </owl:NamedIndividual>
    


    <!-- http://semanticbible.org/ns/2006/NTNames#Zealot -->

    <owl:NamedIndividual rdf:about="http://semanticbible.org/ns/2006/NTNames#Zealot">
        <rdf:type rdf:resource="http://semanticbible.org/ns/2006/NTNames#PoliticalAttribute"/>
        <rdfs:label xml:lang="en">Zealot</rdfs:label>
    </owl:NamedIndividual>
    


    <!-- http://semanticbible.org/ns/2006/NTNames#Zebedee -->

    <owl:NamedIndividual rdf:about="http://semanticbible.org/ns/2006/NTNames#Zebedee">
        <rdf:type rdf:resource="http://semanticbible.org/ns/2006/NTNames#Man"/>
        <parentOf rdf:resource="http://semanticbible.org/ns/2006/NTNames#JamesSonOfZebedee"/>
        <parentOf rdf:resource="http://semanticbible.org/ns/2006/NTNames#JohnSonOfZebedee"/>
        <spouseOf rdf:resource="http://semanticbible.org/ns/2006/NTNames#Salome"/>
        <rdfs:label xml:lang="en">Zebedee</rdfs:label>
    </owl:NamedIndividual>
    


    <!-- http://semanticbible.org/ns/2006/NTNames#Zebulun -->

    <owl:NamedIndividual rdf:about="http://semanticbible.org/ns/2006/NTNames#Zebulun">
        <rdf:type rdf:resource="http://semanticbible.org/ns/2006/NTNames#Man"/>
        <siblingOf rdf:resource="http://semanticbible.org/ns/2006/NTNames#Gad"/>
        <rdfs:label xml:lang="en">Zebulun</rdfs:label>
    </owl:NamedIndividual>
    


    <!-- http://semanticbible.org/ns/2006/NTNames#Zechariah -->

    <owl:NamedIndividual rdf:about="http://semanticbible.org/ns/2006/NTNames#Zechariah">
        <rdf:type rdf:resource="http://semanticbible.org/ns/2006/NTNames#Man"/>
        <parentOf rdf:resource="http://semanticbible.org/ns/2006/NTNames#JohntheBaptist"/>
        <spouseOf rdf:resource="http://semanticbible.org/ns/2006/NTNames#Elizabeth"/>
        <rdfs:label xml:lang="en">Zechariah</rdfs:label>
    </owl:NamedIndividual>
    


    <!-- http://semanticbible.org/ns/2006/NTNames#ZechariahSonOfBarachiah -->

    <owl:NamedIndividual rdf:about="http://semanticbible.org/ns/2006/NTNames#ZechariahSonOfBarachiah">
        <rdf:type rdf:resource="http://semanticbible.org/ns/2006/NTNames#Man"/>
        <childOf rdf:resource="http://semanticbible.org/ns/2006/NTNames#Barachiah"/>
        <ethnicity rdf:resource="http://semanticbible.org/ns/2006/NTNames#Jewish"/>
        <rdfs:label xml:lang="en">Zechariah</rdfs:label>
    </owl:NamedIndividual>
    


    <!-- http://semanticbible.org/ns/2006/NTNames#Zenas -->

    <owl:NamedIndividual rdf:about="http://semanticbible.org/ns/2006/NTNames#Zenas">
        <rdf:type rdf:resource="http://semanticbible.org/ns/2006/NTNames#Man"/>
        <rdfs:label xml:lang="en">Zenas</rdfs:label>
    </owl:NamedIndividual>
    


    <!-- http://semanticbible.org/ns/2006/NTNames#Zerah -->

    <owl:NamedIndividual rdf:about="http://semanticbible.org/ns/2006/NTNames#Zerah">
        <rdf:type rdf:resource="http://semanticbible.org/ns/2006/NTNames#Man"/>
        <childOf rdf:resource="http://semanticbible.org/ns/2006/NTNames#Judah"/>
        <childOf rdf:resource="http://semanticbible.org/ns/2006/NTNames#Tamar"/>
        <ethnicity rdf:resource="http://semanticbible.org/ns/2006/NTNames#Jewish"/>
        <siblingOf rdf:resource="http://semanticbible.org/ns/2006/NTNames#Perez"/>
        <description rdf:datatype="http://www.w3.org/2001/XMLSchema#string">One of the ancestors of Jesus mentioned in Matthew&apos;s geneaology</description>
        <rdfs:label xml:lang="en">Zerah</rdfs:label>
    </owl:NamedIndividual>
    


    <!-- http://semanticbible.org/ns/2006/NTNames#Zerubbabel -->

    <owl:NamedIndividual rdf:about="http://semanticbible.org/ns/2006/NTNames#Zerubbabel">
        <rdf:type rdf:resource="http://semanticbible.org/ns/2006/NTNames#Man"/>
        <childOf rdf:resource="http://semanticbible.org/ns/2006/NTNames#Shealtiel"/>
        <ethnicity rdf:resource="http://semanticbible.org/ns/2006/NTNames#Jewish"/>
        <parentOf rdf:resource="http://semanticbible.org/ns/2006/NTNames#Abiud"/>
        <parentOf rdf:resource="http://semanticbible.org/ns/2006/NTNames#Rhesa"/>
        <hasOnlyGenealogyMention rdf:datatype="http://www.w3.org/2001/XMLSchema#boolean">true</hasOnlyGenealogyMention>
        <rdfs:label xml:lang="en">Zerubbabel</rdfs:label>
    </owl:NamedIndividual>
    


    <!-- http://semanticbible.org/ns/2006/NTNames#Zeus -->

    <owl:NamedIndividual rdf:about="http://semanticbible.org/ns/2006/NTNames#Zeus">
        <rdf:type rdf:resource="http://semanticbible.org/ns/2006/NTNames#SupernaturalBeing"/>
        <rdfs:label xml:lang="en">Zeus</rdfs:label>
    </owl:NamedIndividual>
    


    <!-- http://semanticbible.org/ns/2006/NTNames#Zion -->

    <owl:NamedIndividual rdf:about="http://semanticbible.org/ns/2006/NTNames#Zion">
        <rdf:type rdf:resource="http://semanticbible.org/ns/2006/NTNames#Mountain"/>
        <rdfs:label xml:lang="en">Zion</rdfs:label>
    </owl:NamedIndividual>
    


    <!-- 
    ///////////////////////////////////////////////////////////////////////////////////////
    //
    // General axioms
    //
    ///////////////////////////////////////////////////////////////////////////////////////
     -->

    <rdf:Description>
        <rdf:type rdf:resource="http://www.w3.org/2002/07/owl#AllDifferent"/>
        <owl:distinctMembers rdf:parseType="Collection">
            <rdf:Description rdf:about="http://semanticbible.org/ns/2006/NTNames#Canaanite"/>
            <rdf:Description rdf:about="http://semanticbible.org/ns/2006/NTNames#Jewish"/>
        </owl:distinctMembers>
    </rdf:Description>
    <rdf:Description>
        <rdf:type rdf:resource="http://www.w3.org/2002/07/owl#AllDifferent"/>
        <owl:distinctMembers rdf:parseType="Collection">
            <rdf:Description rdf:about="http://semanticbible.org/ns/2006/NTNames#Egyptian"/>
            <rdf:Description rdf:about="http://semanticbible.org/ns/2006/NTNames#Jewish"/>
        </owl:distinctMembers>
    </rdf:Description>
    <rdf:Description>
        <rdf:type rdf:resource="http://www.w3.org/2002/07/owl#AllDifferent"/>
        <owl:distinctMembers rdf:parseType="Collection">
            <rdf:Description rdf:about="http://semanticbible.org/ns/2006/NTNames#Epaphras"/>
            <rdf:Description rdf:about="http://semanticbible.org/ns/2006/NTNames#Epaphroditus"/>
        </owl:distinctMembers>
    </rdf:Description>
    <rdf:Description>
        <rdf:type rdf:resource="http://www.w3.org/2002/07/owl#AllDifferent"/>
        <owl:distinctMembers rdf:parseType="Collection">
            <rdf:Description rdf:about="http://semanticbible.org/ns/2006/NTNames#Ethiopian"/>
            <rdf:Description rdf:about="http://semanticbible.org/ns/2006/NTNames#Jewish"/>
        </owl:distinctMembers>
    </rdf:Description>
    <rdf:Description>
        <rdf:type rdf:resource="http://www.w3.org/2002/07/owl#AllDifferent"/>
        <owl:distinctMembers rdf:parseType="Collection">
            <rdf:Description rdf:about="http://semanticbible.org/ns/2006/NTNames#Galilean"/>
            <rdf:Description rdf:about="http://semanticbible.org/ns/2006/NTNames#Judean"/>
        </owl:distinctMembers>
    </rdf:Description>
    <rdf:Description>
        <rdf:type rdf:resource="http://www.w3.org/2002/07/owl#AllDifferent"/>
        <owl:distinctMembers rdf:parseType="Collection">
            <rdf:Description rdf:about="http://semanticbible.org/ns/2006/NTNames#Galilean"/>
            <rdf:Description rdf:about="http://semanticbible.org/ns/2006/NTNames#Samaritan"/>
        </owl:distinctMembers>
    </rdf:Description>
    <rdf:Description>
        <rdf:type rdf:resource="http://www.w3.org/2002/07/owl#AllDifferent"/>
        <owl:distinctMembers rdf:parseType="Collection">
            <rdf:Description rdf:about="http://semanticbible.org/ns/2006/NTNames#Gentile"/>
            <rdf:Description rdf:about="http://semanticbible.org/ns/2006/NTNames#Jewish"/>
        </owl:distinctMembers>
    </rdf:Description>
    <rdf:Description>
        <rdf:type rdf:resource="http://www.w3.org/2002/07/owl#AllDifferent"/>
        <owl:distinctMembers rdf:parseType="Collection">
            <rdf:Description rdf:about="http://semanticbible.org/ns/2006/NTNames#Jacob"/>
            <rdf:Description rdf:about="http://semanticbible.org/ns/2006/NTNames#JacobSonOfMatthan"/>
        </owl:distinctMembers>
    </rdf:Description>
    <rdf:Description>
        <rdf:type rdf:resource="http://www.w3.org/2002/07/owl#AllDifferent"/>
        <owl:distinctMembers rdf:parseType="Collection">
            <rdf:Description rdf:about="http://semanticbible.org/ns/2006/NTNames#Judean"/>
            <rdf:Description rdf:about="http://semanticbible.org/ns/2006/NTNames#Samaritan"/>
        </owl:distinctMembers>
    </rdf:Description>
    <rdf:Description>
        <rdf:type rdf:resource="http://www.w3.org/2002/07/owl#AllDifferent"/>
        <owl:distinctMembers rdf:parseType="Collection">
            <rdf:Description rdf:about="http://semanticbible.org/ns/2006/NTNames#Levi"/>
            <rdf:Description rdf:about="http://semanticbible.org/ns/2006/NTNames#LeviSonOfMelki"/>
        </owl:distinctMembers>
    </rdf:Description>
    <rdf:Description>
        <rdf:type rdf:resource="http://www.w3.org/2002/07/owl#AllDifferent"/>
        <owl:distinctMembers rdf:parseType="Collection">
            <rdf:Description rdf:about="http://semanticbible.org/ns/2006/NTNames#Levi"/>
            <rdf:Description rdf:about="http://semanticbible.org/ns/2006/NTNames#LeviSonOfSimeon"/>
        </owl:distinctMembers>
    </rdf:Description>
</rdf:RDF>



<!-- Generated by the OWL API (version 4.5.9.2019-02-01T07:24:44Z) https://github.com/owlcs/owlapi -->

